@prefix dct: <http://purl.org/dc/terms/> .
@prefix rdf: <http://www.w3.org/1999/02/22-rdf-syntax-ns#> .
@prefix dc: <http://purl.org/dc/elements/1.1/> .
@prefix ebucore: <http://www.ebu.ch/metadata/ontologies/ebucore/ebucore#> .
@prefix parentalguidance: <http://www.ebu.ch/metadata/ontologies/skos/ebu_ParentalGuidanceCodeCS#> .
@prefix owl: <http://www.w3.org/2002/07/owl#> .
@prefix skos: <http://www.w3.org/2004/02/skos/core#> .
@prefix rdfs: <http://www.w3.org/2000/01/rdf-schema#> .

parentalguidance:_14.3
        skos:example      "" ;
        skos:historyNote  "" ;
        skos:changeNote   "" ;
        skos:inScheme     <http://www.ebu.ch/metadata/ontologies/skos/ebu_ParentalGuidanceCodeCS> ;
        skos:broader      parentalguidance:_14 ;
        skos:definition   "For ages 12 and older"@en ;
        skos:definition   "Infantil para mayores de 12 años"@es ;
        skos:prefLabel    "I12"@en ;
        rdf:type          ebucore:TargetAudience .

parentalguidance:_47.2.31
        skos:example      "" ;
        skos:historyNote  "" ;
        skos:changeNote   "" ;
        skos:inScheme     <http://www.ebu.ch/metadata/ontologies/skos/ebu_ParentalGuidanceCodeCS> ;
        skos:broader      parentalguidance:_47.2 ;
        skos:definition   "The consumption of tobacco products" ;
        skos:prefLabel    "Use of Tobacco"@en ;
        rdf:type          ebucore:TargetAudience .

parentalguidance:_54.1.4
        skos:example      "" ;
        skos:historyNote  "" ;
        skos:changeNote   "" ;
        skos:inScheme     <http://www.ebu.ch/metadata/ontologies/skos/ebu_ParentalGuidanceCodeCS> ;
        skos:broader      parentalguidance:_54.1 ;
        skos:definition   "not suitable for people under 18. (category IV.) "@en ;
        skos:prefLabel    "18"@en ;
        rdf:type          ebucore:TargetAudience .

parentalguidance:_34.2.7
        skos:example      "" ;
        skos:historyNote  "" ;
        skos:changeNote   "" ;
        skos:inScheme     <http://www.ebu.ch/metadata/ontologies/skos/ebu_ParentalGuidanceCodeCS> ;
        skos:broader      parentalguidance:_34.2 ;
        skos:prefLabel    "Religion"@en ;
        rdf:type          ebucore:TargetAudience .

parentalguidance:_58.1.7
        skos:example      "" ;
        skos:historyNote  "" ;
        skos:changeNote   "" ;
        skos:inScheme     <http://www.ebu.ch/metadata/ontologies/skos/ebu_ParentalGuidanceCodeCS> ;
        skos:broader      parentalguidance:_58.1 ;
        skos:definition   "Younger than 16 Prohibited"@en ;
        skos:prefLabel    "K-16"@en ;
        rdf:type          ebucore:TargetAudience .

parentalguidance:_30.3.1
        skos:example      "" ;
        skos:historyNote  "" ;
        skos:changeNote   "" ;
        skos:inScheme     <http://www.ebu.ch/metadata/ontologies/skos/ebu_ParentalGuidanceCodeCS> ;
        skos:broader      parentalguidance:_30.3 ;
        skos:definition   "No one under the age of 14 admitted"@en ;
        skos:prefLabel    "VM14"@en ;
        rdf:type          ebucore:TargetAudience .

parentalguidance:_48.4
        skos:example      "" ;
        skos:historyNote  "" ;
        skos:changeNote   "" ;
        skos:inScheme     <http://www.ebu.ch/metadata/ontologies/skos/ebu_ParentalGuidanceCodeCS> ;
        skos:broader      parentalguidance:_48 ;
        skos:definition   "Under 17 requires accompyning parent or adult guardian. "@en ;
        skos:prefLabel    "Restricted"@en ;
        skos:prefLabel    "R"@en ;
        rdf:type          ebucore:TargetAudience .

parentalguidance:_26.1
        skos:example      "" ;
        skos:historyNote  "" ;
        skos:changeNote   "" ;
        skos:inScheme     <http://www.ebu.ch/metadata/ontologies/skos/ebu_ParentalGuidanceCodeCS> ;
        skos:broader      parentalguidance:_26 ;
        skos:definition   "Not Recommended for children under 10"@en ;
        skos:definition   "Pas pour les moins de dix ans"@fr ;
        skos:prefLabel    "-10"@en ;
        rdf:type          ebucore:TargetAudience .

parentalguidance:_25.4
        skos:example      "" ;
        skos:historyNote  "" ;
        skos:changeNote   "" ;
        skos:inScheme     <http://www.ebu.ch/metadata/ontologies/skos/ebu_ParentalGuidanceCodeCS> ;
        skos:broader      parentalguidance:_25 ;
        skos:definition   "Unsuitable for minors under 18, may apply to works with\n         non-simulated sexual acts or extreme violence, but do not apply to X rating due to the\n         nature of the theme being treated or the way it has been filmed"@en ;
        skos:definition   "Interdiction de représentation aux moins de dix-huit ans,\n         prévoit que cette restriction peut concerner les œuvres qui comportent « des scènes de sexe\n         non simulées ou de très grande violence mais qui, par la manière dont elles sont filmées et\n         la nature du thème traité ne justifient pas » d’un classement X"@fr ;
        skos:prefLabel    "-18"@en ;
        rdf:type          ebucore:TargetAudience .

parentalguidance:_49  skos:definition  "Recording Industry Association of America scheme. Scheme for\n         music rating as defined by the Recording Industry Association of America"@en ;
        rdf:type          ebucore:TargetAudience ;
        skos:changeNote   "Update" ;
        skos:note         "Valid" ;
        skos:scopeNote    "Region:United States"@en ;
        skos:narrower     parentalguidance:_49.1 ;
        skos:historyNote  "2009-07-28" ;
        skos:prefLabel    "US-RIAA"@en ;
        skos:inScheme     <http://www.ebu.ch/metadata/ontologies/skos/ebu_ParentalGuidanceCodeCS> ;
        skos:example      "" .

parentalguidance:_66.1.2
        skos:example      "" ;
        skos:historyNote  "" ;
        skos:changeNote   "" ;
        skos:inScheme     <http://www.ebu.ch/metadata/ontologies/skos/ebu_ParentalGuidanceCodeCS> ;
        skos:broader      parentalguidance:_66.1 ;
        skos:definition   "Under 13 not admitted unless accompanied by an individual over\n         13. Some material may not be suitable for children "@en ;
        skos:prefLabel    "PG-13"@en ;
        rdf:type          ebucore:TargetAudience .

parentalguidance:_37  skos:example  "" ;
        skos:prefLabel    "NL-NICAM"@en ;
        skos:narrower     parentalguidance:_37.2 ;
        rdf:type          ebucore:TargetAudience ;
        skos:definition   "Nederlands Institute for the Classification of Audio-visual\n         Media"@en ;
        skos:scopeNote    "Region:Netherlands"@en ;
        skos:changeNote   "Update" ;
        skos:note         "Valid" ;
        skos:historyNote  "2009-07-28" ;
        skos:inScheme     <http://www.ebu.ch/metadata/ontologies/skos/ebu_ParentalGuidanceCodeCS> ;
        skos:narrower     parentalguidance:_37.1 .

parentalguidance:_37.1.3
        skos:example      "" ;
        skos:historyNote  "" ;
        skos:changeNote   "" ;
        skos:inScheme     <http://www.ebu.ch/metadata/ontologies/skos/ebu_ParentalGuidanceCodeCS> ;
        skos:broader      parentalguidance:_37.1 ;
        skos:definition   "Let op met kinderen tot 9 jaar"@nl ;
        skos:definition   "Not recommended for viewers younger than 9\n         years"@en ;
        skos:prefLabel    "9"@en ;
        rdf:type          ebucore:TargetAudience .

parentalguidance:_9.2
        skos:example      "" ;
        skos:historyNote  "" ;
        skos:changeNote   "" ;
        skos:inScheme     <http://www.ebu.ch/metadata/ontologies/skos/ebu_ParentalGuidanceCodeCS> ;
        skos:broader      parentalguidance:_9 ;
        skos:definition   "Parental guidance advised. Theme or content may not be suitable\n         for all children."@en ;
        skos:prefLabel    "Parental Guidance"@en ;
        skos:altLabel     "PG"@en ;
        rdf:type          ebucore:TargetAudience .

parentalguidance:_25  skos:narrower  parentalguidance:_25.5 ;
        rdf:type          ebucore:TargetAudience ;
        skos:narrower     parentalguidance:_25.3 ;
        skos:narrower     parentalguidance:_25.1 ;
        skos:definition   "Centre National de Cinematographie"@en ;
        skos:narrower     parentalguidance:_25.4 ;
        skos:historyNote  "2009-07-28" ;
        skos:changeNote   "Update" ;
        skos:prefLabel    "FR-CNC"@en ;
        skos:example      "" ;
        skos:narrower     parentalguidance:_25.2 ;
        skos:inScheme     <http://www.ebu.ch/metadata/ontologies/skos/ebu_ParentalGuidanceCodeCS> ;
        skos:note         "Valid" ;
        skos:scopeNote    "Region:France" .

parentalguidance:_34.2.6
        skos:example      "" ;
        skos:historyNote  "" ;
        skos:changeNote   "" ;
        skos:inScheme     <http://www.ebu.ch/metadata/ontologies/skos/ebu_ParentalGuidanceCodeCS> ;
        skos:broader      parentalguidance:_34.2 ;
        skos:prefLabel    "Harshness of language"@en ;
        rdf:type          ebucore:TargetAudience .

parentalguidance:_49.1
        skos:example      "" ;
        skos:historyNote  "" ;
        skos:changeNote   "" ;
        skos:inScheme     <http://www.ebu.ch/metadata/ontologies/skos/ebu_ParentalGuidanceCodeCS> ;
        skos:broader      parentalguidance:_49 ;
        skos:definition   "The Parental Advisory is a notice to consumers that recordings\n         identified by this value may contain strong language or depiction of violence, sex or\n         substance abuse. Parental discretion is advised" ;
        skos:prefLabel    "Parental Advisory"@en ;
        rdf:type          ebucore:TargetAudience .

parentalguidance:_13  skos:narrower  parentalguidance:_13.4 ;
        rdf:type          ebucore:TargetAudience ;
        skos:scopeNote    "Region:Canada"@en ;
        skos:narrower     parentalguidance:_13.1 ;
        skos:narrower     parentalguidance:_13.5 ;
        skos:narrower     parentalguidance:_13.2 ;
        skos:prefLabel    "CA-CBSC-CCNR-French"@en ;
        skos:changeNote   "Update" ;
        skos:example      "" ;
        skos:inScheme     <http://www.ebu.ch/metadata/ontologies/skos/ebu_ParentalGuidanceCodeCS> ;
        skos:definition   "Ratings Classification for Canadian French-Language\n         Broadcasters"@en ;
        skos:narrower     parentalguidance:_13.3 ;
        skos:note         "Valid" ;
        skos:historyNote  "2009-07-27" .

parentalguidance:_24.7
        skos:example      "" ;
        skos:historyNote  "" ;
        skos:changeNote   "" ;
        skos:narrower     parentalguidance:_24.7.1 ;
        skos:inScheme     <http://www.ebu.ch/metadata/ontologies/skos/ebu_ParentalGuidanceCodeCS> ;
        skos:broader      parentalguidance:_24 ;
        skos:definition   "For people aged 18 years and above"@en ;
        skos:prefLabel    "K-18"@en ;
        rdf:type          ebucore:TargetAudience .

parentalguidance:_8.5
        skos:example      "" ;
        skos:historyNote  "" ;
        skos:changeNote   "" ;
        skos:inScheme     <http://www.ebu.ch/metadata/ontologies/skos/ebu_ParentalGuidanceCodeCS> ;
        skos:broader      parentalguidance:_8 ;
        skos:definition   "Restricted to 18 years and older. No rental or purchase by\n         those under 18. Contents not suitable for minors. Contains frequent sexual activity,\n         brutality/graphic violence, intense horror, and/or other disturbing content. "@en ;
        skos:prefLabel    "R - Restricted"@en ;
        rdf:type          ebucore:TargetAudience .

parentalguidance:_4.1.1
        skos:example      "" ;
        skos:historyNote  "" ;
        skos:changeNote   "" ;
        skos:inScheme     <http://www.ebu.ch/metadata/ontologies/skos/ebu_ParentalGuidanceCodeCS> ;
        skos:broader      parentalguidance:_4.1 ;
        skos:definition   "Pre-school"@en ;
        skos:prefLabel    "P"@en ;
        rdf:type          ebucore:TargetAudience .

parentalguidance:_51.2.6
        skos:example      "" ;
        skos:historyNote  "" ;
        skos:changeNote   "" ;
        skos:inScheme     <http://www.ebu.ch/metadata/ontologies/skos/ebu_ParentalGuidanceCodeCS> ;
        skos:broader      parentalguidance:_51.2 ;
        skos:definition   "Violence"@en ;
        skos:prefLabel    "V"@en ;
        rdf:type          ebucore:TargetAudience .

parentalguidance:_15.1
        skos:example      "" ;
        skos:historyNote  "" ;
        skos:changeNote   "" ;
        skos:inScheme     <http://www.ebu.ch/metadata/ontologies/skos/ebu_ParentalGuidanceCodeCS> ;
        skos:broader      parentalguidance:_15 ;
        skos:definition   "All Audiences"@en ;
        skos:definition   "Todo expectador"@es ;
        skos:prefLabel    "TE"@en ;
        rdf:type          ebucore:TargetAudience .

parentalguidance:_37.2
        skos:narrower     parentalguidance:_37.2.1 ;
        skos:narrower     parentalguidance:_37.2.6 ;
        skos:changeNote   "" ;
        skos:historyNote  "" ;
        skos:prefLabel    "Criteria"@en ;
        skos:inScheme     <http://www.ebu.ch/metadata/ontologies/skos/ebu_ParentalGuidanceCodeCS> ;
        skos:narrower     parentalguidance:_37.2.5 ;
        skos:narrower     parentalguidance:_37.2.3 ;
        skos:example      "" ;
        skos:narrower     parentalguidance:_37.2.4 ;
        skos:broader      parentalguidance:_37 ;
        rdf:type          ebucore:TargetAudience ;
        skos:narrower     parentalguidance:_37.2.2 .

parentalguidance:_47.2.30
        skos:example      "" ;
        skos:historyNote  "" ;
        skos:changeNote   "" ;
        skos:inScheme     <http://www.ebu.ch/metadata/ontologies/skos/ebu_ParentalGuidanceCodeCS> ;
        skos:broader      parentalguidance:_47.2 ;
        skos:definition   "The consumption of alcoholic beverages" ;
        skos:prefLabel    "Use of Alcohol"@en ;
        rdf:type          ebucore:TargetAudience .

_:b0    rdf:rest   _:b1 ;
        rdf:first  parentalguidance:_50 .

parentalguidance:_14.4
        skos:example      "" ;
        skos:historyNote  "" ;
        skos:changeNote   "" ;
        skos:inScheme     <http://www.ebu.ch/metadata/ontologies/skos/ebu_ParentalGuidanceCodeCS> ;
        skos:broader      parentalguidance:_14 ;
        skos:definition   "Shows suitable for all ages, regardless of specific\n         content."@en ;
        skos:definition   "Familiar"@es ;
        skos:prefLabel    "F"@en ;
        rdf:type          ebucore:TargetAudience .

parentalguidance:_54.1.5
        skos:example      "" ;
        skos:historyNote  "" ;
        skos:changeNote   "" ;
        skos:inScheme     <http://www.ebu.ch/metadata/ontologies/skos/ebu_ParentalGuidanceCodeCS> ;
        skos:broader      parentalguidance:_54.1 ;
        skos:definition   "only for adults (category V.) "@en ;
        skos:prefLabel    "X"@en ;
        rdf:type          ebucore:TargetAudience .

parentalguidance:_58.1.8
        skos:example      "" ;
        skos:historyNote  "" ;
        skos:changeNote   "" ;
        skos:inScheme     <http://www.ebu.ch/metadata/ontologies/skos/ebu_ParentalGuidanceCodeCS> ;
        skos:broader      parentalguidance:_58.1 ;
        skos:definition   "Younger than 6 Prohibited. Commonly know as\n         K-E"@en ;
        skos:prefLabel    "K-6"@en ;
        rdf:type          ebucore:TargetAudience .

parentalguidance:_37.1.5
        skos:example      "" ;
        skos:historyNote  "" ;
        skos:changeNote   "" ;
        skos:inScheme     <http://www.ebu.ch/metadata/ontologies/skos/ebu_ParentalGuidanceCodeCS> ;
        skos:broader      parentalguidance:_37.1 ;
        skos:definition   "Let op met kinderen tot 16 jaar"@nl ;
        skos:definition   "Movie shops/cinemas aren't allowed to show these movies to\n         people younger than 16 years"@en ;
        skos:prefLabel    "16"@en ;
        rdf:type          ebucore:TargetAudience .

parentalguidance:_8.6
        skos:example      "" ;
        skos:historyNote  "" ;
        skos:changeNote   "" ;
        skos:inScheme     <http://www.ebu.ch/metadata/ontologies/skos/ebu_ParentalGuidanceCodeCS> ;
        skos:broader      parentalguidance:_8 ;
        skos:definition   "Contains material not subject to classification, such as\n         documentaries, nature, travel, music, arts and culture, sports and leisure, educational and\n         instructional information."@en ;
        skos:prefLabel    "E - Exempt"@en ;
        rdf:type          ebucore:TargetAudience .

parentalguidance:_16.1.1
        skos:example      "" ;
        skos:historyNote  "" ;
        skos:changeNote   "" ;
        skos:inScheme     <http://www.ebu.ch/metadata/ontologies/skos/ebu_ParentalGuidanceCodeCS> ;
        skos:broader      parentalguidance:_16.1 ;
        skos:definition   "Programmes classified \"PG\" may contain adult themes or concepts\n         but must remain suitable for children to watch under the guidance of a parent or\n         guardian."@en ;
        skos:prefLabel    "Parental Guidance"@en ;
        skos:altLabel     "PG"@en ;
        rdf:type          ebucore:TargetAudience .

parentalguidance:_26.2
        skos:example      "" ;
        skos:historyNote  "" ;
        skos:changeNote   "" ;
        skos:inScheme     <http://www.ebu.ch/metadata/ontologies/skos/ebu_ParentalGuidanceCodeCS> ;
        skos:broader      parentalguidance:_26 ;
        skos:definition   "Not Recommended for children under 12"@en ;
        skos:definition   "Pas pour les moins de douze ans"@fr ;
        skos:prefLabel    "-12"@en ;
        rdf:type          ebucore:TargetAudience .

parentalguidance:_38  skos:narrower  parentalguidance:_38.3 ;
        skos:narrower     parentalguidance:_38.1 ;
        skos:example      "" ;
        skos:definition   "Scheme as defined by the Medietilsynet"@en ;
        skos:note         "Valid" ;
        skos:scopeNote    "Region:Norway"@en ;
        skos:historyNote  "2009-07-28" ;
        skos:narrower     parentalguidance:_38.4 ;
        skos:inScheme     <http://www.ebu.ch/metadata/ontologies/skos/ebu_ParentalGuidanceCodeCS> ;
        skos:prefLabel    "NO-Medietilsynet-Om_aldersgrenser"@en ;
        skos:narrower     parentalguidance:_38.2 ;
        rdf:type          ebucore:TargetAudience ;
        skos:narrower     parentalguidance:_38.5 ;
        skos:changeNote   "Update" .

parentalguidance:_37.1.4
        skos:example      "" ;
        skos:historyNote  "" ;
        skos:changeNote   "" ;
        skos:inScheme     <http://www.ebu.ch/metadata/ontologies/skos/ebu_ParentalGuidanceCodeCS> ;
        skos:broader      parentalguidance:_37.1 ;
        skos:definition   "Let op met kinderen tot 12 jaar"@nl ;
        skos:definition   "Not recommended for viewers younger than 12\n         years"@en ;
        skos:prefLabel    "12"@en ;
        rdf:type          ebucore:TargetAudience .

parentalguidance:_26  skos:inScheme  <http://www.ebu.ch/metadata/ontologies/skos/ebu_ParentalGuidanceCodeCS> ;
        skos:note         "Valid" ;
        skos:scopeNote    "Region:France" ;
        skos:narrower     parentalguidance:_26.4 ;
        skos:narrower     parentalguidance:_26.2 ;
        skos:changeNote   "Update" ;
        skos:example      "" ;
        skos:prefLabel    "FR-CSA"@en ;
        skos:narrower     parentalguidance:_26.5 ;
        skos:narrower     parentalguidance:_26.3 ;
        rdf:type          ebucore:TargetAudience ;
        skos:historyNote  "2009-07-28" ;
        skos:definition   "Conseil Superieur de l'Audiovisuel"@en ;
        skos:narrower     parentalguidance:_26.1 .

parentalguidance:_14  skos:narrower  parentalguidance:_14.6 ;
        skos:prefLabel    "CL-ANATEL"@en ;
        skos:prefLabel    "CL-ANATEL"@es ;
        skos:narrower     parentalguidance:_14.4 ;
        skos:narrower     parentalguidance:_14.1 ;
        skos:inScheme     <http://www.ebu.ch/metadata/ontologies/skos/ebu_ParentalGuidanceCodeCS> ;
        rdf:type          ebucore:TargetAudience ;
        skos:narrower     parentalguidance:_14.2 ;
        skos:definition   "National Broadcasting Association rating\n         system"@en ;
        skos:note         "Valid" ;
        skos:narrower     parentalguidance:_14.5 ;
        skos:definition   "Asociación Nacional de Televisión"@es ;
        skos:historyNote  "2009-07-27" ;
        skos:narrower     parentalguidance:_14.3 ;
        skos:changeNote   "Update" ;
        skos:example      "" ;
        skos:scopeNote    "Region:Chile"@en .

parentalguidance:_25.5
        skos:example      "" ;
        skos:historyNote  "" ;
        skos:changeNote   "" ;
        skos:inScheme     <http://www.ebu.ch/metadata/ontologies/skos/ebu_ParentalGuidanceCodeCS> ;
        skos:broader      parentalguidance:_25 ;
        skos:definition   "Adult only, pornographic content"@en ;
        skos:definition   "Programme pour adultes - Contenu de nature\n         pornographie"@fr ;
        skos:prefLabel    "X"@en ;
        rdf:type          ebucore:TargetAudience .

parentalguidance:_9.3
        skos:example      "" ;
        skos:historyNote  "" ;
        skos:changeNote   "" ;
        skos:inScheme     <http://www.ebu.ch/metadata/ontologies/skos/ebu_ParentalGuidanceCodeCS> ;
        skos:broader      parentalguidance:_9 ;
        skos:definition   "Suitable for people 14 years of age or older. Those under 14\n         should view with an adult. No rental or purchase by those under 14 where prohibited by law.\n         Parents cautioned. May contain violence, coarse language and/or sexually suggestive\n         scenes."@en ;
        skos:prefLabel    "14A"@en ;
        rdf:type          ebucore:TargetAudience .

parentalguidance:_66.1.3
        skos:example      "" ;
        skos:historyNote  "" ;
        skos:changeNote   "" ;
        skos:inScheme     <http://www.ebu.ch/metadata/ontologies/skos/ebu_ParentalGuidanceCodeCS> ;
        skos:broader      parentalguidance:_66.1 ;
        skos:definition   "Under 15 not admitted unless accompanied by an individual over\n         15. Some material may not be suitable for children "@en ;
        skos:prefLabel    "PG15"@en ;
        rdf:type          ebucore:TargetAudience .

parentalguidance:_37.2.1
        skos:example      "" ;
        skos:historyNote  "" ;
        skos:changeNote   "" ;
        skos:inScheme     <http://www.ebu.ch/metadata/ontologies/skos/ebu_ParentalGuidanceCodeCS> ;
        skos:broader      parentalguidance:_37.2 ;
        skos:prefLabel    "Geweld"@nl ;
        skos:prefLabel    "Violence"@en ;
        rdf:type          ebucore:TargetAudience .

parentalguidance:_63.1.7
        skos:example      "" ;
        skos:historyNote  "" ;
        skos:changeNote   "" ;
        skos:inScheme     <http://www.ebu.ch/metadata/ontologies/skos/ebu_ParentalGuidanceCodeCS> ;
        skos:broader      parentalguidance:_63.1 ;
        skos:definition   ""@en ;
        skos:prefLabel    "Banned"@en ;
        rdf:type          ebucore:TargetAudience .

parentalguidance:_34.2.5
        skos:example      "" ;
        skos:historyNote  "" ;
        skos:changeNote   "" ;
        skos:inScheme     <http://www.ebu.ch/metadata/ontologies/skos/ebu_ParentalGuidanceCodeCS> ;
        skos:broader      parentalguidance:_34.2 ;
        skos:prefLabel    "Drugs abuse"@en ;
        rdf:type          ebucore:TargetAudience .

parentalguidance:_48.3
        skos:example      "" ;
        skos:historyNote  "" ;
        skos:changeNote   "" ;
        skos:inScheme     <http://www.ebu.ch/metadata/ontologies/skos/ebu_ParentalGuidanceCodeCS> ;
        skos:broader      parentalguidance:_48 ;
        skos:definition   "Some material may be inappropriate for children under 13. "@en ;
        skos:definition   "Parents strongly cautioned"@en ;
        skos:prefLabel    "PG-13"@en ;
        rdf:type          ebucore:TargetAudience .

parentalguidance:_14.1
        skos:example      "" ;
        skos:historyNote  "" ;
        skos:changeNote   "" ;
        skos:inScheme     <http://www.ebu.ch/metadata/ontologies/skos/ebu_ParentalGuidanceCodeCS> ;
        skos:broader      parentalguidance:_14 ;
        skos:definition   "For all ages"@en ;
        skos:definition   "Infantil"@es ;
        skos:prefLabel    "I"@en ;
        rdf:type          ebucore:TargetAudience .

parentalguidance:_4.2.11
        skos:example      "" ;
        skos:historyNote  "" ;
        skos:changeNote   "" ;
        skos:inScheme     <http://www.ebu.ch/metadata/ontologies/skos/ebu_ParentalGuidanceCodeCS> ;
        skos:broader      parentalguidance:_4.2 ;
        skos:definition   "Colorful behaviour"@en ;
        skos:prefLabel    "B"@en ;
        rdf:type          ebucore:TargetAudience .

parentalguidance:_37.1
        skos:narrower     parentalguidance:_37.1.3 ;
        skos:prefLabel    "Rating"@en ;
        skos:inScheme     <http://www.ebu.ch/metadata/ontologies/skos/ebu_ParentalGuidanceCodeCS> ;
        rdf:type          ebucore:TargetAudience ;
        skos:narrower     parentalguidance:_37.1.2 ;
        skos:narrower     parentalguidance:_37.1.5 ;
        skos:changeNote   "" ;
        skos:historyNote  "" ;
        skos:broader      parentalguidance:_37 ;
        skos:example      "" ;
        skos:narrower     parentalguidance:_37.1.4 ;
        skos:narrower     parentalguidance:_37.1.1 .

parentalguidance:_62.1
        skos:inScheme     <http://www.ebu.ch/metadata/ontologies/skos/ebu_ParentalGuidanceCodeCS> ;
        skos:narrower     parentalguidance:_62.1.2 ;
        skos:historyNote  "" ;
        skos:prefLabel    "Rating"@en ;
        skos:changeNote   "" ;
        skos:example      "" ;
        skos:narrower     parentalguidance:_62.1.1 ;
        rdf:type          ebucore:TargetAudience ;
        skos:narrower     parentalguidance:_62.1.3 ;
        skos:broader      parentalguidance:_62 .

parentalguidance:_13.4
        skos:definition   "Le film ne peut être vu, acheté ou loué que par des personnes\n         de 16 ans et plus."@fr ;
        skos:changeNote   "" ;
        skos:broader      parentalguidance:_13 ;
        skos:definition   "Only for 16 and older"@en ;
        rdf:type          ebucore:TargetAudience ;
        skos:prefLabel    "16+"@fr ;
        skos:prefLabel    "16+"@en ;
        skos:historyNote  "" ;
        skos:inScheme     <http://www.ebu.ch/metadata/ontologies/skos/ebu_ParentalGuidanceCodeCS> ;
        skos:example      "" .

parentalguidance:_46.2.3
        skos:example      "" ;
        skos:historyNote  "" ;
        skos:changeNote   "" ;
        skos:inScheme     <http://www.ebu.ch/metadata/ontologies/skos/ebu_ParentalGuidanceCodeCS> ;
        skos:broader      parentalguidance:_46.2 ;
        skos:prefLabel    "Negative behaviour"@en ;
        skos:prefLabel    "Olumsuz örnek oluşturabilecek davranışlar içerir"@tr ;
        rdf:type          ebucore:TargetAudience .

parentalguidance:_54.1.2
        skos:example      "" ;
        skos:historyNote  "" ;
        skos:changeNote   "" ;
        skos:inScheme     <http://www.ebu.ch/metadata/ontologies/skos/ebu_ParentalGuidanceCodeCS> ;
        skos:broader      parentalguidance:_54.1 ;
        skos:definition   "parental guidance suggested for children under 12. (category\n         II.) "@en ;
        skos:prefLabel    "12"@en ;
        rdf:type          ebucore:TargetAudience .

parentalguidance:_23  skos:scopeNote  "Region:Europe"@en ;
        skos:narrower     parentalguidance:_23.2 ;
        skos:note         "Valid" ;
        skos:narrower     parentalguidance:_23.1 ;
        skos:historyNote  "2009-07-28" ;
        skos:example      "" ;
        skos:changeNote   "Update" ;
        skos:definition   "Pan European Game Information"@en ;
        skos:prefLabel    "EU-PEGI"@en ;
        skos:inScheme     <http://www.ebu.ch/metadata/ontologies/skos/ebu_ParentalGuidanceCodeCS> ;
        rdf:type          ebucore:TargetAudience .

parentalguidance:_24.5
        skos:example      "" ;
        skos:historyNote  "" ;
        skos:changeNote   "" ;
        skos:narrower     parentalguidance:_24.5.1 ;
        skos:inScheme     <http://www.ebu.ch/metadata/ontologies/skos/ebu_ParentalGuidanceCodeCS> ;
        skos:broader      parentalguidance:_24 ;
        skos:definition   "For people aged 13 years and above"@en ;
        skos:prefLabel    "K-13"@en ;
        rdf:type          ebucore:TargetAudience .

parentalguidance:_11  skos:narrower  parentalguidance:_11.1 ;
        skos:scopeNote    "Region:Canada"@en ;
        skos:note         "Valid" ;
        skos:historyNote  "2009-07-27" ;
        skos:narrower     parentalguidance:_11.3 ;
        skos:example      "" ;
        skos:changeNote   "Update" ;
        skos:narrower     parentalguidance:_11.2 ;
        skos:inScheme     <http://www.ebu.ch/metadata/ontologies/skos/ebu_ParentalGuidanceCodeCS> ;
        skos:prefLabel    "CA-RCQ"@en ;
        rdf:type          ebucore:TargetAudience ;
        skos:narrower     parentalguidance:_11.4 ;
        skos:definition   "Regie du cinema du Quebec"@fr .

parentalguidance:_16.1.2
        skos:example      "" ;
        skos:historyNote  "" ;
        skos:changeNote   "" ;
        skos:inScheme     <http://www.ebu.ch/metadata/ontologies/skos/ebu_ParentalGuidanceCodeCS> ;
        skos:broader      parentalguidance:_16.1 ;
        skos:definition   "Programmes classified \"M\" are recommended for viewing by\n         grown-up members of the family only."@en ;
        skos:prefLabel    "Mature"@en ;
        skos:prefLabel    "M"@en ;
        rdf:type          ebucore:TargetAudience .

parentalguidance:_25.2
        skos:example      "" ;
        skos:historyNote  "" ;
        skos:changeNote   "" ;
        skos:inScheme     <http://www.ebu.ch/metadata/ontologies/skos/ebu_ParentalGuidanceCodeCS> ;
        skos:broader      parentalguidance:_25 ;
        skos:definition   "Unsuitable for minors under 12"@en ;
        skos:definition   "Interdiction de représentation aux moins de douze\n         ans"@fr ;
        skos:prefLabel    "-12"@en ;
        rdf:type          ebucore:TargetAudience .

parentalguidance:_62.1.1
        skos:example      "" ;
        skos:historyNote  "" ;
        skos:changeNote   "" ;
        skos:inScheme     <http://www.ebu.ch/metadata/ontologies/skos/ebu_ParentalGuidanceCodeCS> ;
        skos:broader      parentalguidance:_62.1 ;
        skos:definition   "General viewing for all ages."@en ;
        skos:prefLabel    "U"@en ;
        rdf:type          ebucore:TargetAudience .

parentalguidance:_37.2.2
        skos:example      "" ;
        skos:historyNote  "" ;
        skos:changeNote   "" ;
        skos:inScheme     <http://www.ebu.ch/metadata/ontologies/skos/ebu_ParentalGuidanceCodeCS> ;
        skos:broader      parentalguidance:_37.2 ;
        skos:prefLabel    "Seks"@nl ;
        skos:prefLabel    "Sex"@en ;
        rdf:type          ebucore:TargetAudience .

parentalguidance:_34.2.4
        skos:example      "" ;
        skos:historyNote  "" ;
        skos:changeNote   "" ;
        skos:inScheme     <http://www.ebu.ch/metadata/ontologies/skos/ebu_ParentalGuidanceCodeCS> ;
        skos:broader      parentalguidance:_34.2 ;
        skos:prefLabel    "Nudity"@en ;
        rdf:type          ebucore:TargetAudience .

parentalguidance:_8.3
        skos:example      "" ;
        skos:historyNote  "" ;
        skos:changeNote   "" ;
        skos:inScheme     <http://www.ebu.ch/metadata/ontologies/skos/ebu_ParentalGuidanceCodeCS> ;
        skos:broader      parentalguidance:_8 ;
        skos:definition   "Suitable for people 14 years of age or older. Those under 14\n         should view with an adult. No rental or purchase by those under 14 where prohibited by law.\n         Parents cautioned. May contain violence, coarse language and/or sexually suggestive\n         scenes."@en ;
        skos:prefLabel    "14A"@en ;
        rdf:type          ebucore:TargetAudience .

parentalguidance:_59  skos:changeNote  "Update" ;
        skos:scopeNote    "Region:Greece"@en ;
        skos:prefLabel    "GR-Film"@en ;
        skos:inScheme     <http://www.ebu.ch/metadata/ontologies/skos/ebu_ParentalGuidanceCodeCS> ;
        skos:example      "" ;
        skos:note         "Valid" ;
        skos:narrower     parentalguidance:_59.1 ;
        skos:historyNote  "2010-08-03" ;
        rdf:type          ebucore:TargetAudience ;
        skos:definition   "Film Board"@en .

parentalguidance:_66.1.4
        skos:example      "" ;
        skos:historyNote  "" ;
        skos:changeNote   "" ;
        skos:inScheme     <http://www.ebu.ch/metadata/ontologies/skos/ebu_ParentalGuidanceCodeCS> ;
        skos:broader      parentalguidance:_66.1 ;
        skos:definition   "No one under the age of 15 admitted "@en ;
        skos:prefLabel    "15+"@en ;
        rdf:type          ebucore:TargetAudience .

parentalguidance:_63.1.6
        skos:example      "" ;
        skos:historyNote  "" ;
        skos:changeNote   "" ;
        skos:inScheme     <http://www.ebu.ch/metadata/ontologies/skos/ebu_ParentalGuidanceCodeCS> ;
        skos:broader      parentalguidance:_63.1 ;
        skos:definition   "Suitable only for persons 18 years and older. No one under this\n         age is admitted. "@en ;
        skos:prefLabel    "18"@en ;
        rdf:type          ebucore:TargetAudience .

parentalguidance:_7.6
        skos:broader      parentalguidance:_7 ;
        skos:prefLabel    "16"@en ;
        skos:prefLabel    "16"@pt ;
        skos:definition   "Não Recomendando para Menores de 16 Anos"@pt ;
        skos:inScheme     <http://www.ebu.ch/metadata/ontologies/skos/ebu_ParentalGuidanceCodeCS> ;
        skos:example      "" ;
        skos:definition   "This film/game is recommended for persons with or over 16 years\n         of age. May contain strong language, sexual innuendo and/or mild sex with or without mild\n         nudity, strong violence, drug use."@en ;
        skos:changeNote   "" ;
        skos:historyNote  "" ;
        rdf:type          ebucore:TargetAudience .

parentalguidance:_47  skos:definition  "Entertainment Software Rating Board scheme"@en ;
        skos:narrower     parentalguidance:_47.2 ;
        rdf:type          ebucore:TargetAudience ;
        skos:scopeNote    "Region:United States"@en ;
        skos:changeNote   "Update" ;
        skos:prefLabel    "US-ESRB"@en ;
        skos:note         "Valid" ;
        skos:historyNote  "2009-07-28" ;
        skos:example      "" ;
        skos:inScheme     <http://www.ebu.ch/metadata/ontologies/skos/ebu_ParentalGuidanceCodeCS> ;
        skos:narrower     parentalguidance:_47.1 .

parentalguidance:_48.2
        skos:example      "" ;
        skos:historyNote  "" ;
        skos:changeNote   "" ;
        skos:inScheme     <http://www.ebu.ch/metadata/ontologies/skos/ebu_ParentalGuidanceCodeCS> ;
        skos:broader      parentalguidance:_48 ;
        skos:definition   "Parental guidance suggested. Theme or content may not be\n         suitable for children."@en ;
        skos:prefLabel    "Parental Guidance"@en ;
        skos:altLabel     "PG"@en ;
        rdf:type          ebucore:TargetAudience .

parentalguidance:_35  skos:narrower  parentalguidance:_35.1 ;
        skos:narrower     parentalguidance:_35.2 ;
        skos:scopeNote    "Region:Mexico"@en ;
        rdf:type          ebucore:TargetAudience ;
        skos:prefLabel    "MX-RTC"@en ;
        skos:changeNote   "Update" ;
        skos:note         "Valid" ;
        skos:definition   "Dirección General de Radio, Televisión y\n         Cinematografía"@en ;
        skos:historyNote  "2009-07-28" ;
        skos:inScheme     <http://www.ebu.ch/metadata/ontologies/skos/ebu_ParentalGuidanceCodeCS> ;
        skos:example      "" .

parentalguidance:_14.2
        skos:example      "" ;
        skos:historyNote  "" ;
        skos:changeNote   "" ;
        skos:inScheme     <http://www.ebu.ch/metadata/ontologies/skos/ebu_ParentalGuidanceCodeCS> ;
        skos:broader      parentalguidance:_14 ;
        skos:definition   "For ages 7 and older"@en ;
        skos:definition   "Infantil para mayores de 7 años"@es ;
        skos:prefLabel    "I7"@en ;
        rdf:type          ebucore:TargetAudience .

parentalguidance:_13.5
        skos:historyNote  "" ;
        skos:example      "" ;
        skos:changeNote   "" ;
        skos:definition   "Only for 18 and older"@en ;
        skos:inScheme     <http://www.ebu.ch/metadata/ontologies/skos/ebu_ParentalGuidanceCodeCS> ;
        skos:broader      parentalguidance:_13 ;
        skos:definition   "Le film ne peut être vu, acheté ou loué que par des personnes\n         de 18 ans et plus."@fr ;
        rdf:type          ebucore:TargetAudience ;
        skos:prefLabel    "18+"@fr ;
        skos:prefLabel    "18+"@en .

parentalguidance:_54.1.3
        skos:example      "" ;
        skos:historyNote  "" ;
        skos:changeNote   "" ;
        skos:inScheme     <http://www.ebu.ch/metadata/ontologies/skos/ebu_ParentalGuidanceCodeCS> ;
        skos:broader      parentalguidance:_54.1 ;
        skos:definition   "not suitable for children under 16. (category III.) "@en ;
        skos:prefLabel    "16"@en ;
        rdf:type          ebucore:TargetAudience .

parentalguidance:_37.2.4
        skos:example      "" ;
        skos:historyNote  "" ;
        skos:changeNote   "" ;
        skos:inScheme     <http://www.ebu.ch/metadata/ontologies/skos/ebu_ParentalGuidanceCodeCS> ;
        skos:broader      parentalguidance:_37.2 ;
        skos:prefLabel    "Discriminatie"@nl ;
        skos:prefLabel    "Discrimination"@en ;
        rdf:type          ebucore:TargetAudience .

parentalguidance:_25.3
        skos:example      "" ;
        skos:historyNote  "" ;
        skos:changeNote   "" ;
        skos:inScheme     <http://www.ebu.ch/metadata/ontologies/skos/ebu_ParentalGuidanceCodeCS> ;
        skos:broader      parentalguidance:_25 ;
        skos:definition   "Unsuitable for minors under 16"@en ;
        skos:definition   "Interdiction de représentation aux moins de seize\n         ans"@fr ;
        skos:prefLabel    "-16"@en ;
        rdf:type          ebucore:TargetAudience .

parentalguidance:_12  skos:note  "Valid" ;
        skos:historyNote  "2009-07-27" ;
        skos:altLabel     "www.cbsc.ca"@en ;
        rdf:type          ebucore:TargetAudience ;
        skos:narrower     parentalguidance:_12.6 ;
        skos:inScheme     <http://www.ebu.ch/metadata/ontologies/skos/ebu_ParentalGuidanceCodeCS> ;
        skos:narrower     parentalguidance:_12.5 ;
        skos:definition   "Ratings Classification for Canadian English-Language and\n         Third-Language Broadcasters"@en ;
        skos:prefLabel    "CA-CBSC-CCNR-English and third-languages"@en ;
        skos:narrower     parentalguidance:_12.4 ;
        skos:narrower     parentalguidance:_12.2 ;
        skos:narrower     parentalguidance:_12.3 ;
        skos:example      "" ;
        skos:changeNote   "Update" ;
        skos:narrower     parentalguidance:_12.1 ;
        skos:scopeNote    "Region:Canada"@en .

parentalguidance:_66.1.5
        skos:example      "" ;
        skos:historyNote  "" ;
        skos:changeNote   "" ;
        skos:inScheme     <http://www.ebu.ch/metadata/ontologies/skos/ebu_ParentalGuidanceCodeCS> ;
        skos:broader      parentalguidance:_66.1 ;
        skos:definition   "No one under the age of 18 admitted "@en ;
        skos:prefLabel    "18+"@en ;
        rdf:type          ebucore:TargetAudience .

parentalguidance:_7.7
        rdf:type          ebucore:TargetAudience ;
        skos:changeNote   "" ;
        skos:example      "" ;
        skos:definition   "Não Recomendando para Menores de 18 Anos"@pt ;
        skos:prefLabel    "18"@en ;
        skos:prefLabel    "18"@pt ;
        skos:historyNote  "" ;
        skos:broader      parentalguidance:_7 ;
        skos:inScheme     <http://www.ebu.ch/metadata/ontologies/skos/ebu_ParentalGuidanceCodeCS> ;
        skos:definition   "This film/game is forbidden for people under 18 years of age.\n         It may contain strong language, intense sex, strong nudity, strong violence, intense drug\n         use. It is also used to rate pornographic films.."@en .

parentalguidance:_9.1
        skos:example      "" ;
        skos:historyNote  "" ;
        skos:changeNote   "" ;
        skos:inScheme     <http://www.ebu.ch/metadata/ontologies/skos/ebu_ParentalGuidanceCodeCS> ;
        skos:broader      parentalguidance:_9 ;
        skos:definition   "Suitable for viewing by all ages"@en ;
        skos:prefLabel    "General"@en ;
        skos:prefLabel    "G"@en ;
        rdf:type          ebucore:TargetAudience .

parentalguidance:_63.1.5
        skos:example      "" ;
        skos:historyNote  "" ;
        skos:changeNote   "" ;
        skos:inScheme     <http://www.ebu.ch/metadata/ontologies/skos/ebu_ParentalGuidanceCodeCS> ;
        skos:broader      parentalguidance:_63.1 ;
        skos:definition   "Suitable only for persons 16 years and older. No one under this\n         age is admitted. "@en ;
        skos:prefLabel    "16"@en ;
        rdf:type          ebucore:TargetAudience .

parentalguidance:_34.2.3
        skos:example      "" ;
        skos:historyNote  "" ;
        skos:changeNote   "" ;
        skos:inScheme     <http://www.ebu.ch/metadata/ontologies/skos/ebu_ParentalGuidanceCodeCS> ;
        skos:broader      parentalguidance:_34.2 ;
        skos:prefLabel    "Angst"@nl ;
        skos:prefLabel    "Scary"@en ;
        rdf:type          ebucore:TargetAudience .

parentalguidance:_48.1
        skos:example      "" ;
        skos:historyNote  "" ;
        skos:changeNote   "" ;
        skos:inScheme     <http://www.ebu.ch/metadata/ontologies/skos/ebu_ParentalGuidanceCodeCS> ;
        skos:broader      parentalguidance:_48 ;
        skos:definition   "General audiences. All ages admitted."@en ;
        skos:prefLabel    "General"@en ;
        skos:prefLabel    "G"@en ;
        rdf:type          ebucore:TargetAudience .

parentalguidance:_37.2.3
        skos:example      "" ;
        skos:historyNote  "" ;
        skos:changeNote   "" ;
        skos:inScheme     <http://www.ebu.ch/metadata/ontologies/skos/ebu_ParentalGuidanceCodeCS> ;
        skos:broader      parentalguidance:_37.2 ;
        skos:prefLabel    "Angst"@nl ;
        skos:prefLabel    "Scary"@en ;
        rdf:type          ebucore:TargetAudience .

parentalguidance:_48  rdf:type  ebucore:TargetAudience ;
        skos:narrower     parentalguidance:_48.6 ;
        skos:narrower     parentalguidance:_48.1 ;
        skos:inScheme     <http://www.ebu.ch/metadata/ontologies/skos/ebu_ParentalGuidanceCodeCS> ;
        skos:definition   "Motion Picture Association of America movie rating\n         scheme"@en ;
        skos:prefLabel    "US-MPAA"@en ;
        skos:scopeNote    "Region:United States"@en ;
        skos:changeNote   "Update" ;
        skos:narrower     parentalguidance:_48.4 ;
        skos:narrower     parentalguidance:_48.2 ;
        skos:example      "" ;
        skos:narrower     parentalguidance:_48.5 ;
        skos:historyNote  "2009-07-27" ;
        skos:narrower     parentalguidance:_48.3 ;
        skos:note         "Valid" .

parentalguidance:_24.6
        skos:example      "" ;
        skos:historyNote  "" ;
        skos:changeNote   "" ;
        skos:narrower     parentalguidance:_24.6.1 ;
        skos:inScheme     <http://www.ebu.ch/metadata/ontologies/skos/ebu_ParentalGuidanceCodeCS> ;
        skos:broader      parentalguidance:_24 ;
        skos:definition   "For people aged 15 years and above"@en ;
        skos:prefLabel    "K-15"@en ;
        rdf:type          ebucore:TargetAudience .

parentalguidance:_8.4
        skos:example      "" ;
        skos:historyNote  "" ;
        skos:changeNote   "" ;
        skos:inScheme     <http://www.ebu.ch/metadata/ontologies/skos/ebu_ParentalGuidanceCodeCS> ;
        skos:broader      parentalguidance:_8 ;
        skos:definition   "Suitable for people 18 years of age or older. Persons under 18\n         should view with an adult. No rental or purchase by those under 18. Parents strongly\n         cautioned. Will likely contain explicit violence, frequent coarse language, sexual activity\n         and/or horror."@en ;
        skos:prefLabel    "18A"@en ;
        rdf:type          ebucore:TargetAudience .

parentalguidance:_36  skos:scopeNote  "Region:Nigeria"@en ;
        skos:narrower     parentalguidance:_36.2 ;
        skos:example      "" ;
        skos:prefLabel    "NG-NFVCB"@en ;
        skos:note         "Valid" ;
        skos:historyNote  "2009-07-28" ;
        skos:inScheme     <http://www.ebu.ch/metadata/ontologies/skos/ebu_ParentalGuidanceCodeCS> ;
        skos:definition   "Natioanl Film and Video Censor Board"@en ;
        skos:narrower     parentalguidance:_36.1 ;
        rdf:type          ebucore:TargetAudience ;
        skos:changeNote   "Update" .

parentalguidance:_24  skos:narrower  parentalguidance:_24.3 ;
        skos:inScheme     <http://www.ebu.ch/metadata/ontologies/skos/ebu_ParentalGuidanceCodeCS> ;
        skos:definition   "Valtion elokuvatarkastamo"@fi ;
        skos:narrower     parentalguidance:_24.1 ;
        skos:note         "Valid" ;
        skos:scopeNote    "Region:Finland"@fi ;
        skos:definition   "Finnish Board of Film Classification"@en ;
        skos:example      "" ;
        skos:changeNote   "Update" ;
        skos:narrower     parentalguidance:_24.4 ;
        skos:narrower     parentalguidance:_24.6 ;
        skos:narrower     parentalguidance:_24.2 ;
        skos:historyNote  "2009-07-28" ;
        skos:narrower     parentalguidance:_24.7 ;
        skos:narrower     parentalguidance:_24.5 ;
        skos:prefLabel    "FI-VET"@en ;
        rdf:type          ebucore:TargetAudience .

parentalguidance:_39.1
        skos:example      "" ;
        skos:historyNote  "" ;
        skos:changeNote   "" ;
        skos:inScheme     <http://www.ebu.ch/metadata/ontologies/skos/ebu_ParentalGuidanceCodeCS> ;
        skos:broader      parentalguidance:_39 ;
        skos:definition   "Suitable for general audiences (awarded by the Film and Video\n         Labelling Body and the Office of Film and Literature Classification)"@en ;
        skos:prefLabel    "General"@en ;
        skos:prefLabel    "G"@en ;
        rdf:type          ebucore:TargetAudience .

parentalguidance:_16.1
        skos:example      "" ;
        skos:historyNote  "" ;
        skos:changeNote   "" ;
        skos:narrower     parentalguidance:_16.1.2 ;
        skos:narrower     parentalguidance:_16.1.1 ;
        skos:inScheme     <http://www.ebu.ch/metadata/ontologies/skos/ebu_ParentalGuidanceCodeCS> ;
        skos:broader      parentalguidance:_16 ;
        skos:prefLabel    "Rating"@en ;
        rdf:type          ebucore:TargetAudience .

parentalguidance:_46.2.1
        skos:example      "" ;
        skos:historyNote  "" ;
        skos:changeNote   "" ;
        skos:inScheme     <http://www.ebu.ch/metadata/ontologies/skos/ebu_ParentalGuidanceCodeCS> ;
        skos:broader      parentalguidance:_46.2 ;
        skos:prefLabel    "Sexual content"@en ;
        skos:prefLabel    "Cinsellik içerir"@tr ;
        rdf:type          ebucore:TargetAudience .

parentalguidance:_15.4
        skos:example      "" ;
        skos:historyNote  "" ;
        skos:changeNote   "" ;
        skos:inScheme     <http://www.ebu.ch/metadata/ontologies/skos/ebu_ParentalGuidanceCodeCS> ;
        skos:broader      parentalguidance:_15 ;
        skos:definition   "Suitable for people aged 18 and over with sexually explicit\n         content"@en ;
        skos:prefLabel    "18/S"@en ;
        rdf:type          ebucore:TargetAudience .

parentalguidance:_57.1.2
        skos:example      "" ;
        skos:historyNote  "" ;
        skos:changeNote   "" ;
        skos:inScheme     <http://www.ebu.ch/metadata/ontologies/skos/ebu_ParentalGuidanceCodeCS> ;
        skos:broader      parentalguidance:_57.1 ;
        skos:definition   "Restricted to audiences aged 18 and above"@en ;
        skos:prefLabel    "Adults Only"@en ;
        rdf:type          ebucore:TargetAudience .

parentalguidance:_38.4
        skos:example      "" ;
        skos:historyNote  "" ;
        skos:changeNote   "" ;
        skos:inScheme     <http://www.ebu.ch/metadata/ontologies/skos/ebu_ParentalGuidanceCodeCS> ;
        skos:broader      parentalguidance:_38 ;
        skos:definition   "15 and older, not under 12, above 12 in presence of an\n         accompanying adult"@en ;
        skos:definition   "15 år (unge ned til 12 år i følgje med\n         føresette)"@no ;
        skos:prefLabel    "15"@en ;
        rdf:type          ebucore:TargetAudience .

parentalguidance:_46.1.4
        skos:example      "" ;
        skos:historyNote  "" ;
        skos:changeNote   "" ;
        skos:inScheme     <http://www.ebu.ch/metadata/ontologies/skos/ebu_ParentalGuidanceCodeCS> ;
        skos:broader      parentalguidance:_46.1 ;
        skos:definition   "No one under 15 years of age admitted"@en ;
        skos:definition   "18 yaş ve üzeri için uygun"@tr ;
        skos:prefLabel    "18+"@en ;
        rdf:type          ebucore:TargetAudience .

parentalguidance:_45  rdf:type  ebucore:TargetAudience ;
        skos:narrower     parentalguidance:_45.5 ;
        skos:changeNote   "Update" ;
        skos:narrower     parentalguidance:_45.2 ;
        skos:definition   "Media Development Authority"@en ;
        skos:prefLabel    "SG-MDA"@en ;
        skos:historyNote  "2009-07-28" ;
        skos:narrower     parentalguidance:_45.3 ;
        skos:scopeNote    "Region:Singapore" ;
        skos:example      "" ;
        skos:narrower     parentalguidance:_45.1 ;
        skos:narrower     parentalguidance:_45.4 ;
        skos:inScheme     <http://www.ebu.ch/metadata/ontologies/skos/ebu_ParentalGuidanceCodeCS> ;
        skos:note         "Valid" .

parentalguidance:_51.1
        skos:historyNote  "" ;
        skos:narrower     parentalguidance:_51.1.6 ;
        skos:narrower     parentalguidance:_51.1.5 ;
        rdf:type          ebucore:TargetAudience ;
        skos:example      "" ;
        skos:narrower     parentalguidance:_51.1.7 ;
        skos:changeNote   "" ;
        skos:inScheme     <http://www.ebu.ch/metadata/ontologies/skos/ebu_ParentalGuidanceCodeCS> ;
        skos:narrower     parentalguidance:_51.1.2 ;
        skos:prefLabel    "Rating"@en ;
        skos:narrower     parentalguidance:_51.1.1 ;
        skos:broader      parentalguidance:_51 ;
        skos:narrower     parentalguidance:_51.1.4 ;
        skos:narrower     parentalguidance:_51.1.3 .

parentalguidance:_4.1.5
        skos:example      "" ;
        skos:historyNote  "" ;
        skos:changeNote   "" ;
        skos:inScheme     <http://www.ebu.ch/metadata/ontologies/skos/ebu_ParentalGuidanceCodeCS> ;
        skos:broader      parentalguidance:_4.1 ;
        skos:definition   "Mature"@en ;
        skos:prefLabel    "M"@en ;
        rdf:type          ebucore:TargetAudience .

parentalguidance:_33  skos:narrower  parentalguidance:_33.4 ;
        rdf:type          ebucore:TargetAudience ;
        skos:prefLabel    "KR-KMRB"@en ;
        skos:changeNote   "" ;
        skos:narrower     parentalguidance:_33.3 ;
        skos:scopeNote    "Region:South Korea"@en ;
        skos:narrower     parentalguidance:_33.5 ;
        skos:inScheme     <http://www.ebu.ch/metadata/ontologies/skos/ebu_ParentalGuidanceCodeCS> ;
        skos:example      "" ;
        skos:historyNote  "" ;
        skos:definition   "Scheme as defined by the Korea Media Rating\n         Board"@en ;
        skos:narrower     parentalguidance:_33.2 ;
        skos:narrower     parentalguidance:_33.1 .

parentalguidance:_50.4
        skos:example      "" ;
        skos:historyNote  "" ;
        skos:changeNote   "" ;
        skos:inScheme     <http://www.ebu.ch/metadata/ontologies/skos/ebu_ParentalGuidanceCodeCS> ;
        skos:broader      parentalguidance:_50 ;
        skos:definition   "General Audience - All ages admitted"@en ;
        skos:prefLabel    "TV-G"@en ;
        rdf:type          ebucore:TargetAudience .

parentalguidance:_27.2
        skos:example      "" ;
        skos:historyNote  "" ;
        skos:changeNote   "" ;
        skos:inScheme     <http://www.ebu.ch/metadata/ontologies/skos/ebu_ParentalGuidanceCodeCS> ;
        skos:broader      parentalguidance:_27 ;
        skos:definition   "General viewing but some scenes may be unsuitable for young\n         children"@en ;
        skos:prefLabel    "PG"@en ;
        rdf:type          ebucore:TargetAudience .

parentalguidance:_21  skos:narrower  parentalguidance:_21.2 ;
        skos:changeNote   "Update Update" ;
        skos:note         "Valid" ;
        skos:scopeNote    "Region:Denmark"@en ;
        skos:example      "" ;
        skos:narrower     parentalguidance:_21.3 ;
        skos:definition   "Denmark Radio"@en ;
        skos:inScheme     <http://www.ebu.ch/metadata/ontologies/skos/ebu_ParentalGuidanceCodeCS> ;
        skos:historyNote  "2009-07-28 2009-07-28" ;
        skos:prefLabel    "DK-DR"@en ;
        skos:narrower     parentalguidance:_21.1 ;
        rdf:type          ebucore:TargetAudience .

parentalguidance:_4.2.2
        skos:example      "" ;
        skos:historyNote  "" ;
        skos:changeNote   "" ;
        skos:inScheme     <http://www.ebu.ch/metadata/ontologies/skos/ebu_ParentalGuidanceCodeCS> ;
        skos:broader      parentalguidance:_4.2 ;
        skos:definition   "Violence"@en ;
        skos:prefLabel    "V"@en ;
        rdf:type          ebucore:TargetAudience .

parentalguidance:_16.2.1
        skos:example      "" ;
        skos:historyNote  "" ;
        skos:changeNote   "" ;
        skos:inScheme     <http://www.ebu.ch/metadata/ontologies/skos/ebu_ParentalGuidanceCodeCS> ;
        skos:broader      parentalguidance:_16.2 ;
        skos:prefLabel    "Violence"@en ;
        rdf:type          ebucore:TargetAudience .

parentalguidance:_7.4
        rdf:type          ebucore:TargetAudience ;
        skos:broader      parentalguidance:_7 ;
        skos:example      "" ;
        skos:inScheme     <http://www.ebu.ch/metadata/ontologies/skos/ebu_ParentalGuidanceCodeCS> ;
        skos:definition   "This film/game is recommended for persons with or over 12 years\n         of age. May contain a little inappropriate language, sexual innuendo, or mild\n         violence."@en ;
        skos:changeNote   "" ;
        skos:historyNote  "" ;
        skos:definition   "Não Recomendando para Menores de 12 Anos"@pt ;
        skos:prefLabel    "12"@en ;
        skos:prefLabel    "12"@pt .

parentalguidance:_26.5
        skos:example      "" ;
        skos:historyNote  "" ;
        skos:changeNote   "" ;
        skos:inScheme     <http://www.ebu.ch/metadata/ontologies/skos/ebu_ParentalGuidanceCodeCS> ;
        skos:broader      parentalguidance:_26 ;
        skos:definition   "Adult, pornographic content"@en ;
        skos:definition   "Adulte - Contenu de nature pornographie"@fr ;
        skos:prefLabel    "X"@en ;
        rdf:type          ebucore:TargetAudience .

parentalguidance:_69  skos:example  "" ;
        skos:scopeNote    "Region:Italy"@en ;
        skos:definition   "Direzione generale Cinema e audiovisivo"@en ;
        skos:altLabel     "AGCOM"@en ;
        skos:inScheme     <http://www.ebu.ch/metadata/ontologies/skos/ebu_ParentalGuidanceCodeCS> ;
        skos:note         "Valid" ;
        skos:narrower     parentalguidance:_69.2 ;
        skos:prefLabel    "IT-AGCOM"@en ;
        skos:changeNote   "Created" ;
        skos:narrower     parentalguidance:_69.1 ;
        rdf:type          ebucore:TargetAudience ;
        skos:historyNote  "2024-04-10" .

parentalguidance:_57  skos:definition  "Film Board"@en ;
        skos:inScheme     <http://www.ebu.ch/metadata/ontologies/skos/ebu_ParentalGuidanceCodeCS> ;
        skos:example      "" ;
        skos:note         "Valid" ;
        skos:narrower     parentalguidance:_57.1 ;
        skos:prefLabel    "EG-Film"@en ;
        skos:scopeNote    "Region:Egypt"@en ;
        skos:historyNote  "2010-08-03" ;
        skos:changeNote   "Update" ;
        rdf:type          ebucore:TargetAudience .

parentalguidance:_8.1
        skos:example      "" ;
        skos:historyNote  "" ;
        skos:changeNote   "" ;
        skos:inScheme     <http://www.ebu.ch/metadata/ontologies/skos/ebu_ParentalGuidanceCodeCS> ;
        skos:broader      parentalguidance:_8 ;
        skos:definition   "Suitable for viewing by all ages"@en ;
        skos:prefLabel    "G - General"@en ;
        rdf:type          ebucore:TargetAudience .

parentalguidance:_60.1
        skos:narrower     parentalguidance:_60.1.4 ;
        skos:broader      parentalguidance:_60 ;
        skos:prefLabel    "Rating"@en ;
        skos:historyNote  "" ;
        skos:narrower     parentalguidance:_60.1.5 ;
        skos:inScheme     <http://www.ebu.ch/metadata/ontologies/skos/ebu_ParentalGuidanceCodeCS> ;
        rdf:type          ebucore:TargetAudience ;
        skos:changeNote   "" ;
        skos:example      "" ;
        skos:narrower     parentalguidance:_60.1.1 ;
        skos:narrower     parentalguidance:_60.1.3 ;
        skos:narrower     parentalguidance:_60.1.2 .

parentalguidance:_16.2
        skos:narrower     parentalguidance:_16.2.11 ;
        skos:narrower     parentalguidance:_16.2.7 ;
        skos:narrower     parentalguidance:_16.2.2 ;
        skos:narrower     parentalguidance:_16.2.5 ;
        skos:changeNote   "" ;
        skos:inScheme     <http://www.ebu.ch/metadata/ontologies/skos/ebu_ParentalGuidanceCodeCS> ;
        skos:narrower     parentalguidance:_16.2.6 ;
        skos:narrower     parentalguidance:_16.2.1 ;
        skos:narrower     parentalguidance:_16.2.4 ;
        skos:historyNote  "" ;
        skos:example      "" ;
        rdf:type          ebucore:TargetAudience ;
        skos:narrower     parentalguidance:_16.2.9 ;
        skos:narrower     parentalguidance:_16.2.8 ;
        skos:narrower     parentalguidance:_16.2.10 ;
        skos:broader      parentalguidance:_16 ;
        skos:narrower     parentalguidance:_16.2.3 ;
        skos:prefLabel    "Criteria"@en .

parentalguidance:_57.1.1
        skos:example      "" ;
        skos:historyNote  "" ;
        skos:changeNote   "" ;
        skos:inScheme     <http://www.ebu.ch/metadata/ontologies/skos/ebu_ParentalGuidanceCodeCS> ;
        skos:broader      parentalguidance:_57.1 ;
        skos:definition   "Everyone is admitted"@en ;
        skos:prefLabel    "General Audience"@en ;
        rdf:type          ebucore:TargetAudience .

parentalguidance:_46.2.2
        skos:example      "" ;
        skos:historyNote  "" ;
        skos:changeNote   "" ;
        skos:inScheme     <http://www.ebu.ch/metadata/ontologies/skos/ebu_ParentalGuidanceCodeCS> ;
        skos:broader      parentalguidance:_46.2 ;
        skos:prefLabel    "Violence"@en ;
        skos:prefLabel    "Şiddet ya da korku içerir"@tr ;
        rdf:type          ebucore:TargetAudience .

parentalguidance:_15.5
        skos:example      "" ;
        skos:historyNote  "" ;
        skos:changeNote   "" ;
        skos:inScheme     <http://www.ebu.ch/metadata/ontologies/skos/ebu_ParentalGuidanceCodeCS> ;
        skos:broader      parentalguidance:_15 ;
        skos:definition   "Suitable for people aged 18 and over with extreme violence\n         content"@en ;
        skos:prefLabel    "18/V"@en ;
        rdf:type          ebucore:TargetAudience .

parentalguidance:_38.3
        skos:example      "" ;
        skos:historyNote  "" ;
        skos:changeNote   "" ;
        skos:inScheme     <http://www.ebu.ch/metadata/ontologies/skos/ebu_ParentalGuidanceCodeCS> ;
        skos:broader      parentalguidance:_38 ;
        skos:definition   "11 and older or from 8 in presence of an accompanying\n         adult"@en ;
        skos:definition   "11 år (barn ned til 8 år i følgje med\n         føresette)"@no ;
        skos:prefLabel    "11"@en ;
        rdf:type          ebucore:TargetAudience .

parentalguidance:_16.2.3
        skos:example      "" ;
        skos:historyNote  "" ;
        skos:changeNote   "" ;
        skos:inScheme     <http://www.ebu.ch/metadata/ontologies/skos/ebu_ParentalGuidanceCodeCS> ;
        skos:broader      parentalguidance:_16.2 ;
        skos:prefLabel    "Sex and nudity"@en ;
        rdf:type          ebucore:TargetAudience .

parentalguidance:_50.3
        skos:example      "" ;
        skos:historyNote  "" ;
        skos:changeNote   "" ;
        skos:inScheme     <http://www.ebu.ch/metadata/ontologies/skos/ebu_ParentalGuidanceCodeCS> ;
        skos:broader      parentalguidance:_50 ;
        skos:definition   "Directed to other children above 7 due to fantasy and violent\n         content"@en ;
        skos:prefLabel    "TV-Y7-FV"@en ;
        rdf:type          ebucore:TargetAudience .

parentalguidance:_34  skos:example  "" ;
        skos:narrower     parentalguidance:_34.2 ;
        skos:historyNote  "2009-07-28" ;
        skos:definition   "National Bureau of Classification"@en ;
        skos:narrower     parentalguidance:_34.1 ;
        skos:inScheme     <http://www.ebu.ch/metadata/ontologies/skos/ebu_ParentalGuidanceCodeCS> ;
        rdf:type          ebucore:TargetAudience ;
        skos:changeNote   "Update" ;
        skos:scopeNote    "Region:Maldives"@en ;
        skos:prefLabel    "MV-NBC"@en ;
        skos:note         "Valid" .

parentalguidance:_22  skos:inScheme  <http://www.ebu.ch/metadata/ontologies/skos/ebu_ParentalGuidanceCodeCS> ;
        skos:changeNote   "Update" ;
        skos:narrower     parentalguidance:_22.1 ;
        skos:example      "" ;
        skos:historyNote  "2009-07-28" ;
        skos:narrower     parentalguidance:_22.4 ;
        skos:note         "Valid" ;
        skos:scopeNote    "Region:Spain"@en ;
        skos:narrower     parentalguidance:_22.5 ;
        rdf:type          ebucore:TargetAudience ;
        skos:narrower     parentalguidance:_22.2 ;
        skos:narrower     parentalguidance:_22.3 ;
        skos:prefLabel    "ES"@en .

parentalguidance:_10  skos:historyNote  "2009-07-27" ;
        skos:prefLabel    "CA-OFRB"@en ;
        skos:narrower     parentalguidance:_10.3 ;
        skos:narrower     parentalguidance:_10.5 ;
        skos:inScheme     <http://www.ebu.ch/metadata/ontologies/skos/ebu_ParentalGuidanceCodeCS> ;
        rdf:type          ebucore:TargetAudience ;
        skos:narrower     parentalguidance:_10.2 ;
        skos:changeNote   "Update" ;
        skos:example      "" ;
        skos:narrower     parentalguidance:_10.1 ;
        skos:scopeNote    "Region:Canada"@en ;
        skos:definition   "Ontario Film Review Board"@en ;
        skos:note         "Valid" ;
        skos:narrower     parentalguidance:_10.4 .

parentalguidance:_4.1.4
        skos:example      "" ;
        skos:historyNote  "" ;
        skos:changeNote   "" ;
        skos:inScheme     <http://www.ebu.ch/metadata/ontologies/skos/ebu_ParentalGuidanceCodeCS> ;
        skos:broader      parentalguidance:_4.1 ;
        skos:definition   "Parental Guidance"@en ;
        skos:prefLabel    "PG"@en ;
        rdf:type          ebucore:TargetAudience .

parentalguidance:_16.2.2
        skos:example      "" ;
        skos:historyNote  "" ;
        skos:changeNote   "" ;
        skos:inScheme     <http://www.ebu.ch/metadata/ontologies/skos/ebu_ParentalGuidanceCodeCS> ;
        skos:broader      parentalguidance:_16.2 ;
        skos:prefLabel    "Language"@en ;
        rdf:type          ebucore:TargetAudience .

parentalguidance:_8.2
        skos:example      "" ;
        skos:historyNote  "" ;
        skos:changeNote   "" ;
        skos:inScheme     <http://www.ebu.ch/metadata/ontologies/skos/ebu_ParentalGuidanceCodeCS> ;
        skos:broader      parentalguidance:_8 ;
        skos:definition   "Parental guidance advised. Theme or content may not be suitable\n         for all children."@en ;
        skos:prefLabel    "PG - Parental Guidance"@en ;
        rdf:type          ebucore:TargetAudience .

parentalguidance:_27.3
        skos:hiddenLabel  "12"@en ;
        skos:example      "" ;
        skos:historyNote  "" ;
        skos:changeNote   "" ;
        skos:inScheme     <http://www.ebu.ch/metadata/ontologies/skos/ebu_ParentalGuidanceCodeCS> ;
        skos:broader      parentalguidance:_27 ;
        skos:definition   "Suitable for 12 years and older. No 12 year old child may see a\n         12A film without the presence of an accompanying adult."@en ;
        skos:prefLabel    "12A/12"@en ;
        rdf:type          ebucore:TargetAudience .

parentalguidance:_58  skos:narrower  parentalguidance:_58.1 ;
        skos:changeNote   "Update" ;
        skos:note         "Valid" ;
        rdf:type          ebucore:TargetAudience ;
        skos:prefLabel    "ES-Film"@en ;
        skos:example      "" ;
        skos:historyNote  "2010-08-03" ;
        skos:definition   "Film Board"@en ;
        skos:inScheme     <http://www.ebu.ch/metadata/ontologies/skos/ebu_ParentalGuidanceCodeCS> ;
        skos:scopeNote    "Region:Estonia"@en .

parentalguidance:_7.5
        skos:definition   "Não Recomendando para Menores de 14 Anos"@pt ;
        skos:example      "" ;
        skos:broader      parentalguidance:_7 ;
        skos:definition   "This film/game is recommended for persons with or over 14 years\n         of age. May contain inappropriate language, sexual innuendo and/or mild sex with no nudity\n         or the act being explicit shown, violence, mention to drug use."@en ;
        skos:changeNote   "" ;
        skos:inScheme     <http://www.ebu.ch/metadata/ontologies/skos/ebu_ParentalGuidanceCodeCS> ;
        skos:historyNote  "" ;
        rdf:type          ebucore:TargetAudience ;
        skos:prefLabel    "14"@en ;
        skos:prefLabel    "14"@pt .

parentalguidance:_46  skos:narrower  parentalguidance:_46.2 ;
        skos:definition   "Symbol system for content rating"@en ;
        skos:inScheme     <http://www.ebu.ch/metadata/ontologies/skos/ebu_ParentalGuidanceCodeCS> ;
        skos:changeNote   "Update" ;
        rdf:type          ebucore:TargetAudience ;
        skos:example      "" ;
        skos:narrower     parentalguidance:_46.1 ;
        skos:note         "Valid" ;
        skos:scopeNote    "Region:Turkey" ;
        skos:historyNote  "2009-07-28" ;
        skos:definition   "Akıllı İşaretler Sembol Sistemi"@tr ;
        skos:prefLabel    "TR-AISS"@en .

parentalguidance:_4.2.1
        skos:example      "" ;
        skos:historyNote  "" ;
        skos:changeNote   "" ;
        skos:inScheme     <http://www.ebu.ch/metadata/ontologies/skos/ebu_ParentalGuidanceCodeCS> ;
        skos:broader      parentalguidance:_4.2 ;
        skos:definition   "Adult"@en ;
        skos:prefLabel    "A"@en ;
        rdf:type          ebucore:TargetAudience .

parentalguidance:_46.1.2
        skos:example      "" ;
        skos:historyNote  "" ;
        skos:changeNote   "" ;
        skos:inScheme     <http://www.ebu.ch/metadata/ontologies/skos/ebu_ParentalGuidanceCodeCS> ;
        skos:broader      parentalguidance:_46.1 ;
        skos:definition   "Suitable for children of at least 7 years of\n         age"@en ;
        skos:definition   "7 yaş ve üzeri için uygun"@tr ;
        skos:prefLabel    "7+"@en ;
        rdf:type          ebucore:TargetAudience .

parentalguidance:_38.2
        skos:example      "" ;
        skos:historyNote  "" ;
        skos:changeNote   "" ;
        skos:inScheme     <http://www.ebu.ch/metadata/ontologies/skos/ebu_ParentalGuidanceCodeCS> ;
        skos:broader      parentalguidance:_38 ;
        skos:definition   "7 and older or from 4 in presence of an accompanying\n         adult"@en ;
        skos:definition   "7 år (barn ned til 4 år i følgje med\n         føresette)"@no ;
        skos:prefLabel    "7"@en ;
        rdf:type          ebucore:TargetAudience .

parentalguidance:_15.2
        skos:example      "" ;
        skos:historyNote  "" ;
        skos:changeNote   "" ;
        skos:inScheme     <http://www.ebu.ch/metadata/ontologies/skos/ebu_ParentalGuidanceCodeCS> ;
        skos:broader      parentalguidance:_15 ;
        skos:definition   "Inappropriate for children under 14"@en ;
        skos:definition   "Mayor de 14 anos"@es ;
        skos:prefLabel    "14"@en ;
        rdf:type          ebucore:TargetAudience .

parentalguidance:_14.5
        skos:example      "" ;
        skos:historyNote  "" ;
        skos:changeNote   "" ;
        skos:inScheme     <http://www.ebu.ch/metadata/ontologies/skos/ebu_ParentalGuidanceCodeCS> ;
        skos:broader      parentalguidance:_14 ;
        skos:definition   "Shared responsibility - Children accompanied by an\n         adult."@en ;
        skos:definition   "Responsabilidad compartida"@es ;
        skos:prefLabel    "R"@en ;
        rdf:type          ebucore:TargetAudience .

parentalguidance:_16.2.4
        skos:example      "" ;
        skos:historyNote  "" ;
        skos:changeNote   "" ;
        skos:inScheme     <http://www.ebu.ch/metadata/ontologies/skos/ebu_ParentalGuidanceCodeCS> ;
        skos:broader      parentalguidance:_16.2 ;
        skos:prefLabel    "Sexual Violence"@en ;
        rdf:type          ebucore:TargetAudience .

parentalguidance:_67  skos:note  "Valid" ;
        skos:historyNote  "2023-07-13" ;
        skos:narrower     parentalguidance:_67.2 ;
        skos:narrower     parentalguidance:_67.1 ;
        skos:inScheme     <http://www.ebu.ch/metadata/ontologies/skos/ebu_ParentalGuidanceCodeCS> ;
        skos:definition   ""@en ;
        skos:prefLabel    "simple"@en ;
        rdf:type          ebucore:TargetAudience .

parentalguidance:_55  skos:scopeNote  "Region:Iceland"@en ;
        skos:example      "" ;
        skos:inScheme     <http://www.ebu.ch/metadata/ontologies/skos/ebu_ParentalGuidanceCodeCS> ;
        skos:narrower     parentalguidance:_55.1 ;
        skos:historyNote  "2019-06-24" ;
        skos:prefLabel    "IS-Smais"@en ;
        rdf:type          ebucore:TargetAudience ;
        skos:definition   "National Film Office"@en ;
        skos:changeNote   "Correct subterm termId 54.1.5 into 55.1.5" ;
        skos:note         "Valid" .

parentalguidance:_43  skos:narrower  parentalguidance:_43.3 ;
        skos:narrower     parentalguidance:_43.4 ;
        skos:changeNote   "Update" ;
        rdf:type          ebucore:TargetAudience ;
        skos:definition   "Scheme as defined by the Radio Televisão\n         Portugal"@en ;
        skos:narrower     parentalguidance:_43.1 ;
        skos:scopeNote    "Region:Portugal"@en ;
        skos:prefLabel    "PT-RTP"@en ;
        skos:historyNote  "2009-07-28" ;
        skos:example      "" ;
        skos:narrower     parentalguidance:_43.2 ;
        skos:inScheme     <http://www.ebu.ch/metadata/ontologies/skos/ebu_ParentalGuidanceCodeCS> ;
        skos:note         "Valid" .

parentalguidance:_4.1.3
        skos:example      "" ;
        skos:historyNote  "" ;
        skos:changeNote   "" ;
        skos:inScheme     <http://www.ebu.ch/metadata/ontologies/skos/ebu_ParentalGuidanceCodeCS> ;
        skos:broader      parentalguidance:_4.1 ;
        skos:definition   "General"@en ;
        skos:prefLabel    "G"@en ;
        rdf:type          ebucore:TargetAudience .

parentalguidance:_48.6
        skos:example      "" ;
        skos:historyNote  "" ;
        skos:changeNote   "" ;
        skos:inScheme     <http://www.ebu.ch/metadata/ontologies/skos/ebu_ParentalGuidanceCodeCS> ;
        skos:broader      parentalguidance:_48 ;
        skos:definition   "Not rated or Unrated"@en ;
        skos:altLabel     "UR"@en ;
        skos:prefLabel    "NR"@en ;
        rdf:type          ebucore:TargetAudience .

parentalguidance:_26.3
        skos:example      "" ;
        skos:historyNote  "" ;
        skos:changeNote   "" ;
        skos:inScheme     <http://www.ebu.ch/metadata/ontologies/skos/ebu_ParentalGuidanceCodeCS> ;
        skos:broader      parentalguidance:_26 ;
        skos:definition   "Not Recommended for children under 16"@en ;
        skos:definition   "Pas pour les moins de seize ans"@fr ;
        skos:prefLabel    "-16"@en ;
        rdf:type          ebucore:TargetAudience .

parentalguidance:_50.2
        skos:example      "" ;
        skos:historyNote  "" ;
        skos:changeNote   "" ;
        skos:inScheme     <http://www.ebu.ch/metadata/ontologies/skos/ebu_ParentalGuidanceCodeCS> ;
        skos:broader      parentalguidance:_50 ;
        skos:definition   "Directed to other children above 7"@en ;
        skos:prefLabel    "TV-Y7"@en ;
        rdf:type          ebucore:TargetAudience .

parentalguidance:_31  skos:definition  "Computer Entertainment Rating Organization"@en ;
        skos:changeNote   "Update" ;
        skos:scopeNote    "Region:Japan"@en ;
        skos:narrower     parentalguidance:_31.1 ;
        rdf:type          ebucore:TargetAudience ;
        skos:example      "" ;
        skos:narrower     parentalguidance:_31.2 ;
        skos:inScheme     <http://www.ebu.ch/metadata/ontologies/skos/ebu_ParentalGuidanceCodeCS> ;
        skos:historyNote  "2009-07-27" ;
        skos:prefLabel    "JA-CERO"@en ;
        skos:definition   "Tokutei Hieiri Katsudō Hōjin Konpyūta Entāteinmento Rētingu\n         Kikō - 特定非営利活動法人 コンピュータエンターテインメントレーティング機構"@ja ;
        skos:note         "Valid" .

parentalguidance:_6.5
        skos:example      "" ;
        skos:historyNote  "" ;
        skos:changeNote   "" ;
        skos:inScheme     <http://www.ebu.ch/metadata/ontologies/skos/ebu_ParentalGuidanceCodeCS> ;
        skos:broader      parentalguidance:_6 ;
        skos:definition   "When the film is naturalistically erotic or shows violence in\n         an ostentatious manner"@en ;
        skos:prefLabel    "X"@en ;
        skos:prefLabel    "D"@po ;
        rdf:type          ebucore:TargetAudience .

parentalguidance:_55.1.6
        skos:example      "" ;
        skos:historyNote  "" ;
        skos:changeNote   "" ;
        skos:inScheme     <http://www.ebu.ch/metadata/ontologies/skos/ebu_ParentalGuidanceCodeCS> ;
        skos:broader      parentalguidance:_55.1 ;
        skos:definition   "Passed only for 18 and older "@en ;
        skos:prefLabel    "18"@en ;
        rdf:type          ebucore:TargetAudience .

parentalguidance:_37.1.1
        skos:example      "" ;
        skos:historyNote  "" ;
        skos:changeNote   "" ;
        skos:inScheme     <http://www.ebu.ch/metadata/ontologies/skos/ebu_ParentalGuidanceCodeCS> ;
        skos:broader      parentalguidance:_37.1 ;
        skos:definition   "Alle leeftijden"@nl ;
        skos:definition   "Suitable for all ages"@en ;
        skos:prefLabel    "AL"@en ;
        rdf:type          ebucore:TargetAudience .

parentalguidance:_7.2
        skos:definition   "Livre para Todos os Públicos"@pt ;
        skos:changeNote   "" ;
        skos:inScheme     <http://www.ebu.ch/metadata/ontologies/skos/ebu_ParentalGuidanceCodeCS> ;
        skos:prefLabel    "L"@en ;
        skos:prefLabel    "L"@pt ;
        skos:historyNote  "" ;
        rdf:type          ebucore:TargetAudience ;
        skos:definition   "This rating means that the film/game can be watched/played by\n         anyone and doesn't have any inappropriate content"@en ;
        skos:broader      parentalguidance:_7 ;
        skos:example      "" .

parentalguidance:_38.1
        skos:prefLabel    "All"@en ;
        skos:definition   "For all"@en ;
        skos:prefLabel    "Alle"@no ;
        skos:changeNote   "" ;
        skos:inScheme     <http://www.ebu.ch/metadata/ontologies/skos/ebu_ParentalGuidanceCodeCS> ;
        skos:broader      parentalguidance:_38 ;
        skos:historyNote  "" ;
        rdf:type          ebucore:TargetAudience ;
        skos:definition   "Tillaten for alle"@no ;
        skos:example      "" .

parentalguidance:_61.1
        skos:example      "" ;
        skos:narrower     parentalguidance:_61.1.4 ;
        skos:changeNote   "" ;
        skos:narrower     parentalguidance:_61.1.1 ;
        skos:narrower     parentalguidance:_61.1.3 ;
        skos:narrower     parentalguidance:_61.1.6 ;
        skos:historyNote  "" ;
        rdf:type          ebucore:TargetAudience ;
        skos:narrower     parentalguidance:_61.1.5 ;
        skos:broader      parentalguidance:_61 ;
        skos:prefLabel    "Rating"@en ;
        skos:inScheme     <http://www.ebu.ch/metadata/ontologies/skos/ebu_ParentalGuidanceCodeCS> ;
        skos:narrower     parentalguidance:_61.1.2 .

parentalguidance:_15.3
        skos:example      "" ;
        skos:historyNote  "" ;
        skos:changeNote   "" ;
        skos:inScheme     <http://www.ebu.ch/metadata/ontologies/skos/ebu_ParentalGuidanceCodeCS> ;
        skos:broader      parentalguidance:_15 ;
        skos:definition   "Suitable for people aged 18 and over"@en ;
        skos:definition   "Mayor de 18 anos"@es ;
        skos:prefLabel    "18"@en ;
        rdf:type          ebucore:TargetAudience .

parentalguidance:_14.6
        skos:example      "" ;
        skos:historyNote  "" ;
        skos:changeNote   "" ;
        skos:inScheme     <http://www.ebu.ch/metadata/ontologies/skos/ebu_ParentalGuidanceCodeCS> ;
        skos:broader      parentalguidance:_14 ;
        skos:definition   "For adult audiences only (ages 18 or older). Shows that contain\n         explicit language, sex scenes, explicit situations"@en ;
        skos:definition   "Adulto"@es ;
        skos:prefLabel    "A"@en ;
        rdf:type          ebucore:TargetAudience .

parentalguidance:_46.1.3
        skos:example      "" ;
        skos:historyNote  "" ;
        skos:changeNote   "" ;
        skos:inScheme     <http://www.ebu.ch/metadata/ontologies/skos/ebu_ParentalGuidanceCodeCS> ;
        skos:broader      parentalguidance:_46.1 ;
        skos:definition   "Suitable for children of at least 11 years of\n         age"@en ;
        skos:definition   "13 yaş ve üzeri için uygun"@tr ;
        skos:prefLabel    "13+"@en ;
        rdf:type          ebucore:TargetAudience .

parentalguidance:_16.2.5
        skos:example      "" ;
        skos:historyNote  "" ;
        skos:changeNote   "" ;
        skos:inScheme     <http://www.ebu.ch/metadata/ontologies/skos/ebu_ParentalGuidanceCodeCS> ;
        skos:broader      parentalguidance:_16.2 ;
        skos:prefLabel    "Drugs and alcohol"@en ;
        rdf:type          ebucore:TargetAudience .

parentalguidance:_56  skos:changeNote  "Update" ;
        skos:narrower     parentalguidance:_56.1 ;
        skos:example      "" ;
        skos:historyNote  "2010-08-03" ;
        skos:prefLabel    "IN-CFBC"@en ;
        skos:note         "Valid" ;
        skos:scopeNote    "Region:India"@en ;
        skos:definition   "Film Board"@en ;
        skos:inScheme     <http://www.ebu.ch/metadata/ontologies/skos/ebu_ParentalGuidanceCodeCS> ;
        rdf:type          ebucore:TargetAudience .

parentalguidance:_44  skos:narrower  parentalguidance:_44.2 ;
        skos:inScheme     <http://www.ebu.ch/metadata/ontologies/skos/ebu_ParentalGuidanceCodeCS> ;
        skos:changeNote   "Update" ;
        skos:narrower     parentalguidance:_44.3 ;
        skos:definition   "Swedish National Board of Film Censors"@en ;
        skos:note         "Valid" ;
        skos:definition   "Statens biografbyrå"@sv ;
        skos:example      "" ;
        skos:narrower     parentalguidance:_44.1 ;
        skos:scopeNote    "Region:Sweden" ;
        skos:narrower     parentalguidance:_44.5 ;
        skos:historyNote  "2009-07-28" ;
        skos:prefLabel    "SE-SB"@en ;
        skos:narrower     parentalguidance:_44.4 ;
        rdf:type          ebucore:TargetAudience .

parentalguidance:_48.5
        skos:hiddenLabel  "adult"@en ;
        skos:example      "" ;
        skos:historyNote  "" ;
        skos:changeNote   "" ;
        skos:inScheme     <http://www.ebu.ch/metadata/ontologies/skos/ebu_ParentalGuidanceCodeCS> ;
        skos:broader      parentalguidance:_48 ;
        skos:definition   "Not one 17 and under admitted."@en ;
        skos:prefLabel    "NC-17"@en ;
        rdf:type          ebucore:TargetAudience .

parentalguidance:_32  skos:narrower  parentalguidance:_32.1 ;
        skos:scopeNote    "Region:South Korea"@en ;
        skos:definition   "Scheme as defined by the Korea Broadcasting\n         Station"@en ;
        skos:narrower     parentalguidance:_32.4 ;
        skos:inScheme     <http://www.ebu.ch/metadata/ontologies/skos/ebu_ParentalGuidanceCodeCS> ;
        skos:prefLabel    "KR-KBS"@en ;
        skos:narrower     parentalguidance:_32.5 ;
        skos:changeNote   "" ;
        rdf:type          ebucore:TargetAudience ;
        skos:narrower     parentalguidance:_32.3 ;
        skos:narrower     parentalguidance:_32.2 ;
        skos:example      "" ;
        skos:historyNote  "" .

parentalguidance:_50.1
        skos:example      "" ;
        skos:historyNote  "" ;
        skos:changeNote   "" ;
        skos:inScheme     <http://www.ebu.ch/metadata/ontologies/skos/ebu_ParentalGuidanceCodeCS> ;
        skos:broader      parentalguidance:_50 ;
        skos:definition   "All children"@en ;
        skos:prefLabel    "TV-Y"@en ;
        rdf:type          ebucore:TargetAudience .

parentalguidance:_20  skos:definition  "Medieradet for barn och unga - Media Advice for Children and\n         Youths (Denmark)"@en ;
        skos:narrower     parentalguidance:_20.4 ;
        skos:definition   "Scheme as defined by the Danish Media Council for Children and\n         Young People"@en ;
        skos:historyNote  "2009-07-28" ;
        skos:scopeNote    "Region:Denmark"@en ;
        skos:note         "Valid" ;
        skos:prefLabel    "DK-MBU"@en ;
        skos:narrower     parentalguidance:_20.2 ;
        skos:narrower     parentalguidance:_20.3 ;
        skos:narrower     parentalguidance:_20.1 ;
        rdf:type          ebucore:TargetAudience ;
        skos:example      "" ;
        skos:inScheme     <http://www.ebu.ch/metadata/ontologies/skos/ebu_ParentalGuidanceCodeCS> ;
        skos:changeNote   "Update" .

parentalguidance:_27.1
        skos:example      "" ;
        skos:historyNote  "" ;
        skos:changeNote   "" ;
        skos:inScheme     <http://www.ebu.ch/metadata/ontologies/skos/ebu_ParentalGuidanceCodeCS> ;
        skos:broader      parentalguidance:_27 ;
        skos:definition   "Suitable for all"@en ;
        skos:prefLabel    "U"@en ;
        rdf:type          ebucore:TargetAudience .

parentalguidance:_55.1.5
        skos:example      "" ;
        skos:historyNote  "" ;
        skos:changeNote   "" ;
        skos:inScheme     <http://www.ebu.ch/metadata/ontologies/skos/ebu_ParentalGuidanceCodeCS> ;
        skos:broader      parentalguidance:_55.1 ;
        skos:definition   "Passed only for 16 and older "@en ;
        skos:prefLabel    "16"@en ;
        rdf:type          ebucore:TargetAudience .

parentalguidance:_26.4
        skos:example      "" ;
        skos:historyNote  "" ;
        skos:changeNote   "" ;
        skos:inScheme     <http://www.ebu.ch/metadata/ontologies/skos/ebu_ParentalGuidanceCodeCS> ;
        skos:broader      parentalguidance:_26 ;
        skos:definition   "Unsuitable for minors under 18, may apply to works with\n         non-simulated sexual acts or extreme violence, but do not apply to X rating due to the\n         nature of the theme being treated or the way it has been filmed"@en ;
        skos:definition   "Pas pour les moins de dix-huit ans, prévoit que cette\n         restriction peut concerner les œuvres qui comportent « des scènes de sexe non simulées ou\n         de très grande violence mais qui, par la manière dont elles sont filmées et la nature du\n         thème traité ne justifient pas » d’un classement X"@fr ;
        skos:prefLabel    "-18"@en ;
        rdf:type          ebucore:TargetAudience .

parentalguidance:_66.1.1
        skos:example      "" ;
        skos:historyNote  "" ;
        skos:changeNote   "" ;
        skos:inScheme     <http://www.ebu.ch/metadata/ontologies/skos/ebu_ParentalGuidanceCodeCS> ;
        skos:broader      parentalguidance:_66.1 ;
        skos:definition   "Suitable for general audiences "@en ;
        skos:prefLabel    "G"@en ;
        rdf:type          ebucore:TargetAudience .

parentalguidance:_7.3
        skos:prefLabel    "10"@en ;
        skos:prefLabel    "10"@pt ;
        skos:broader      parentalguidance:_7 ;
        skos:definition   "This film/game is recommended for persons with or over 10 years\n         of age. May contain a little inappropriate language, sexual innuendo, or mild\n         violence."@en ;
        skos:changeNote   "" ;
        skos:historyNote  "" ;
        skos:definition   "Não Recomendando para Menores de 10 Anos"@pt ;
        skos:inScheme     <http://www.ebu.ch/metadata/ontologies/skos/ebu_ParentalGuidanceCodeCS> ;
        rdf:type          ebucore:TargetAudience ;
        skos:example      "" .

parentalguidance:_37.1.2
        skos:example      "" ;
        skos:historyNote  "" ;
        skos:changeNote   "" ;
        skos:inScheme     <http://www.ebu.ch/metadata/ontologies/skos/ebu_ParentalGuidanceCodeCS> ;
        skos:broader      parentalguidance:_37.1 ;
        skos:definition   "Let op met kinderen tot 6 jaar"@nl ;
        skos:definition   "Not recommended for viewers younger than 6\n         years"@en ;
        skos:prefLabel    "6"@en ;
        rdf:type          ebucore:TargetAudience .

parentalguidance:_68  skos:altLabel  "MBACT"@en ;
        skos:definition   "Direzione generale Cinema e audiovisivo"@en ;
        skos:narrower     parentalguidance:_68.1 ;
        skos:inScheme     <http://www.ebu.ch/metadata/ontologies/skos/ebu_ParentalGuidanceCodeCS> ;
        skos:note         "Valid" ;
        rdf:type          ebucore:TargetAudience ;
        skos:historyNote  "2024-04-10" ;
        skos:example      "" ;
        skos:scopeNote    "Region:Italy"@en ;
        skos:narrower     parentalguidance:_68.2 ;
        skos:changeNote   "Created" ;
        skos:prefLabel    "IT-MBACT"@en .

parentalguidance:_4.1.2
        skos:example      "" ;
        skos:historyNote  "" ;
        skos:changeNote   "" ;
        skos:inScheme     <http://www.ebu.ch/metadata/ontologies/skos/ebu_ParentalGuidanceCodeCS> ;
        skos:broader      parentalguidance:_4.1 ;
        skos:definition   "Children"@en ;
        skos:prefLabel    "C"@en ;
        rdf:type          ebucore:TargetAudience .

parentalguidance:_11.4
        skos:example      "" ;
        skos:definition   "Le film ne peut être vu, acheté ou loué que par des personnes\n         de 18 ans et plus."@fr ;
        skos:historyNote  "" ;
        skos:prefLabel    "18+"@fr ;
        skos:prefLabel    "18+"@en ;
        rdf:type          ebucore:TargetAudience ;
        skos:broader      parentalguidance:_11 ;
        skos:changeNote   "" ;
        skos:definition   "Only for 18 and older"@en ;
        skos:inScheme     <http://www.ebu.ch/metadata/ontologies/skos/ebu_ParentalGuidanceCodeCS> .

parentalguidance:_47.2.6
        skos:example      "" ;
        skos:historyNote  "" ;
        skos:changeNote   "" ;
        skos:inScheme     <http://www.ebu.ch/metadata/ontologies/skos/ebu_ParentalGuidanceCodeCS> ;
        skos:broader      parentalguidance:_47.2 ;
        skos:definition   "Depictions or dialogue involving slapstick or suggestive\n         humour" ;
        skos:prefLabel    "Comic Mischief"@en ;
        rdf:type          ebucore:TargetAudience .

parentalguidance:_58.1
        skos:changeNote   "" ;
        skos:narrower     parentalguidance:_58.1.8 ;
        skos:broader      parentalguidance:_58 ;
        skos:narrower     parentalguidance:_58.1.7 ;
        rdf:type          ebucore:TargetAudience ;
        skos:prefLabel    "Rating"@en ;
        skos:historyNote  "" ;
        skos:narrower     parentalguidance:_58.1.5 ;
        skos:narrower     parentalguidance:_58.1.4 ;
        skos:narrower     parentalguidance:_58.1.3 ;
        skos:narrower     parentalguidance:_58.1.2 ;
        skos:inScheme     <http://www.ebu.ch/metadata/ontologies/skos/ebu_ParentalGuidanceCodeCS> ;
        skos:narrower     parentalguidance:_58.1.6 ;
        skos:narrower     parentalguidance:_58.1.1 ;
        skos:example      "" .

parentalguidance:_35.1
        skos:example      "" ;
        skos:historyNote  "" ;
        skos:broader      parentalguidance:_35 ;
        skos:narrower     parentalguidance:_35.1.5 ;
        skos:changeNote   "" ;
        skos:inScheme     <http://www.ebu.ch/metadata/ontologies/skos/ebu_ParentalGuidanceCodeCS> ;
        skos:narrower     parentalguidance:_35.1.6 ;
        skos:prefLabel    "Rating"@en ;
        skos:narrower     parentalguidance:_35.1.3 ;
        skos:narrower     parentalguidance:_35.1.1 ;
        skos:narrower     parentalguidance:_35.1.4 ;
        skos:narrower     parentalguidance:_35.1.2 ;
        rdf:type          ebucore:TargetAudience .

parentalguidance:_2  skos:narrower  parentalguidance:_2.5 ;
        skos:prefLabel    "AT-BMUKK"@en ;
        skos:definition   "Bundesministerium für Unterricht, Kunst und\n         Kultur"@de ;
        skos:narrower     parentalguidance:_2.4 ;
        skos:narrower     parentalguidance:_2.1 ;
        skos:note         "Valid" ;
        skos:narrower     parentalguidance:_2.6 ;
        skos:scopeNote    "Region:Austria"@en ;
        skos:historyNote  "2009-07-27" ;
        skos:definition   "Federal Ministry for Education, the Arts and\n         Culture"@en ;
        rdf:type          ebucore:TargetAudience ;
        skos:inScheme     <http://www.ebu.ch/metadata/ontologies/skos/ebu_ParentalGuidanceCodeCS> ;
        skos:narrower     parentalguidance:_2.3 ;
        skos:example      "" ;
        skos:changeNote   "Update" ;
        skos:narrower     parentalguidance:_2.2 .

parentalguidance:_16.2.10
        skos:example      "" ;
        skos:historyNote  "" ;
        skos:changeNote   "" ;
        skos:inScheme     <http://www.ebu.ch/metadata/ontologies/skos/ebu_ParentalGuidanceCodeCS> ;
        skos:broader      parentalguidance:_16.2 ;
        skos:prefLabel    "Exorcism, psychic or occultic practice and depiction of the\n         supernatural"@en ;
        rdf:type          ebucore:TargetAudience .

parentalguidance:_12.1
        skos:example      "" ;
        skos:historyNote  "" ;
        skos:changeNote   "" ;
        skos:inScheme     <http://www.ebu.ch/metadata/ontologies/skos/ebu_ParentalGuidanceCodeCS> ;
        skos:broader      parentalguidance:_12 ;
        skos:definition   "Children"@en ;
        skos:prefLabel    "C"@en ;
        rdf:type          ebucore:TargetAudience .

parentalguidance:_34.1.1
        skos:example      "" ;
        rdf:type          ebucore:TargetAudience ;
        skos:changeNote   "" ;
        skos:prefLabel    "G"@en ;
        skos:definition   "Suitable for all ages"@en ;
        skos:historyNote  "" ;
        skos:broader      parentalguidance:_34.1 ;
        skos:prefLabel    "General"@en ;
        skos:inScheme     <http://www.ebu.ch/metadata/ontologies/skos/ebu_ParentalGuidanceCodeCS> ;
        skos:prefLabel    "Green"@en .

parentalguidance:_69.1.4
        skos:example      "" ;
        skos:historyNote  "" ;
        skos:changeNote   "" ;
        skos:inScheme     <http://www.ebu.ch/metadata/ontologies/skos/ebu_ParentalGuidanceCodeCS> ;
        skos:broader      parentalguidance:_69.1 ;
        skos:definition   "Films prohibited to minors under 18 years"@en ;
        skos:definition   "Film Vietati ai minori di 18 anni"@it ;
        skos:prefLabel    "VM18"@en ;
        rdf:type          ebucore:TargetAudience .

parentalguidance:_22.5
        skos:example      "" ;
        skos:historyNote  "" ;
        skos:changeNote   "" ;
        skos:inScheme     <http://www.ebu.ch/metadata/ontologies/skos/ebu_ParentalGuidanceCodeCS> ;
        skos:broader      parentalguidance:_22 ;
        skos:definition   "For 18 and older"@en ;
        skos:prefLabel    "18"@en ;
        rdf:type          ebucore:TargetAudience .

parentalguidance:_45.5
        skos:example      "" ;
        skos:historyNote  "" ;
        skos:changeNote   "" ;
        skos:inScheme     <http://www.ebu.ch/metadata/ontologies/skos/ebu_ParentalGuidanceCodeCS> ;
        skos:broader      parentalguidance:_45 ;
        skos:definition   "Restricted to persons 21 years and above"@en ;
        skos:prefLabel    "R21"@en ;
        rdf:type          ebucore:TargetAudience .

parentalguidance:_46.2
        skos:changeNote   "" ;
        skos:narrower     parentalguidance:_46.2.3 ;
        rdf:type          ebucore:TargetAudience ;
        skos:historyNote  "" ;
        skos:narrower     parentalguidance:_46.2.1 ;
        skos:inScheme     <http://www.ebu.ch/metadata/ontologies/skos/ebu_ParentalGuidanceCodeCS> ;
        skos:example      "" ;
        skos:broader      parentalguidance:_46 ;
        skos:prefLabel    "Criteria"@en ;
        skos:narrower     parentalguidance:_46.2.2 .

parentalguidance:_4.2.6
        skos:example      "" ;
        skos:historyNote  "" ;
        skos:changeNote   "" ;
        skos:inScheme     <http://www.ebu.ch/metadata/ontologies/skos/ebu_ParentalGuidanceCodeCS> ;
        skos:broader      parentalguidance:_4.2 ;
        skos:definition   "Drugs"@en ;
        skos:prefLabel    "D"@en ;
        rdf:type          ebucore:TargetAudience .

parentalguidance:_23.2
        skos:narrower     parentalguidance:_23.2.7 ;
        skos:example      "" ;
        skos:narrower     parentalguidance:_23.2.6 ;
        skos:inScheme     <http://www.ebu.ch/metadata/ontologies/skos/ebu_ParentalGuidanceCodeCS> ;
        rdf:type          ebucore:TargetAudience ;
        skos:narrower     parentalguidance:_23.2.4 ;
        skos:narrower     parentalguidance:_23.2.2 ;
        skos:historyNote  "" ;
        skos:narrower     parentalguidance:_23.2.5 ;
        skos:prefLabel    "Criteria"@en ;
        skos:changeNote   "" ;
        skos:narrower     parentalguidance:_23.2.1 ;
        skos:broader      parentalguidance:_23 ;
        skos:narrower     parentalguidance:_23.2.3 .

parentalguidance:_36.1.2
        skos:example      "" ;
        skos:historyNote  "" ;
        skos:changeNote   "" ;
        skos:inScheme     <http://www.ebu.ch/metadata/ontologies/skos/ebu_ParentalGuidanceCodeCS> ;
        skos:broader      parentalguidance:_36.1 ;
        skos:definition   "the themes or content of the film may not, in the opinion of\n         the board, be suitable for all children."@en ;
        skos:prefLabel    "Parental Guidance"@en ;
        skos:altLabel     "PG"@en ;
        rdf:type          ebucore:TargetAudience .

parentalguidance:_1.2
        rdf:type          ebucore:TargetAudience ;
        skos:example      "" ;
        skos:inScheme     <http://www.ebu.ch/metadata/ontologies/skos/ebu_ParentalGuidanceCodeCS> ;
        skos:historyNote  "" ;
        skos:broader      parentalguidance:_1 ;
        skos:definition   "Apto para mayores de 13 años"@es ;
        skos:definition   "Not under 13"@en ;
        skos:changeNote   "" ;
        skos:prefLabel    "13"@es ;
        skos:prefLabel    "13"@en .

parentalguidance:_46.1.1
        skos:example      "" ;
        skos:historyNote  "" ;
        skos:changeNote   "" ;
        skos:inScheme     <http://www.ebu.ch/metadata/ontologies/skos/ebu_ParentalGuidanceCodeCS> ;
        skos:broader      parentalguidance:_46.1 ;
        skos:definition   "Suitable for all ages"@en ;
        skos:definition   "Genel izleyici kitlesi"@tr ;
        skos:prefLabel    "All"@en ;
        rdf:type          ebucore:TargetAudience .

parentalguidance:_47.2.5
        skos:example      "" ;
        skos:historyNote  "" ;
        skos:changeNote   "" ;
        skos:inScheme     <http://www.ebu.ch/metadata/ontologies/skos/ebu_ParentalGuidanceCodeCS> ;
        skos:broader      parentalguidance:_47.2 ;
        skos:definition   "Violent actions involving cartoon-like situations and characters.\n         May include violence where a character is unharmed after the action has been\n         inflicted" ;
        skos:prefLabel    "Cartoon Violence"@en ;
        rdf:type          ebucore:TargetAudience .

parentalguidance:_3  skos:narrower  parentalguidance:_3.4 ;
        skos:narrower     parentalguidance:_3.3 ;
        skos:scopeNote    "Region:Australia"@en ;
        skos:example      "" ;
        skos:changeNote   "Update" ;
        skos:note         "Valid" ;
        skos:narrower     parentalguidance:_3.6 ;
        skos:prefLabel    "AU-OFLC"@en ;
        skos:historyNote  "2009-07-27" ;
        skos:inScheme     <http://www.ebu.ch/metadata/ontologies/skos/ebu_ParentalGuidanceCodeCS> ;
        skos:narrower     parentalguidance:_3.5 ;
        skos:narrower     parentalguidance:_3.2 ;
        skos:narrower     parentalguidance:_3.1 ;
        skos:definition   "Office of Film and Literature Classification"@en ;
        rdf:type          ebucore:TargetAudience .

parentalguidance:_12.2
        skos:example      "" ;
        skos:historyNote  "" ;
        skos:changeNote   "" ;
        skos:inScheme     <http://www.ebu.ch/metadata/ontologies/skos/ebu_ParentalGuidanceCodeCS> ;
        skos:broader      parentalguidance:_12 ;
        skos:definition   "Children over 8 years"@en ;
        skos:prefLabel    "C8"@en ;
        rdf:type          ebucore:TargetAudience .

parentalguidance:_4.2.5
        skos:example      "" ;
        skos:historyNote  "" ;
        skos:changeNote   "" ;
        skos:inScheme     <http://www.ebu.ch/metadata/ontologies/skos/ebu_ParentalGuidanceCodeCS> ;
        skos:broader      parentalguidance:_4.2 ;
        skos:definition   "Horror"@en ;
        skos:prefLabel    "H"@en ;
        rdf:type          ebucore:TargetAudience .

parentalguidance:_69.1.3
        skos:example      "" ;
        skos:historyNote  "" ;
        skos:changeNote   "" ;
        skos:inScheme     <http://www.ebu.ch/metadata/ontologies/skos/ebu_ParentalGuidanceCodeCS> ;
        skos:broader      parentalguidance:_69.1 ;
        skos:definition   "Films prohibited to minors under 14 years"@en ;
        skos:definition   "Film Vietati ai minori di 14 anni"@it ;
        skos:prefLabel    "VM14"@en ;
        rdf:type          ebucore:TargetAudience .

parentalguidance:_4  skos:note  "Valid" ;
        skos:narrower     parentalguidance:_4.1 ;
        skos:historyNote  "2009-07-27" ;
        skos:scopeNote    "Region:Australia"@en ;
        rdf:type          ebucore:TargetAudience ;
        skos:changeNote   "Update" ;
        skos:example      "" ;
        skos:inScheme     <http://www.ebu.ch/metadata/ontologies/skos/ebu_ParentalGuidanceCodeCS> ;
        skos:prefLabel    "AU-ACMA"@en ;
        skos:narrower     parentalguidance:_4.2 ;
        skos:altLabel     "www.acma.gov.au"@en ;
        skos:definition   "Australian Communications and Media Authority"@en .

parentalguidance:_45.4
        skos:example      "" ;
        skos:historyNote  "" ;
        skos:changeNote   "" ;
        skos:inScheme     <http://www.ebu.ch/metadata/ontologies/skos/ebu_ParentalGuidanceCodeCS> ;
        skos:broader      parentalguidance:_45 ;
        skos:definition   "Mature 18 for persons 18 years and above"@en ;
        skos:prefLabel    "M18"@en ;
        rdf:type          ebucore:TargetAudience .

parentalguidance:_46.1
        skos:prefLabel    "Rating"@en ;
        skos:narrower     parentalguidance:_46.1.3 ;
        skos:narrower     parentalguidance:_46.1.1 ;
        skos:historyNote  "" ;
        skos:broader      parentalguidance:_46 ;
        skos:example      "" ;
        skos:changeNote   "" ;
        skos:narrower     parentalguidance:_46.1.4 ;
        skos:narrower     parentalguidance:_46.1.2 ;
        rdf:type          ebucore:TargetAudience ;
        skos:inScheme     <http://www.ebu.ch/metadata/ontologies/skos/ebu_ParentalGuidanceCodeCS> .

parentalguidance:_47.2.4
        skos:example      "" ;
        skos:historyNote  "" ;
        skos:changeNote   "" ;
        skos:inScheme     <http://www.ebu.ch/metadata/ontologies/skos/ebu_ParentalGuidanceCodeCS> ;
        skos:broader      parentalguidance:_47.2 ;
        skos:definition   "Depictions of blood or the mutilation of body\n         parts" ;
        skos:prefLabel    "Blood and Gore"@en ;
        rdf:type          ebucore:TargetAudience .

parentalguidance:_1.3
        skos:prefLabel    "16"@es ;
        skos:prefLabel    "16"@en ;
        skos:broader      parentalguidance:_1 ;
        skos:example      "" ;
        skos:historyNote  "" ;
        skos:definition   "Not under 16"@en ;
        skos:changeNote   "" ;
        skos:definition   "Apto para mayores de 16 años"@es ;
        skos:inScheme     <http://www.ebu.ch/metadata/ontologies/skos/ebu_ParentalGuidanceCodeCS> ;
        rdf:type          ebucore:TargetAudience .

parentalguidance:_36.1.3
        skos:example      "" ;
        skos:historyNote  "" ;
        skos:changeNote   "" ;
        skos:inScheme     <http://www.ebu.ch/metadata/ontologies/skos/ebu_ParentalGuidanceCodeCS> ;
        skos:broader      parentalguidance:_36.1 ;
        skos:definition   "Suitable for viewing by persons 12 years of age or older but\n         not for children under 12 years of age unless accompanied by an adult"@en ;
        skos:prefLabel    "12A/12"@en ;
        rdf:type          ebucore:TargetAudience .

parentalguidance:_10.5
        skos:example      "" ;
        skos:historyNote  "" ;
        skos:changeNote   "" ;
        skos:inScheme     <http://www.ebu.ch/metadata/ontologies/skos/ebu_ParentalGuidanceCodeCS> ;
        skos:broader      parentalguidance:_10 ;
        skos:definition   "Restricted to 18 years and older. No rental or purchase by\n         those under 18. Contents not suitable for minors. Contains frequent sexual activity,\n         brutality/graphic violence, intense horror, and/or other disturbing content. "@en ;
        skos:prefLabel    "Restricted"@en ;
        skos:prefLabel    "R"@en ;
        rdf:type          ebucore:TargetAudience .

parentalguidance:_47.1.7
        skos:example      "" ;
        skos:historyNote  "" ;
        skos:changeNote   "" ;
        skos:inScheme     <http://www.ebu.ch/metadata/ontologies/skos/ebu_ParentalGuidanceCodeCS> ;
        skos:broader      parentalguidance:_47.1 ;
        skos:definition   "Titles listed as RP (Rating Pending) have been submitted to the\n         ESRB and are awaiting final rating. (This symbol appears only in advertising prior to a\n         game's release)" ;
        skos:prefLabel    "RP"@en ;
        rdf:type          ebucore:TargetAudience .

parentalguidance:_33.5
        skos:example      "" ;
        skos:historyNote  "" ;
        skos:changeNote   "" ;
        skos:inScheme     <http://www.ebu.ch/metadata/ontologies/skos/ebu_ParentalGuidanceCodeCS> ;
        skos:broader      parentalguidance:_33 ;
        skos:definition   "Suitable for those aged 18 and over"@en ;
        skos:prefLabel    "Restricted"@en ;
        rdf:type          ebucore:TargetAudience .

parentalguidance:_34.2
        skos:narrower     parentalguidance:_34.2.6 ;
        skos:historyNote  "" ;
        skos:narrower     parentalguidance:_34.2.3 ;
        skos:narrower     parentalguidance:_34.2.1 ;
        skos:example      "" ;
        skos:narrower     parentalguidance:_34.2.4 ;
        skos:prefLabel    "Criteria"@en ;
        skos:narrower     parentalguidance:_34.2.2 ;
        skos:narrower     parentalguidance:_34.2.7 ;
        skos:broader      parentalguidance:_34 ;
        skos:inScheme     <http://www.ebu.ch/metadata/ontologies/skos/ebu_ParentalGuidanceCodeCS> ;
        rdf:type          ebucore:TargetAudience ;
        skos:changeNote   "" ;
        skos:narrower     parentalguidance:_34.2.5 .

parentalguidance:_11.2
        skos:historyNote  "" ;
        rdf:type          ebucore:TargetAudience ;
        skos:definition   "For 13 and older in presence of an adult"@en ;
        skos:prefLabel    "13+"@fr ;
        skos:prefLabel    "13+"@en ;
        skos:inScheme     <http://www.ebu.ch/metadata/ontologies/skos/ebu_ParentalGuidanceCodeCS> ;
        skos:definition   "Le film ne peut être vu, acheté ou loué que par des personnes\n         de 13 ans et plus. Les enfants de moins de 13 ans peuvent y avoir accès s’ils sont\n         accompagnés par un adulte."@fr ;
        skos:example      "" ;
        skos:changeNote   "" ;
        skos:broader      parentalguidance:_11 .

parentalguidance:_4.2.4
        skos:example      "" ;
        skos:historyNote  "" ;
        skos:changeNote   "" ;
        skos:inScheme     <http://www.ebu.ch/metadata/ontologies/skos/ebu_ParentalGuidanceCodeCS> ;
        skos:broader      parentalguidance:_4.2 ;
        skos:definition   "Sex"@en ;
        skos:prefLabel    "S"@en ;
        rdf:type          ebucore:TargetAudience .

parentalguidance:_45.3
        skos:example      "" ;
        skos:historyNote  "" ;
        skos:changeNote   "" ;
        skos:inScheme     <http://www.ebu.ch/metadata/ontologies/skos/ebu_ParentalGuidanceCodeCS> ;
        skos:broader      parentalguidance:_45 ;
        skos:definition   "No children below 16 years old"@en ;
        skos:prefLabel    "NC16"@en ;
        rdf:type          ebucore:TargetAudience .

parentalguidance:_4.1.7
        skos:example      "" ;
        skos:historyNote  "" ;
        skos:changeNote   "" ;
        skos:inScheme     <http://www.ebu.ch/metadata/ontologies/skos/ebu_ParentalGuidanceCodeCS> ;
        skos:broader      parentalguidance:_4.1 ;
        skos:definition   "15 or older with violent content"@en ;
        skos:prefLabel    "AV15+"@en ;
        rdf:type          ebucore:TargetAudience .

parentalguidance:_19  skos:narrower  parentalguidance:_19.3 ;
        skos:historyNote  "2009-07-28" ;
        skos:note         "Valid" ;
        skos:narrower     parentalguidance:_19.2 ;
        skos:changeNote   "Update" ;
        skos:narrower     parentalguidance:_19.4 ;
        skos:inScheme     <http://www.ebu.ch/metadata/ontologies/skos/ebu_ParentalGuidanceCodeCS> ;
        skos:definition   "Voluntary Self-Control of the Film Business'\n         rating"@en ;
        skos:altLabel     "www.fsk.de"@en ;
        rdf:type          ebucore:TargetAudience ;
        skos:scopeNote    "Region:Germany"@en ;
        skos:narrower     parentalguidance:_19.1 ;
        skos:narrower     parentalguidance:_19.5 ;
        skos:example      "" ;
        skos:definition   "Freiwillige Selbstkontrolle der Filmwirtschaft\n         Altersfreigabe"@en ;
        skos:prefLabel    "DE-FSK"@en .

parentalguidance:_47.2.3
        skos:example      "" ;
        skos:historyNote  "" ;
        skos:changeNote   "" ;
        skos:inScheme     <http://www.ebu.ch/metadata/ontologies/skos/ebu_ParentalGuidanceCodeCS> ;
        skos:broader      parentalguidance:_47.2 ;
        skos:definition   "Depictions of blood" ;
        skos:prefLabel    "Blood"@en ;
        rdf:type          ebucore:TargetAudience .

parentalguidance:_22.3
        skos:example      "" ;
        skos:historyNote  "" ;
        skos:changeNote   "" ;
        skos:inScheme     <http://www.ebu.ch/metadata/ontologies/skos/ebu_ParentalGuidanceCodeCS> ;
        skos:broader      parentalguidance:_22 ;
        skos:definition   "For 7 and older"@en ;
        skos:prefLabel    "7"@en ;
        rdf:type          ebucore:TargetAudience .

parentalguidance:_60.1.4
        skos:example      "" ;
        skos:historyNote  "" ;
        skos:changeNote   "" ;
        skos:inScheme     <http://www.ebu.ch/metadata/ontologies/skos/ebu_ParentalGuidanceCodeCS> ;
        skos:broader      parentalguidance:_60.1 ;
        skos:definition   "Remaja): Teen (13–15 years and over) "@en ;
        skos:prefLabel    "R"@en ;
        rdf:type          ebucore:TargetAudience .

parentalguidance:_57.1.3
        skos:example      "" ;
        skos:historyNote  "" ;
        skos:changeNote   "" ;
        skos:inScheme     <http://www.ebu.ch/metadata/ontologies/skos/ebu_ParentalGuidanceCodeCS> ;
        skos:broader      parentalguidance:_57.1 ;
        skos:definition   ""@en ;
        skos:prefLabel    "Exempt from classification"@en ;
        rdf:type          ebucore:TargetAudience .

parentalguidance:_47.1.6
        skos:example      "" ;
        skos:historyNote  "" ;
        skos:changeNote   "" ;
        skos:inScheme     <http://www.ebu.ch/metadata/ontologies/skos/ebu_ParentalGuidanceCodeCS> ;
        skos:broader      parentalguidance:_47.1 ;
        skos:definition   "Titles rated AO (Adults Only) have content that should only be\n         played by persons 18 years and older. Titles in this category may include prolonged scenes\n         of intense violence and/or graphic sexual content and nudity" ;
        skos:prefLabel    "AO"@en ;
        rdf:type          ebucore:TargetAudience .

parentalguidance:_33.4
        skos:example      "" ;
        skos:historyNote  "" ;
        skos:changeNote   "" ;
        skos:inScheme     <http://www.ebu.ch/metadata/ontologies/skos/ebu_ParentalGuidanceCodeCS> ;
        skos:broader      parentalguidance:_33 ;
        skos:definition   "Unsuitable for those aged under 18"@en ;
        skos:prefLabel    "Teenager Restricted"@en ;
        rdf:type          ebucore:TargetAudience .

parentalguidance:_59.1
        rdf:type          ebucore:TargetAudience ;
        skos:prefLabel    "Rating"@en ;
        skos:changeNote   "" ;
        skos:narrower     parentalguidance:_59.1.4 ;
        skos:narrower     parentalguidance:_59.1.3 ;
        skos:broader      parentalguidance:_59 ;
        skos:historyNote  "" ;
        skos:narrower     parentalguidance:_59.1.2 ;
        skos:example      "" ;
        skos:inScheme     <http://www.ebu.ch/metadata/ontologies/skos/ebu_ParentalGuidanceCodeCS> ;
        skos:narrower     parentalguidance:_59.1.1 .

parentalguidance:_34.1
        skos:broader      parentalguidance:_34 ;
        skos:example      "" ;
        skos:inScheme     <http://www.ebu.ch/metadata/ontologies/skos/ebu_ParentalGuidanceCodeCS> ;
        skos:prefLabel    "Rating"@en ;
        skos:narrower     parentalguidance:_34.1.4 ;
        skos:narrower     parentalguidance:_34.1.2 ;
        rdf:type          ebucore:TargetAudience ;
        skos:narrower     parentalguidance:_34.1.5 ;
        skos:changeNote   "" ;
        skos:narrower     parentalguidance:_34.1.3 ;
        skos:historyNote  "" ;
        skos:narrower     parentalguidance:_34.1.1 .

parentalguidance:_11.3
        skos:changeNote   "" ;
        skos:definition   "Only for 16 and older"@en ;
        skos:inScheme     <http://www.ebu.ch/metadata/ontologies/skos/ebu_ParentalGuidanceCodeCS> ;
        skos:prefLabel    "16+"@fr ;
        skos:definition   "Le film ne peut être vu, acheté ou loué que par des personnes\n         de 16 ans et plus."@fr ;
        skos:prefLabel    "16+"@en ;
        skos:historyNote  "" ;
        rdf:type          ebucore:TargetAudience ;
        skos:broader      parentalguidance:_11 ;
        skos:example      "" .

parentalguidance:_1  skos:example  "" ;
        skos:narrower     parentalguidance:_1.6 ;
        skos:prefLabel    "AR-INCAA"@en ;
        skos:changeNote   "Update" ;
        rdf:type          ebucore:TargetAudience ;
        skos:narrower     parentalguidance:_1.5 ;
        skos:definition   "Institute of Film and Audiovisual Arts through the Advisory\n         Commission of Cinematographic Exhibition"@en ;
        skos:note         "Valid" ;
        skos:narrower     parentalguidance:_1.3 ;
        skos:historyNote  "2009-07-27" ;
        skos:inScheme     <http://www.ebu.ch/metadata/ontologies/skos/ebu_ParentalGuidanceCodeCS> ;
        skos:definition   "Instituto de Cine y Artes Audiovisuales, Comisión Asesora de\n         Exhibición Cinematográfica"@es ;
        skos:narrower     parentalguidance:_1.4 ;
        skos:narrower     parentalguidance:_1.2 ;
        skos:scopeNote    "Region:Argentina"@en ;
        skos:narrower     parentalguidance:_1.1 .

parentalguidance:_4.1.6
        skos:example      "" ;
        skos:historyNote  "" ;
        skos:changeNote   "" ;
        skos:inScheme     <http://www.ebu.ch/metadata/ontologies/skos/ebu_ParentalGuidanceCodeCS> ;
        skos:broader      parentalguidance:_4.1 ;
        skos:definition   "15 or older"@en ;
        skos:prefLabel    "MA15+"@en ;
        rdf:type          ebucore:TargetAudience .

parentalguidance:_4.2.3
        skos:example      "" ;
        skos:historyNote  "" ;
        skos:changeNote   "" ;
        skos:inScheme     <http://www.ebu.ch/metadata/ontologies/skos/ebu_ParentalGuidanceCodeCS> ;
        skos:broader      parentalguidance:_4.2 ;
        skos:definition   "Language"@en ;
        skos:prefLabel    "L"@en ;
        rdf:type          ebucore:TargetAudience .

parentalguidance:_24.3.1
        skos:example      "" ;
        skos:historyNote  "" ;
        skos:changeNote   "" ;
        skos:inScheme     <http://www.ebu.ch/metadata/ontologies/skos/ebu_ParentalGuidanceCodeCS> ;
        skos:broader      parentalguidance:_24.3 ;
        skos:definition   "Parental Guidance option - children 2 years of age under the K\n         limits may access the show in presence of an accompanying adult"@en ;
        skos:prefLabel    "PG"@en ;
        rdf:type          ebucore:TargetAudience .

parentalguidance:_22.4
        skos:example      "" ;
        skos:historyNote  "" ;
        skos:changeNote   "" ;
        skos:inScheme     <http://www.ebu.ch/metadata/ontologies/skos/ebu_ParentalGuidanceCodeCS> ;
        skos:broader      parentalguidance:_22 ;
        skos:definition   "For 13 and older"@en ;
        skos:prefLabel    "13"@en ;
        rdf:type          ebucore:TargetAudience .

parentalguidance:_44.5
        skos:example      "" ;
        skos:historyNote  "" ;
        skos:changeNote   "" ;
        skos:inScheme     <http://www.ebu.ch/metadata/ontologies/skos/ebu_ParentalGuidanceCodeCS> ;
        skos:broader      parentalguidance:_44 ;
        skos:definition   "No one under 18 years of age admitted"@en ;
        skos:prefLabel    "18"@en ;
        rdf:type          ebucore:TargetAudience .

parentalguidance:_47.2.2
        skos:example      "" ;
        skos:historyNote  "" ;
        skos:changeNote   "" ;
        skos:inScheme     <http://www.ebu.ch/metadata/ontologies/skos/ebu_ParentalGuidanceCodeCS> ;
        skos:broader      parentalguidance:_47.2 ;
        skos:definition   "Discoloured and/or unrealistic depictions of\n         blood" ;
        skos:prefLabel    "Animated Blood"@en ;
        rdf:type          ebucore:TargetAudience .

parentalguidance:_45.2
        skos:example      "" ;
        skos:historyNote  "" ;
        skos:changeNote   "" ;
        skos:inScheme     <http://www.ebu.ch/metadata/ontologies/skos/ebu_ParentalGuidanceCodeCS> ;
        skos:broader      parentalguidance:_45 ;
        skos:definition   "Parental supervision is advised"@en ;
        skos:prefLabel    "Parental Guidance"@en ;
        skos:altLabel     "PG"@en ;
        rdf:type          ebucore:TargetAudience .

parentalguidance:_47.1.5
        skos:example      "" ;
        skos:historyNote  "" ;
        skos:changeNote   "" ;
        skos:inScheme     <http://www.ebu.ch/metadata/ontologies/skos/ebu_ParentalGuidanceCodeCS> ;
        skos:broader      parentalguidance:_47.1 ;
        skos:definition   "Titles rated M (Mature) have content that may be suitable for\n         persons ages 17 and older. Titles in this category may contain intense violence, blood and\n         gore, sexual content and/or strong language" ;
        skos:prefLabel    "M"@en ;
        rdf:type          ebucore:TargetAudience .

parentalguidance:_36.1.1
        skos:example      "" ;
        skos:historyNote  "" ;
        skos:changeNote   "" ;
        skos:inScheme     <http://www.ebu.ch/metadata/ontologies/skos/ebu_ParentalGuidanceCodeCS> ;
        skos:broader      parentalguidance:_36.1 ;
        skos:definition   "The content is considered by the board to be suitable for\n         viewing by persons of all ages."@en ;
        skos:prefLabel    "General"@en ;
        skos:prefLabel    "G"@en ;
        rdf:type          ebucore:TargetAudience .

parentalguidance:_60.1.5
        skos:example      "" ;
        skos:historyNote  "" ;
        skos:changeNote   "" ;
        skos:inScheme     <http://www.ebu.ch/metadata/ontologies/skos/ebu_ParentalGuidanceCodeCS> ;
        skos:broader      parentalguidance:_60.1 ;
        skos:definition   "(Dewasa): Mature (17 years and over) "@en ;
        skos:prefLabel    "D"@en ;
        rdf:type          ebucore:TargetAudience .

parentalguidance:_23.1
        skos:narrower     parentalguidance:_23.1.3 ;
        skos:narrower     parentalguidance:_23.1.5 ;
        skos:broader      parentalguidance:_23 ;
        skos:historyNote  "" ;
        skos:prefLabel    "Rating"@en ;
        rdf:type          ebucore:TargetAudience ;
        skos:narrower     parentalguidance:_23.1.1 ;
        skos:narrower     parentalguidance:_23.1.4 ;
        skos:narrower     parentalguidance:_23.1.2 ;
        skos:changeNote   "" ;
        skos:inScheme     <http://www.ebu.ch/metadata/ontologies/skos/ebu_ParentalGuidanceCodeCS> ;
        skos:example      "" .

parentalguidance:_1.1
        rdf:type          ebucore:TargetAudience ;
        skos:example      "" ;
        skos:historyNote  "" ;
        skos:prefLabel    "ATP"@es ;
        skos:prefLabel    "ATP"@en ;
        skos:broader      parentalguidance:_1 ;
        skos:changeNote   "" ;
        skos:definition   "For all ages"@en ;
        skos:inScheme     <http://www.ebu.ch/metadata/ontologies/skos/ebu_ParentalGuidanceCodeCS> ;
        skos:definition   "Apta (para) Todo Público"@es .

parentalguidance:_13.2
        skos:definition   "General – Not Suitable for Young Children"@en ;
        skos:prefLabel    "8+"@fr ;
        skos:prefLabel    "8+"@en ;
        skos:example      "" ;
        rdf:type          ebucore:TargetAudience ;
        skos:inScheme     <http://www.ebu.ch/metadata/ontologies/skos/ebu_ParentalGuidanceCodeCS> ;
        skos:broader      parentalguidance:_13 ;
        skos:changeNote   "" ;
        skos:historyNote  "" ;
        skos:definition   "General, non approprié pour jeunes enfants de moins e 8\n         ans"@fr .

<http://www.ebu.ch/metadata/ontologies/skos/ebu_ParentalGuidanceCodeCS.rdf>
        dct:rights       "http://creativecommons.org/licenses/by-nc-sa/3.0/" ;
        dct:publisher    "EBU" ;
        dct:creator      "Jean-Pierre Evain, EBU, metadata@ebu.ch" ;
        dct:description  "An RDF vocabulary defining television, radio and associated\n         pafental guidance codes"@en ;
        dct:contributor  "EBU metadata community experts" ;
        dct:title        "EBU SKOS Classification Scheme for Parental Guidance"@en ;
        rdf:type         owl:Ontology .

parentalguidance:_36.2
        rdf:type          ebucore:TargetAudience ;
        skos:narrower     parentalguidance:_36.2.5 ;
        skos:changeNote   "" ;
        skos:historyNote  "" ;
        skos:narrower     parentalguidance:_36.2.4 ;
        skos:inScheme     <http://www.ebu.ch/metadata/ontologies/skos/ebu_ParentalGuidanceCodeCS> ;
        skos:narrower     parentalguidance:_36.2.3 ;
        skos:narrower     parentalguidance:_36.2.2 ;
        skos:narrower     parentalguidance:_36.2.1 ;
        skos:broader      parentalguidance:_36 ;
        skos:prefLabel    "Criteria"@en ;
        skos:example      "" .

parentalguidance:_12.5
        skos:example      "" ;
        skos:historyNote  "" ;
        skos:changeNote   "" ;
        skos:inScheme     <http://www.ebu.ch/metadata/ontologies/skos/ebu_ParentalGuidanceCodeCS> ;
        skos:broader      parentalguidance:_12 ;
        skos:definition   "Over 14 Years"@en ;
        skos:prefLabel    "14+"@en ;
        rdf:type          ebucore:TargetAudience .

parentalguidance:_68.1
        skos:narrower     parentalguidance:_68.1.3 ;
        skos:inScheme     <http://www.ebu.ch/metadata/ontologies/skos/ebu_ParentalGuidanceCodeCS> ;
        skos:narrower     parentalguidance:_68.1.1 ;
        skos:historyNote  "" ;
        rdf:type          ebucore:TargetAudience ;
        skos:example      "" ;
        skos:broader      parentalguidance:_4 ;
        skos:prefLabel    "Rating"@en ;
        skos:definition   ""@en ;
        skos:changeNote   "" ;
        skos:narrower     parentalguidance:_68.1.4 ;
        skos:narrower     parentalguidance:_68.1.2 .

parentalguidance:_37.2.5
        skos:example      "" ;
        skos:historyNote  "" ;
        skos:changeNote   "" ;
        skos:inScheme     <http://www.ebu.ch/metadata/ontologies/skos/ebu_ParentalGuidanceCodeCS> ;
        skos:broader      parentalguidance:_37.2 ;
        skos:prefLabel    "Drugs- en alcoholmisbruik"@nl ;
        skos:prefLabel    "Drugs & alcohol"@en ;
        rdf:type          ebucore:TargetAudience .

parentalguidance:_59.1.3
        skos:example      "" ;
        skos:historyNote  "" ;
        skos:changeNote   "" ;
        skos:inScheme     <http://www.ebu.ch/metadata/ontologies/skos/ebu_ParentalGuidanceCodeCS> ;
        skos:broader      parentalguidance:_59.1 ;
        skos:definition   "Suitable film for adults over the age of 17. The film may\n         contain violence, drug abuse, and mild pornographic scenes. An ID card certifying the age\n         is required in all Greek cinemas and DVD rental shops in order to get a cinema ticket or\n         rent a DVD of a \"K-17\" rated film. This category is legally restricted. "@en ;
        skos:prefLabel    "K-17"@en ;
        rdf:type          ebucore:TargetAudience .

_:b2    rdf:rest   _:b3 ;
        rdf:first  parentalguidance:_25 .

parentalguidance:_9.6
        skos:example      "" ;
        skos:historyNote  "" ;
        skos:changeNote   "" ;
        skos:inScheme     <http://www.ebu.ch/metadata/ontologies/skos/ebu_ParentalGuidanceCodeCS> ;
        skos:broader      parentalguidance:_9 ;
        skos:definition   "Admittance restricted to persons 18 years of age or older.\n         Content not suitable for minors. Contains predominantly sexually explicit activity. "@en ;
        skos:prefLabel    "Adult"@en ;
        skos:prefLabel    "A"@en ;
        rdf:type          ebucore:TargetAudience .

parentalguidance:_34.2.2
        skos:example      "" ;
        skos:historyNote  "" ;
        skos:changeNote   "" ;
        skos:inScheme     <http://www.ebu.ch/metadata/ontologies/skos/ebu_ParentalGuidanceCodeCS> ;
        skos:broader      parentalguidance:_34.2 ;
        skos:prefLabel    "Sexual acts"@en ;
        rdf:type          ebucore:TargetAudience .

parentalguidance:_24.3
        skos:example      "" ;
        skos:historyNote  "" ;
        skos:changeNote   "" ;
        skos:narrower     parentalguidance:_24.3.1 ;
        skos:inScheme     <http://www.ebu.ch/metadata/ontologies/skos/ebu_ParentalGuidanceCodeCS> ;
        skos:broader      parentalguidance:_24 ;
        skos:definition   "For people aged 7 years and above"@en ;
        skos:prefLabel    "K-7"@en ;
        rdf:type          ebucore:TargetAudience .

parentalguidance:_34.1.5
        skos:example      "" ;
        skos:historyNote  "" ;
        skos:changeNote   "" ;
        skos:inScheme     <http://www.ebu.ch/metadata/ontologies/skos/ebu_ParentalGuidanceCodeCS> ;
        skos:broader      parentalguidance:_34.1 ;
        skos:definition   "For Professional Use Only"@en ;
        skos:prefLabel    "PU"@en ;
        rdf:type          ebucore:TargetAudience .

parentalguidance:_62.1.3
        skos:example      "" ;
        skos:historyNote  "" ;
        skos:changeNote   "" ;
        skos:inScheme     <http://www.ebu.ch/metadata/ontologies/skos/ebu_ParentalGuidanceCodeCS> ;
        skos:broader      parentalguidance:_62.1 ;
        skos:definition   "For aged 18 and above only"@en ;
        skos:prefLabel    "18"@en ;
        rdf:type          ebucore:TargetAudience .

parentalguidance:_29  skos:prefLabel  "IE-RTE"@en ;
        skos:narrower     parentalguidance:_29.4 ;
        skos:narrower     parentalguidance:_29.1 ;
        skos:narrower     parentalguidance:_29.5 ;
        skos:inScheme     <http://www.ebu.ch/metadata/ontologies/skos/ebu_ParentalGuidanceCodeCS> ;
        skos:narrower     parentalguidance:_29.3 ;
        skos:example      "" ;
        rdf:type          ebucore:TargetAudience ;
        skos:scopeNote    "Region:Ireland"@en ;
        skos:changeNote   "Update" ;
        skos:definition   "Irish Film Classification Office"@en ;
        skos:historyNote  "2009-07-28" ;
        skos:narrower     parentalguidance:_29.2 ;
        skos:note         "Valid" .

parentalguidance:_17  skos:note  "Valid" ;
        skos:scopeNote    "Region:Columbia"@en ;
        skos:historyNote  "2009-07-27" ;
        skos:prefLabel    "CO"@en ;
        skos:narrower     parentalguidance:_17.5 ;
        skos:narrower     parentalguidance:_17.2 ;
        skos:inScheme     <http://www.ebu.ch/metadata/ontologies/skos/ebu_ParentalGuidanceCodeCS> ;
        skos:narrower     parentalguidance:_17.6 ;
        skos:narrower     parentalguidance:_17.4 ;
        skos:narrower     parentalguidance:_17.1 ;
        skos:example      "" ;
        skos:definition   "Movie ratings as defined by the Colombian Ministry of\n         Culture"@en ;
        rdf:type          ebucore:TargetAudience ;
        skos:changeNote   "Update" ;
        skos:narrower     parentalguidance:_17.3 .

parentalguidance:_47.2.9
        skos:example      "" ;
        skos:historyNote  "" ;
        skos:changeNote   "" ;
        skos:inScheme     <http://www.ebu.ch/metadata/ontologies/skos/ebu_ParentalGuidanceCodeCS> ;
        skos:broader      parentalguidance:_47.2 ;
        skos:definition   "Content of product provides user with specific skills development\n         or reinforcement learning within an entertainment setting. Skill development is an integral\n         part of product" ;
        skos:prefLabel    "Edutainment"@en ;
        rdf:type          ebucore:TargetAudience .

parentalguidance:_13.3
        skos:inScheme     <http://www.ebu.ch/metadata/ontologies/skos/ebu_ParentalGuidanceCodeCS> ;
        skos:historyNote  "" ;
        skos:broader      parentalguidance:_13 ;
        skos:prefLabel    "13+"@fr ;
        skos:prefLabel    "13+"@en ;
        skos:example      "" ;
        rdf:type          ebucore:TargetAudience ;
        skos:definition   "Le film ne peut être vu, acheté ou loué que par des personnes\n         de 13 ans et plus. Les enfants de moins de 13 ans peuvent y avoir accès s’ils sont\n         accompagnés par un adulte."@fr ;
        skos:definition   "For 13 and older in presence of an adult"@en ;
        skos:changeNote   "" .

parentalguidance:_12.6
        skos:example      "" ;
        skos:historyNote  "" ;
        skos:changeNote   "" ;
        skos:inScheme     <http://www.ebu.ch/metadata/ontologies/skos/ebu_ParentalGuidanceCodeCS> ;
        skos:broader      parentalguidance:_12 ;
        skos:definition   "Over 18 Years"@en ;
        skos:prefLabel    "18+"@en ;
        rdf:type          ebucore:TargetAudience .

parentalguidance:_36.1
        skos:historyNote  "" ;
        skos:narrower     parentalguidance:_36.1.3 ;
        skos:narrower     parentalguidance:_36.1.6 ;
        skos:narrower     parentalguidance:_36.1.2 ;
        skos:narrower     parentalguidance:_36.1.1 ;
        skos:inScheme     <http://www.ebu.ch/metadata/ontologies/skos/ebu_ParentalGuidanceCodeCS> ;
        skos:example      "" ;
        skos:prefLabel    "Rating"@en ;
        rdf:type          ebucore:TargetAudience ;
        skos:changeNote   "" ;
        skos:narrower     parentalguidance:_36.1.5 ;
        skos:narrower     parentalguidance:_36.1.4 ;
        skos:broader      parentalguidance:_36 .

parentalguidance:_37.2.6
        skos:example      "" ;
        skos:historyNote  "" ;
        skos:changeNote   "" ;
        skos:inScheme     <http://www.ebu.ch/metadata/ontologies/skos/ebu_ParentalGuidanceCodeCS> ;
        skos:broader      parentalguidance:_37.2 ;
        skos:prefLabel    "Grof taalgebruik"@nl ;
        skos:prefLabel    "Bad language"@en ;
        rdf:type          ebucore:TargetAudience .

parentalguidance:_57.1
        skos:example      "" ;
        skos:prefLabel    "Rating"@en ;
        rdf:type          ebucore:TargetAudience ;
        skos:inScheme     <http://www.ebu.ch/metadata/ontologies/skos/ebu_ParentalGuidanceCodeCS> ;
        skos:broader      parentalguidance:_57 ;
        skos:changeNote   "" ;
        skos:narrower     parentalguidance:_57.1.1 ;
        skos:narrower     parentalguidance:_57.1.2 ;
        skos:narrower     parentalguidance:_57.1.3 ;
        skos:historyNote  "" .

parentalguidance:_59.1.4
        skos:example      "" ;
        skos:historyNote  "" ;
        skos:changeNote   "" ;
        skos:inScheme     <http://www.ebu.ch/metadata/ontologies/skos/ebu_ParentalGuidanceCodeCS> ;
        skos:broader      parentalguidance:_59.1 ;
        skos:definition   "Exempt from classification "@en ;
        skos:prefLabel    "E"@en ;
        rdf:type          ebucore:TargetAudience .

parentalguidance:_54.1.1
        skos:example      "" ;
        skos:historyNote  "" ;
        skos:changeNote   "" ;
        skos:inScheme     <http://www.ebu.ch/metadata/ontologies/skos/ebu_ParentalGuidanceCodeCS> ;
        skos:broader      parentalguidance:_54.1 ;
        skos:definition   "suitable for all (category I.) "@en ;
        skos:prefLabel    "KN"@en ;
        rdf:type          ebucore:TargetAudience .

parentalguidance:_24.4
        skos:example      "" ;
        skos:historyNote  "" ;
        skos:changeNote   "" ;
        skos:narrower     parentalguidance:_24.4.1 ;
        skos:inScheme     <http://www.ebu.ch/metadata/ontologies/skos/ebu_ParentalGuidanceCodeCS> ;
        skos:broader      parentalguidance:_24 ;
        skos:definition   "For people aged 11 years and above"@en ;
        skos:prefLabel    "K-11"@en ;
        rdf:type          ebucore:TargetAudience .

parentalguidance:_25.1
        skos:example      "" ;
        skos:historyNote  "" ;
        skos:changeNote   "" ;
        skos:inScheme     <http://www.ebu.ch/metadata/ontologies/skos/ebu_ParentalGuidanceCodeCS> ;
        skos:broader      parentalguidance:_25 ;
        skos:definition   "For all audiences"@en ;
        skos:prefLabel    "For all audiences"@en ;
        skos:prefLabel    "Tout public"@fr ;
        rdf:type          ebucore:TargetAudience .

parentalguidance:_34.2.1
        skos:example      "" ;
        skos:historyNote  "" ;
        skos:changeNote   "" ;
        skos:inScheme     <http://www.ebu.ch/metadata/ontologies/skos/ebu_ParentalGuidanceCodeCS> ;
        skos:broader      parentalguidance:_34.2 ;
        skos:prefLabel    "Violence"@en ;
        rdf:type          ebucore:TargetAudience .

parentalguidance:_47.2
        skos:narrower     parentalguidance:_47.2.17 ;
        skos:narrower     parentalguidance:_47.2.7 ;
        skos:narrower     parentalguidance:_47.2.21 ;
        skos:narrower     parentalguidance:_47.2.16 ;
        skos:narrower     parentalguidance:_47.2.10 ;
        skos:narrower     parentalguidance:_47.2.6 ;
        skos:narrower     parentalguidance:_47.2.3 ;
        skos:broader      parentalguidance:_47 ;
        skos:narrower     parentalguidance:_47.2.1 ;
        skos:narrower     parentalguidance:_47.2.20 ;
        skos:narrower     parentalguidance:_47.2.2 ;
        skos:narrower     parentalguidance:_47.2.31 ;
        skos:narrower     parentalguidance:_47.2.5 ;
        rdf:type          ebucore:TargetAudience ;
        skos:historyNote  "" ;
        skos:narrower     parentalguidance:_47.2.30 ;
        skos:changeNote   "" ;
        skos:inScheme     <http://www.ebu.ch/metadata/ontologies/skos/ebu_ParentalGuidanceCodeCS> ;
        skos:narrower     parentalguidance:_47.2.26 ;
        skos:example      "" ;
        skos:narrower     parentalguidance:_47.2.32 ;
        skos:narrower     parentalguidance:_47.2.15 ;
        skos:narrower     parentalguidance:_47.2.25 ;
        skos:narrower     parentalguidance:_47.2.14 ;
        skos:narrower     parentalguidance:_47.2.24 ;
        skos:narrower     parentalguidance:_47.2.13 ;
        skos:narrower     parentalguidance:_47.2.19 ;
        skos:narrower     parentalguidance:_47.2.9 ;
        skos:narrower     parentalguidance:_47.2.23 ;
        skos:narrower     parentalguidance:_47.2.29 ;
        skos:narrower     parentalguidance:_47.2.27 ;
        skos:narrower     parentalguidance:_47.2.12 ;
        skos:narrower     parentalguidance:_47.2.18 ;
        skos:narrower     parentalguidance:_47.2.8 ;
        skos:narrower     parentalguidance:_47.2.28 ;
        skos:narrower     parentalguidance:_47.2.22 ;
        skos:prefLabel    "Criteria"@en ;
        skos:narrower     parentalguidance:_47.2.11 ;
        skos:narrower     parentalguidance:_47.2.4 .

parentalguidance:_34.1.4
        skos:example      "" ;
        skos:historyNote  "" ;
        skos:changeNote   "" ;
        skos:inScheme     <http://www.ebu.ch/metadata/ontologies/skos/ebu_ParentalGuidanceCodeCS> ;
        skos:broader      parentalguidance:_34.1 ;
        skos:definition   "Suitable for ages 18 and above"@en ;
        skos:prefLabel    "18+"@en ;
        rdf:type          ebucore:TargetAudience .

parentalguidance:_62.1.2
        skos:example      "" ;
        skos:historyNote  "" ;
        skos:changeNote   "" ;
        skos:inScheme     <http://www.ebu.ch/metadata/ontologies/skos/ebu_ParentalGuidanceCodeCS> ;
        skos:broader      parentalguidance:_62.1 ;
        skos:definition   "Parental guidance is suggested for viewers under\n         13"@en ;
        skos:prefLabel    "PG13"@en ;
        rdf:type          ebucore:TargetAudience .

parentalguidance:_4.2.9
        skos:example      "" ;
        skos:historyNote  "" ;
        skos:changeNote   "" ;
        skos:inScheme     <http://www.ebu.ch/metadata/ontologies/skos/ebu_ParentalGuidanceCodeCS> ;
        skos:broader      parentalguidance:_4.2 ;
        skos:definition   "Medical"@en ;
        skos:prefLabel    "M"@en ;
        rdf:type          ebucore:TargetAudience .

parentalguidance:_18  skos:narrower  parentalguidance:_18.3 ;
        skos:inScheme     <http://www.ebu.ch/metadata/ontologies/skos/ebu_ParentalGuidanceCodeCS> ;
        rdf:type          ebucore:TargetAudience ;
        skos:changeNote   "Update" ;
        skos:definition   "German TV content classification"@en ;
        skos:definition   "Freiwillige Selbskontrolle Fernsehen\n         Altersfreigabe"@de ;
        skos:narrower     parentalguidance:_18.2 ;
        skos:narrower     parentalguidance:_18.5 ;
        skos:historyNote  "2009-07-28" ;
        skos:scopeNote    "Region:Germany"@en ;
        skos:narrower     parentalguidance:_18.1 ;
        skos:narrower     parentalguidance:_18.4 ;
        skos:note         "Valid" ;
        skos:prefLabel    "DE-FSF"@en ;
        skos:example      "" .

parentalguidance:_12.3
        skos:example      "" ;
        skos:historyNote  "" ;
        skos:changeNote   "" ;
        skos:inScheme     <http://www.ebu.ch/metadata/ontologies/skos/ebu_ParentalGuidanceCodeCS> ;
        skos:broader      parentalguidance:_12 ;
        skos:definition   "Considered acceptable for all age groups. Appropriate viewing\n         for the entire family."@en ;
        skos:prefLabel    "General"@en ;
        skos:prefLabel    "G"@en ;
        rdf:type          ebucore:TargetAudience .

parentalguidance:_47.2.8
        skos:example      "" ;
        skos:historyNote  "" ;
        skos:changeNote   "" ;
        skos:inScheme     <http://www.ebu.ch/metadata/ontologies/skos/ebu_ParentalGuidanceCodeCS> ;
        skos:broader      parentalguidance:_47.2 ;
        skos:definition   "Reference to and/or images of illegal drugs" ;
        skos:prefLabel    "Drug Reference"@en ;
        rdf:type          ebucore:TargetAudience .

parentalguidance:_59.1.1
        skos:example      "" ;
        skos:historyNote  "" ;
        skos:changeNote   "" ;
        skos:inScheme     <http://www.ebu.ch/metadata/ontologies/skos/ebu_ParentalGuidanceCodeCS> ;
        skos:broader      parentalguidance:_59.1 ;
        skos:definition   "Suitable film for everyone, including children. The film does\n         not contain violence, drug abuse, or sexual content."@en ;
        skos:prefLabel    "K"@en ;
        rdf:type          ebucore:TargetAudience .

parentalguidance:_34.1.3
        skos:example      "" ;
        skos:historyNote  "" ;
        skos:changeNote   "" ;
        skos:inScheme     <http://www.ebu.ch/metadata/ontologies/skos/ebu_ParentalGuidanceCodeCS> ;
        skos:broader      parentalguidance:_34.1 ;
        skos:definition   "Suitable for ages 15 and above"@en ;
        skos:prefLabel    "15+"@en ;
        rdf:type          ebucore:TargetAudience .

parentalguidance:_69.1.2
        skos:example      "" ;
        skos:historyNote  "" ;
        skos:changeNote   "" ;
        skos:inScheme     <http://www.ebu.ch/metadata/ontologies/skos/ebu_ParentalGuidanceCodeCS> ;
        skos:broader      parentalguidance:_69.1 ;
        skos:definition   "Films prohibited to minors under 6 years"@en ;
        skos:definition   "Film Vietati ai minori di 6 anni"@it ;
        skos:prefLabel    "VM6"@en ;
        rdf:type          ebucore:TargetAudience .

parentalguidance:_27  skos:narrower  parentalguidance:_27.3 ;
        skos:definition   "British Board of Film Classification"@en ;
        skos:narrower     parentalguidance:_27.4 ;
        skos:example      "" ;
        skos:inScheme     <http://www.ebu.ch/metadata/ontologies/skos/ebu_ParentalGuidanceCodeCS> ;
        skos:narrower     parentalguidance:_27.5 ;
        rdf:type          ebucore:TargetAudience ;
        skos:note         "Valid" ;
        skos:narrower     parentalguidance:_27.6 ;
        skos:prefLabel    "GB-BBFC"@en ;
        skos:narrower     parentalguidance:_27.1 ;
        skos:altLabel     "www.bbfc.co.uk"@en ;
        skos:narrower     parentalguidance:_27.2 ;
        skos:historyNote  "2009-07-28" ;
        skos:changeNote   "Update" ;
        skos:scopeNote    "Region:Britain" .

parentalguidance:_4.2.8
        skos:example      "" ;
        skos:historyNote  "" ;
        skos:changeNote   "" ;
        skos:inScheme     <http://www.ebu.ch/metadata/ontologies/skos/ebu_ParentalGuidanceCodeCS> ;
        skos:broader      parentalguidance:_4.2 ;
        skos:definition   "Supernatural"@en ;
        skos:prefLabel    "SN"@en ;
        rdf:type          ebucore:TargetAudience .

parentalguidance:_47.1
        skos:historyNote  "" ;
        skos:narrower     parentalguidance:_47.1.2 ;
        skos:prefLabel    "Rating"@en ;
        rdf:type          ebucore:TargetAudience ;
        skos:changeNote   "" ;
        skos:narrower     parentalguidance:_47.1.1 ;
        skos:example      "" ;
        skos:broader      parentalguidance:_47 ;
        skos:narrower     parentalguidance:_47.1.7 ;
        skos:narrower     parentalguidance:_47.1.6 ;
        skos:inScheme     <http://www.ebu.ch/metadata/ontologies/skos/ebu_ParentalGuidanceCodeCS> ;
        skos:narrower     parentalguidance:_47.1.4 ;
        skos:narrower     parentalguidance:_47.1.5 ;
        skos:narrower     parentalguidance:_47.1.3 .

parentalguidance:_15  skos:definition  "Consejo de Calificacion Cinematografica"@es ;
        skos:scopeNote    "Region:Chile"@en ;
        skos:inScheme     <http://www.ebu.ch/metadata/ontologies/skos/ebu_ParentalGuidanceCodeCS> ;
        skos:narrower     parentalguidance:_15.4 ;
        skos:example      "" ;
        skos:definition   "Movie ratings as defined by the Chilean Council of\n         Cinematographic Classification"@en ;
        skos:narrower     parentalguidance:_15.5 ;
        rdf:type          ebucore:TargetAudience ;
        skos:note         "Valid" ;
        skos:historyNote  "2009-07-27" ;
        skos:changeNote   "Update" ;
        skos:prefLabel    "CL-CCC"@es ;
        skos:narrower     parentalguidance:_15.1 ;
        skos:prefLabel    "CL-CCC"@en ;
        skos:narrower     parentalguidance:_15.2 ;
        skos:narrower     parentalguidance:_15.3 .

parentalguidance:_9.4
        skos:example      "" ;
        skos:historyNote  "" ;
        skos:changeNote   "" ;
        skos:inScheme     <http://www.ebu.ch/metadata/ontologies/skos/ebu_ParentalGuidanceCodeCS> ;
        skos:broader      parentalguidance:_9 ;
        skos:definition   "Suitable for people 18 years of age or older. Persons under 18\n         should view with an adult. No rental or purchase by those under 18. Parents strongly\n         cautioned. Will likely contain explicit violence, frequent coarse language, sexual activity\n         and/or horror."@en ;
        skos:prefLabel    "18A"@en ;
        rdf:type          ebucore:TargetAudience .

parentalguidance:_39  skos:scopeNote  "Region:New Zealand"@en ;
        skos:narrower     parentalguidance:_39.3 ;
        skos:prefLabel    "NZ-OFLC"@en ;
        rdf:type          ebucore:TargetAudience ;
        skos:narrower     parentalguidance:_39.7 ;
        skos:narrower     parentalguidance:_39.2 ;
        skos:narrower     parentalguidance:_39.5 ;
        skos:inScheme     <http://www.ebu.ch/metadata/ontologies/skos/ebu_ParentalGuidanceCodeCS> ;
        skos:historyNote  "2009-07-27" ;
        skos:narrower     parentalguidance:_39.4 ;
        skos:narrower     parentalguidance:_39.6 ;
        skos:note         "Valid" ;
        skos:narrower     parentalguidance:_39.1 ;
        skos:definition   "Office of Film and Literature Classification"@en ;
        skos:example      "" ;
        skos:changeNote   "Update" ;
        skos:narrower     parentalguidance:_39.8 .

parentalguidance:_24.1
        skos:example      "" ;
        skos:historyNote  "" ;
        skos:changeNote   "" ;
        skos:inScheme     <http://www.ebu.ch/metadata/ontologies/skos/ebu_ParentalGuidanceCodeCS> ;
        skos:broader      parentalguidance:_24 ;
        skos:definition   "For all ages"@en ;
        skos:prefLabel    "S"@en ;
        rdf:type          ebucore:TargetAudience .

parentalguidance:_12.4
        skos:example      "" ;
        skos:historyNote  "" ;
        skos:changeNote   "" ;
        skos:inScheme     <http://www.ebu.ch/metadata/ontologies/skos/ebu_ParentalGuidanceCodeCS> ;
        skos:broader      parentalguidance:_12 ;
        skos:definition   "This programming, while intended for a general audience, may\n         not be suitable for younger children (under the age of 8). Parents/guardians should be\n         aware that there might be content elements which some could consider inappropriate for\n         unsupervised viewing by children in the 8-13 age range."@en ;
        skos:prefLabel    "Parental Guidance"@en ;
        skos:altLabel     "PG"@en ;
        rdf:type          ebucore:TargetAudience .

parentalguidance:_35.2
        skos:example      "" ;
        skos:changeNote   "" ;
        skos:broader      parentalguidance:_35 ;
        skos:prefLabel    "Criteria"@en ;
        skos:narrower     parentalguidance:_35.2.4 ;
        skos:inScheme     <http://www.ebu.ch/metadata/ontologies/skos/ebu_ParentalGuidanceCodeCS> ;
        skos:narrower     parentalguidance:_35.2.3 ;
        skos:historyNote  "" ;
        skos:narrower     parentalguidance:_35.2.2 ;
        rdf:type          ebucore:TargetAudience ;
        skos:narrower     parentalguidance:_35.2.1 .

parentalguidance:_47.2.7
        skos:example      "" ;
        skos:historyNote  "" ;
        skos:changeNote   "" ;
        skos:inScheme     <http://www.ebu.ch/metadata/ontologies/skos/ebu_ParentalGuidanceCodeCS> ;
        skos:broader      parentalguidance:_47.2 ;
        skos:definition   "Depictions or dialogue involving vulgar antics, including\n         'bathroom\" humour" ;
        skos:prefLabel    "Crude Humour"@en ;
        rdf:type          ebucore:TargetAudience .

parentalguidance:_59.1.2
        skos:example      "" ;
        skos:historyNote  "" ;
        skos:changeNote   "" ;
        skos:inScheme     <http://www.ebu.ch/metadata/ontologies/skos/ebu_ParentalGuidanceCodeCS> ;
        skos:broader      parentalguidance:_59.1 ;
        skos:definition   "Suitable film for children over the age of 13. The film may\n         contain mild violence and adult themes. "@en ;
        skos:prefLabel    "K-13"@en ;
        rdf:type          ebucore:TargetAudience .

parentalguidance:_69.1
        skos:historyNote  "" ;
        skos:narrower     parentalguidance:_69.1.2 ;
        skos:narrower     parentalguidance:_69.1.3 ;
        skos:changeNote   "" ;
        rdf:type          ebucore:TargetAudience ;
        skos:definition   ""@en ;
        skos:narrower     parentalguidance:_69.1.1 ;
        skos:prefLabel    "Rating"@en ;
        skos:broader      parentalguidance:_4 ;
        skos:inScheme     <http://www.ebu.ch/metadata/ontologies/skos/ebu_ParentalGuidanceCodeCS> ;
        skos:narrower     parentalguidance:_69.1.4 ;
        skos:example      "" .

parentalguidance:_16.2.11
        skos:example      "" ;
        skos:historyNote  "" ;
        skos:changeNote   "" ;
        skos:inScheme     <http://www.ebu.ch/metadata/ontologies/skos/ebu_ParentalGuidanceCodeCS> ;
        skos:broader      parentalguidance:_16.2 ;
        skos:prefLabel    "Triad expressions and ceremonies"@en ;
        rdf:type          ebucore:TargetAudience .

parentalguidance:_13.1
        rdf:type          ebucore:TargetAudience ;
        skos:changeNote   "" ;
        skos:definition   "For all ages"@en ;
        skos:example      "" ;
        skos:broader      parentalguidance:_13 ;
        skos:prefLabel    "G"@fr ;
        skos:prefLabel    "G"@en ;
        skos:definition   "General"@fr ;
        skos:inScheme     <http://www.ebu.ch/metadata/ontologies/skos/ebu_ParentalGuidanceCodeCS> ;
        skos:definition   "Le film peut être vu, loué ou acheté sans risque par des\n         personnes de tout âge"@fr ;
        skos:historyNote  "" .

parentalguidance:_9.5
        skos:example      "" ;
        skos:historyNote  "" ;
        skos:changeNote   "" ;
        skos:inScheme     <http://www.ebu.ch/metadata/ontologies/skos/ebu_ParentalGuidanceCodeCS> ;
        skos:broader      parentalguidance:_9 ;
        skos:definition   "Restricted to 18 years and older. No rental or purchase by\n         those under 18. Contents not suitable for minors. Contains frequent sexual activity,\n         brutality/graphic violence, intense horror, and/or other disturbing content. "@en ;
        skos:prefLabel    "Restricted"@en ;
        skos:prefLabel    "R"@en ;
        rdf:type          ebucore:TargetAudience .

parentalguidance:_24.2
        skos:example      "" ;
        skos:historyNote  "" ;
        skos:changeNote   "" ;
        skos:inScheme     <http://www.ebu.ch/metadata/ontologies/skos/ebu_ParentalGuidanceCodeCS> ;
        skos:broader      parentalguidance:_24 ;
        skos:definition   "For all ages"@en ;
        skos:prefLabel    "K-3"@en ;
        rdf:type          ebucore:TargetAudience .

parentalguidance:_34.1.2
        skos:example      "" ;
        skos:historyNote  "" ;
        skos:changeNote   "" ;
        skos:inScheme     <http://www.ebu.ch/metadata/ontologies/skos/ebu_ParentalGuidanceCodeCS> ;
        skos:broader      parentalguidance:_34.1 ;
        skos:definition   "Ages 12 and above"@en ;
        skos:prefLabel    "12+"@en ;
        rdf:type          ebucore:TargetAudience .

parentalguidance:_69.1.1
        skos:example      "" ;
        skos:historyNote  "" ;
        skos:changeNote   "" ;
        skos:inScheme     <http://www.ebu.ch/metadata/ontologies/skos/ebu_ParentalGuidanceCodeCS> ;
        skos:broader      parentalguidance:_69.1 ;
        skos:definition   "Pellicola per tutti"@it ;
        skos:definition   "Film for everyone"@en ;
        skos:prefLabel    "T"@en ;
        rdf:type          ebucore:TargetAudience .

parentalguidance:_16  skos:changeNote  "Update" ;
        skos:note         "Valid" ;
        skos:narrower     parentalguidance:_16.1 ;
        skos:narrower     parentalguidance:_16.2 ;
        skos:scopeNote    "Region:Hong-Kong"@en ;
        skos:historyNote  "2009-07-28" ;
        skos:example      "" ;
        skos:prefLabel    "CN-HK-HKBA"@en ;
        rdf:type          ebucore:TargetAudience ;
        skos:inScheme     <http://www.ebu.ch/metadata/ontologies/skos/ebu_ParentalGuidanceCodeCS> ;
        skos:definition   "Hong-Kong Broadcasting Authority"@en .

parentalguidance:_4.2.7
        skos:example      "" ;
        skos:historyNote  "" ;
        skos:changeNote   "" ;
        skos:inScheme     <http://www.ebu.ch/metadata/ontologies/skos/ebu_ParentalGuidanceCodeCS> ;
        skos:broader      parentalguidance:_4.2 ;
        skos:definition   "Nudity"@en ;
        skos:prefLabel    "N"@en ;
        rdf:type          ebucore:TargetAudience .

parentalguidance:_28  skos:scopeNote  "Region:Ireland"@en ;
        skos:historyNote  "2009-07-28" ;
        skos:narrower     parentalguidance:_28.3 ;
        skos:narrower     parentalguidance:_28.6 ;
        skos:note         "Valid" ;
        skos:example      "" ;
        skos:narrower     parentalguidance:_28.5 ;
        skos:definition   "Irish Film Classification Office"@en ;
        skos:narrower     parentalguidance:_28.2 ;
        rdf:type          ebucore:TargetAudience ;
        skos:changeNote   "Update" ;
        skos:inScheme     <http://www.ebu.ch/metadata/ontologies/skos/ebu_ParentalGuidanceCodeCS> ;
        skos:prefLabel    "IE-IFCO"@en ;
        skos:narrower     parentalguidance:_28.1 ;
        skos:narrower     parentalguidance:_28.4 .

parentalguidance:_64.1.1
        skos:example      "" ;
        skos:historyNote  "" ;
        skos:changeNote   "" ;
        skos:inScheme     <http://www.ebu.ch/metadata/ontologies/skos/ebu_ParentalGuidanceCodeCS> ;
        skos:broader      parentalguidance:_64.1 ;
        skos:definition   "General viewing for all ages."@en ;
        skos:prefLabel    "0"@en ;
        rdf:type          ebucore:TargetAudience .

parentalguidance:_32.2
        skos:example      "" ;
        skos:historyNote  "" ;
        skos:changeNote   "" ;
        skos:inScheme     <http://www.ebu.ch/metadata/ontologies/skos/ebu_ParentalGuidanceCodeCS> ;
        skos:broader      parentalguidance:_32 ;
        skos:definition   "This rating is for programming that may contain material\n         inappropriate for children younger than 7, and parental discretion should be\n         used."@en ;
        skos:prefLabel    "7"@en ;
        rdf:type          ebucore:TargetAudience .

parentalguidance:_35.1.2
        skos:example      "" ;
        skos:historyNote  "" ;
        skos:changeNote   "" ;
        skos:inScheme     <http://www.ebu.ch/metadata/ontologies/skos/ebu_ParentalGuidanceCodeCS> ;
        skos:broader      parentalguidance:_35.1 ;
        skos:definition   "Para todo público. Todos los programas bajo esta clasificación\n         son aptos para todo público y no deben contener elementos inadecuados para que los niños\n         los vean sin la supervisión de personas adultas."@es ;
        skos:definition   "For all audiences containing no content requiring parent\n         supervision" ;
        skos:prefLabel    "A"@en ;
        rdf:type          ebucore:TargetAudience .

parentalguidance:_55.1
        rdf:type          ebucore:TargetAudience ;
        skos:narrower     parentalguidance:_55.1.5 ;
        skos:changeNote   "" ;
        skos:example      "" ;
        skos:narrower     parentalguidance:_55.1.6 ;
        skos:narrower     parentalguidance:_55.1.1 ;
        skos:narrower     parentalguidance:_55.1.2 ;
        skos:prefLabel    "Rating"@en ;
        skos:narrower     parentalguidance:_55.1.3 ;
        skos:inScheme     <http://www.ebu.ch/metadata/ontologies/skos/ebu_ParentalGuidanceCodeCS> ;
        skos:narrower     parentalguidance:_55.1.4 ;
        skos:broader      parentalguidance:_55 ;
        skos:historyNote  "" .

parentalguidance:_42.6
        skos:example      "" ;
        skos:historyNote  "" ;
        skos:changeNote   "" ;
        skos:inScheme     <http://www.ebu.ch/metadata/ontologies/skos/ebu_ParentalGuidanceCodeCS> ;
        skos:broader      parentalguidance:_42 ;
        skos:definition   "Serão classificados no 1º escalão (hard-core) os espectáculos\n         que apresentem uma descrição ostensiva e insistente de actos sexuais realmente praticados\n         com exibição dos órgãos genitais; Serão classificados no 2º escalão (soft-core) os\n         espectáculos que apresentem uma descrição ostensiva e insistente de actos sexuais\n         simulados."@pt ;
        skos:definition   "For persons of age 18 and above, sexual\n         content"@en ;
        skos:prefLabel    "Pornográficos"@en ;
        rdf:type          ebucore:TargetAudience .

parentalguidance:_19.5
        skos:definition   "\"No youth admitted\", only adults"@en ;
        skos:changeNote   "" ;
        skos:inScheme     <http://www.ebu.ch/metadata/ontologies/skos/ebu_ParentalGuidanceCodeCS> ;
        skos:historyNote  "" ;
        skos:definition   "Keine Jugendfreigabe"@de ;
        skos:broader      parentalguidance:_19 ;
        rdf:type          ebucore:TargetAudience ;
        skos:prefLabel    "FSK 18"@de ;
        skos:prefLabel    "FSK 18"@en ;
        skos:example      "" .

parentalguidance:_43.3
        skos:example      "" ;
        skos:historyNote  "" ;
        skos:changeNote   "" ;
        skos:inScheme     <http://www.ebu.ch/metadata/ontologies/skos/ebu_ParentalGuidanceCodeCS> ;
        skos:broader      parentalguidance:_43 ;
        skos:definition   "For persons of age 12 and above. Parental Guidance is\n         suggested."@en ;
        skos:prefLabel    "12"@en ;
        rdf:type          ebucore:TargetAudience .

parentalguidance:_20.3
        skos:example      "" ;
        skos:historyNote  "" ;
        skos:changeNote   "" ;
        skos:inScheme     <http://www.ebu.ch/metadata/ontologies/skos/ebu_ParentalGuidanceCodeCS> ;
        skos:broader      parentalguidance:_20 ;
        skos:definition   "Approval of the film for admittance of children from the age of\n         11"@en ;
        skos:prefLabel    "11"@en ;
        rdf:type          ebucore:TargetAudience .

parentalguidance:_3.4
        skos:example      "" ;
        skos:historyNote  "" ;
        skos:changeNote   "" ;
        skos:inScheme     <http://www.ebu.ch/metadata/ontologies/skos/ebu_ParentalGuidanceCodeCS> ;
        skos:broader      parentalguidance:_3 ;
        skos:definition   "The MA 15+ category is a legally restricted category. The\n         impact of the content is strong. A person under the age of 15 years must be accompanied by\n         a parent or adult guardian if viewing or buying a film or computer game classified MA\n         15+."@en ;
        skos:prefLabel    "MA15+"@en ;
        rdf:type          ebucore:TargetAudience .

parentalguidance:_4.1
        skos:narrower     parentalguidance:_4.1.2 ;
        skos:inScheme     <http://www.ebu.ch/metadata/ontologies/skos/ebu_ParentalGuidanceCodeCS> ;
        skos:example      "" ;
        skos:broader      parentalguidance:_4 ;
        skos:narrower     parentalguidance:_4.1.7 ;
        skos:narrower     parentalguidance:_4.1.1 ;
        skos:definition   ""@en ;
        skos:changeNote   "" ;
        skos:narrower     parentalguidance:_4.1.6 ;
        skos:narrower     parentalguidance:_4.1.5 ;
        skos:prefLabel    "Rating"@en ;
        skos:narrower     parentalguidance:_4.1.4 ;
        skos:narrower     parentalguidance:_4.1.3 ;
        skos:historyNote  "" ;
        rdf:type          ebucore:TargetAudience .

parentalguidance:_23.1.3
        skos:example      "" ;
        skos:historyNote  "" ;
        skos:changeNote   "" ;
        skos:inScheme     <http://www.ebu.ch/metadata/ontologies/skos/ebu_ParentalGuidanceCodeCS> ;
        skos:broader      parentalguidance:_23.1 ;
        skos:definition   "Suitable only for persons of over ages 12 and older. This\n         rating contains mild action violence or suggestive themes and mildly suggestive song\n         lyrics."@en ;
        skos:prefLabel    "12+"@en ;
        rdf:type          ebucore:TargetAudience .

parentalguidance:_68.1.3
        skos:example      "" ;
        skos:historyNote  "" ;
        skos:changeNote   "" ;
        skos:inScheme     <http://www.ebu.ch/metadata/ontologies/skos/ebu_ParentalGuidanceCodeCS> ;
        skos:broader      parentalguidance:_68.1 ;
        skos:definition   "14 years"@en ;
        skos:definition   "14 anni"@it ;
        skos:prefLabel    "VM14"@en ;
        rdf:type          ebucore:TargetAudience .

parentalguidance:_67.1
        skos:inScheme    <http://www.ebu.ch/metadata/ontologies/skos/ebu_ParentalGuidanceCodeCS> ;
        skos:broader     parentalguidance:_67 ;
        skos:definition  "Viewing for all ages"@en ;
        skos:altLabel    "children"@en ;
        skos:altLabel    "family"@en ;
        skos:prefLabel   "nonadult"@en ;
        rdf:type         ebucore:TargetAudience .

parentalguidance:_32.1
        skos:example      "" ;
        skos:historyNote  "" ;
        skos:changeNote   "" ;
        skos:inScheme     <http://www.ebu.ch/metadata/ontologies/skos/ebu_ParentalGuidanceCodeCS> ;
        skos:broader      parentalguidance:_32 ;
        skos:definition   "Suitable for all ages"@en ;
        skos:prefLabel    "All"@en ;
        rdf:type          ebucore:TargetAudience .

parentalguidance:_56.1.4
        skos:example      "" ;
        skos:historyNote  "" ;
        skos:changeNote   "" ;
        skos:inScheme     <http://www.ebu.ch/metadata/ontologies/skos/ebu_ParentalGuidanceCodeCS> ;
        skos:broader      parentalguidance:_56.1 ;
        skos:definition   "Exhibition to restricted audience such as doctors\n         etc."@en ;
        skos:prefLabel    "S"@en ;
        rdf:type          ebucore:TargetAudience .

parentalguidance:_35.1.1
        skos:example      "" ;
        skos:historyNote  "" ;
        skos:changeNote   "" ;
        skos:inScheme     <http://www.ebu.ch/metadata/ontologies/skos/ebu_ParentalGuidanceCodeCS> ;
        skos:broader      parentalguidance:_35.1 ;
        skos:definition   "Comprensible para niños menores de 7 años"@es ;
        skos:definition   "Particularly recommended for children under 7" ;
        skos:prefLabel    "AA"@en ;
        rdf:type          ebucore:TargetAudience .

parentalguidance:_24.5.1
        skos:example      "" ;
        skos:historyNote  "" ;
        skos:changeNote   "" ;
        skos:inScheme     <http://www.ebu.ch/metadata/ontologies/skos/ebu_ParentalGuidanceCodeCS> ;
        skos:broader      parentalguidance:_24.5 ;
        skos:definition   "Parental Guidance option - children 2 years of age under the K\n         limits may access the show in presence of an accompanying adult"@en ;
        skos:prefLabel    "PG"@en ;
        rdf:type          ebucore:TargetAudience .

parentalguidance:_68.1.2
        skos:example      "" ;
        skos:historyNote  "" ;
        skos:changeNote   "" ;
        skos:inScheme     <http://www.ebu.ch/metadata/ontologies/skos/ebu_ParentalGuidanceCodeCS> ;
        skos:broader      parentalguidance:_68.1 ;
        skos:definition   "Works not suitable for children under 6 years"@en ;
        skos:definition   "Opere non adatte ai minori di anni 6"@it ;
        skos:prefLabel    "VM6"@en ;
        rdf:type          ebucore:TargetAudience .

parentalguidance:_21.1
        skos:example      "" ;
        skos:historyNote  "" ;
        skos:changeNote   "" ;
        skos:inScheme     <http://www.ebu.ch/metadata/ontologies/skos/ebu_ParentalGuidanceCodeCS> ;
        skos:broader      parentalguidance:_21 ;
        skos:definition   "All ages"@en ;
        skos:prefLabel    "Green"@en ;
        rdf:type          ebucore:TargetAudience .

parentalguidance:_42.5
        skos:example      "" ;
        skos:historyNote  "" ;
        skos:changeNote   "" ;
        skos:inScheme     <http://www.ebu.ch/metadata/ontologies/skos/ebu_ParentalGuidanceCodeCS> ;
        skos:broader      parentalguidance:_42 ;
        skos:definition   "os espectáculos pornográficos e os que explorem formas\n         patológicas de violência física e psíquica."@pt ;
        skos:definition   "For persons of age 18 and above"@en ;
        skos:prefLabel    "M/18"@en ;
        rdf:type          ebucore:TargetAudience .

parentalguidance:_3.5
        skos:example      "" ;
        skos:historyNote  "" ;
        skos:changeNote   "" ;
        skos:inScheme     <http://www.ebu.ch/metadata/ontologies/skos/ebu_ParentalGuidanceCodeCS> ;
        skos:broader      parentalguidance:_3 ;
        skos:definition   "R 18+ classified films are legally restricted to persons 18\n         years and over because of the high impact content. Some material in this classification may\n         be offensive to some sections of the adult community. "@en ;
        skos:prefLabel    "R18+"@en ;
        rdf:type          ebucore:TargetAudience .

parentalguidance:_23.1.4
        skos:example      "" ;
        skos:historyNote  "" ;
        skos:changeNote   "" ;
        skos:inScheme     <http://www.ebu.ch/metadata/ontologies/skos/ebu_ParentalGuidanceCodeCS> ;
        skos:broader      parentalguidance:_23.1 ;
        skos:definition   "This rating is suitable only for persons of 16 years of age or\n         older. Some situations include strong action violence, mild references to gambling, and\n         rude humor."@en ;
        skos:prefLabel    "16+"@en ;
        rdf:type          ebucore:TargetAudience .

parentalguidance:_20.4
        skos:example      "" ;
        skos:historyNote  "" ;
        skos:changeNote   "" ;
        skos:inScheme     <http://www.ebu.ch/metadata/ontologies/skos/ebu_ParentalGuidanceCodeCS> ;
        skos:broader      parentalguidance:_20 ;
        skos:definition   "Approval of the film for admittance of children from the age of\n         15"@en ;
        skos:prefLabel    "15"@en ;
        rdf:type          ebucore:TargetAudience .

parentalguidance:_43.2
        skos:example      "" ;
        skos:historyNote  "" ;
        skos:changeNote   "" ;
        skos:inScheme     <http://www.ebu.ch/metadata/ontologies/skos/ebu_ParentalGuidanceCodeCS> ;
        skos:broader      parentalguidance:_43 ;
        skos:definition   "For persons of age 10 and above. Parental Guidance is\n         suggested."@en ;
        skos:prefLabel    "10"@en ;
        rdf:type          ebucore:TargetAudience .

parentalguidance:_4.2
        skos:example      "" ;
        rdf:type          ebucore:TargetAudience ;
        skos:narrower     parentalguidance:_4.2.11 ;
        skos:narrower     parentalguidance:_4.2.8 ;
        skos:narrower     parentalguidance:_4.2.5 ;
        skos:narrower     parentalguidance:_4.2.2 ;
        skos:broader      parentalguidance:_4 ;
        skos:narrower     parentalguidance:_4.2.1 ;
        skos:definition   ""@en ;
        skos:inScheme     <http://www.ebu.ch/metadata/ontologies/skos/ebu_ParentalGuidanceCodeCS> ;
        skos:narrower     parentalguidance:_4.2.9 ;
        skos:narrower     parentalguidance:_4.2.6 ;
        skos:prefLabel    "Criteria"@en ;
        skos:narrower     parentalguidance:_4.2.3 ;
        skos:changeNote   "" ;
        skos:narrower     parentalguidance:_4.2.10 ;
        skos:historyNote  "" ;
        skos:narrower     parentalguidance:_4.2.7 ;
        skos:narrower     parentalguidance:_4.2.4 .

parentalguidance:_23.2.1
        skos:example      "" ;
        skos:historyNote  "" ;
        skos:changeNote   "" ;
        skos:inScheme     <http://www.ebu.ch/metadata/ontologies/skos/ebu_ParentalGuidanceCodeCS> ;
        skos:broader      parentalguidance:_23.2 ;
        skos:prefLabel    "Profanity"@en ;
        rdf:type          ebucore:TargetAudience .

parentalguidance:_67.2
        skos:inScheme    <http://www.ebu.ch/metadata/ontologies/skos/ebu_ParentalGuidanceCodeCS> ;
        skos:broader     parentalguidance:_67 ;
        skos:definition  "Only for adult viewing"@en ;
        skos:prefLabel   "adult"@en ;
        rdf:type         ebucore:TargetAudience .

parentalguidance:_35.1.4
        skos:example      "" ;
        skos:historyNote  "" ;
        skos:changeNote   "" ;
        skos:inScheme     <http://www.ebu.ch/metadata/ontologies/skos/ebu_ParentalGuidanceCodeCS> ;
        skos:broader      parentalguidance:_35.1 ;
        skos:definition   "No recomendada para menores de 15 años. Aptos para mayores de\n         15 años. El material clasificado contiene temas o conceptos para adultos, pero sigue siendo\n         adecuado para ser visto por adolescentes, preferentemente con la guía de personas\n         adultas."@es ;
        skos:definition   "For ages 15 and older preferably in presence of supervising\n         adults"@en ;
        skos:prefLabel    "B15"@en ;
        rdf:type          ebucore:TargetAudience .

parentalguidance:_19.2
        skos:definition   "Freigegeben ab 6 Jahren"@de ;
        skos:inScheme     <http://www.ebu.ch/metadata/ontologies/skos/ebu_ParentalGuidanceCodeCS> ;
        skos:changeNote   "" ;
        skos:prefLabel    "FSK 6"@de ;
        skos:prefLabel    "FSK 6"@en ;
        rdf:type          ebucore:TargetAudience ;
        skos:example      "" ;
        skos:broader      parentalguidance:_19 ;
        skos:historyNote  "" ;
        skos:definition   "No one under 6 years admitted"@en .

parentalguidance:_56.1
        skos:changeNote   "" ;
        skos:broader      parentalguidance:_56 ;
        skos:inScheme     <http://www.ebu.ch/metadata/ontologies/skos/ebu_ParentalGuidanceCodeCS> ;
        skos:narrower     parentalguidance:_56.1.2 ;
        skos:narrower     parentalguidance:_56.1.1 ;
        skos:prefLabel    "Rating"@en ;
        skos:example      "" ;
        skos:narrower     parentalguidance:_56.1.3 ;
        rdf:type          ebucore:TargetAudience ;
        skos:narrower     parentalguidance:_56.1.4 ;
        skos:historyNote  "" .

parentalguidance:_35.2.1
        skos:example      "" ;
        skos:historyNote  "" ;
        skos:changeNote   "" ;
        skos:inScheme     <http://www.ebu.ch/metadata/ontologies/skos/ebu_ParentalGuidanceCodeCS> ;
        skos:broader      parentalguidance:_35.2 ;
        skos:prefLabel    "Violencia"@es ;
        skos:prefLabel    "Violence"@en ;
        rdf:type          ebucore:TargetAudience .

parentalguidance:_64.1.3
        skos:example      "" ;
        skos:historyNote  "" ;
        skos:changeNote   "" ;
        skos:inScheme     <http://www.ebu.ch/metadata/ontologies/skos/ebu_ParentalGuidanceCodeCS> ;
        skos:broader      parentalguidance:_64.1 ;
        skos:definition   "No one under the age of 10 admitted "@en ;
        skos:prefLabel    "10"@en ;
        rdf:type          ebucore:TargetAudience .

parentalguidance:_9  skos:narrower  parentalguidance:_9.4 ;
        skos:narrower     parentalguidance:_9.1 ;
        skos:inScheme     <http://www.ebu.ch/metadata/ontologies/skos/ebu_ParentalGuidanceCodeCS> ;
        skos:prefLabel    "CA-AFR"@en ;
        skos:narrower     parentalguidance:_9.5 ;
        skos:historyNote  "2009-07-27" ;
        skos:narrower     parentalguidance:_9.2 ;
        rdf:type          ebucore:TargetAudience ;
        skos:definition   "Alberta Film rating"@en ;
        skos:changeNote   "Update" ;
        skos:scopeNote    "Region:Canada"@en ;
        skos:narrower     parentalguidance:_9.6 ;
        skos:narrower     parentalguidance:_9.3 ;
        skos:note         "Valid" ;
        skos:example      "" .

parentalguidance:_68.1.1
        skos:example      "" ;
        skos:historyNote  "" ;
        skos:changeNote   "" ;
        skos:inScheme     <http://www.ebu.ch/metadata/ontologies/skos/ebu_ParentalGuidanceCodeCS> ;
        skos:broader      parentalguidance:_68.1 ;
        skos:definition   "Pellicola per tutti"@it ;
        skos:definition   "Film for everyone"@en ;
        skos:prefLabel    "T"@en ;
        rdf:type          ebucore:TargetAudience .

parentalguidance:_42.4
        skos:example      "" ;
        skos:historyNote  "" ;
        skos:changeNote   "" ;
        skos:inScheme     <http://www.ebu.ch/metadata/ontologies/skos/ebu_ParentalGuidanceCodeCS> ;
        skos:broader      parentalguidance:_42 ;
        skos:definition   "os espectáculos que explorem, em termos excessivos, aspectos da\n         sexualidade e da violência física e psíquica."@pt ;
        skos:definition   "For persons of age 16 and above"@en ;
        skos:prefLabel    "M/16"@en ;
        rdf:type          ebucore:TargetAudience .

parentalguidance:_2.5
        skos:example      "" ;
        skos:historyNote  "" ;
        skos:changeNote   "" ;
        skos:inScheme     <http://www.ebu.ch/metadata/ontologies/skos/ebu_ParentalGuidanceCodeCS> ;
        skos:broader      parentalguidance:_2 ;
        skos:definition   "14 years and above"@en ;
        skos:prefLabel    "14"@en ;
        rdf:type          ebucore:TargetAudience .

parentalguidance:_43.1
        skos:example      "" ;
        skos:historyNote  "" ;
        skos:changeNote   "" ;
        skos:inScheme     <http://www.ebu.ch/metadata/ontologies/skos/ebu_ParentalGuidanceCodeCS> ;
        skos:broader      parentalguidance:_43 ;
        skos:definition   "Todos"@pt ;
        skos:definition   "For all audiences"@en ;
        skos:prefLabel    "T"@en ;
        rdf:type          ebucore:TargetAudience .

parentalguidance:_23.1.1
        skos:example      "" ;
        skos:historyNote  "" ;
        skos:changeNote   "" ;
        skos:inScheme     <http://www.ebu.ch/metadata/ontologies/skos/ebu_ParentalGuidanceCodeCS> ;
        skos:broader      parentalguidance:_23.1 ;
        skos:definition   "Suitable for ages 3 and over. Contains very mild violence or\n         suggestive themes."@en ;
        skos:prefLabel    "3+"@en ;
        rdf:type          ebucore:TargetAudience .

parentalguidance:_3.2
        skos:example      "" ;
        skos:historyNote  "" ;
        skos:changeNote   "" ;
        skos:inScheme     <http://www.ebu.ch/metadata/ontologies/skos/ebu_ParentalGuidanceCodeCS> ;
        skos:broader      parentalguidance:_3 ;
        skos:definition   "PG classified films and computer games may contain material\n         that needs to be explained to children therefore parental guidance is recommended. The\n         impact of the content is mild."@en ;
        skos:prefLabel    "Parental Guidance"@en ;
        skos:altLabel     "PG"@en ;
        rdf:type          ebucore:TargetAudience .

parentalguidance:_20.1
        skos:example      "" ;
        skos:historyNote  "" ;
        skos:changeNote   "" ;
        skos:inScheme     <http://www.ebu.ch/metadata/ontologies/skos/ebu_ParentalGuidanceCodeCS> ;
        skos:broader      parentalguidance:_20 ;
        skos:definition   "Approval of the film for general admittance"@en ;
        skos:prefLabel    "A"@en ;
        rdf:type          ebucore:TargetAudience .

parentalguidance:_64.1.2
        skos:example      "" ;
        skos:historyNote  "" ;
        skos:changeNote   "" ;
        skos:inScheme     <http://www.ebu.ch/metadata/ontologies/skos/ebu_ParentalGuidanceCodeCS> ;
        skos:broader      parentalguidance:_64.1 ;
        skos:definition   "No one under the age of 7 admitted "@en ;
        skos:prefLabel    "7"@en ;
        rdf:type          ebucore:TargetAudience .

parentalguidance:_35.1.3
        skos:example      "" ;
        skos:historyNote  "" ;
        skos:changeNote   "" ;
        skos:inScheme     <http://www.ebu.ch/metadata/ontologies/skos/ebu_ParentalGuidanceCodeCS> ;
        skos:broader      parentalguidance:_35.1 ;
        skos:definition   "Para adolescentes de 12 años en adelante. Son programas aptos\n         para adolescentes y adultos. El material contiene temas o conceptos para adultos, sin\n         embargo es adecuado para que lo vean adolescentes mayores de 12 años."@es ;
        skos:definition   "For teenagers (ages 12 and older) and adults"@en ;
        skos:prefLabel    "B"@en ;
        rdf:type          ebucore:TargetAudience .

parentalguidance:_19.3
        skos:inScheme     <http://www.ebu.ch/metadata/ontologies/skos/ebu_ParentalGuidanceCodeCS> ;
        skos:definition   "Freigegeben ab 12 Jahren"@de ;
        skos:historyNote  "" ;
        skos:definition   "People 12 or older admitted, children between 6 and 11 only\n         when accompanied by parent or legal guardian"@en ;
        skos:prefLabel    "FSK 12"@de ;
        skos:prefLabel    "FSK 12"@en ;
        skos:changeNote   "" ;
        skos:hiddenLabel  "12"@en ;
        rdf:type          ebucore:TargetAudience ;
        skos:example      "" ;
        skos:broader      parentalguidance:_19 .

parentalguidance:_31.2
        skos:changeNote   "" ;
        skos:narrower     parentalguidance:_31.2.7 ;
        skos:narrower     parentalguidance:_31.2.8 ;
        skos:narrower     parentalguidance:_31.2.9 ;
        skos:narrower     parentalguidance:_31.2.2 ;
        skos:prefLabel    "コンテンツアイコン"@ja ;
        skos:narrower     parentalguidance:_31.2.3 ;
        skos:narrower     parentalguidance:_31.2.4 ;
        skos:narrower     parentalguidance:_31.2.5 ;
        skos:narrower     parentalguidance:_31.2.1 ;
        skos:broader      parentalguidance:_31 ;
        skos:inScheme     <http://www.ebu.ch/metadata/ontologies/skos/ebu_ParentalGuidanceCodeCS> ;
        rdf:type          ebucore:TargetAudience ;
        skos:prefLabel    "Criteria"@en ;
        skos:example      "" ;
        skos:historyNote  "" ;
        skos:narrower     parentalguidance:_31.2.6 .

parentalguidance:_54.1
        skos:historyNote  "" ;
        skos:narrower     parentalguidance:_54.1.2 ;
        skos:narrower     parentalguidance:_54.1.3 ;
        skos:narrower     parentalguidance:_54.1.1 ;
        skos:narrower     parentalguidance:_54.1.4 ;
        skos:narrower     parentalguidance:_54.1.5 ;
        skos:changeNote   "" ;
        skos:example      "" ;
        skos:broader      parentalguidance:_54 ;
        skos:prefLabel    "Rating"@en ;
        rdf:type          ebucore:TargetAudience ;
        skos:inScheme     <http://www.ebu.ch/metadata/ontologies/skos/ebu_ParentalGuidanceCodeCS> .

parentalguidance:_19.4
        skos:prefLabel    "FSK 16"@de ;
        skos:prefLabel    "FSK 16"@en ;
        skos:historyNote  "" ;
        skos:definition   "People 16 or older admitted"@en ;
        skos:hiddenLabel  "16"@en ;
        skos:inScheme     <http://www.ebu.ch/metadata/ontologies/skos/ebu_ParentalGuidanceCodeCS> ;
        skos:broader      parentalguidance:_19 ;
        rdf:type          ebucore:TargetAudience ;
        skos:example      "" ;
        skos:changeNote   "" ;
        skos:definition   "Freigegeben ab 16 Jahren"@de .

parentalguidance:_20.2
        skos:example      "" ;
        skos:historyNote  "" ;
        skos:changeNote   "" ;
        skos:inScheme     <http://www.ebu.ch/metadata/ontologies/skos/ebu_ParentalGuidanceCodeCS> ;
        skos:broader      parentalguidance:_20 ;
        skos:definition   "Approval of the film for general admittance, but not\n         recommended for children under the age of 7"@en ;
        skos:prefLabel    "7"@en ;
        rdf:type          ebucore:TargetAudience .

parentalguidance:_2.6
        skos:example      "" ;
        skos:historyNote  "" ;
        skos:changeNote   "" ;
        skos:inScheme     <http://www.ebu.ch/metadata/ontologies/skos/ebu_ParentalGuidanceCodeCS> ;
        skos:broader      parentalguidance:_2 ;
        skos:definition   "16 years and above"@en ;
        skos:prefLabel    "16"@en ;
        rdf:type          ebucore:TargetAudience .

parentalguidance:_42.3
        skos:example      "" ;
        skos:historyNote  "" ;
        skos:changeNote   "" ;
        skos:inScheme     <http://www.ebu.ch/metadata/ontologies/skos/ebu_ParentalGuidanceCodeCS> ;
        skos:broader      parentalguidance:_42 ;
        skos:definition   "os espectáculos que, pela sua extensão e complexidade, possam\n         provocar nos espectadores de nível etário inferior fadiga excessiva e ou traumatismo\n         psíquico."@pt ;
        skos:definition   "For persons of age 12 and above"@en ;
        skos:prefLabel    "M/12"@en ;
        rdf:type          ebucore:TargetAudience .

parentalguidance:_3.3
        skos:example      "" ;
        skos:historyNote  "" ;
        skos:changeNote   "" ;
        skos:inScheme     <http://www.ebu.ch/metadata/ontologies/skos/ebu_ParentalGuidanceCodeCS> ;
        skos:broader      parentalguidance:_3 ;
        skos:definition   "The M category is recommended for mature audiences. A mature\n         perspective is required to view this material. The impact of the content is\n         moderate."@en ;
        skos:prefLabel    "Mature"@en ;
        skos:prefLabel    "M"@en ;
        rdf:type          ebucore:TargetAudience .

parentalguidance:_23.1.2
        skos:example      "" ;
        skos:historyNote  "" ;
        skos:changeNote   "" ;
        skos:inScheme     <http://www.ebu.ch/metadata/ontologies/skos/ebu_ParentalGuidanceCodeCS> ;
        skos:broader      parentalguidance:_23.1 ;
        skos:definition   "These games are the same as Early Childhood ratings but may\n         include content descriptors like mild violence and in a rare case, very mild action\n         violence."@en ;
        skos:prefLabel    "7+"@en ;
        rdf:type          ebucore:TargetAudience .

parentalguidance:_36.2.4
        skos:example      "" ;
        skos:historyNote  "" ;
        skos:changeNote   "" ;
        skos:inScheme     <http://www.ebu.ch/metadata/ontologies/skos/ebu_ParentalGuidanceCodeCS> ;
        skos:broader      parentalguidance:_36.2 ;
        skos:prefLabel    "Strong themes"@en ;
        rdf:type          ebucore:TargetAudience .

parentalguidance:_35.2.3
        skos:example      "" ;
        skos:historyNote  "" ;
        skos:changeNote   "" ;
        skos:inScheme     <http://www.ebu.ch/metadata/ontologies/skos/ebu_ParentalGuidanceCodeCS> ;
        skos:broader      parentalguidance:_35.2 ;
        skos:prefLabel    "Lenguaje"@es ;
        skos:prefLabel    "Language"@en ;
        rdf:type          ebucore:TargetAudience .

parentalguidance:_47.2.19
        skos:example      "" ;
        skos:historyNote  "" ;
        skos:changeNote   "" ;
        skos:inScheme     <http://www.ebu.ch/metadata/ontologies/skos/ebu_ParentalGuidanceCodeCS> ;
        skos:broader      parentalguidance:_47.2 ;
        skos:definition   "Player can gamble, including betting or wagering real cash or\n         currency" ;
        skos:prefLabel    "Real Gambling"@en ;
        rdf:type          ebucore:TargetAudience .

parentalguidance:_33.3
        skos:example      "" ;
        skos:historyNote  "" ;
        skos:changeNote   "" ;
        skos:inScheme     <http://www.ebu.ch/metadata/ontologies/skos/ebu_ParentalGuidanceCodeCS> ;
        skos:broader      parentalguidance:_33 ;
        skos:definition   "Suitable for those aged 15 and over"@en ;
        skos:prefLabel    "15+"@en ;
        rdf:type          ebucore:TargetAudience .

parentalguidance:_35.1.6
        skos:example      "" ;
        skos:historyNote  "" ;
        skos:changeNote   "" ;
        skos:inScheme     <http://www.ebu.ch/metadata/ontologies/skos/ebu_ParentalGuidanceCodeCS> ;
        skos:broader      parentalguidance:_35.1 ;
        skos:definition   "Para Adultos. Programas exclusivamente para mayores de 18\n         años"@es ;
        skos:definition   "For ages 18 and above, strictly"@en ;
        skos:prefLabel    "D"@en ;
        rdf:type          ebucore:TargetAudience .

parentalguidance:_56.1.1
        skos:example      "" ;
        skos:historyNote  "" ;
        skos:changeNote   "" ;
        skos:inScheme     <http://www.ebu.ch/metadata/ontologies/skos/ebu_ParentalGuidanceCodeCS> ;
        skos:broader      parentalguidance:_56.1 ;
        skos:definition   "Unrestricted Public Exhibition throughout\n         India,"@en ;
        skos:prefLabel    "U"@en ;
        rdf:type          ebucore:TargetAudience .

parentalguidance:_10.3
        skos:example      "" ;
        skos:historyNote  "" ;
        skos:changeNote   "" ;
        skos:inScheme     <http://www.ebu.ch/metadata/ontologies/skos/ebu_ParentalGuidanceCodeCS> ;
        skos:broader      parentalguidance:_10 ;
        skos:definition   "Suitable for people 14 years of age or older. Those under 14\n         should view with an adult. No rental or purchase by those under 14 where prohibited by law.\n         Parents cautioned. May contain violence, coarse language and/or sexually suggestive\n         scenes."@en ;
        skos:prefLabel    "14A"@en ;
        rdf:type          ebucore:TargetAudience .

parentalguidance:_64.1.5
        skos:example      "" ;
        skos:historyNote  "" ;
        skos:changeNote   "" ;
        skos:inScheme     <http://www.ebu.ch/metadata/ontologies/skos/ebu_ParentalGuidanceCodeCS> ;
        skos:broader      parentalguidance:_64.1 ;
        skos:definition   "No one under the age of 14 admitted "@en ;
        skos:prefLabel    "14"@en ;
        rdf:type          ebucore:TargetAudience .

parentalguidance:_31.1.3
        skos:prefLabel    "青"@ja ;
        skos:inScheme     <http://www.ebu.ch/metadata/ontologies/skos/ebu_ParentalGuidanceCodeCS> ;
        skos:example      "" ;
        skos:definition   "15 and over"@en ;
        rdf:type          ebucore:TargetAudience ;
        skos:broader      parentalguidance:_31.1 ;
        skos:changeNote   "" ;
        skos:historyNote  "" ;
        skos:definition   "15歳以上のみ"@ja ;
        skos:prefLabel    "Blue"@en ;
        skos:prefLabel    "C"@en .

parentalguidance:_7  skos:inScheme  <http://www.ebu.ch/metadata/ontologies/skos/ebu_ParentalGuidanceCodeCS> ;
        skos:narrower     parentalguidance:_7.6 ;
        rdf:type          ebucore:TargetAudience ;
        skos:narrower     parentalguidance:_7.3 ;
        skos:changeNote   "Update" ;
        skos:note         "Valid" ;
        skos:narrower     parentalguidance:_7.4 ;
        skos:definition   "Department of Justice, Rating, Titles and\n         Qualification"@en ;
        skos:scopeNote    "Region:Brazil"@en ;
        skos:narrower     parentalguidance:_7.7 ;
        skos:narrower     parentalguidance:_7.1 ;
        skos:definition   "Departamento de Justiça, Classificação, Títulos e\n         Qualificação"@pt ;
        skos:narrower     parentalguidance:_7.2 ;
        skos:example      "" ;
        skos:historyNote  "2009-07-27" ;
        skos:prefLabel    "BR-DJCTQ"@en ;
        skos:narrower     parentalguidance:_7.5 .

parentalguidance:_44.4
        skos:example      "" ;
        skos:historyNote  "" ;
        skos:changeNote   "" ;
        skos:inScheme     <http://www.ebu.ch/metadata/ontologies/skos/ebu_ParentalGuidanceCodeCS> ;
        skos:broader      parentalguidance:_44 ;
        skos:definition   "No one under 15 years of age admitted"@en ;
        skos:prefLabel    "15"@en ;
        rdf:type          ebucore:TargetAudience .

parentalguidance:_47.2.1
        skos:example      "" ;
        skos:historyNote  "" ;
        skos:changeNote   "" ;
        skos:inScheme     <http://www.ebu.ch/metadata/ontologies/skos/ebu_ParentalGuidanceCodeCS> ;
        skos:broader      parentalguidance:_47.2 ;
        skos:definition   "Reference to and/or images of alcoholic\n         beverages" ;
        skos:prefLabel    "Alcohol Reference"@en ;
        rdf:type          ebucore:TargetAudience .

parentalguidance:_45.1
        skos:example      "" ;
        skos:historyNote  "" ;
        skos:changeNote   "" ;
        skos:inScheme     <http://www.ebu.ch/metadata/ontologies/skos/ebu_ParentalGuidanceCodeCS> ;
        skos:broader      parentalguidance:_45 ;
        skos:definition   "Suitable for all ages and audiences"@en ;
        skos:prefLabel    "General"@en ;
        skos:prefLabel    "G"@en ;
        rdf:type          ebucore:TargetAudience .

parentalguidance:_60.1.2
        skos:example      "" ;
        skos:historyNote  "" ;
        skos:changeNote   "" ;
        skos:inScheme     <http://www.ebu.ch/metadata/ontologies/skos/ebu_ParentalGuidanceCodeCS> ;
        skos:broader      parentalguidance:_60.1 ;
        skos:definition   "(Anak-anak): Children (3–12 years) "@en ;
        skos:prefLabel    "A"@en ;
        rdf:type          ebucore:TargetAudience .

parentalguidance:_65.1.5
        skos:example      "" ;
        skos:historyNote  "" ;
        skos:changeNote   "" ;
        skos:inScheme     <http://www.ebu.ch/metadata/ontologies/skos/ebu_ParentalGuidanceCodeCS> ;
        skos:broader      parentalguidance:_65.1 ;
        skos:definition   "No one under the age of 18 admitted "@en ;
        skos:prefLabel    "18+"@en ;
        rdf:type          ebucore:TargetAudience .

parentalguidance:_1.6
        skos:example      "" ;
        skos:historyNote  "" ;
        skos:changeNote   "" ;
        skos:inScheme     <http://www.ebu.ch/metadata/ontologies/skos/ebu_ParentalGuidanceCodeCS> ;
        skos:broader      parentalguidance:_1 ;
        skos:definition   "Exempt: sports, music, etc."@en ;
        skos:prefLabel    "E"@en ;
        rdf:type          ebucore:TargetAudience .

parentalguidance:_47.1.4
        skos:example      "" ;
        skos:historyNote  "" ;
        skos:changeNote   "" ;
        skos:inScheme     <http://www.ebu.ch/metadata/ontologies/skos/ebu_ParentalGuidanceCodeCS> ;
        skos:broader      parentalguidance:_47.1 ;
        skos:definition   "Titles rated T (Teen) have content that may be suitable for ages\n         13 and older. Titles in this category may contain violence, suggestive themes, crude\n         humour, minimal blood, simulated gambling, and/or infrequent use of strong\n         language" ;
        skos:prefLabel    "T"@en ;
        rdf:type          ebucore:TargetAudience .

parentalguidance:_2.3
        skos:example      "" ;
        skos:historyNote  "" ;
        skos:changeNote   "" ;
        skos:inScheme     <http://www.ebu.ch/metadata/ontologies/skos/ebu_ParentalGuidanceCodeCS> ;
        skos:broader      parentalguidance:_2 ;
        skos:definition   "10 years and above"@en ;
        skos:prefLabel    "10"@en ;
        rdf:type          ebucore:TargetAudience .

parentalguidance:_22.1
        skos:example      "" ;
        skos:historyNote  "" ;
        skos:changeNote   "" ;
        skos:inScheme     <http://www.ebu.ch/metadata/ontologies/skos/ebu_ParentalGuidanceCodeCS> ;
        skos:broader      parentalguidance:_22 ;
        skos:definition   "Specially recommended for children under 7"@en ;
        skos:definition   "Especial recomendado para la infancia"@es ;
        skos:prefLabel    "ERI"@en ;
        rdf:type          ebucore:TargetAudience .

parentalguidance:_36.2.5
        skos:example      "" ;
        skos:historyNote  "" ;
        skos:changeNote   "" ;
        skos:inScheme     <http://www.ebu.ch/metadata/ontologies/skos/ebu_ParentalGuidanceCodeCS> ;
        skos:broader      parentalguidance:_36.2 ;
        skos:prefLabel    "Horror or ritual scenes"@en ;
        rdf:type          ebucore:TargetAudience .

parentalguidance:_36.2.3
        skos:example      "" ;
        skos:historyNote  "" ;
        skos:changeNote   "" ;
        skos:inScheme     <http://www.ebu.ch/metadata/ontologies/skos/ebu_ParentalGuidanceCodeCS> ;
        skos:broader      parentalguidance:_36.2 ;
        skos:prefLabel    "Coarse language"@en ;
        rdf:type          ebucore:TargetAudience .

parentalguidance:_32.5
        skos:example      "" ;
        skos:historyNote  "" ;
        skos:changeNote   "" ;
        skos:inScheme     <http://www.ebu.ch/metadata/ontologies/skos/ebu_ParentalGuidanceCodeCS> ;
        skos:broader      parentalguidance:_32 ;
        skos:definition   "This rating is for programs that are not recommended to those\n         younger than 19."@en ;
        skos:prefLabel    "19"@en ;
        rdf:type          ebucore:TargetAudience .

parentalguidance:_35.2.2
        skos:example      "" ;
        skos:historyNote  "" ;
        skos:changeNote   "" ;
        skos:inScheme     <http://www.ebu.ch/metadata/ontologies/skos/ebu_ParentalGuidanceCodeCS> ;
        skos:broader      parentalguidance:_35.2 ;
        skos:prefLabel    "Sexualidad"@es ;
        skos:prefLabel    "Sexuality"@en ;
        rdf:type          ebucore:TargetAudience .

parentalguidance:_47.2.18
        skos:example      "" ;
        skos:historyNote  "" ;
        skos:changeNote   "" ;
        skos:inScheme     <http://www.ebu.ch/metadata/ontologies/skos/ebu_ParentalGuidanceCodeCS> ;
        skos:broader      parentalguidance:_47.2 ;
        skos:definition   "Brief and/or mild depictions of nudity" ;
        skos:prefLabel    "Partial Nudity"@en ;
        rdf:type          ebucore:TargetAudience .

parentalguidance:_33.2
        skos:example      "" ;
        skos:historyNote  "" ;
        skos:changeNote   "" ;
        skos:inScheme     <http://www.ebu.ch/metadata/ontologies/skos/ebu_ParentalGuidanceCodeCS> ;
        skos:broader      parentalguidance:_33 ;
        skos:definition   "Suitable for those aged 12 and over"@en ;
        skos:prefLabel    "12+"@en ;
        rdf:type          ebucore:TargetAudience .

parentalguidance:_35.1.5
        skos:example      "" ;
        skos:historyNote  "" ;
        skos:changeNote   "" ;
        skos:inScheme     <http://www.ebu.ch/metadata/ontologies/skos/ebu_ParentalGuidanceCodeCS> ;
        skos:broader      parentalguidance:_35.1 ;
        skos:definition   "Para adultos de 18 años en adelante. Programas aptos para\n         mayores de 18 años."@es ;
        skos:definition   "For ages 18 and above"@en ;
        skos:prefLabel    "C"@en ;
        rdf:type          ebucore:TargetAudience .

parentalguidance:_10.4
        skos:example      "" ;
        skos:historyNote  "" ;
        skos:changeNote   "" ;
        skos:inScheme     <http://www.ebu.ch/metadata/ontologies/skos/ebu_ParentalGuidanceCodeCS> ;
        skos:broader      parentalguidance:_10 ;
        skos:definition   "Suitable for people 18 years of age or older. Persons under 18\n         should view with an adult. No rental or purchase by those under 18. Parents strongly\n         cautioned. Will likely contain explicit violence, frequent coarse language, sexual activity\n         and/or horror."@en ;
        skos:prefLabel    "18A"@en ;
        rdf:type          ebucore:TargetAudience .

parentalguidance:_64.1.4
        skos:example      "" ;
        skos:historyNote  "" ;
        skos:changeNote   "" ;
        skos:inScheme     <http://www.ebu.ch/metadata/ontologies/skos/ebu_ParentalGuidanceCodeCS> ;
        skos:broader      parentalguidance:_64.1 ;
        skos:definition   "No one under the age of 12 admitted "@en ;
        skos:prefLabel    "12"@en ;
        rdf:type          ebucore:TargetAudience .

parentalguidance:_11.1
        skos:definition   "Le film peut être vu, loué ou acheté sans risque par des\n         personnes de tout âge"@fr ;
        rdf:type          ebucore:TargetAudience ;
        skos:definition   "General"@fr ;
        skos:definition   "For all ages"@en ;
        skos:example      "" ;
        skos:historyNote  "" ;
        skos:inScheme     <http://www.ebu.ch/metadata/ontologies/skos/ebu_ParentalGuidanceCodeCS> ;
        skos:broader      parentalguidance:_11 ;
        skos:prefLabel    "G"@fr ;
        skos:prefLabel    "G"@en ;
        skos:changeNote   "" .

parentalguidance:_31.1.4
        skos:changeNote   "" ;
        skos:historyNote  "" ;
        skos:prefLabel    "Orange"@en ;
        skos:example      "" ;
        skos:broader      parentalguidance:_31.1 ;
        skos:definition   "17 and over"@en ;
        rdf:type          ebucore:TargetAudience ;
        skos:prefLabel    "橙"@ja ;
        skos:prefLabel    "D"@en ;
        skos:inScheme     <http://www.ebu.ch/metadata/ontologies/skos/ebu_ParentalGuidanceCodeCS> ;
        skos:definition   "17歳以上のみ"@ja .

_:b3    rdf:rest   _:b4 ;
        rdf:first  parentalguidance:_19 .

parentalguidance:_8  skos:definition  "Canadian Home Video Rating System"@en ;
        skos:changeNote   "Update" ;
        skos:note         "Valid" ;
        skos:narrower     parentalguidance:_8.5 ;
        skos:narrower     parentalguidance:_8.1 ;
        rdf:type          ebucore:TargetAudience ;
        skos:narrower     parentalguidance:_8.6 ;
        skos:inScheme     <http://www.ebu.ch/metadata/ontologies/skos/ebu_ParentalGuidanceCodeCS> ;
        skos:prefLabel    "CA-CHVRS"@en ;
        skos:narrower     parentalguidance:_8.3 ;
        skos:example      "" ;
        skos:historyNote  "2009-07-27" ;
        skos:narrower     parentalguidance:_8.4 ;
        skos:scopeNote    "Region:Canada"@en ;
        skos:narrower     parentalguidance:_8.2 .

parentalguidance:_47.1.3
        skos:example      "" ;
        skos:historyNote  "" ;
        skos:changeNote   "" ;
        skos:inScheme     <http://www.ebu.ch/metadata/ontologies/skos/ebu_ParentalGuidanceCodeCS> ;
        skos:broader      parentalguidance:_47.1 ;
        skos:definition   "Titles rated E10+ (Everyone 10 and older) have content that may\n         be suitable for ages 10 and older. Titles in this category may contain more cartoon,\n         fantasy or mild violence, mild language and/or minimal suggestive themes" ;
        skos:prefLabel    "E10+"@en ;
        rdf:type          ebucore:TargetAudience .

parentalguidance:_44.3
        skos:example      "" ;
        skos:historyNote  "" ;
        skos:changeNote   "" ;
        skos:inScheme     <http://www.ebu.ch/metadata/ontologies/skos/ebu_ParentalGuidanceCodeCS> ;
        skos:broader      parentalguidance:_44 ;
        skos:definition   "Suitable for children of at least 11 years of\n         age"@en ;
        skos:prefLabel    "11"@en ;
        rdf:type          ebucore:TargetAudience .

parentalguidance:_2.4
        skos:example      "" ;
        skos:historyNote  "" ;
        skos:changeNote   "" ;
        skos:inScheme     <http://www.ebu.ch/metadata/ontologies/skos/ebu_ParentalGuidanceCodeCS> ;
        skos:broader      parentalguidance:_2 ;
        skos:definition   "12 years and above"@en ;
        skos:prefLabel    "12"@en ;
        rdf:type          ebucore:TargetAudience .

parentalguidance:_3.1
        skos:example      "" ;
        skos:historyNote  "" ;
        skos:changeNote   "" ;
        skos:inScheme     <http://www.ebu.ch/metadata/ontologies/skos/ebu_ParentalGuidanceCodeCS> ;
        skos:broader      parentalguidance:_3 ;
        skos:definition   "G classified films and computer games are for general viewing.\n         Many of the films and computer games contain content that would be of no interest to\n         children. The impact of the content is very mild."@en ;
        skos:prefLabel    "General"@en ;
        skos:prefLabel    "G"@en ;
        rdf:type          ebucore:TargetAudience .

parentalguidance:_22.2
        skos:example      "" ;
        skos:historyNote  "" ;
        skos:changeNote   "" ;
        skos:inScheme     <http://www.ebu.ch/metadata/ontologies/skos/ebu_ParentalGuidanceCodeCS> ;
        skos:broader      parentalguidance:_22 ;
        skos:definition   "Suitable for the general public"@en ;
        skos:definition   "Todos los publicos"@en ;
        skos:prefLabel    "TP"@en ;
        rdf:type          ebucore:TargetAudience .

parentalguidance:_60.1.3
        skos:example      "" ;
        skos:historyNote  "" ;
        skos:changeNote   "" ;
        skos:inScheme     <http://www.ebu.ch/metadata/ontologies/skos/ebu_ParentalGuidanceCodeCS> ;
        skos:broader      parentalguidance:_60.1 ;
        skos:definition   "BO (Bimbingan Orangtua): Parental Guidance (parental\n         supervision is recommended for persons under 13 years) "@en ;
        skos:prefLabel    "BO"@en ;
        rdf:type          ebucore:TargetAudience .

parentalguidance:_65.1.6
        skos:example      "" ;
        skos:historyNote  "" ;
        skos:changeNote   "" ;
        skos:inScheme     <http://www.ebu.ch/metadata/ontologies/skos/ebu_ParentalGuidanceCodeCS> ;
        skos:broader      parentalguidance:_65.1 ;
        skos:definition   "For views over 20 years old only "@en ;
        skos:prefLabel    "20+"@en ;
        rdf:type          ebucore:TargetAudience .

parentalguidance:_31.2.1
        skos:example      "" ;
        skos:historyNote  "" ;
        skos:changeNote   "" ;
        skos:inScheme     <http://www.ebu.ch/metadata/ontologies/skos/ebu_ParentalGuidanceCodeCS> ;
        skos:broader      parentalguidance:_31.2 ;
        skos:prefLabel    "Love"@en ;
        skos:prefLabel    "恋愛"@ja ;
        rdf:type          ebucore:TargetAudience .

parentalguidance:_36.2.2
        skos:example      "" ;
        skos:historyNote  "" ;
        skos:changeNote   "" ;
        skos:inScheme     <http://www.ebu.ch/metadata/ontologies/skos/ebu_ParentalGuidanceCodeCS> ;
        skos:broader      parentalguidance:_36.2 ;
        skos:prefLabel    "Sex"@en ;
        rdf:type          ebucore:TargetAudience .

parentalguidance:_66.1
        skos:example      "" ;
        skos:broader      parentalguidance:_66 ;
        skos:changeNote   "" ;
        rdf:type          ebucore:TargetAudience ;
        skos:narrower     parentalguidance:_66.1.5 ;
        skos:prefLabel    "Rating"@en ;
        skos:narrower     parentalguidance:_66.1.1 ;
        skos:historyNote  "" ;
        skos:inScheme     <http://www.ebu.ch/metadata/ontologies/skos/ebu_ParentalGuidanceCodeCS> ;
        skos:narrower     parentalguidance:_66.1.2 ;
        skos:narrower     parentalguidance:_66.1.3 ;
        skos:narrower     parentalguidance:_66.1.4 .

parentalguidance:_56.1.3
        skos:example      "" ;
        skos:historyNote  "" ;
        skos:changeNote   "" ;
        skos:inScheme     <http://www.ebu.ch/metadata/ontologies/skos/ebu_ParentalGuidanceCodeCS> ;
        skos:broader      parentalguidance:_56.1 ;
        skos:definition   "Public exhibition restricted to adults above 18 years only, "@en ;
        skos:prefLabel    "A"@en ;
        rdf:type          ebucore:TargetAudience .

parentalguidance:_47.2.29
        skos:example      "" ;
        skos:historyNote  "" ;
        skos:changeNote   "" ;
        skos:inScheme     <http://www.ebu.ch/metadata/ontologies/skos/ebu_ParentalGuidanceCodeCS> ;
        skos:broader      parentalguidance:_47.2 ;
        skos:definition   "The consumption or use of illegal drugs" ;
        skos:prefLabel    "Use of Drugs"@en ;
        rdf:type          ebucore:TargetAudience .

_:b1    rdf:rest   _:b2 ;
        rdf:first  parentalguidance:_27 .

parentalguidance:_33.1
        skos:example      "" ;
        skos:historyNote  "" ;
        skos:changeNote   "" ;
        skos:inScheme     <http://www.ebu.ch/metadata/ontologies/skos/ebu_ParentalGuidanceCodeCS> ;
        skos:broader      parentalguidance:_33 ;
        skos:definition   "Suitable for all ages"@en ;
        skos:prefLabel    "All"@en ;
        rdf:type          ebucore:TargetAudience .

parentalguidance:_32.4
        skos:example      "" ;
        skos:historyNote  "" ;
        skos:changeNote   "" ;
        skos:inScheme     <http://www.ebu.ch/metadata/ontologies/skos/ebu_ParentalGuidanceCodeCS> ;
        skos:broader      parentalguidance:_32 ;
        skos:definition   "This rating is for programs that contain material that may be\n         inappropriate for children under 15, and that parental discretion should be\n         used."@en ;
        skos:prefLabel    "15"@en ;
        rdf:type          ebucore:TargetAudience .

parentalguidance:_47.2.17
        skos:example      "" ;
        skos:historyNote  "" ;
        skos:changeNote   "" ;
        skos:inScheme     <http://www.ebu.ch/metadata/ontologies/skos/ebu_ParentalGuidanceCodeCS> ;
        skos:broader      parentalguidance:_47.2 ;
        skos:definition   "Graphic or prolonged depictions of nudity" ;
        skos:prefLabel    "Nudity"@en ;
        rdf:type          ebucore:TargetAudience .

parentalguidance:_64.1.7
        skos:example      "" ;
        skos:historyNote  "" ;
        skos:changeNote   "" ;
        skos:inScheme     <http://www.ebu.ch/metadata/ontologies/skos/ebu_ParentalGuidanceCodeCS> ;
        skos:broader      parentalguidance:_64.1 ;
        skos:definition   "No one under the age of 18 admitted "@en ;
        skos:prefLabel    "18"@en ;
        rdf:type          ebucore:TargetAudience .

parentalguidance:_10.1
        skos:example      "" ;
        skos:historyNote  "" ;
        skos:changeNote   "" ;
        skos:inScheme     <http://www.ebu.ch/metadata/ontologies/skos/ebu_ParentalGuidanceCodeCS> ;
        skos:broader      parentalguidance:_10 ;
        skos:definition   "Suitable for viewing by all ages"@en ;
        skos:prefLabel    "General"@en ;
        skos:prefLabel    "G"@en ;
        rdf:type          ebucore:TargetAudience .

parentalguidance:_5  skos:example  "" ;
        skos:historyNote  "" ;
        skos:changeNote   "" ;
        skos:narrower     parentalguidance:_5.2 ;
        skos:narrower     parentalguidance:_5.1 ;
        skos:inScheme     <http://www.ebu.ch/metadata/ontologies/skos/ebu_ParentalGuidanceCodeCS> ;
        skos:scopeNote    "Region:Belgium"@en ;
        skos:prefLabel    "BE"@en ;
        rdf:type          ebucore:TargetAudience .

parentalguidance:_24.4.1
        skos:example      "" ;
        skos:historyNote  "" ;
        skos:changeNote   "" ;
        skos:inScheme     <http://www.ebu.ch/metadata/ontologies/skos/ebu_ParentalGuidanceCodeCS> ;
        skos:broader      parentalguidance:_24.4 ;
        skos:definition   "Parental Guidance option - children 2 years of age under the K\n         limits may access the show in presence of an accompanying adult"@en ;
        skos:prefLabel    "PG"@en ;
        rdf:type          ebucore:TargetAudience .

parentalguidance:_44.2
        skos:example      "" ;
        skos:historyNote  "" ;
        skos:changeNote   "" ;
        skos:inScheme     <http://www.ebu.ch/metadata/ontologies/skos/ebu_ParentalGuidanceCodeCS> ;
        skos:broader      parentalguidance:_44 ;
        skos:definition   "Suitable for children of at least 7 years of\n         age"@en ;
        skos:prefLabel    "7"@en ;
        rdf:type          ebucore:TargetAudience .

parentalguidance:_47.1.2
        skos:example      "" ;
        skos:historyNote  "" ;
        skos:changeNote   "" ;
        skos:inScheme     <http://www.ebu.ch/metadata/ontologies/skos/ebu_ParentalGuidanceCodeCS> ;
        skos:broader      parentalguidance:_47.1 ;
        skos:definition   "Titles rated E (Everyone) have content that may be suitable for\n         ages 6 and older. Titles in this category may contain minimal cartoon, fantasy or mild\n         violence and/or infrequent use of mild language" ;
        skos:prefLabel    "E"@en ;
        rdf:type          ebucore:TargetAudience .

parentalguidance:_21.2
        skos:example      "" ;
        skos:historyNote  "" ;
        skos:changeNote   "" ;
        skos:inScheme     <http://www.ebu.ch/metadata/ontologies/skos/ebu_ParentalGuidanceCodeCS> ;
        skos:broader      parentalguidance:_21 ;
        skos:definition   "Adult supervision"@en ;
        skos:prefLabel    "Yellow"@en ;
        rdf:type          ebucore:TargetAudience .

parentalguidance:_65.1.3
        skos:example      "" ;
        skos:historyNote  "" ;
        skos:changeNote   "" ;
        skos:inScheme     <http://www.ebu.ch/metadata/ontologies/skos/ebu_ParentalGuidanceCodeCS> ;
        skos:broader      parentalguidance:_65.1 ;
        skos:definition   "No one under the age of 13 admitted "@en ;
        skos:prefLabel    "13+"@en ;
        rdf:type          ebucore:TargetAudience .

parentalguidance:_1.4
        skos:inScheme     <http://www.ebu.ch/metadata/ontologies/skos/ebu_ParentalGuidanceCodeCS> ;
        skos:definition   "Not under 18"@en ;
        skos:historyNote  "" ;
        skos:definition   "Apto para mayores de 18 años"@es ;
        rdf:type          ebucore:TargetAudience ;
        skos:prefLabel    "18"@es ;
        skos:prefLabel    "18"@en ;
        skos:example      "" ;
        skos:broader      parentalguidance:_1 ;
        skos:changeNote   "" .

parentalguidance:_31.1.1
        skos:changeNote   "" ;
        skos:prefLabel    "黒"@ja ;
        skos:definition   ""@ja ;
        skos:prefLabel    "A"@en ;
        skos:definition   "All ages"@en ;
        skos:broader      parentalguidance:_31.1 ;
        skos:historyNote  "" ;
        skos:prefLabel    "Black"@en ;
        skos:example      "" ;
        skos:inScheme     <http://www.ebu.ch/metadata/ontologies/skos/ebu_ParentalGuidanceCodeCS> ;
        rdf:type          ebucore:TargetAudience .

parentalguidance:_2.1
        skos:inScheme     <http://www.ebu.ch/metadata/ontologies/skos/ebu_ParentalGuidanceCodeCS> ;
        skos:definition   "For all ages"@en ;
        skos:changeNote   "" ;
        skos:broader      parentalguidance:_2 ;
        rdf:type          ebucore:TargetAudience ;
        skos:prefLabel    "None"@en ;
        skos:definition   "Freigegeben fur alle Altersstufen"@de ;
        skos:historyNote  "" ;
        skos:prefLabel    "Ohne"@de ;
        skos:example      "" .

parentalguidance:_36.1.4
        skos:example      "" ;
        skos:historyNote  "" ;
        skos:changeNote   "" ;
        skos:inScheme     <http://www.ebu.ch/metadata/ontologies/skos/ebu_ParentalGuidanceCodeCS> ;
        skos:broader      parentalguidance:_36.1 ;
        skos:definition   "Suitable for viewing by persons over 15 years of\n         age"@en ;
        skos:prefLabel    "15"@en ;
        rdf:type          ebucore:TargetAudience .

parentalguidance:_36.1.6
        skos:example      "" ;
        skos:historyNote  "" ;
        skos:changeNote   "" ;
        skos:inScheme     <http://www.ebu.ch/metadata/ontologies/skos/ebu_ParentalGuidanceCodeCS> ;
        skos:broader      parentalguidance:_36.1 ;
        skos:definition   "not suitable for viewing by persons under 18 years of age with\n         certain sensitvities to classification criteria"@en ;
        skos:prefLabel    "RE"@en ;
        rdf:type          ebucore:TargetAudience .

parentalguidance:_36.2.1
        skos:example      "" ;
        skos:historyNote  "" ;
        skos:changeNote   "" ;
        skos:inScheme     <http://www.ebu.ch/metadata/ontologies/skos/ebu_ParentalGuidanceCodeCS> ;
        skos:broader      parentalguidance:_36.2 ;
        skos:prefLabel    "Violence"@en ;
        rdf:type          ebucore:TargetAudience .

parentalguidance:_56.1.2
        skos:example      "" ;
        skos:historyNote  "" ;
        skos:changeNote   "" ;
        skos:inScheme     <http://www.ebu.ch/metadata/ontologies/skos/ebu_ParentalGuidanceCodeCS> ;
        skos:broader      parentalguidance:_56.1 ;
        skos:definition   "Unrestricted public exhibition with parental guidance for\n         children below the age of 12 "@en ;
        skos:prefLabel    "U/A"@en ;
        rdf:type          ebucore:TargetAudience .

parentalguidance:_47.2.16
        skos:example      "" ;
        skos:historyNote  "" ;
        skos:changeNote   "" ;
        skos:inScheme     <http://www.ebu.ch/metadata/ontologies/skos/ebu_ParentalGuidanceCodeCS> ;
        skos:broader      parentalguidance:_47.2 ;
        skos:definition   "Mild scenes depicting characters in unsafe and/or violent\n         situations" ;
        skos:prefLabel    "Mild Violence"@en ;
        rdf:type          ebucore:TargetAudience .

parentalguidance:_35.2.4
        skos:example      "" ;
        skos:historyNote  "" ;
        skos:changeNote   "" ;
        skos:inScheme     <http://www.ebu.ch/metadata/ontologies/skos/ebu_ParentalGuidanceCodeCS> ;
        skos:broader      parentalguidance:_35.2 ;
        skos:prefLabel    "Drugs and aclohol"@en ;
        skos:prefLabel    "Adicciones"@es ;
        rdf:type          ebucore:TargetAudience .

parentalguidance:_47.2.28
        skos:example      "" ;
        skos:historyNote  "" ;
        skos:changeNote   "" ;
        skos:inScheme     <http://www.ebu.ch/metadata/ontologies/skos/ebu_ParentalGuidanceCodeCS> ;
        skos:broader      parentalguidance:_47.2 ;
        skos:definition   "Reference to and/or images of tobacco products" ;
        skos:prefLabel    "Tobacco Reference"@en ;
        rdf:type          ebucore:TargetAudience .

parentalguidance:_32.3
        skos:example      "" ;
        skos:historyNote  "" ;
        skos:changeNote   "" ;
        skos:inScheme     <http://www.ebu.ch/metadata/ontologies/skos/ebu_ParentalGuidanceCodeCS> ;
        skos:broader      parentalguidance:_32 ;
        skos:definition   "This rating is for programs that may contain material\n         inappropriate for those younger than 12, and parental discretion should be used. Usually\n         used for animations that have stronger themes or violence then those designed for\n         childrens, or for reality variety programs that have mild violence, theme, or\n         language."@en ;
        skos:prefLabel    "12"@en ;
        rdf:type          ebucore:TargetAudience .

parentalguidance:_64.1.6
        skos:example      "" ;
        skos:historyNote  "" ;
        skos:changeNote   "" ;
        skos:inScheme     <http://www.ebu.ch/metadata/ontologies/skos/ebu_ParentalGuidanceCodeCS> ;
        skos:broader      parentalguidance:_64.1 ;
        skos:definition   "No one under the age of 16 admitted "@en ;
        skos:prefLabel    "16"@en ;
        rdf:type          ebucore:TargetAudience .

parentalguidance:_10.2
        skos:example      "" ;
        skos:historyNote  "" ;
        skos:changeNote   "" ;
        skos:inScheme     <http://www.ebu.ch/metadata/ontologies/skos/ebu_ParentalGuidanceCodeCS> ;
        skos:broader      parentalguidance:_10 ;
        skos:definition   "Parental guidance advised. Theme or content may not be suitable\n         for all children."@en ;
        skos:prefLabel    "Parental Guidance"@en ;
        skos:altLabel     "PG"@en ;
        rdf:type          ebucore:TargetAudience .

parentalguidance:_6  rdf:type  ebucore:TargetAudience ;
        skos:historyNote  "2009-07-27" ;
        skos:changeNote   "Update" ;
        skos:scopeNote    "Region:Bulgaria"@en ;
        skos:prefLabel    "BG-FIA"@en ;
        skos:definition   "National Film Rating Committee"@en ;
        skos:narrower     parentalguidance:_6.2 ;
        skos:inScheme     <http://www.ebu.ch/metadata/ontologies/skos/ebu_ParentalGuidanceCodeCS> ;
        skos:narrower     parentalguidance:_6.3 ;
        skos:example      "" ;
        skos:narrower     parentalguidance:_6.4 ;
        skos:narrower     parentalguidance:_6.5 ;
        skos:note         "Valid" ;
        skos:altLabel     "BG-NFRC"@en ;
        skos:definition   "Film Industry Act"@en ;
        skos:narrower     parentalguidance:_6.1 .

parentalguidance:_42.7
        skos:example      "" ;
        skos:historyNote  "" ;
        skos:changeNote   "" ;
        skos:inScheme     <http://www.ebu.ch/metadata/ontologies/skos/ebu_ParentalGuidanceCodeCS> ;
        skos:broader      parentalguidance:_42 ;
        skos:definition   "Os espectáculos que, pelos seus aspectos artístico, temático,\n         pedagógico e técnico mereçam esse atributo."@pt ;
        skos:definition   "Of quality from an artistic, thematic, pedagogic or technical\n         realisation perspective"@en ;
        skos:prefLabel    "De Qualidade"@en ;
        rdf:type          ebucore:TargetAudience .

parentalguidance:_60.1.1
        skos:example      "" ;
        skos:historyNote  "" ;
        skos:changeNote   "" ;
        skos:inScheme     <http://www.ebu.ch/metadata/ontologies/skos/ebu_ParentalGuidanceCodeCS> ;
        skos:broader      parentalguidance:_60.1 ;
        skos:definition   "(Semua Umur): All ages "@en ;
        skos:prefLabel    "SU"@en ;
        rdf:type          ebucore:TargetAudience .

parentalguidance:_43.4
        skos:example      "" ;
        skos:historyNote  "" ;
        skos:changeNote   "" ;
        skos:inScheme     <http://www.ebu.ch/metadata/ontologies/skos/ebu_ParentalGuidanceCodeCS> ;
        skos:broader      parentalguidance:_43 ;
        skos:definition   "For persons of age 16 and above."@en ;
        skos:prefLabel    "16"@en ;
        rdf:type          ebucore:TargetAudience .

parentalguidance:_65.1.4
        skos:example      "" ;
        skos:historyNote  "" ;
        skos:changeNote   "" ;
        skos:inScheme     <http://www.ebu.ch/metadata/ontologies/skos/ebu_ParentalGuidanceCodeCS> ;
        skos:broader      parentalguidance:_65.1 ;
        skos:definition   "No one under the age of 15 admitted "@en ;
        skos:prefLabel    "15+"@en ;
        rdf:type          ebucore:TargetAudience .

parentalguidance:_21.3
        skos:example      "" ;
        skos:historyNote  "" ;
        skos:changeNote   "" ;
        skos:inScheme     <http://www.ebu.ch/metadata/ontologies/skos/ebu_ParentalGuidanceCodeCS> ;
        skos:broader      parentalguidance:_21 ;
        skos:definition   "Adult"@en ;
        skos:prefLabel    "Red"@en ;
        rdf:type          ebucore:TargetAudience .

parentalguidance:_44.1
        skos:example      "" ;
        skos:historyNote  "" ;
        skos:changeNote   "" ;
        skos:inScheme     <http://www.ebu.ch/metadata/ontologies/skos/ebu_ParentalGuidanceCodeCS> ;
        skos:broader      parentalguidance:_44 ;
        skos:definition   "Suitable for all ages"@en ;
        skos:definition   "Barntillåten"@sv ;
        skos:prefLabel    "Btl"@en ;
        rdf:type          ebucore:TargetAudience .

parentalguidance:_1.5
        skos:example      "" ;
        skos:historyNote  "" ;
        skos:changeNote   "" ;
        skos:inScheme     <http://www.ebu.ch/metadata/ontologies/skos/ebu_ParentalGuidanceCodeCS> ;
        skos:broader      parentalguidance:_1 ;
        skos:definition   "Explicit"@en ;
        skos:prefLabel    "X"@en ;
        rdf:type          ebucore:TargetAudience .

parentalguidance:_2.2
        skos:example      "" ;
        skos:historyNote  "" ;
        skos:changeNote   "" ;
        skos:inScheme     <http://www.ebu.ch/metadata/ontologies/skos/ebu_ParentalGuidanceCodeCS> ;
        skos:broader      parentalguidance:_2 ;
        skos:definition   "6 years and above"@en ;
        skos:prefLabel    "6"@en ;
        rdf:type          ebucore:TargetAudience .

parentalguidance:_47.1.1
        skos:example      "" ;
        skos:historyNote  "" ;
        skos:changeNote   "" ;
        skos:inScheme     <http://www.ebu.ch/metadata/ontologies/skos/ebu_ParentalGuidanceCodeCS> ;
        skos:broader      parentalguidance:_47.1 ;
        skos:definition   "Titles rated EC (Early Childhood) have content that may be\n         suitable for ages 3 and older. Contains no material that parents would find\n         inappropriate" ;
        skos:prefLabel    "EC"@en ;
        rdf:type          ebucore:TargetAudience .

parentalguidance:_36.1.5
        skos:example      "" ;
        skos:historyNote  "" ;
        skos:changeNote   "" ;
        skos:inScheme     <http://www.ebu.ch/metadata/ontologies/skos/ebu_ParentalGuidanceCodeCS> ;
        skos:broader      parentalguidance:_36.1 ;
        skos:definition   "Suitable for viewing by persons over 18 years of\n         ages"@en ;
        skos:prefLabel    "18"@en ;
        rdf:type          ebucore:TargetAudience .

parentalguidance:_31.1.2
        skos:prefLabel    "Green"@en ;
        skos:example      "" ;
        rdf:type          ebucore:TargetAudience ;
        skos:definition   "12 and over"@en ;
        skos:broader      parentalguidance:_31.1 ;
        skos:prefLabel    "緑"@ja ;
        skos:changeNote   "" ;
        skos:definition   "12歳以上のみ"@ja ;
        skos:inScheme     <http://www.ebu.ch/metadata/ontologies/skos/ebu_ParentalGuidanceCodeCS> ;
        skos:prefLabel    "B"@en ;
        skos:historyNote  "" .

parentalguidance:_64.1
        skos:broader      parentalguidance:_64 ;
        skos:historyNote  "" ;
        skos:narrower     parentalguidance:_64.1.2 ;
        skos:inScheme     <http://www.ebu.ch/metadata/ontologies/skos/ebu_ParentalGuidanceCodeCS> ;
        skos:narrower     parentalguidance:_64.1.1 ;
        skos:narrower     parentalguidance:_64.1.6 ;
        skos:narrower     parentalguidance:_64.1.7 ;
        skos:narrower     parentalguidance:_64.1.5 ;
        skos:example      "" ;
        rdf:type          ebucore:TargetAudience ;
        skos:narrower     parentalguidance:_64.1.4 ;
        skos:narrower     parentalguidance:_64.1.3 ;
        skos:prefLabel    "Rating"@en ;
        skos:changeNote   "" .

parentalguidance:_41.1
        skos:example      "" ;
        skos:historyNote  "" ;
        skos:changeNote   "" ;
        skos:inScheme     <http://www.ebu.ch/metadata/ontologies/skos/ebu_ParentalGuidanceCodeCS> ;
        skos:broader      parentalguidance:_41 ;
        skos:definition   "For all audiences"@en ;
        skos:prefLabel    "G"@en ;
        rdf:type          ebucore:TargetAudience .

parentalguidance:_40.4
        skos:example      "" ;
        skos:historyNote  "" ;
        skos:changeNote   "" ;
        skos:inScheme     <http://www.ebu.ch/metadata/ontologies/skos/ebu_ParentalGuidanceCodeCS> ;
        skos:broader      parentalguidance:_40 ;
        skos:definition   "Only those who are 13 and above may view an “R-13”\n         film."@en ;
        skos:prefLabel    "R-18"@en ;
        rdf:type          ebucore:TargetAudience .

parentalguidance:_47.2.15
        skos:example      "" ;
        skos:historyNote  "" ;
        skos:changeNote   "" ;
        skos:inScheme     <http://www.ebu.ch/metadata/ontologies/skos/ebu_ParentalGuidanceCodeCS> ;
        skos:broader      parentalguidance:_47.2 ;
        skos:definition   "Depictions or dialogue involving \"adult\" humour, including sexual\n         references" ;
        skos:prefLabel    "Mature Humour"@en ;
        rdf:type          ebucore:TargetAudience .

parentalguidance:_39.5
        skos:example      "" ;
        skos:historyNote  "" ;
        skos:changeNote   "" ;
        skos:inScheme     <http://www.ebu.ch/metadata/ontologies/skos/ebu_ParentalGuidanceCodeCS> ;
        skos:broader      parentalguidance:_39 ;
        skos:definition   "Suitable to persons 15 years of age and over (awarded by the\n         Office of Film and Literature Classification only)"@en ;
        skos:prefLabel    "R15"@en ;
        rdf:type          ebucore:TargetAudience .

parentalguidance:_51.1.2
        skos:example      "" ;
        skos:historyNote  "" ;
        skos:changeNote   "" ;
        skos:inScheme     <http://www.ebu.ch/metadata/ontologies/skos/ebu_ParentalGuidanceCodeCS> ;
        skos:broader      parentalguidance:_51.1 ;
        skos:definition   "A category with content that may be disturbing to or\n         inappropriate for children"@en ;
        skos:prefLabel    "PG"@en ;
        rdf:type          ebucore:TargetAudience .

parentalguidance:_47.2.27
        skos:example      "" ;
        skos:historyNote  "" ;
        skos:changeNote   "" ;
        skos:inScheme     <http://www.ebu.ch/metadata/ontologies/skos/ebu_ParentalGuidanceCodeCS> ;
        skos:broader      parentalguidance:_47.2 ;
        skos:definition   "Mild provocative references or materials" ;
        skos:prefLabel    "Suggestive Themes"@en ;
        rdf:type          ebucore:TargetAudience .

parentalguidance:_53.1.3
        skos:example      "" ;
        skos:historyNote  "" ;
        skos:changeNote   "" ;
        skos:inScheme     <http://www.ebu.ch/metadata/ontologies/skos/ebu_ParentalGuidanceCodeCS> ;
        skos:broader      parentalguidance:_53.1 ;
        skos:definition   ""@en ;
        skos:prefLabel    "15"@en ;
        rdf:type          ebucore:TargetAudience .

parentalguidance:_17.2
        skos:example      "" ;
        skos:historyNote  "" ;
        skos:changeNote   "" ;
        skos:inScheme     <http://www.ebu.ch/metadata/ontologies/skos/ebu_ParentalGuidanceCodeCS> ;
        skos:broader      parentalguidance:_17 ;
        skos:definition   "Suitable for people aged 7 and over"@en ;
        skos:prefLabel    "7"@en ;
        rdf:type          ebucore:TargetAudience .

parentalguidance:_41  skos:example  "" ;
        skos:narrower     parentalguidance:_41.2 ;
        skos:narrower     parentalguidance:_41.4 ;
        skos:historyNote  "2009-07-28" ;
        skos:narrower     parentalguidance:_41.1 ;
        skos:narrower     parentalguidance:_41.3 ;
        skos:definition   "Scheme as used by the Radio Telewisja Polska"@en ;
        skos:prefLabel    "PL-RTP"@en ;
        skos:scopeNote    "Region:Portugal"@en ;
        rdf:type          ebucore:TargetAudience ;
        skos:narrower     parentalguidance:_41.5 ;
        skos:changeNote   "Update" ;
        skos:note         "Valid" ;
        skos:inScheme     <http://www.ebu.ch/metadata/ontologies/skos/ebu_ParentalGuidanceCodeCS> .

parentalguidance:_16.2.6
        skos:example      "" ;
        skos:historyNote  "" ;
        skos:changeNote   "" ;
        skos:inScheme     <http://www.ebu.ch/metadata/ontologies/skos/ebu_ParentalGuidanceCodeCS> ;
        skos:broader      parentalguidance:_16.2 ;
        skos:prefLabel    "Dangerous behaviour"@en ;
        rdf:type          ebucore:TargetAudience .

parentalguidance:_52.2
        skos:inScheme     <http://www.ebu.ch/metadata/ontologies/skos/ebu_ParentalGuidanceCodeCS> ;
        skos:example      "" ;
        skos:historyNote  "2019-06-24" ;
        skos:definition   "Freigegeben ab 6 Jahren"@de ;
        skos:changeNote   "Change termId from 18.x to 52.x" ;
        skos:definition   "No one under 6 years admitted"@en ;
        skos:prefLabel    "6+"@de ;
        skos:prefLabel    "6+"@en ;
        rdf:type          ebucore:TargetAudience ;
        skos:broader      parentalguidance:_52 .

parentalguidance:_31.2.4
        skos:example      "" ;
        skos:historyNote  "" ;
        skos:changeNote   "" ;
        skos:inScheme     <http://www.ebu.ch/metadata/ontologies/skos/ebu_ParentalGuidanceCodeCS> ;
        skos:broader      parentalguidance:_31.2 ;
        skos:prefLabel    "Surnatural"@en ;
        skos:prefLabel    "恐怖"@ja ;
        rdf:type          ebucore:TargetAudience .

parentalguidance:_65  skos:scopeNote  "Region:Thailand"@en ;
        skos:note         "Valid" ;
        skos:example      "" ;
        skos:definition   ""@en ;
        rdf:type          ebucore:TargetAudience ;
        skos:changeNote   "Update" ;
        skos:inScheme     <http://www.ebu.ch/metadata/ontologies/skos/ebu_ParentalGuidanceCodeCS> ;
        skos:historyNote  "2010-08-03" ;
        skos:prefLabel    "TH"@en ;
        skos:narrower     parentalguidance:_65.1 .

parentalguidance:_55.1.4
        skos:example      "" ;
        skos:historyNote  "" ;
        skos:changeNote   "" ;
        skos:inScheme     <http://www.ebu.ch/metadata/ontologies/skos/ebu_ParentalGuidanceCodeCS> ;
        skos:broader      parentalguidance:_55.1 ;
        skos:definition   "Passed only for 14 and older "@en ;
        skos:prefLabel    "14"@en ;
        rdf:type          ebucore:TargetAudience .

parentalguidance:_53  skos:definition  ""@en ;
        skos:scopeNote    "Region:Czech republic"@en ;
        skos:narrower     parentalguidance:_53.1 ;
        skos:example      "" ;
        rdf:type          ebucore:TargetAudience ;
        skos:changeNote   "Update" ;
        skos:prefLabel    "CZ-Film"@en ;
        skos:historyNote  "2010-08-03" ;
        skos:inScheme     <http://www.ebu.ch/metadata/ontologies/skos/ebu_ParentalGuidanceCodeCS> ;
        skos:note         "Valid" .

parentalguidance:_28.3
        skos:example      "" ;
        skos:historyNote  "" ;
        skos:changeNote   "" ;
        skos:inScheme     <http://www.ebu.ch/metadata/ontologies/skos/ebu_ParentalGuidanceCodeCS> ;
        skos:broader      parentalguidance:_28 ;
        skos:definition   "Films classified in this category are considered to be suitable\n         for those of twelve and upwards. They may also be seen by younger children provided a\n         parent or adult guardian accompanies them."@en ;
        skos:prefLabel    "12A"@en ;
        rdf:type          ebucore:TargetAudience .

parentalguidance:_65.1.1
        skos:example      "" ;
        skos:historyNote  "" ;
        skos:changeNote   "" ;
        skos:inScheme     <http://www.ebu.ch/metadata/ontologies/skos/ebu_ParentalGuidanceCodeCS> ;
        skos:broader      parentalguidance:_65.1 ;
        skos:definition   "Promotional, film is educational and viewing is encouraged for\n         all Thai people.."@en ;
        skos:prefLabel    "P"@en ;
        rdf:type          ebucore:TargetAudience .

parentalguidance:_27.6
        skos:example      "" ;
        skos:historyNote  "" ;
        skos:changeNote   "" ;
        skos:inScheme     <http://www.ebu.ch/metadata/ontologies/skos/ebu_ParentalGuidanceCodeCS> ;
        skos:broader      parentalguidance:_27 ;
        skos:definition   "To be supplied only in licensed sex shops or cinemas to adults\n         of not less than 18 years of age"@en ;
        skos:prefLabel    "R18"@en ;
        rdf:type          ebucore:TargetAudience .

parentalguidance:_6.3
        skos:example      "" ;
        skos:historyNote  "" ;
        skos:changeNote   "" ;
        skos:inScheme     <http://www.ebu.ch/metadata/ontologies/skos/ebu_ParentalGuidanceCodeCS> ;
        skos:broader      parentalguidance:_6 ;
        skos:definition   "For 12 and over - When the film contains certain erotic scenes\n         or scenes with drinking, taking drugs or stimulants or a few scenes of\n         violence"@en ;
        skos:prefLabel    "C"@en ;
        rdf:type          ebucore:TargetAudience .

parentalguidance:_39.6
        skos:example      "" ;
        skos:historyNote  "" ;
        skos:changeNote   "" ;
        skos:inScheme     <http://www.ebu.ch/metadata/ontologies/skos/ebu_ParentalGuidanceCodeCS> ;
        skos:broader      parentalguidance:_39 ;
        skos:definition   "Suitable to persons 16 years of age and over (awarded by the\n         Office of Film and Literature Classification only)"@en ;
        skos:prefLabel    "R16"@en ;
        rdf:type          ebucore:TargetAudience .

parentalguidance:_40.3
        skos:example      "" ;
        skos:historyNote  "" ;
        skos:changeNote   "" ;
        skos:inScheme     <http://www.ebu.ch/metadata/ontologies/skos/ebu_ParentalGuidanceCodeCS> ;
        skos:broader      parentalguidance:_40 ;
        skos:definition   "Only those who are 13 and above may view an “R-13”\n         film."@en ;
        skos:prefLabel    "R-13"@en ;
        rdf:type          ebucore:TargetAudience .

parentalguidance:_47.2.14
        skos:example      "" ;
        skos:historyNote  "" ;
        skos:changeNote   "" ;
        skos:inScheme     <http://www.ebu.ch/metadata/ontologies/skos/ebu_ParentalGuidanceCodeCS> ;
        skos:broader      parentalguidance:_47.2 ;
        skos:definition   "Mild references to profanity, sexuality, violence, alcohol or\n         drug use in music" ;
        skos:prefLabel    "Lyrics"@en ;
        rdf:type          ebucore:TargetAudience .

parentalguidance:_39.4
        skos:example      "" ;
        skos:historyNote  "" ;
        skos:changeNote   "" ;
        skos:inScheme     <http://www.ebu.ch/metadata/ontologies/skos/ebu_ParentalGuidanceCodeCS> ;
        skos:broader      parentalguidance:_39 ;
        skos:definition   "Suitable to persons 13 years of age and over (awarded by the\n         Office of Film and Literature Classification only)"@en ;
        skos:prefLabel    "R13"@en ;
        rdf:type          ebucore:TargetAudience .

parentalguidance:_47.2.26
        skos:example      "" ;
        skos:historyNote  "" ;
        skos:changeNote   "" ;
        skos:inScheme     <http://www.ebu.ch/metadata/ontologies/skos/ebu_ParentalGuidanceCodeCS> ;
        skos:broader      parentalguidance:_47.2 ;
        skos:definition   "Graphic references to and/or depictions of sexual behaviour,\n         possibly including nudity" ;
        skos:prefLabel    "Strong Sexual Content"@en ;
        rdf:type          ebucore:TargetAudience .

parentalguidance:_16.2.7
        skos:example      "" ;
        skos:historyNote  "" ;
        skos:changeNote   "" ;
        skos:inScheme     <http://www.ebu.ch/metadata/ontologies/skos/ebu_ParentalGuidanceCodeCS> ;
        skos:broader      parentalguidance:_16.2 ;
        skos:prefLabel    "Hanging scenes"@en ;
        rdf:type          ebucore:TargetAudience .

parentalguidance:_51.1.1
        skos:example      "" ;
        skos:historyNote  "" ;
        skos:changeNote   "" ;
        skos:inScheme     <http://www.ebu.ch/metadata/ontologies/skos/ebu_ParentalGuidanceCodeCS> ;
        skos:broader      parentalguidance:_51.1 ;
        skos:definition   "All ages"@en ;
        skos:prefLabel    "A"@en ;
        rdf:type          ebucore:TargetAudience .

parentalguidance:_17.3
        skos:example      "" ;
        skos:historyNote  "" ;
        skos:changeNote   "" ;
        skos:inScheme     <http://www.ebu.ch/metadata/ontologies/skos/ebu_ParentalGuidanceCodeCS> ;
        skos:broader      parentalguidance:_17 ;
        skos:definition   "Suitable for people aged 12 and over"@en ;
        skos:prefLabel    "12"@en ;
        rdf:type          ebucore:TargetAudience .

parentalguidance:_53.1.4
        skos:example      "" ;
        skos:historyNote  "" ;
        skos:changeNote   "" ;
        skos:inScheme     <http://www.ebu.ch/metadata/ontologies/skos/ebu_ParentalGuidanceCodeCS> ;
        skos:broader      parentalguidance:_53.1 ;
        skos:definition   ""@en ;
        skos:prefLabel    "18"@en ;
        rdf:type          ebucore:TargetAudience .

parentalguidance:_30  skos:inScheme  <http://www.ebu.ch/metadata/ontologies/skos/ebu_ParentalGuidanceCodeCS> ;
        skos:note         "Valid" ;
        skos:example      "" ;
        skos:changeNote   "Update" ;
        skos:narrower     parentalguidance:_30.1 ;
        skos:narrower     parentalguidance:_30.3 ;
        skos:definition   "Rating used by Radio Televisione Italiana"@en ;
        skos:prefLabel    "IT-RAI"@en ;
        skos:historyNote  "2009-07-27" ;
        skos:narrower     parentalguidance:_30.2 ;
        rdf:type          ebucore:TargetAudience ;
        skos:scopeNote    "Region:Italy"@en .

parentalguidance:_66  rdf:type  ebucore:TargetAudience ;
        skos:example      "" ;
        skos:historyNote  "2019-06-24" ;
        skos:prefLabel    "UAB"@en ;
        skos:scopeNote    "Region:United Arab Emirates"@en ;
        skos:changeNote   "Correct subterm termId starting with 65.x into\n         66.x" ;
        skos:definition   ""@en ;
        skos:note         "Valid" ;
        skos:narrower     parentalguidance:_66.1 ;
        skos:inScheme     <http://www.ebu.ch/metadata/ontologies/skos/ebu_ParentalGuidanceCodeCS> .

parentalguidance:_55.1.3
        skos:example      "" ;
        skos:historyNote  "" ;
        skos:changeNote   "" ;
        skos:inScheme     <http://www.ebu.ch/metadata/ontologies/skos/ebu_ParentalGuidanceCodeCS> ;
        skos:broader      parentalguidance:_55.1 ;
        skos:definition   "Passed only for 12 and older "@en ;
        skos:prefLabel    "12"@en ;
        rdf:type          ebucore:TargetAudience .

parentalguidance:_54  skos:historyNote  "2010-08-03" ;
        skos:scopeNote    "Region:Hungary"@en ;
        skos:inScheme     <http://www.ebu.ch/metadata/ontologies/skos/ebu_ParentalGuidanceCodeCS> ;
        skos:note         "Valid" ;
        skos:definition   "National Film Office"@en ;
        skos:example      "" ;
        rdf:type          ebucore:TargetAudience ;
        skos:narrower     parentalguidance:_54.1 ;
        skos:changeNote   "Update" ;
        skos:prefLabel    "HU-Film"@en .

parentalguidance:_31.2.5
        skos:example      "" ;
        skos:historyNote  "" ;
        skos:changeNote   "" ;
        skos:inScheme     <http://www.ebu.ch/metadata/ontologies/skos/ebu_ParentalGuidanceCodeCS> ;
        skos:broader      parentalguidance:_31.2 ;
        skos:prefLabel    "Alcohol & Tobacco"@en ;
        skos:prefLabel    "飲酒・喫煙"@ja ;
        rdf:type          ebucore:TargetAudience .

parentalguidance:_42  skos:narrower  parentalguidance:_42.2 ;
        skos:narrower     parentalguidance:_42.4 ;
        skos:scopeNote    "Region:Portugal"@en ;
        skos:definition   "Scheme as defined by the Comissão de Classificação de\n         Espectáculos"@en ;
        skos:narrower     parentalguidance:_42.3 ;
        skos:historyNote  "2009-07-28" ;
        skos:inScheme     <http://www.ebu.ch/metadata/ontologies/skos/ebu_ParentalGuidanceCodeCS> ;
        skos:narrower     parentalguidance:_42.5 ;
        skos:narrower     parentalguidance:_42.6 ;
        skos:note         "Valid" ;
        skos:example      "" ;
        rdf:type          ebucore:TargetAudience ;
        skos:prefLabel    "PT-CCE"@en ;
        skos:changeNote   "Update" ;
        skos:narrower     parentalguidance:_42.7 ;
        skos:narrower     parentalguidance:_42.1 .

parentalguidance:_52.1
        skos:definition   "Ohne Altersbeschränkung"@de ;
        skos:example      "" ;
        skos:changeNote   "Change termId from 18.x to 52.x" ;
        skos:prefLabel    "ALL"@en ;
        skos:prefLabel    "ALL AGES"@de ;
        skos:inScheme     <http://www.ebu.ch/metadata/ontologies/skos/ebu_ParentalGuidanceCodeCS> ;
        skos:definition   "For all ages"@en ;
        rdf:type          ebucore:TargetAudience ;
        skos:broader      parentalguidance:_52 ;
        skos:historyNote  "2019-06-24" .

parentalguidance:_29.1
        skos:changeNote   "" ;
        rdf:type          ebucore:TargetAudience ;
        skos:example      "" ;
        skos:prefLabel    "GA"@en ;
        skos:inScheme     <http://www.ebu.ch/metadata/ontologies/skos/ebu_ParentalGuidanceCodeCS> ;
        skos:historyNote  "" ;
        skos:prefLabel    "General Audience"@en ;
        skos:prefLabel    "Lucht Féachana Ginearálta"@ga ;
        skos:definition   "A programme that would be acceptable to all ages and\n         tastes."@en ;
        skos:broader      parentalguidance:_29 .

parentalguidance:_50.7
        skos:hiddenLabel  "adult"@en ;
        skos:example      "" ;
        skos:historyNote  "" ;
        skos:changeNote   "" ;
        skos:inScheme     <http://www.ebu.ch/metadata/ontologies/skos/ebu_ParentalGuidanceCodeCS> ;
        skos:broader      parentalguidance:_50 ;
        skos:definition   "Mature audience only"@en ;
        skos:prefLabel    "TV-MA"@en ;
        rdf:type          ebucore:TargetAudience .

parentalguidance:_6.4
        skos:example      "" ;
        skos:historyNote  "" ;
        skos:changeNote   "" ;
        skos:inScheme     <http://www.ebu.ch/metadata/ontologies/skos/ebu_ParentalGuidanceCodeCS> ;
        skos:broader      parentalguidance:_6 ;
        skos:definition   "For 16 and over - When the film contains quite a number of\n         erotic scenes or scenes with drinking, taking drugs or stimulants or a considerable number\n         of scenes showing violence"@en ;
        skos:prefLabel    "D"@en ;
        skos:prefLabel    "D"@po ;
        rdf:type          ebucore:TargetAudience .

parentalguidance:_28.4
        skos:example      "" ;
        skos:historyNote  "" ;
        skos:changeNote   "" ;
        skos:inScheme     <http://www.ebu.ch/metadata/ontologies/skos/ebu_ParentalGuidanceCodeCS> ;
        skos:broader      parentalguidance:_28 ;
        skos:definition   "Films classified in this category are considered to be suitable\n         for those of fifteen and upwards. They may also be seen by younger children provided a\n         parent or adult guardian accompanies them."@en ;
        skos:prefLabel    "15A"@en ;
        rdf:type          ebucore:TargetAudience .

parentalguidance:_65.1.2
        skos:example      "" ;
        skos:historyNote  "" ;
        skos:changeNote   "" ;
        skos:inScheme     <http://www.ebu.ch/metadata/ontologies/skos/ebu_ParentalGuidanceCodeCS> ;
        skos:broader      parentalguidance:_65.1 ;
        skos:definition   "Suitable for general audiences "@en ;
        skos:prefLabel    "G"@en ;
        rdf:type          ebucore:TargetAudience .

parentalguidance:_7.1
        rdf:type          ebucore:TargetAudience ;
        skos:example      "" ;
        skos:definition   "Especially Recommended for Children and Adolescents. This\n         rating means that the film is especially advised for children and adolescents. Contains\n         educational material, and doesn't have any inappropriate content. "@en ;
        skos:broader      parentalguidance:_7 ;
        skos:changeNote   "" ;
        skos:historyNote  "" ;
        skos:prefLabel    "ER"@en ;
        skos:prefLabel    "ER"@pt ;
        skos:inScheme     <http://www.ebu.ch/metadata/ontologies/skos/ebu_ParentalGuidanceCodeCS> ;
        skos:definition   "Especialmente Recomendado para Crianças e\n         Adolescentes"@pt .

parentalguidance:_40.2
        skos:example      "" ;
        skos:historyNote  "" ;
        skos:changeNote   "" ;
        skos:inScheme     <http://www.ebu.ch/metadata/ontologies/skos/ebu_ParentalGuidanceCodeCS> ;
        skos:broader      parentalguidance:_40 ;
        skos:definition   "Viewers below 13 years old must be accompanied by a parent or\n         an adult."@en ;
        skos:prefLabel    "PG-13"@en ;
        rdf:type          ebucore:TargetAudience .

parentalguidance:_23.2.7
        skos:example      "" ;
        skos:historyNote  "" ;
        skos:changeNote   "" ;
        skos:inScheme     <http://www.ebu.ch/metadata/ontologies/skos/ebu_ParentalGuidanceCodeCS> ;
        skos:broader      parentalguidance:_23.2 ;
        skos:prefLabel    "Gambling"@en ;
        rdf:type          ebucore:TargetAudience .

parentalguidance:_47.2.25
        skos:example      "" ;
        skos:historyNote  "" ;
        skos:changeNote   "" ;
        skos:inScheme     <http://www.ebu.ch/metadata/ontologies/skos/ebu_ParentalGuidanceCodeCS> ;
        skos:broader      parentalguidance:_47.2 ;
        skos:definition   "Explicit and/or frequent references to profanity, sex, violence,\n         alcohol or drug use in music" ;
        skos:prefLabel    "Strong Lyrics"@en ;
        rdf:type          ebucore:TargetAudience .

parentalguidance:_61.1.1
        skos:example      "" ;
        skos:historyNote  "" ;
        skos:changeNote   "" ;
        skos:inScheme     <http://www.ebu.ch/metadata/ontologies/skos/ebu_ParentalGuidanceCodeCS> ;
        skos:broader      parentalguidance:_61.1 ;
        skos:definition   "rated for all ages (added in July 2007)."@en ;
        skos:prefLabel    "U"@en ;
        rdf:type          ebucore:TargetAudience .

parentalguidance:_47.2.13
        skos:example      "" ;
        skos:historyNote  "" ;
        skos:changeNote   "" ;
        skos:inScheme     <http://www.ebu.ch/metadata/ontologies/skos/ebu_ParentalGuidanceCodeCS> ;
        skos:broader      parentalguidance:_47.2 ;
        skos:definition   "Mild to moderate use of profanity" ;
        skos:prefLabel    "Language"@en ;
        rdf:type          ebucore:TargetAudience .

parentalguidance:_39.3
        skos:example      "" ;
        skos:historyNote  "" ;
        skos:changeNote   "" ;
        skos:inScheme     <http://www.ebu.ch/metadata/ontologies/skos/ebu_ParentalGuidanceCodeCS> ;
        skos:broader      parentalguidance:_39 ;
        skos:definition   "Suitable for (but not restricted to) mature audiences 16 years\n         and over (awarded by the Film and Video Labelling Body and the Office of Film and\n         Literature Classification)"@en ;
        skos:prefLabel    "Mature"@en ;
        skos:prefLabel    "M"@en ;
        rdf:type          ebucore:TargetAudience .

parentalguidance:_53.1.5
        skos:example      "" ;
        skos:historyNote  "" ;
        skos:changeNote   "" ;
        skos:inScheme     <http://www.ebu.ch/metadata/ontologies/skos/ebu_ParentalGuidanceCodeCS> ;
        skos:broader      parentalguidance:_53.1 ;
        skos:definition   "Exempt from classification"@en ;
        skos:prefLabel    "E"@en ;
        rdf:type          ebucore:TargetAudience .

parentalguidance:_16.2.8
        skos:example      "" ;
        skos:historyNote  "" ;
        skos:changeNote   "" ;
        skos:inScheme     <http://www.ebu.ch/metadata/ontologies/skos/ebu_ParentalGuidanceCodeCS> ;
        skos:broader      parentalguidance:_16.2 ;
        skos:prefLabel    "Bad taste and indecency"@en ;
        rdf:type          ebucore:TargetAudience .

parentalguidance:_51.1.4
        skos:example      "" ;
        skos:historyNote  "" ;
        skos:changeNote   "" ;
        skos:inScheme     <http://www.ebu.ch/metadata/ontologies/skos/ebu_ParentalGuidanceCodeCS> ;
        skos:broader      parentalguidance:_51.1 ;
        skos:definition   "Persons under the age of 13 must be accompanied by an adult to\n         any filem classfied 13M, while a DVB or VHS or an interactive computer game classfied 13 PG\n         requires Parental Guidance for persons under the age of 13"@en ;
        skos:prefLabel    "10M-13PG"@en ;
        rdf:type          ebucore:TargetAudience .

parentalguidance:_63  skos:changeNote  "Update" ;
        skos:example      "" ;
        skos:inScheme     <http://www.ebu.ch/metadata/ontologies/skos/ebu_ParentalGuidanceCodeCS> ;
        skos:narrower     parentalguidance:_63.1 ;
        skos:historyNote  "2010-08-03" ;
        skos:note         "Valid" ;
        skos:definition   ""@en ;
        skos:prefLabel    "MA-BBFC"@en ;
        skos:scopeNote    "Region:Malta"@en ;
        rdf:type          ebucore:TargetAudience .

parentalguidance:_51  rdf:type  ebucore:TargetAudience ;
        skos:changeNote   "Update" ;
        skos:note         "Valid" ;
        skos:scopeNote    "Region:South Africa"@en ;
        skos:narrower     parentalguidance:_51.2 ;
        skos:example      "" ;
        skos:prefLabel    "ZA-FPB"@en ;
        skos:inScheme     <http://www.ebu.ch/metadata/ontologies/skos/ebu_ParentalGuidanceCodeCS> ;
        skos:narrower     parentalguidance:_51.1 ;
        skos:historyNote  "2009-07-28" ;
        skos:definition   "Film and Publication Board"@en .

parentalguidance:_51.2.1
        skos:example      "" ;
        skos:historyNote  "" ;
        skos:changeNote   "" ;
        skos:inScheme     <http://www.ebu.ch/metadata/ontologies/skos/ebu_ParentalGuidanceCodeCS> ;
        skos:broader      parentalguidance:_51.2 ;
        skos:definition   "Drug and alocohol abuse"@en ;
        skos:prefLabel    "D"@en ;
        rdf:type          ebucore:TargetAudience .

parentalguidance:_31.2.2
        skos:example      "" ;
        skos:historyNote  "" ;
        skos:changeNote   "" ;
        skos:inScheme     <http://www.ebu.ch/metadata/ontologies/skos/ebu_ParentalGuidanceCodeCS> ;
        skos:broader      parentalguidance:_31.2 ;
        skos:prefLabel    "Sex"@en ;
        skos:prefLabel    "セクシャル"@ja ;
        rdf:type          ebucore:TargetAudience .

parentalguidance:_55.1.2
        skos:example      "" ;
        skos:historyNote  "" ;
        skos:changeNote   "" ;
        skos:inScheme     <http://www.ebu.ch/metadata/ontologies/skos/ebu_ParentalGuidanceCodeCS> ;
        skos:broader      parentalguidance:_55.1 ;
        skos:definition   "Passed only for 7 and older "@en ;
        skos:prefLabel    "7"@en ;
        rdf:type          ebucore:TargetAudience .

parentalguidance:_31.1.5
        skos:changeNote   "" ;
        skos:prefLabel    "Z"@en ;
        skos:definition   "18歳以上のみ"@ja ;
        skos:prefLabel    "赤"@ja ;
        skos:inScheme     <http://www.ebu.ch/metadata/ontologies/skos/ebu_ParentalGuidanceCodeCS> ;
        skos:prefLabel    "Red"@en ;
        rdf:type          ebucore:TargetAudience ;
        skos:broader      parentalguidance:_31.1 ;
        skos:definition   "18 and over"@en ;
        skos:historyNote  "" ;
        skos:example      "" .

parentalguidance:_28.1
        skos:example      "" ;
        skos:historyNote  "" ;
        skos:changeNote   "" ;
        skos:inScheme     <http://www.ebu.ch/metadata/ontologies/skos/ebu_ParentalGuidanceCodeCS> ;
        skos:broader      parentalguidance:_28 ;
        skos:definition   "'A film classified as 'General' should be suitable for children\n         of school going age."@en ;
        skos:prefLabel    "G"@en ;
        rdf:type          ebucore:TargetAudience .

parentalguidance:_27.4
        skos:example      "" ;
        skos:historyNote  "" ;
        skos:changeNote   "" ;
        skos:inScheme     <http://www.ebu.ch/metadata/ontologies/skos/ebu_ParentalGuidanceCodeCS> ;
        skos:broader      parentalguidance:_27 ;
        skos:definition   "No one under 15 years of age may see a \"15\" film or rent or buy\n         a \"15\" video"@en ;
        skos:prefLabel    "15"@en ;
        rdf:type          ebucore:TargetAudience .

parentalguidance:_50.6
        skos:example      "" ;
        skos:historyNote  "" ;
        skos:changeNote   "" ;
        skos:inScheme     <http://www.ebu.ch/metadata/ontologies/skos/ebu_ParentalGuidanceCodeCS> ;
        skos:broader      parentalguidance:_50 ;
        skos:definition   "Parents strongly cautioned"@en ;
        skos:prefLabel    "TV-14"@en ;
        rdf:type          ebucore:TargetAudience .

parentalguidance:_6.1
        skos:example      "" ;
        skos:historyNote  "" ;
        skos:changeNote   "" ;
        skos:inScheme     <http://www.ebu.ch/metadata/ontologies/skos/ebu_ParentalGuidanceCodeCS> ;
        skos:broader      parentalguidance:_6 ;
        skos:definition   "When the film confirms the ideals of humanism or popularizes\n         the national and world cultures or contributes to upbringing children"@en ;
        skos:prefLabel    "A"@en ;
        skos:prefLabel    "A"@po ;
        rdf:type          ebucore:TargetAudience .

parentalguidance:_23.2.6
        skos:example      "" ;
        skos:historyNote  "" ;
        skos:changeNote   "" ;
        skos:inScheme     <http://www.ebu.ch/metadata/ontologies/skos/ebu_ParentalGuidanceCodeCS> ;
        skos:broader      parentalguidance:_23.2 ;
        skos:prefLabel    "Violence"@en ;
        rdf:type          ebucore:TargetAudience .

parentalguidance:_40.1
        skos:example      "" ;
        skos:historyNote  "" ;
        skos:changeNote   "" ;
        skos:inScheme     <http://www.ebu.ch/metadata/ontologies/skos/ebu_ParentalGuidanceCodeCS> ;
        skos:broader      parentalguidance:_40 ;
        skos:definition   "General Patronage. All ages admitted."@en ;
        skos:prefLabel    "G"@en ;
        rdf:type          ebucore:TargetAudience .

parentalguidance:_61.1.2
        skos:example      "" ;
        skos:historyNote  "" ;
        skos:changeNote   "" ;
        skos:inScheme     <http://www.ebu.ch/metadata/ontologies/skos/ebu_ParentalGuidanceCodeCS> ;
        skos:broader      parentalguidance:_61.1 ;
        skos:definition   "Not recommended until 7 "@en ;
        skos:prefLabel    "7+"@en ;
        rdf:type          ebucore:TargetAudience .

parentalguidance:_38.5
        skos:example      "" ;
        skos:historyNote  "" ;
        skos:changeNote   "" ;
        skos:inScheme     <http://www.ebu.ch/metadata/ontologies/skos/ebu_ParentalGuidanceCodeCS> ;
        skos:broader      parentalguidance:_38 ;
        skos:definition   "Not under 18"@en ;
        skos:definition   "18 år (absolutt nedre grense)"@no ;
        skos:prefLabel    "18"@en ;
        rdf:type          ebucore:TargetAudience .

parentalguidance:_47.2.12
        skos:example      "" ;
        skos:historyNote  "" ;
        skos:changeNote   "" ;
        skos:inScheme     <http://www.ebu.ch/metadata/ontologies/skos/ebu_ParentalGuidanceCodeCS> ;
        skos:broader      parentalguidance:_47.2 ;
        skos:definition   "Graphic and realistic-looking depictions of physical conflict.\n         May involve extreme and/or realistic blood, gore, weapons and depictions of human injury\n         and death" ;
        skos:prefLabel    "Intense Violence"@en ;
        rdf:type          ebucore:TargetAudience .

parentalguidance:_65.1
        skos:narrower     parentalguidance:_65.1.3 ;
        skos:example      "" ;
        skos:historyNote  "" ;
        skos:narrower     parentalguidance:_65.1.1 ;
        skos:changeNote   "" ;
        skos:narrower     parentalguidance:_65.1.6 ;
        skos:inScheme     <http://www.ebu.ch/metadata/ontologies/skos/ebu_ParentalGuidanceCodeCS> ;
        skos:narrower     parentalguidance:_65.1.4 ;
        skos:prefLabel    "Rating"@en ;
        rdf:type          ebucore:TargetAudience ;
        skos:broader      parentalguidance:_65 ;
        skos:narrower     parentalguidance:_65.1.5 ;
        skos:narrower     parentalguidance:_65.1.2 .

parentalguidance:_39.2
        skos:example      "" ;
        skos:historyNote  "" ;
        skos:changeNote   "" ;
        skos:inScheme     <http://www.ebu.ch/metadata/ontologies/skos/ebu_ParentalGuidanceCodeCS> ;
        skos:broader      parentalguidance:_39 ;
        skos:definition   "Parental guidance recommended for younger viewers (awarded by\n         the Film and Video Labelling Body and the Office of Film and Literature\n         Classification)"@en ;
        skos:prefLabel    "Parental Guidance"@en ;
        skos:altLabel     "PG"@en ;
        rdf:type          ebucore:TargetAudience .

parentalguidance:_47.2.24
        skos:example      "" ;
        skos:historyNote  "" ;
        skos:changeNote   "" ;
        skos:inScheme     <http://www.ebu.ch/metadata/ontologies/skos/ebu_ParentalGuidanceCodeCS> ;
        skos:broader      parentalguidance:_47.2 ;
        skos:definition   "Explicit and/or frequent use of profanity" ;
        skos:prefLabel    "Strong Language"@en ;
        rdf:type          ebucore:TargetAudience .

parentalguidance:_51.1.3
        skos:example      "" ;
        skos:historyNote  "" ;
        skos:changeNote   "" ;
        skos:inScheme     <http://www.ebu.ch/metadata/ontologies/skos/ebu_ParentalGuidanceCodeCS> ;
        skos:broader      parentalguidance:_51.1 ;
        skos:definition   "Children under the age of 10 years must be accompanied by an\n         adult"@en ;
        skos:prefLabel    "10M"@en ;
        rdf:type          ebucore:TargetAudience .

parentalguidance:_16.2.9
        skos:example      "" ;
        skos:historyNote  "" ;
        skos:changeNote   "" ;
        skos:inScheme     <http://www.ebu.ch/metadata/ontologies/skos/ebu_ParentalGuidanceCodeCS> ;
        skos:broader      parentalguidance:_16.2 ;
        skos:prefLabel    "Scenes of extreme suffering and distress"@en ;
        rdf:type          ebucore:TargetAudience .

parentalguidance:_17.1
        skos:inScheme     <http://www.ebu.ch/metadata/ontologies/skos/ebu_ParentalGuidanceCodeCS> ;
        skos:prefLabel    "T"@es ;
        skos:prefLabel    "T"@en ;
        skos:changeNote   "" ;
        skos:historyNote  "" ;
        skos:broader      parentalguidance:_17 ;
        skos:example      "" ;
        skos:definition   "All Audiences"@en ;
        skos:definition   "Todos"@es ;
        rdf:type          ebucore:TargetAudience .

parentalguidance:_52  skos:note  "Valid" ;
        skos:definition   "UnterhaltungSoftware SebstKontrolle"@de ;
        skos:narrower     parentalguidance:_52.1 ;
        rdf:type          ebucore:TargetAudience ;
        skos:inScheme     <http://www.ebu.ch/metadata/ontologies/skos/ebu_ParentalGuidanceCodeCS> ;
        skos:narrower     parentalguidance:_52.3 ;
        skos:changeNote   "Change subterm termId from 18.x to 52.x" ;
        skos:scopeNote    "Region:Germany" ;
        skos:historyNote  "2019-06-24" ;
        skos:narrower     parentalguidance:_52.2 ;
        skos:example      "" ;
        skos:narrower     parentalguidance:_52.4 ;
        skos:narrower     parentalguidance:_52.5 ;
        skos:prefLabel    "DE-USK"@en ;
        skos:definition   "Entertianment and software self control"@en .

parentalguidance:_40  skos:narrower  parentalguidance:_40.4 ;
        skos:scopeNote    "Region:Philippines"@en ;
        skos:note         "Valid" ;
        skos:definition   "Movie and Television Review and Classification\n         Board"@en ;
        skos:inScheme     <http://www.ebu.ch/metadata/ontologies/skos/ebu_ParentalGuidanceCodeCS> ;
        skos:prefLabel    "PH-MTRCB"@en ;
        rdf:type          ebucore:TargetAudience ;
        skos:historyNote  "2009-07-28" ;
        skos:narrower     parentalguidance:_40.1 ;
        skos:changeNote   "Update" ;
        skos:example      "" ;
        skos:definition   "Lupon sa Pagrerepaso at Pag-uuri ng Sine at\n         Telebisyon" ;
        skos:narrower     parentalguidance:_40.3 ;
        skos:narrower     parentalguidance:_40.2 .

parentalguidance:_55.1.1
        skos:example      "" ;
        skos:historyNote  "" ;
        skos:changeNote   "" ;
        skos:inScheme     <http://www.ebu.ch/metadata/ontologies/skos/ebu_ParentalGuidanceCodeCS> ;
        skos:broader      parentalguidance:_55.1 ;
        skos:definition   "Suitable for all "@en ;
        skos:prefLabel    "L"@en ;
        rdf:type          ebucore:TargetAudience .

parentalguidance:_58.1.1
        skos:example      "" ;
        skos:historyNote  "" ;
        skos:changeNote   "" ;
        skos:inScheme     <http://www.ebu.ch/metadata/ontologies/skos/ebu_ParentalGuidanceCodeCS> ;
        skos:broader      parentalguidance:_58.1 ;
        skos:definition   "Family film"@en ;
        skos:prefLabel    "Pere"@en ;
        rdf:type          ebucore:TargetAudience .

parentalguidance:_31.2.3
        skos:example      "" ;
        skos:historyNote  "" ;
        skos:changeNote   "" ;
        skos:inScheme     <http://www.ebu.ch/metadata/ontologies/skos/ebu_ParentalGuidanceCodeCS> ;
        skos:broader      parentalguidance:_31.2 ;
        skos:prefLabel    "Violence"@en ;
        skos:prefLabel    "暴力"@ja ;
        rdf:type          ebucore:TargetAudience .

parentalguidance:_64  skos:example  "" ;
        rdf:type          ebucore:TargetAudience ;
        skos:scopeNote    "Region:Switzerland"@en ;
        skos:changeNote   "Update" ;
        skos:note         "Valid" ;
        skos:definition   ""@en ;
        skos:prefLabel    "CH"@en ;
        skos:narrower     parentalguidance:_64.1 ;
        skos:inScheme     <http://www.ebu.ch/metadata/ontologies/skos/ebu_ParentalGuidanceCodeCS> ;
        skos:historyNote  "2010-08-03" .

parentalguidance:_51.2
        skos:narrower     parentalguidance:_51.2.2 ;
        skos:narrower     parentalguidance:_51.2.5 ;
        skos:narrower     parentalguidance:_51.2.6 ;
        skos:inScheme     <http://www.ebu.ch/metadata/ontologies/skos/ebu_ParentalGuidanceCodeCS> ;
        skos:narrower     parentalguidance:_51.2.4 ;
        skos:broader      parentalguidance:_51 ;
        rdf:type          ebucore:TargetAudience ;
        skos:prefLabel    "Criteria"@en ;
        skos:narrower     parentalguidance:_51.2.3 ;
        skos:historyNote  "" ;
        skos:changeNote   "" ;
        skos:example      "" ;
        skos:narrower     parentalguidance:_51.2.1 .

parentalguidance:_28.2
        skos:example      "" ;
        skos:historyNote  "" ;
        skos:changeNote   "" ;
        skos:inScheme     <http://www.ebu.ch/metadata/ontologies/skos/ebu_ParentalGuidanceCodeCS> ;
        skos:broader      parentalguidance:_28 ;
        skos:definition   "A film with a 'PG' cert may be watched by unaccompanied\n         children of any age."@en ;
        skos:prefLabel    "PG"@en ;
        rdf:type          ebucore:TargetAudience .

parentalguidance:_50.5
        skos:example      "" ;
        skos:historyNote  "" ;
        skos:changeNote   "" ;
        skos:inScheme     <http://www.ebu.ch/metadata/ontologies/skos/ebu_ParentalGuidanceCodeCS> ;
        skos:broader      parentalguidance:_50 ;
        skos:definition   "Parental guidance suggested"@en ;
        skos:prefLabel    "TV-PG"@en ;
        rdf:type          ebucore:TargetAudience .

parentalguidance:_27.5
        skos:example      "" ;
        skos:historyNote  "" ;
        skos:changeNote   "" ;
        skos:inScheme     <http://www.ebu.ch/metadata/ontologies/skos/ebu_ParentalGuidanceCodeCS> ;
        skos:broader      parentalguidance:_27 ;
        skos:definition   "Suitable only for adults"@en ;
        skos:prefLabel    "18"@en ;
        rdf:type          ebucore:TargetAudience .

parentalguidance:_6.2
        skos:example      "" ;
        skos:historyNote  "" ;
        skos:changeNote   "" ;
        skos:inScheme     <http://www.ebu.ch/metadata/ontologies/skos/ebu_ParentalGuidanceCodeCS> ;
        skos:broader      parentalguidance:_6 ;
        skos:definition   "All ages - When the film is in no way contrary to the universal\n         rules of morality in this country, has no restrictive recommendations from the Committee\n         and does not fall in rating A"@en ;
        skos:prefLabel    "B"@en ;
        rdf:type          ebucore:TargetAudience .

parentalguidance:_61.1.3
        skos:example      "" ;
        skos:historyNote  "" ;
        skos:changeNote   "" ;
        skos:inScheme     <http://www.ebu.ch/metadata/ontologies/skos/ebu_ParentalGuidanceCodeCS> ;
        skos:broader      parentalguidance:_61.1 ;
        skos:definition   "Not recommended until 12 "@en ;
        skos:prefLabel    "12+"@en ;
        rdf:type          ebucore:TargetAudience .

parentalguidance:_47.2.11
        skos:example      "" ;
        skos:historyNote  "" ;
        skos:changeNote   "" ;
        skos:inScheme     <http://www.ebu.ch/metadata/ontologies/skos/ebu_ParentalGuidanceCodeCS> ;
        skos:broader      parentalguidance:_47.2 ;
        skos:definition   "Overall content of product contains data, facts, resource\n         information, reference materials or instructional text" ;
        skos:prefLabel    "Informational"@en ;
        rdf:type          ebucore:TargetAudience .

parentalguidance:_51.1.6
        skos:example      "" ;
        skos:historyNote  "" ;
        skos:changeNote   "" ;
        skos:inScheme     <http://www.ebu.ch/metadata/ontologies/skos/ebu_ParentalGuidanceCodeCS> ;
        skos:broader      parentalguidance:_51.1 ;
        skos:definition   "16 years and older only"@en ;
        skos:prefLabel    "16"@en ;
        rdf:type          ebucore:TargetAudience .

parentalguidance:_41.5
        skos:example      "" ;
        skos:historyNote  "" ;
        skos:changeNote   "" ;
        skos:inScheme     <http://www.ebu.ch/metadata/ontologies/skos/ebu_ParentalGuidanceCodeCS> ;
        skos:broader      parentalguidance:_41 ;
        skos:definition   "Adults only (18 and over)"@en ;
        skos:prefLabel    "R"@en ;
        rdf:type          ebucore:TargetAudience .

parentalguidance:_47.2.23
        skos:example      "" ;
        skos:historyNote  "" ;
        skos:changeNote   "" ;
        skos:inScheme     <http://www.ebu.ch/metadata/ontologies/skos/ebu_ParentalGuidanceCodeCS> ;
        skos:broader      parentalguidance:_47.2 ;
        skos:definition   "Intended for very young ages" ;
        skos:prefLabel    "Some Adult Assistance May Be Needed"@en ;
        rdf:type          ebucore:TargetAudience .

parentalguidance:_29.5
        skos:prefLabel    "Mature Audience"@en ;
        skos:prefLabel    "MA"@en ;
        skos:broader      parentalguidance:_29 ;
        skos:changeNote   "" ;
        skos:example      "" ;
        skos:historyNote  "" ;
        rdf:type          ebucore:TargetAudience ;
        skos:inScheme     <http://www.ebu.ch/metadata/ontologies/skos/ebu_ParentalGuidanceCodeCS> ;
        skos:definition   "a typical \"post-watershed\" program which might contain scenes\n         of strong sexual activity and heavy violence, or the dialogue might be\n         profane."@en ;
        skos:prefLabel    "Lucht Féachana Lánfhásta Amháin"@ga .

parentalguidance:_18.3
        rdf:type          ebucore:TargetAudience ;
        skos:prefLabel    "12"@de ;
        skos:prefLabel    "12"@en ;
        skos:definition   "Freigegeben ab 12 Jahren"@de ;
        skos:inScheme     <http://www.ebu.ch/metadata/ontologies/skos/ebu_ParentalGuidanceCodeCS> ;
        skos:historyNote  "" ;
        skos:example      "" ;
        skos:changeNote   "" ;
        skos:broader      parentalguidance:_18 ;
        skos:definition   "People 12 or older admitted, children between 6 and 11 only\n         when accompanied by parent or legal guardian"@en .

parentalguidance:_51.2.3
        skos:example      "" ;
        skos:historyNote  "" ;
        skos:changeNote   "" ;
        skos:inScheme     <http://www.ebu.ch/metadata/ontologies/skos/ebu_ParentalGuidanceCodeCS> ;
        skos:broader      parentalguidance:_51.2 ;
        skos:definition   "Nudity"@en ;
        skos:prefLabel    "N"@en ;
        rdf:type          ebucore:TargetAudience .

parentalguidance:_31.1
        skos:prefLabel    "レーティングマーク"@ja ;
        skos:narrower     parentalguidance:_31.1.4 ;
        skos:historyNote  "" ;
        skos:narrower     parentalguidance:_31.1.2 ;
        rdf:type          ebucore:TargetAudience ;
        skos:narrower     parentalguidance:_31.1.3 ;
        skos:changeNote   "" ;
        skos:narrower     parentalguidance:_31.1.1 ;
        skos:broader      parentalguidance:_31 ;
        skos:example      "" ;
        skos:prefLabel    "Rating"@en ;
        skos:narrower     parentalguidance:_31.1.5 ;
        skos:inScheme     <http://www.ebu.ch/metadata/ontologies/skos/ebu_ParentalGuidanceCodeCS> .

parentalguidance:_61  skos:narrower  parentalguidance:_61.1 ;
        rdf:type          ebucore:TargetAudience ;
        skos:example      "" ;
        skos:prefLabel    "LV-NCC"@en ;
        skos:inScheme     <http://www.ebu.ch/metadata/ontologies/skos/ebu_ParentalGuidanceCodeCS> ;
        skos:definition   "Nacionālais Kino Centrs"@lv ;
        skos:definition   "National Cinema Center"@en ;
        skos:note         "Valid" ;
        skos:historyNote  "2010-08-03" ;
        skos:changeNote   "Update" ;
        skos:scopeNote    "Region:Latvia"@en .

_:b5    rdf:rest   _:b0 ;
        rdf:first  parentalguidance:_48 .

parentalguidance:_24.6.1
        skos:example      "" ;
        skos:historyNote  "" ;
        skos:changeNote   "" ;
        skos:inScheme     <http://www.ebu.ch/metadata/ontologies/skos/ebu_ParentalGuidanceCodeCS> ;
        skos:broader      parentalguidance:_24.6 ;
        skos:definition   "Parental Guidance option - children 2 years of age under the K\n         limits may access the show in presence of an accompanying adult"@en ;
        skos:prefLabel    "PG"@en ;
        rdf:type          ebucore:TargetAudience .

parentalguidance:defaultSchemesList
        skos:memberList  _:b5 ;
        skos:definition  "The ordered list of Parental Guidance top concepts to be considered when no scheme is provided for a rating"@en ;
        rdfs:label       "Default PG Schemes List"@en ;
        rdf:type         skos:OrderedCollection .

parentalguidance:_63.1.4
        skos:example      "" ;
        skos:historyNote  "" ;
        skos:changeNote   "" ;
        skos:inScheme     <http://www.ebu.ch/metadata/ontologies/skos/ebu_ParentalGuidanceCodeCS> ;
        skos:broader      parentalguidance:_63.1 ;
        skos:definition   "Suitable only for persons 14 years and older. No one under this\n         age is admitted. "@en ;
        skos:prefLabel    "14"@en ;
        rdf:type          ebucore:TargetAudience .

parentalguidance:_31.2.8
        skos:example      "" ;
        skos:historyNote  "" ;
        skos:changeNote   "" ;
        skos:inScheme     <http://www.ebu.ch/metadata/ontologies/skos/ebu_ParentalGuidanceCodeCS> ;
        skos:broader      parentalguidance:_31.2 ;
        skos:prefLabel    "Drugs"@en ;
        skos:prefLabel    "麻薬"@ja ;
        rdf:type          ebucore:TargetAudience .

parentalguidance:_58.1.2
        skos:example      "" ;
        skos:historyNote  "" ;
        skos:changeNote   "" ;
        skos:inScheme     <http://www.ebu.ch/metadata/ontologies/skos/ebu_ParentalGuidanceCodeCS> ;
        skos:broader      parentalguidance:_58.1 ;
        skos:definition   "For all audiences"@en ;
        skos:prefLabel    "L"@en ;
        rdf:type          ebucore:TargetAudience .

parentalguidance:_29.4
        skos:prefLabel    "Parental Supervision"@en ;
        skos:prefLabel    "PS"@en ;
        rdf:type          ebucore:TargetAudience ;
        skos:broader      parentalguidance:_29 ;
        skos:definition   "a programme aimed at a mature audience (i.e. It might deal with\n         adult themes, be moderately violent, frightening or contain an occasional swear word.) and\n         the classification label invites parents or guardians to consider restricting children's\n         access."@en ;
        skos:changeNote   "" ;
        skos:prefLabel    "Treoir Tuismitheora"@ga ;
        skos:inScheme     <http://www.ebu.ch/metadata/ontologies/skos/ebu_ParentalGuidanceCodeCS> ;
        skos:example      "" ;
        skos:historyNote  "" .

parentalguidance:_23.2.4
        skos:example      "" ;
        skos:historyNote  "" ;
        skos:changeNote   "" ;
        skos:inScheme     <http://www.ebu.ch/metadata/ontologies/skos/ebu_ParentalGuidanceCodeCS> ;
        skos:broader      parentalguidance:_23.2 ;
        skos:prefLabel    "Fear"@en ;
        rdf:type          ebucore:TargetAudience .

parentalguidance:_42.2
        skos:example      "" ;
        skos:historyNote  "" ;
        skos:changeNote   "" ;
        skos:inScheme     <http://www.ebu.ch/metadata/ontologies/skos/ebu_ParentalGuidanceCodeCS> ;
        skos:broader      parentalguidance:_42 ;
        skos:definition   "os espectáculos que, pela sua temática ou extensão, não sejam\n         abrangidos pelos critérios fixados para os níveis etários superiores."@pt ;
        skos:definition   "For persons of age 6 and above"@en ;
        skos:prefLabel    "M/6"@en ;
        rdf:type          ebucore:TargetAudience .

parentalguidance:_5.2
        skos:example      "" ;
        skos:historyNote  "" ;
        skos:definition   "Kinderen Niet Toegelaten"@nl ;
        skos:changeNote   "" ;
        skos:broader      parentalguidance:_5 ;
        skos:definition   "Children not admitted (below 16 years of age)"@en ;
        skos:prefLabel    "KNT"@nl ;
        skos:prefLabel    "ENA"@fr ;
        rdf:type          ebucore:TargetAudience ;
        skos:inScheme     <http://www.ebu.ch/metadata/ontologies/skos/ebu_ParentalGuidanceCodeCS> ;
        skos:definition   "Enfants Non admis"@fr ;
        skos:prefLabel    "Children Not Allowed"@en .

parentalguidance:_47.2.10
        skos:example      "" ;
        skos:historyNote  "" ;
        skos:changeNote   "" ;
        skos:inScheme     <http://www.ebu.ch/metadata/ontologies/skos/ebu_ParentalGuidanceCodeCS> ;
        skos:broader      parentalguidance:_47.2 ;
        skos:definition   "Violent actions of a fantasy nature, involving human or non-human\n         characters in situations easily distinguishable from real life" ;
        skos:prefLabel    "Fantasy Violence"@en ;
        rdf:type          ebucore:TargetAudience .

parentalguidance:_63.1
        skos:historyNote  "" ;
        skos:example      "" ;
        skos:narrower     parentalguidance:_63.1.6 ;
        skos:prefLabel    "Rating"@en ;
        skos:broader      parentalguidance:_63 ;
        skos:narrower     parentalguidance:_63.1.4 ;
        skos:narrower     parentalguidance:_63.1.7 ;
        skos:narrower     parentalguidance:_63.1.2 ;
        skos:narrower     parentalguidance:_63.1.3 ;
        skos:inScheme     <http://www.ebu.ch/metadata/ontologies/skos/ebu_ParentalGuidanceCodeCS> ;
        rdf:type          ebucore:TargetAudience ;
        skos:narrower     parentalguidance:_63.1.5 ;
        skos:changeNote   "" ;
        skos:narrower     parentalguidance:_63.1.1 .

parentalguidance:_47.2.22
        skos:example      "" ;
        skos:historyNote  "" ;
        skos:changeNote   "" ;
        skos:inScheme     <http://www.ebu.ch/metadata/ontologies/skos/ebu_ParentalGuidanceCodeCS> ;
        skos:broader      parentalguidance:_47.2 ;
        skos:definition   "Player can gamble without betting or wagering real cash or\n         currency" ;
        skos:prefLabel    "Simulated Gambling"@en ;
        rdf:type          ebucore:TargetAudience .

parentalguidance:_61.1.4
        skos:example      "" ;
        skos:historyNote  "" ;
        skos:changeNote   "" ;
        skos:inScheme     <http://www.ebu.ch/metadata/ontologies/skos/ebu_ParentalGuidanceCodeCS> ;
        skos:broader      parentalguidance:_61.1 ;
        skos:definition   "Not recommended until 16 "@en ;
        skos:prefLabel    "16+"@en ;
        rdf:type          ebucore:TargetAudience .

parentalguidance:_51.1.5
        skos:example      "" ;
        skos:historyNote  "" ;
        skos:changeNote   "" ;
        skos:inScheme     <http://www.ebu.ch/metadata/ontologies/skos/ebu_ParentalGuidanceCodeCS> ;
        skos:broader      parentalguidance:_51.1 ;
        skos:definition   "10 years and older only"@en ;
        skos:prefLabel    "10"@en ;
        rdf:type          ebucore:TargetAudience .

parentalguidance:_41.4
        skos:example      "" ;
        skos:historyNote  "" ;
        skos:changeNote   "" ;
        skos:inScheme     <http://www.ebu.ch/metadata/ontologies/skos/ebu_ParentalGuidanceCodeCS> ;
        skos:broader      parentalguidance:_41 ;
        skos:definition   "For persons of age 16 and above."@en ;
        skos:prefLabel    "16"@en ;
        rdf:type          ebucore:TargetAudience .

<http://www.ebu.ch/metadata/ontologies/skos/ebu_ParentalGuidanceCodeCS>
        skos:hasTopConcept  parentalguidance:_46 ;
        skos:hasTopConcept  parentalguidance:_33 ;
        skos:hasTopConcept  parentalguidance:_14 ;
        skos:hasTopConcept  parentalguidance:_41 ;
        skos:hasTopConcept  parentalguidance:_64 ;
        skos:hasTopConcept  parentalguidance:_69 ;
        rdfs:isDefinedBy    <http://www.ebu.ch/metadata/ontologies/skos/ebu_ParentalGuidanceCodeCS> ;
        skos:hasTopConcept  parentalguidance:_27 ;
        skos:hasTopConcept  parentalguidance:_28 ;
        skos:hasTopConcept  parentalguidance:_57 ;
        skos:hasTopConcept  parentalguidance:_32 ;
        skos:hasTopConcept  parentalguidance:_38 ;
        skos:hasTopConcept  parentalguidance:_5 ;
        skos:hasTopConcept  parentalguidance:_60 ;
        skos:hasTopConcept  parentalguidance:_6 ;
        skos:hasTopConcept  parentalguidance:_15 ;
        skos:hasTopConcept  parentalguidance:_2 ;
        skos:hasTopConcept  parentalguidance:_56 ;
        skos:hasTopConcept  parentalguidance:_39 ;
        skos:hasTopConcept  parentalguidance:_1 ;
        rdf:type            skos:ConceptScheme ;
        skos:hasTopConcept  parentalguidance:_20 ;
        skos:hasTopConcept  parentalguidance:_25 ;
        skos:hasTopConcept  parentalguidance:_26 ;
        rdfs:label          "EBU SKOS Classification Scheme for Parental Guidance"@en ;
        skos:hasTopConcept  parentalguidance:_4 ;
        skos:hasTopConcept  parentalguidance:_13 ;
        skos:hasTopConcept  parentalguidance:_43 ;
        skos:hasTopConcept  parentalguidance:_44 ;
        skos:hasTopConcept  parentalguidance:_49 ;
        skos:hasTopConcept  parentalguidance:_52 ;
        skos:hasTopConcept  parentalguidance:_31 ;
        skos:hasTopConcept  parentalguidance:_12 ;
        skos:hasTopConcept  parentalguidance:_37 ;
        skos:hasTopConcept  parentalguidance:_18 ;
        skos:hasTopConcept  parentalguidance:_40 ;
        skos:hasTopConcept  parentalguidance:_67 ;
        skos:hasTopConcept  parentalguidance:_68 ;
        skos:hasTopConcept  parentalguidance:_55 ;
        skos:hasTopConcept  parentalguidance:_36 ;
        skos:hasTopConcept  parentalguidance:_63 ;
        skos:hasTopConcept  parentalguidance:_54 ;
        skos:hasTopConcept  parentalguidance:_9 ;
        skos:hasTopConcept  parentalguidance:_19 ;
        skos:hasTopConcept  parentalguidance:_42 ;
        skos:hasTopConcept  parentalguidance:_50 ;
        skos:hasTopConcept  parentalguidance:_10 ;
        skos:hasTopConcept  parentalguidance:_65 ;
        skos:hasTopConcept  parentalguidance:_66 ;
        skos:hasTopConcept  parentalguidance:_23 ;
        skos:hasTopConcept  parentalguidance:_24 ;
        skos:hasTopConcept  parentalguidance:_29 ;
        skos:hasTopConcept  parentalguidance:_51 ;
        skos:hasTopConcept  parentalguidance:_34 ;
        skos:hasTopConcept  parentalguidance:_61 ;
        skos:hasTopConcept  parentalguidance:_11 ;
        skos:hasTopConcept  parentalguidance:_7 ;
        skos:hasTopConcept  parentalguidance:_62 ;
        skos:hasTopConcept  parentalguidance:_8 ;
        skos:hasTopConcept  parentalguidance:_17 ;
        skos:hasTopConcept  parentalguidance:_47 ;
        skos:hasTopConcept  parentalguidance:_48 ;
        skos:hasTopConcept  parentalguidance:_58 ;
        skos:hasTopConcept  parentalguidance:_35 ;
        skos:hasTopConcept  parentalguidance:_53 ;
        skos:hasTopConcept  parentalguidance:_16 ;
        skos:hasTopConcept  parentalguidance:_3 ;
        skos:hasTopConcept  parentalguidance:_21 ;
        skos:hasTopConcept  parentalguidance:_22 ;
        skos:hasTopConcept  parentalguidance:_59 ;
        skos:hasTopConcept  parentalguidance:_30 ;
        skos:hasTopConcept  parentalguidance:_45 .

parentalguidance:_18.4
        skos:historyNote  "" ;
        skos:example      "" ;
        skos:changeNote   "" ;
        skos:broader      parentalguidance:_18 ;
        skos:inScheme     <http://www.ebu.ch/metadata/ontologies/skos/ebu_ParentalGuidanceCodeCS> ;
        skos:definition   "Freigegeben ab 16 Jahren"@de ;
        skos:definition   "People 16 or older admitted"@en ;
        rdf:type          ebucore:TargetAudience ;
        skos:prefLabel    "16"@de ;
        skos:prefLabel    "16"@en .

parentalguidance:_30.3
        skos:example      "" ;
        skos:historyNote  "" ;
        skos:changeNote   "" ;
        skos:narrower     parentalguidance:_30.3.1 ;
        skos:inScheme     <http://www.ebu.ch/metadata/ontologies/skos/ebu_ParentalGuidanceCodeCS> ;
        skos:broader      parentalguidance:_30 ;
        skos:definition   "adults only."@en ;
        skos:prefLabel    "Red"@en ;
        rdf:type          ebucore:TargetAudience .

parentalguidance:_19.1
        skos:historyNote  "" ;
        skos:example      "" ;
        skos:changeNote   "" ;
        skos:prefLabel    "FSK 0"@en ;
        skos:prefLabel    "FSK 0"@de ;
        skos:inScheme     <http://www.ebu.ch/metadata/ontologies/skos/ebu_ParentalGuidanceCodeCS> ;
        rdf:type          ebucore:TargetAudience ;
        skos:definition   "Ohne Altersbeschränkung"@de ;
        skos:definition   "For all ages"@en ;
        skos:broader      parentalguidance:_19 .

parentalguidance:_62  skos:example  "" ;
        skos:narrower     parentalguidance:_62.1 ;
        skos:scopeNote    "Region:Malaysia"@en ;
        skos:definition   "Film Censorship Board"@en ;
        skos:prefLabel    "MA-FCB"@en ;
        skos:inScheme     <http://www.ebu.ch/metadata/ontologies/skos/ebu_ParentalGuidanceCodeCS> ;
        skos:changeNote   "Update" ;
        rdf:type          ebucore:TargetAudience ;
        skos:note         "Valid" ;
        skos:historyNote  "2010-08-03" .

parentalguidance:_51.2.2
        skos:example      "" ;
        skos:historyNote  "" ;
        skos:changeNote   "" ;
        skos:inScheme     <http://www.ebu.ch/metadata/ontologies/skos/ebu_ParentalGuidanceCodeCS> ;
        skos:broader      parentalguidance:_51.2 ;
        skos:definition   "Strong language"@en ;
        skos:prefLabel    "L"@en ;
        rdf:type          ebucore:TargetAudience .

parentalguidance:_50  skos:narrower  parentalguidance:_50.2 ;
        skos:narrower     parentalguidance:_50.6 ;
        skos:historyNote  "2009-07-27" ;
        skos:changeNote   "Update" ;
        skos:inScheme     <http://www.ebu.ch/metadata/ontologies/skos/ebu_ParentalGuidanceCodeCS> ;
        skos:narrower     parentalguidance:_50.3 ;
        skos:narrower     parentalguidance:_50.7 ;
        skos:definition   "The TV Parental Guidelines"@en ;
        skos:narrower     parentalguidance:_50.4 ;
        rdf:type          ebucore:TargetAudience ;
        skos:example      "" ;
        skos:altLabel     "USA_PR"@en ;
        skos:prefLabel    "US-TVPG"@en ;
        skos:altLabel     "V-Chip"@en ;
        skos:narrower     parentalguidance:_50.1 ;
        skos:note         "Valid" ;
        skos:scopeNote    "Region:United States"@en ;
        skos:narrower     parentalguidance:_50.5 .

parentalguidance:_4.2.10
        skos:example      "" ;
        skos:historyNote  "" ;
        skos:changeNote   "" ;
        skos:inScheme     <http://www.ebu.ch/metadata/ontologies/skos/ebu_ParentalGuidanceCodeCS> ;
        skos:broader      parentalguidance:_4.2 ;
        skos:definition   "War"@en ;
        skos:prefLabel    "W"@en ;
        rdf:type          ebucore:TargetAudience .

parentalguidance:_31.2.9
        skos:example      "" ;
        skos:historyNote  "" ;
        skos:changeNote   "" ;
        skos:inScheme     <http://www.ebu.ch/metadata/ontologies/skos/ebu_ParentalGuidanceCodeCS> ;
        skos:broader      parentalguidance:_31.2 ;
        skos:prefLabel    "Strong vocabulary"@en ;
        skos:prefLabel    "言葉・その他"@ja ;
        rdf:type          ebucore:TargetAudience .

parentalguidance:_58.1.3
        skos:example      "" ;
        skos:historyNote  "" ;
        skos:changeNote   "" ;
        skos:inScheme     <http://www.ebu.ch/metadata/ontologies/skos/ebu_ParentalGuidanceCodeCS> ;
        skos:broader      parentalguidance:_58.1 ;
        skos:definition   "Younger than 6 Not Recommended "@en ;
        skos:prefLabel    "MS-6"@en ;
        rdf:type          ebucore:TargetAudience .

parentalguidance:_18.5
        skos:broader      parentalguidance:_18 ;
        rdf:type          ebucore:TargetAudience ;
        skos:changeNote   "" ;
        skos:prefLabel    "18"@de ;
        skos:prefLabel    "18"@en ;
        skos:definition   "Keine Jugendfreigabe"@de ;
        skos:inScheme     <http://www.ebu.ch/metadata/ontologies/skos/ebu_ParentalGuidanceCodeCS> ;
        skos:example      "" ;
        skos:definition   "\"No youth admitted\", only adults"@en ;
        skos:historyNote  "" .

parentalguidance:_52.5
        skos:historyNote  "2019-06-24" ;
        skos:changeNote   "Change termId from 18.x to 52.x" ;
        skos:prefLabel    "18+"@de ;
        skos:prefLabel    "18+"@en ;
        skos:definition   "\"No youth admitted\", only adults"@en ;
        skos:example      "" ;
        skos:definition   "Keine Jugendfreigabe"@de ;
        skos:inScheme     <http://www.ebu.ch/metadata/ontologies/skos/ebu_ParentalGuidanceCodeCS> ;
        rdf:type          ebucore:TargetAudience ;
        skos:broader      parentalguidance:_52 .

parentalguidance:_23.2.5
        skos:example      "" ;
        skos:historyNote  "" ;
        skos:changeNote   "" ;
        skos:inScheme     <http://www.ebu.ch/metadata/ontologies/skos/ebu_ParentalGuidanceCodeCS> ;
        skos:broader      parentalguidance:_23.2 ;
        skos:prefLabel    "Sex"@en ;
        rdf:type          ebucore:TargetAudience .

parentalguidance:_63.1.3
        skos:example      "" ;
        skos:historyNote  "" ;
        skos:changeNote   "" ;
        skos:inScheme     <http://www.ebu.ch/metadata/ontologies/skos/ebu_ParentalGuidanceCodeCS> ;
        skos:broader      parentalguidance:_63.1 ;
        skos:definition   "Suitable only for persons 12 years and older. No one under this\n         age is admitted. "@en ;
        skos:prefLabel    "12"@en ;
        rdf:type          ebucore:TargetAudience .

parentalguidance:_42.1
        skos:example      "" ;
        skos:historyNote  "" ;
        skos:changeNote   "" ;
        skos:inScheme     <http://www.ebu.ch/metadata/ontologies/skos/ebu_ParentalGuidanceCodeCS> ;
        skos:broader      parentalguidance:_42 ;
        skos:definition   "os espectáculos de curta duração e de fácil compreensão que não\n         provoquem reacções de pavor e que não colidam com a fantasia e com o sentido lúdico deste\n         nível etário."@pt ;
        skos:definition   "For persons of age 4 and above"@en ;
        skos:prefLabel    "M/4"@en ;
        rdf:type          ebucore:TargetAudience .

parentalguidance:_47.2.21
        skos:example      "" ;
        skos:historyNote  "" ;
        skos:changeNote   "" ;
        skos:inScheme     <http://www.ebu.ch/metadata/ontologies/skos/ebu_ParentalGuidanceCodeCS> ;
        skos:broader      parentalguidance:_47.2 ;
        skos:definition   "Depictions of rape or other violent sexual acts" ;
        skos:prefLabel    "Sexual Violence"@en ;
        rdf:type          ebucore:TargetAudience .

parentalguidance:_61.1.5
        skos:example      "" ;
        skos:historyNote  "" ;
        skos:changeNote   "" ;
        skos:inScheme     <http://www.ebu.ch/metadata/ontologies/skos/ebu_ParentalGuidanceCodeCS> ;
        skos:broader      parentalguidance:_61.1 ;
        skos:definition   "Not recommended until 18 "@en ;
        skos:prefLabel    "18+ (blue)"@en ;
        rdf:type          ebucore:TargetAudience .

parentalguidance:_51.2.5
        skos:example      "" ;
        skos:historyNote  "" ;
        skos:changeNote   "" ;
        skos:inScheme     <http://www.ebu.ch/metadata/ontologies/skos/ebu_ParentalGuidanceCodeCS> ;
        skos:broader      parentalguidance:_51.2 ;
        skos:definition   "Sex"@en ;
        skos:prefLabel    "S"@en ;
        rdf:type          ebucore:TargetAudience .

parentalguidance:_53.1.1
        skos:example      "" ;
        skos:historyNote  "" ;
        skos:changeNote   "" ;
        skos:inScheme     <http://www.ebu.ch/metadata/ontologies/skos/ebu_ParentalGuidanceCodeCS> ;
        skos:broader      parentalguidance:_53.1 ;
        skos:definition   "Suitable for all audiences "@en ;
        skos:prefLabel    "U"@en ;
        rdf:type          ebucore:TargetAudience .

parentalguidance:_41.3
        skos:example      "" ;
        skos:historyNote  "" ;
        skos:changeNote   "" ;
        skos:inScheme     <http://www.ebu.ch/metadata/ontologies/skos/ebu_ParentalGuidanceCodeCS> ;
        skos:broader      parentalguidance:_41 ;
        skos:definition   "For persons of age 12 and above. Parental Guidance is\n         suggested."@en ;
        skos:prefLabel    "12"@en ;
        rdf:type          ebucore:TargetAudience .

parentalguidance:_28.6
        skos:example      "" ;
        skos:historyNote  "" ;
        skos:changeNote   "" ;
        skos:inScheme     <http://www.ebu.ch/metadata/ontologies/skos/ebu_ParentalGuidanceCodeCS> ;
        skos:broader      parentalguidance:_28 ;
        skos:definition   "Adults only"@en ;
        skos:prefLabel    "18"@en ;
        rdf:type          ebucore:TargetAudience .

parentalguidance:_17.4
        skos:example      "" ;
        skos:historyNote  "" ;
        skos:changeNote   "" ;
        skos:inScheme     <http://www.ebu.ch/metadata/ontologies/skos/ebu_ParentalGuidanceCodeCS> ;
        skos:broader      parentalguidance:_17 ;
        skos:definition   "Suitable for people aged 15 and over"@en ;
        skos:prefLabel    "15"@en ;
        rdf:type          ebucore:TargetAudience .

parentalguidance:_18.1
        skos:broader      parentalguidance:_18 ;
        skos:definition   "Ohne Altersbeschränkung"@de ;
        skos:definition   "For all ages"@en ;
        skos:inScheme     <http://www.ebu.ch/metadata/ontologies/skos/ebu_ParentalGuidanceCodeCS> ;
        rdf:type          ebucore:TargetAudience ;
        skos:historyNote  "" ;
        skos:example      "" ;
        skos:changeNote   "" ;
        skos:prefLabel    "0"@de ;
        skos:prefLabel    "0"@en .

parentalguidance:_30.2
        skos:example      "" ;
        skos:historyNote  "" ;
        skos:changeNote   "" ;
        skos:inScheme     <http://www.ebu.ch/metadata/ontologies/skos/ebu_ParentalGuidanceCodeCS> ;
        skos:broader      parentalguidance:_30 ;
        skos:definition   "Children allowed, but parental guidance is strongly\n         advised."@en ;
        skos:prefLabel    "Yellow"@en ;
        rdf:type          ebucore:TargetAudience .

parentalguidance:_24.7.1
        skos:example      "" ;
        skos:historyNote  "" ;
        skos:changeNote   "" ;
        skos:inScheme     <http://www.ebu.ch/metadata/ontologies/skos/ebu_ParentalGuidanceCodeCS> ;
        skos:broader      parentalguidance:_24.7 ;
        skos:definition   "Parental Guidance option - children 2 years of age under the K\n         limits may access the show in presence of an accompanying adult"@en ;
        skos:prefLabel    "PG"@en ;
        rdf:type          ebucore:TargetAudience .

parentalguidance:_53.1
        skos:example      "" ;
        skos:historyNote  "" ;
        skos:prefLabel    "Rating"@en ;
        skos:narrower     parentalguidance:_53.1.5 ;
        rdf:type          ebucore:TargetAudience ;
        skos:changeNote   "" ;
        skos:narrower     parentalguidance:_53.1.2 ;
        skos:inScheme     <http://www.ebu.ch/metadata/ontologies/skos/ebu_ParentalGuidanceCodeCS> ;
        skos:narrower     parentalguidance:_53.1.4 ;
        skos:broader      parentalguidance:_53 ;
        skos:narrower     parentalguidance:_53.1.1 ;
        skos:narrower     parentalguidance:_53.1.3 .

parentalguidance:_52.4
        skos:broader      parentalguidance:_52 ;
        skos:definition   "People 16 or older admitted"@en ;
        skos:prefLabel    "16+"@de ;
        skos:prefLabel    "16+"@en ;
        skos:inScheme     <http://www.ebu.ch/metadata/ontologies/skos/ebu_ParentalGuidanceCodeCS> ;
        skos:changeNote   "Change termId from 18.x to 52.x" ;
        skos:example      "" ;
        skos:historyNote  "2019-06-24" ;
        skos:definition   "Freigegeben ab 16 Jahren"@de ;
        rdf:type          ebucore:TargetAudience .

parentalguidance:_58.1.4
        skos:example      "" ;
        skos:historyNote  "" ;
        skos:changeNote   "" ;
        skos:inScheme     <http://www.ebu.ch/metadata/ontologies/skos/ebu_ParentalGuidanceCodeCS> ;
        skos:broader      parentalguidance:_58.1 ;
        skos:definition   "Younger than 12 Not Recommended "@en ;
        skos:prefLabel    "MS-12"@en ;
        rdf:type          ebucore:TargetAudience .

parentalguidance:_31.2.6
        skos:example      "" ;
        skos:historyNote  "" ;
        skos:changeNote   "" ;
        skos:inScheme     <http://www.ebu.ch/metadata/ontologies/skos/ebu_ParentalGuidanceCodeCS> ;
        skos:broader      parentalguidance:_31.2 ;
        skos:prefLabel    "Gambling"@en ;
        skos:prefLabel    "ギャンブル"@ja ;
        rdf:type          ebucore:TargetAudience .

parentalguidance:_29.2
        skos:changeNote   "" ;
        skos:definition   "a programme aimed specifically at children ages 5–10. May\n         contain mild cartoon or fantasy violence."@en ;
        rdf:type          ebucore:TargetAudience ;
        skos:inScheme     <http://www.ebu.ch/metadata/ontologies/skos/ebu_ParentalGuidanceCodeCS> ;
        skos:broader      parentalguidance:_29 ;
        skos:prefLabel    "CH"@en ;
        skos:example      "" ;
        skos:prefLabel    "Páistí"@ga ;
        skos:historyNote  "" ;
        skos:prefLabel    "Children"@en .

parentalguidance:_28.5
        skos:example      "" ;
        skos:historyNote  "" ;
        skos:changeNote   "" ;
        skos:inScheme     <http://www.ebu.ch/metadata/ontologies/skos/ebu_ParentalGuidanceCodeCS> ;
        skos:broader      parentalguidance:_28 ;
        skos:definition   "Films classified in this category are considered to be suitable\n         for persons of sixteen or over. Children under this age cannot be admitted to\n         cinemas."@en ;
        skos:prefLabel    "16"@en ;
        rdf:type          ebucore:TargetAudience .

parentalguidance:_23.1.5
        skos:example      "" ;
        skos:historyNote  "" ;
        skos:changeNote   "" ;
        skos:inScheme     <http://www.ebu.ch/metadata/ontologies/skos/ebu_ParentalGuidanceCodeCS> ;
        skos:broader      parentalguidance:_23.1 ;
        skos:definition   "This rating is suitable only for persons 18 years of age and\n         older with graphic violence, strong sexual content, explicit references to gambling, and\n         vulgar language (spoken and used in song lyrics)"@en ;
        skos:prefLabel    "18+"@en ;
        rdf:type          ebucore:TargetAudience .

parentalguidance:_39.8
        skos:example      "" ;
        skos:historyNote  "" ;
        skos:changeNote   "" ;
        skos:inScheme     <http://www.ebu.ch/metadata/ontologies/skos/ebu_ParentalGuidanceCodeCS> ;
        skos:broader      parentalguidance:_39 ;
        skos:definition   "Restricted to a particular class of persons, or for particular\n         purposes, or both, specified by the Office of Film and Literature\n         Classification"@en ;
        skos:prefLabel    "Restricted"@en ;
        skos:prefLabel    "R"@en ;
        rdf:type          ebucore:TargetAudience .

parentalguidance:_3.6
        skos:example      "" ;
        skos:historyNote  "" ;
        skos:changeNote   "" ;
        skos:inScheme     <http://www.ebu.ch/metadata/ontologies/skos/ebu_ParentalGuidanceCodeCS> ;
        skos:broader      parentalguidance:_3 ;
        skos:definition   "The X 18+ classification only applies to films that contain\n         sexually explicit material between consenting adults. It is restricted to persons aged 18\n         years and over and can only be sold or hired legally in the ACT and the Northern Territory.\n         The possession and supply of X 18+ films is prohibited in prescribed areas of the Northern\n         Territory."@en ;
        skos:prefLabel    "Restricted to 18 and over"@en ;
        skos:prefLabel    "X18+"@en ;
        rdf:type          ebucore:TargetAudience .

parentalguidance:_63.1.2
        skos:example      "" ;
        skos:historyNote  "" ;
        skos:changeNote   "" ;
        skos:inScheme     <http://www.ebu.ch/metadata/ontologies/skos/ebu_ParentalGuidanceCodeCS> ;
        skos:broader      parentalguidance:_63.1 ;
        skos:definition   "Some material may be unsuitable for younger children. Children\n         under the age of 12 are to be accompanied by an adult. "@en ;
        skos:prefLabel    "PG (Parental Guidance)"@en ;
        rdf:type          ebucore:TargetAudience .

parentalguidance:_23.2.2
        skos:example      "" ;
        skos:historyNote  "" ;
        skos:changeNote   "" ;
        skos:inScheme     <http://www.ebu.ch/metadata/ontologies/skos/ebu_ParentalGuidanceCodeCS> ;
        skos:broader      parentalguidance:_23.2 ;
        skos:prefLabel    "Discrimination"@en ;
        rdf:type          ebucore:TargetAudience .

parentalguidance:_47.2.32
        skos:example      "" ;
        skos:historyNote  "" ;
        skos:changeNote   "" ;
        skos:inScheme     <http://www.ebu.ch/metadata/ontologies/skos/ebu_ParentalGuidanceCodeCS> ;
        skos:broader      parentalguidance:_47.2 ;
        skos:definition   "Scenes involving aggressive conflict" ;
        skos:prefLabel    "Violence"@en ;
        rdf:type          ebucore:TargetAudience .

parentalguidance:_41.2
        skos:example      "" ;
        skos:historyNote  "" ;
        skos:changeNote   "" ;
        skos:inScheme     <http://www.ebu.ch/metadata/ontologies/skos/ebu_ParentalGuidanceCodeCS> ;
        skos:broader      parentalguidance:_41 ;
        skos:definition   "For persons of age 10 and above. Parental Guidance is\n         suggested."@en ;
        skos:prefLabel    "7"@en ;
        rdf:type          ebucore:TargetAudience .

parentalguidance:_47.2.20
        skos:example      "" ;
        skos:historyNote  "" ;
        skos:changeNote   "" ;
        skos:inScheme     <http://www.ebu.ch/metadata/ontologies/skos/ebu_ParentalGuidanceCodeCS> ;
        skos:broader      parentalguidance:_47.2 ;
        skos:definition   "Mild to moderate sexual references and/or depictions. May include\n         partial nudity" ;
        skos:prefLabel    "Sexual Themes"@en ;
        rdf:type          ebucore:TargetAudience .

parentalguidance:_51.2.4
        skos:example      "" ;
        skos:historyNote  "" ;
        skos:changeNote   "" ;
        skos:inScheme     <http://www.ebu.ch/metadata/ontologies/skos/ebu_ParentalGuidanceCodeCS> ;
        skos:broader      parentalguidance:_51.2 ;
        skos:definition   "Biased or prejudiced with regard to race, ethnicity, gender,\n         religion, or other group identifiable characteristics"@en ;
        skos:prefLabel    "P"@en ;
        rdf:type          ebucore:TargetAudience .

parentalguidance:_53.1.2
        skos:example      "" ;
        skos:historyNote  "" ;
        skos:changeNote   "" ;
        skos:inScheme     <http://www.ebu.ch/metadata/ontologies/skos/ebu_ParentalGuidanceCodeCS> ;
        skos:broader      parentalguidance:_53.1 ;
        skos:definition   ""@en ;
        skos:prefLabel    "12"@en ;
        rdf:type          ebucore:TargetAudience .

parentalguidance:_51.1.7
        skos:example      "" ;
        skos:historyNote  "" ;
        skos:changeNote   "" ;
        skos:inScheme     <http://www.ebu.ch/metadata/ontologies/skos/ebu_ParentalGuidanceCodeCS> ;
        skos:broader      parentalguidance:_51.1 ;
        skos:definition   "Adults only"@en ;
        skos:prefLabel    "18"@en ;
        rdf:type          ebucore:TargetAudience .

parentalguidance:_17.5
        skos:example      "" ;
        skos:historyNote  "" ;
        skos:changeNote   "" ;
        skos:inScheme     <http://www.ebu.ch/metadata/ontologies/skos/ebu_ParentalGuidanceCodeCS> ;
        skos:broader      parentalguidance:_17 ;
        skos:definition   "Suitable for people aged 18 and over"@en ;
        skos:prefLabel    "18"@en ;
        rdf:type          ebucore:TargetAudience .

parentalguidance:_58.1.6
        skos:example      "" ;
        skos:historyNote  "" ;
        skos:changeNote   "" ;
        skos:inScheme     <http://www.ebu.ch/metadata/ontologies/skos/ebu_ParentalGuidanceCodeCS> ;
        skos:broader      parentalguidance:_58.1 ;
        skos:definition   "Younger than 14 Prohibited"@en ;
        skos:prefLabel    "K-14"@en ;
        rdf:type          ebucore:TargetAudience .

parentalguidance:_18.2
        skos:changeNote   "" ;
        skos:definition   "Freigegeben ab 6 Jahren"@de ;
        skos:inScheme     <http://www.ebu.ch/metadata/ontologies/skos/ebu_ParentalGuidanceCodeCS> ;
        skos:broader      parentalguidance:_18 ;
        skos:definition   "No one under 6 years admitted"@en ;
        skos:prefLabel    "6"@de ;
        skos:prefLabel    "6"@en ;
        rdf:type          ebucore:TargetAudience ;
        skos:historyNote  "" ;
        skos:example      "" .

parentalguidance:_30.1
        skos:example      "" ;
        skos:historyNote  "" ;
        skos:changeNote   "" ;
        skos:inScheme     <http://www.ebu.ch/metadata/ontologies/skos/ebu_ParentalGuidanceCodeCS> ;
        skos:broader      parentalguidance:_30 ;
        skos:definition   "All audiences allowed"@en ;
        skos:prefLabel    "Green"@en ;
        rdf:type          ebucore:TargetAudience .

parentalguidance:_61.1.6
        skos:example      "" ;
        skos:historyNote  "" ;
        skos:changeNote   "" ;
        skos:inScheme     <http://www.ebu.ch/metadata/ontologies/skos/ebu_ParentalGuidanceCodeCS> ;
        skos:broader      parentalguidance:_61.1 ;
        skos:definition   "Prohibited for minors "@en ;
        skos:prefLabel    "18+ (red)"@en ;
        rdf:type          ebucore:TargetAudience .

parentalguidance:_60  skos:definition  "Lembaga Sensor Film"@en ;
        skos:inScheme     <http://www.ebu.ch/metadata/ontologies/skos/ebu_ParentalGuidanceCodeCS> ;
        skos:changeNote   "Update" ;
        skos:historyNote  "2010-08-03" ;
        skos:prefLabel    "ID-LSF"@en ;
        skos:note         "Valid" ;
        skos:scopeNote    "Region:Indonesia"@en ;
        skos:example      "" ;
        rdf:type          ebucore:TargetAudience ;
        skos:narrower     parentalguidance:_60.1 .

parentalguidance:_52.3
        skos:changeNote   "Change termId from 18.x to 52.x" ;
        skos:example      "" ;
        skos:inScheme     <http://www.ebu.ch/metadata/ontologies/skos/ebu_ParentalGuidanceCodeCS> ;
        skos:prefLabel    "12+"@de ;
        skos:prefLabel    "12+"@en ;
        skos:definition   "Freigegeben ab 12 Jahren"@de ;
        skos:broader      parentalguidance:_52 ;
        rdf:type          ebucore:TargetAudience ;
        skos:historyNote  "2019-06-24" ;
        skos:definition   "People 12 or older admitted, children between 6 and 11 only\n         when accompanied by parent or legal guardian"@en .

parentalguidance:_58.1.5
        skos:example      "" ;
        skos:historyNote  "" ;
        skos:changeNote   "" ;
        skos:inScheme     <http://www.ebu.ch/metadata/ontologies/skos/ebu_ParentalGuidanceCodeCS> ;
        skos:broader      parentalguidance:_58.1 ;
        skos:definition   "Younger than 12 Prohibited"@en ;
        skos:prefLabel    "K-12"@en ;
        rdf:type          ebucore:TargetAudience .

parentalguidance:_31.2.7
        skos:example      "" ;
        skos:historyNote  "" ;
        skos:changeNote   "" ;
        skos:inScheme     <http://www.ebu.ch/metadata/ontologies/skos/ebu_ParentalGuidanceCodeCS> ;
        skos:broader      parentalguidance:_31.2 ;
        skos:prefLabel    "Murder"@en ;
        skos:prefLabel    "犯罪"@ja ;
        rdf:type          ebucore:TargetAudience .

parentalguidance:_29.3
        skos:broader      parentalguidance:_29 ;
        skos:prefLabel    "Young Adult"@en ;
        skos:definition   "a programme aimed at an adolescent audience. That is to say it\n         would not be of great interest to an adult. However, it might deal with issues which affect\n         the teenage and late preteen audience, e.g. relationships, sexual activity, sexuality, soft\n         drugs. Parents and guardians could expect that \"YA\" programmes might contain such material\n         and may choose to limit their children's access."@en ;
        skos:example      "" ;
        skos:prefLabel    "Ógra"@ga ;
        skos:historyNote  "" ;
        skos:inScheme     <http://www.ebu.ch/metadata/ontologies/skos/ebu_ParentalGuidanceCodeCS> ;
        skos:prefLabel    "YA"@en ;
        rdf:type          ebucore:TargetAudience ;
        skos:changeNote   "" .

parentalguidance:_17.6
        skos:example      "" ;
        skos:historyNote  "" ;
        skos:changeNote   "" ;
        skos:inScheme     <http://www.ebu.ch/metadata/ontologies/skos/ebu_ParentalGuidanceCodeCS> ;
        skos:broader      parentalguidance:_17 ;
        skos:definition   "Adult - Pornographic Content"@en ;
        skos:definition   "Adulto"@es ;
        skos:prefLabel    "X"@en ;
        rdf:type          ebucore:TargetAudience .

parentalguidance:_23.2.3
        skos:example      "" ;
        skos:historyNote  "" ;
        skos:changeNote   "" ;
        skos:inScheme     <http://www.ebu.ch/metadata/ontologies/skos/ebu_ParentalGuidanceCodeCS> ;
        skos:broader      parentalguidance:_23.2 ;
        skos:prefLabel    "Drugs"@en ;
        rdf:type          ebucore:TargetAudience .

parentalguidance:_63.1.1
        skos:example      "" ;
        skos:historyNote  "" ;
        skos:changeNote   "" ;
        skos:inScheme     <http://www.ebu.ch/metadata/ontologies/skos/ebu_ParentalGuidanceCodeCS> ;
        skos:broader      parentalguidance:_63.1 ;
        skos:definition   "General viewing for all ages."@en ;
        skos:prefLabel    "U /Universal)"@en ;
        rdf:type          ebucore:TargetAudience .

parentalguidance:_5.1
        skos:prefLabel    "EA"@fr ;
        skos:broader      parentalguidance:_5 ;
        rdf:type          ebucore:TargetAudience ;
        skos:prefLabel    "KT"@nl ;
        skos:prefLabel    "Children Allowed"@en ;
        skos:definition   "Kinderen Toegelaten"@nl ;
        skos:example      "" ;
        skos:historyNote  "" ;
        skos:inScheme     <http://www.ebu.ch/metadata/ontologies/skos/ebu_ParentalGuidanceCodeCS> ;
        skos:definition   "Children admitted - Suitable for all"@en ;
        skos:changeNote   "" ;
        skos:definition   "Enfants admis"@fr .

parentalguidance:_39.7
        skos:example      "" ;
        skos:historyNote  "" ;
        skos:changeNote   "" ;
        skos:inScheme     <http://www.ebu.ch/metadata/ontologies/skos/ebu_ParentalGuidanceCodeCS> ;
        skos:broader      parentalguidance:_39 ;
        skos:definition   "Suitable to persons 18 years of age and over (awarded by the\n         Office of Film and Literature Classification only)"@en ;
        skos:prefLabel    "R18"@en ;
        rdf:type          ebucore:TargetAudience .

_:b4    rdf:rest   rdf:nil ;
        rdf:first  parentalguidance:_31 .

parentalguidance:_68.1.4
        skos:example      "" ;
        skos:historyNote  "" ;
        skos:changeNote   "" ;
        skos:inScheme     <http://www.ebu.ch/metadata/ontologies/skos/ebu_ParentalGuidanceCodeCS> ;
        skos:broader      parentalguidance:_68.1 ;
        skos:definition   "18 years"@en ;
        skos:definition   "18 anni"@it ;
        skos:prefLabel    "VM18"@en ;
        rdf:type          ebucore:TargetAudience .
