@prefix rdf: <http://www.w3.org/1999/02/22-rdf-syntax-ns#> .
@prefix ebucore: <http://www.ebu.ch/metadata/ontologies/ebucore/ebucore#> .
@prefix skos: <http://www.w3.org/2004/02/skos/core#> .
@prefix owl: <http://www.w3.org/2002/07/owl#> .
@prefix dc: <http://purl.org/dc/elements/1.1/> .
@prefix dct: <http://purl.org/dc/terms/> .
@prefix rdfs: <http://www.w3.org/2000/01/rdf-schema#> .


<https://metadata.amagi.tv/skos/amagi_ebu_IdentifierTypeCS>
    a skos:ConceptScheme ;
    rdfs:isDefinedBy <https://metadata.amagi.tv/skos/amagi_ebu_IdentifierTypeCS> ;
    rdfs:label "EBU SKOS Classification Scheme for media IdentifierType"@en .

<https://metadata.amagi.tv/skos/amagi_ebu_IdentifierTypeCS#_amgastid>
    a ebucore:IdentifierType ;
    skos:changeNote """First version""" ;
    skos:definition """unique identifier for asset ingested using amagi"""@en ;
    skos:example "" ;
    skos:historyNote "2023-11-03" ;
    skos:inScheme <https://metadata.amagi.tv/skos/amagi_ebu_IdentifierTypeCS> ;
    skos:note "Valid" ;
    skos:prefLabel "AMAGI-ASSETID"@en .


<https://metadata.amagi.tv/skos/amagi_ebu_IdentifierTypeCS#_tmsid>
    a ebucore:IdentifierType ;
    skos:changeNote """First version""" ;
    skos:definition """Gracenote TMSID. Check https://en.wikipedia.org/wiki/TMS_(entertainment_data) and https://www.gracenote.com/gracenote-id/"""@en ;
    skos:example "MV003331980000" ;
    skos:historyNote "2022-11-29" ;
    skos:inScheme <https://metadata.amagi.tv/skos/amagi_ebu_IdentifierTypeCS> ;
    skos:note "Valid" ;
    skos:prefLabel "TMSID"@en .


<https://metadata.amagi.tv/skos/amagi_ebu_IdentifierTypeCS#_eidr>
    a ebucore:IdentifierType ;
    skos:changeNote """First version""" ;
    skos:definition """The universal media identifier. Check https://www.eidr.org/"""@en ;
    skos:example "" ;
    skos:historyNote "2022-11-29" ;
    skos:inScheme <https://metadata.amagi.tv/skos/amagi_ebu_IdentifierTypeCS> ;
    skos:note "Valid" ;
    skos:prefLabel "EIDR"@en .

<https://metadata.amagi.tv/skos/amagi_ebu_IdentifierTypeCS#_imdb>
    a ebucore:IdentifierType ;
    skos:changeNote """First version""" ;
    skos:definition """IMDB identifier. Check https://www.imdb.org/"""@en ;
    skos:example "" ;
    skos:historyNote "2022-11-29" ;
    skos:inScheme <https://metadata.amagi.tv/skos/amagi_ebu_IdentifierTypeCS> ;
    skos:note "Valid" ;
    skos:prefLabel "IMDB"@en .

<https://metadata.amagi.tv/skos/amagi_ebu_IdentifierTypeCS#_wikidata>
    a ebucore:IdentifierType ;
    skos:changeNote """First version""" ;
    skos:definition """Wikidata identifier. Check https://www.wikidata.org/"""@en ;
    skos:example "" ;
    skos:historyNote "2023-10-25" ;
    skos:inScheme <https://metadata.amagi.tv/skos/amagi_ebu_IdentifierTypeCS> ;
    skos:note "Valid" ;
    skos:prefLabel "WIKI"@en .

<https://metadata.amagi.tv/skos/amagi_ebu_IdentifierTypeCS#_iptcmediatopic>
    a ebucore:IdentifierType ;
    skos:changeNote """First version""" ;
    skos:definition """iptc mediatopic identifier. Check http://cv.iptc.org/newscodes/mediatopic/"""@en ;
    skos:example "" ;
    skos:historyNote "2023-11-03" ;
    skos:inScheme <https://metadata.amagi.tv/skos/amagi_ebu_IdentifierTypeCS> ;
    skos:note "Valid" ;
    skos:prefLabel "IPTC-MEDIATOPIC"@en .

<https://metadata.amagi.tv/skos/amagi_ebu_IdentifierTypeCS#_iab30>
    a ebucore:IdentifierType ;
    skos:changeNote """First version""" ;
    skos:definition """iab 3.0 content taxonomy. Check https://github.com/InteractiveAdvertisingBureau/Taxonomies/blob/main/Content%20Taxonomies/Content%20Taxonomy%203.0.tsv"""@en ;
    skos:example "" ;
    skos:historyNote "2023-11-10" ;
    skos:inScheme <https://metadata.amagi.tv/skos/amagi_ebu_IdentifierTypeCS> ;
    skos:note "Valid" ;
    skos:prefLabel "IAB-3.0"@en .

<https://metadata.amagi.tv/skos/amagi_ebu_IdentifierTypeCS#_gracenote>
    a ebucore:IdentifierType ;
    skos:changeNote """First version""" ;
    skos:definition """Gracenote TMSID. Check https://en.wikipedia.org/wiki/TMS_(entertainment_data) and https://www.gracenote.com/gracenote-id"""@en ;
    skos:example "MV003331980000" ;
    skos:historyNote "2023-11-10" ;
    skos:inScheme <https://metadata.amagi.tv/skos/amagi_ebu_IdentifierTypeCS> ;
    skos:note "Valid" ;
    skos:prefLabel "gracenote"@en .

<https://metadata.amagi.tv/skos/amagi_ebu_IdentifierTypeCS#_provider_guid>
    a ebucore:IdentifierType ;
    skos:changeNote """First version""" ;
    skos:definition """Unique id from the provider"""@en ;
    skos:example "tmk-video-2779f930951347e0ad939b05f43a8ff8" ;
    skos:historyNote "2023-11-10" ;
    skos:inScheme <https://metadata.amagi.tv/skos/amagi_ebu_IdentifierTypeCS> ;
    skos:note "Valid" ;
    skos:prefLabel "provider_guid"@en .

<https://metadata.amagi.tv/skos/amagi_ebu_IdentifierTypeCS#_tastemade>
    a ebucore:IdentifierType ;
    skos:changeNote """First version""" ;
    skos:definition """external id provided from tastemade"""@en ;
    skos:example "37190" ;
    skos:historyNote "2023-11-10" ;
    skos:inScheme <https://metadata.amagi.tv/skos/amagi_ebu_IdentifierTypeCS> ;
    skos:note "Valid" ;
    skos:prefLabel "tastemade"@en .

<https://metadata.amagi.tv/skos/amagi_ebu_IdentifierTypeCS#_amagi>
    a ebucore:IdentifierType ;
    skos:changeNote """First version""" ;
    skos:definition """external id provided by amagi"""@en ;
    skos:example "ACm1io6d5z76aehcyESGbki" ;
    skos:historyNote "2023-11-10" ;
    skos:inScheme <https://metadata.amagi.tv/skos/amagi_ebu_IdentifierTypeCS> ;
    skos:note "Valid" ;
    skos:prefLabel "Amagi"@en .

<https://metadata.amagi.tv/skos/amagi_ebu_IdentifierTypeCS#_cpaltid>
    a ebucore:IdentifierType ;
    skos:changeNote """First version""" ;
    skos:definition """Content partner alternate identifier. 
        Can be used to allow the content partner who is the amagi 
        account holder ingesting the assets to store an additional identifier. 
        This e.g. can be used to store additional identifiers for collections."""@en ;
    skos:example "S0_A0_123" ;
    skos:historyNote "2024-10-25" ;
    skos:inScheme <https://metadata.amagi.tv/skos/amagi_ebu_IdentifierTypeCS> ;
    skos:note "Valid" ;
    skos:prefLabel "ALTERNATE-ID"@en .

<https://metadata.amagi.tv/skos/amagi_ebu_IdentifierTypeCS#_aichatid>
    a ebucore:IdentifierType ;
    skos:changeNote """First version""" ;
    skos:definition """Chat-ID provided in response of AI metadata generation. This chat-id will be used in the UI to call chat interaction to fine tune the response"""@en ;
    skos:example "39ij490jk" ;
    skos:historyNote "2025-03-25" ;
    skos:inScheme <https://metadata.amagi.tv/skos/amagi_ebu_IdentifierTypeCS> ;
    skos:note "Valid" ;
    skos:prefLabel "ai_chat_id"@en .

<https://metadata.amagi.tv/skos/amagi_ebu_IdentifierTypeCS#_aisummarychatid>
    a ebucore:IdentifierType ;
    skos:changeNote """First version""" ;
    skos:definition """Chat-ID provided in response of AI summary metadata generation. This chat-id will be used in the UI to call chat interaction to fine tune the response"""@en ;
    skos:example "39ij490jk" ;
    skos:historyNote "2025-03-25" ;
    skos:inScheme <https://metadata.amagi.tv/skos/amagi_ebu_IdentifierTypeCS> ;
    skos:note "Valid" ;
    skos:prefLabel "ai_summary_chat_id"@en .

<https://metadata.amagi.tv/skos/amagi_ebu_IdentifierTypeCS#_aisynopsischatid>
    a ebucore:IdentifierType ;
    skos:changeNote """First version""" ;
    skos:definition """Chat-ID provided in response of AI synopsis metadata generation. This chat-id will be used in the UI to call chat interaction to fine tune the response"""@en ;
    skos:example "39ij490jk" ;
    skos:historyNote "2025-03-25" ;
    skos:inScheme <https://metadata.amagi.tv/skos/amagi_ebu_IdentifierTypeCS> ;
    skos:note "Valid" ;
    skos:prefLabel "ai_synopsis_chat_id"@en .
