@prefix rdf: <http://www.w3.org/1999/02/22-rdf-syntax-ns#> .
@prefix ebucore: <http://www.ebu.ch/metadata/ontologies/ebucore/ebucore#> .
@prefix skos: <http://www.w3.org/2004/02/skos/core#> .
@prefix owl: <http://www.w3.org/2002/07/owl#> .
@prefix dc: <http://purl.org/dc/elements/1.1/> .
@prefix dct: <http://purl.org/dc/terms/> .
@prefix rdfs: <http://www.w3.org/2000/01/rdf-schema#> .
@prefix ast_type: <https://metadata.amagi.tv/skos/amagi_ebu_AssetTypeCS#> .

<https://metadata.amagi.tv/skos/amagi_ebu_AssetTypeCS.rdf>
        rdf:type         owl:Ontology ;
        dct:title        "EBU Based SKOS Classification Scheme for Asset Types"@en ;
        dct:contributor  "Amagi metadata community" ;
        dct:description  "An RDF vocabulary defining additional types to be used for assets"@en ;
        dct:creator      "Shashidhar, Amagi, shashidhar@amagi.com" ;
        dct:publisher    "EBU" ;
        dct:rights       "http://creativecommons.org/licenses/by-nc-sa/3.0/" .

<https://metadata.amagi.tv/skos/amagi_ebu_AssetTypeCS>
        rdf:type            skos:ConceptScheme ;
        rdfs:label          "EBU SKOS Classification Scheme for Asset Type"@en ;
        rdfs:isDefinedBy    <https://metadata.amagi.tv/skos/amagi_ebu_AssetTypeCS> ;
        skos:hasTopConcept  ast_type:_1 ;
        skos:hasTopConcept  ast_type:_2 ;
        skos:hasTopConcept  ast_type:_3 ;
        skos:hasTopConcept  ast_type:_4 .

ast_type:_1
        rdf:type        ebucore:AssetType ;
        skos:prefLabel  "Video"@en ;
        skos:definition   "Video Asset Type Top Concept" ;
        skos:inScheme    <https://metadata.amagi.tv/skos/amagi_ebu_AssetTypeCS> ;
        skos:narrower    ast_type:_1.1 ;
        skos:narrower    ast_type:_1.2 ;
        skos:changeNote "" ;
        skos:historyNote "2023-08-27" ;
        skos:note "Valid" . 

ast_type:_1.1
        rdf:type        ebucore:AssetType ;
        skos:prefLabel  "Feature"@en ;
        skos:definition   "Standalone feature videos e.g. movies, ads etc." ;
        skos:inScheme    <https://metadata.amagi.tv/skos/amagi_ebu_AssetTypeCS> ;
        skos:broader     ast_type:_1 ;
        skos:narrower    ast_type:_1.1.1 ;
        skos:narrower    ast_type:_1.1.2 ;
        skos:narrower    ast_type:_1.1.3 ;
        skos:narrower    ast_type:_1.1.4 ;
        skos:narrower    ast_type:_1.1.5 ;
        skos:narrower    ast_type:_1.1.6 ;
        skos:narrower    ast_type:_1.1.7 ;
        skos:narrower    ast_type:_1.1.8 ;
        skos:narrower    ast_type:_1.1.9 ;
        skos:narrower    ast_type:_1.1.10 ;
        skos:narrower    ast_type:_1.1.11 ;
        skos:narrower    ast_type:_1.1.12 ;
        skos:narrower    ast_type:_1.1.13 ;
        skos:narrower    ast_type:_1.1.14 ;
        skos:narrower    ast_type:_1.1.15 ;
        skos:narrower    ast_type:_1.1.16 ;
        skos:narrower    ast_type:_1.1.17 ;
        skos:changeNote "" ;
        skos:historyNote "2023-08-27" ;
        skos:note "Valid" . 

ast_type:_1.2 
        rdf:type        ebucore:AssetType ;
        skos:prefLabel  "Episode"@en ;
        skos:definition   "Episode of a TV Show or a Program" ;
        skos:inScheme    <https://metadata.amagi.tv/skos/amagi_ebu_AssetTypeCS> ;
        skos:broader     ast_type:_1 ;
        skos:narrower    ast_type:_1.2.1 ;
        skos:narrower    ast_type:_1.2.2 ;
        skos:changeNote "" ;
        skos:historyNote "2023-08-27" ;
        skos:note "Valid" .

ast_type:_1.1.1
        rdf:type        ebucore:AssetType ;
        skos:prefLabel  "Movie"@en ;
        skos:definition   "A film – also called a movie, motion picture, moving picture, picture, photoplay is is a series of moving images shown on a screen, usually with sound, that make up a story" ;
        skos:inScheme    <https://metadata.amagi.tv/skos/amagi_ebu_AssetTypeCS> ;
        skos:broader    ast_type:_1.1 ;
        skos:changeNote "" ;
        skos:historyNote "2023-08-27" ;
        skos:note "Valid" .

ast_type:_1.1.2
        rdf:type        ebucore:AssetType ;
        skos:prefLabel  "Short Form"@en ;
        skos:definition   "Any video that is under 10 minutes is classified as a short-form video" ;
        skos:inScheme    <https://metadata.amagi.tv/skos/amagi_ebu_AssetTypeCS> ;
        skos:broader    ast_type:_1.1 ;
        skos:narrower    ast_type:_1.1.2.1 ;
        skos:changeNote "" ;
        skos:historyNote "2023-08-27" ;
        skos:note "Valid" .

ast_type:_1.1.2.1
        rdf:type        ebucore:AssetType ;
        skos:prefLabel  "Shorts Sponsored"@en ;
        skos:definition   "A feature that is short form and sponsored" ;
        skos:inScheme    <https://metadata.amagi.tv/skos/amagi_ebu_AssetTypeCS> ;
        skos:broader    ast_type:_1.1.2 ;
        skos:changeNote "" ;
        skos:historyNote "2024-11-18" ;
        skos:note "Valid" .

ast_type:_1.1.3
        rdf:type        ebucore:AssetType ;
        skos:prefLabel  "TV Show"@en ;
        skos:definition   "Asset Type TV Program or a Show" ;
        skos:inScheme    <https://metadata.amagi.tv/skos/amagi_ebu_AssetTypeCS> ;
        skos:broader    ast_type:_1.1 ;
        skos:narrower    ast_type:_1.1.3.1 ;
        skos:changeNote "" ;
        skos:historyNote "2023-08-27" ;
        skos:note "Valid" .

ast_type:_1.1.3.1
        rdf:type        ebucore:AssetType ;
        skos:prefLabel  "Program"@en ;
        skos:definition   "Asset Type TV Program or a Show" ;
        skos:inScheme    <https://metadata.amagi.tv/skos/amagi_ebu_AssetTypeCS> ;
        skos:broader    ast_type:_1.1.3 ;
        skos:changeNote "" ;
        skos:historyNote "2024-12-12" ;
        skos:note "Valid" .

ast_type:_1.1.4
        rdf:type        ebucore:AssetType ;
        skos:prefLabel  "Advertisement"@en ;
        skos:altLabel  "Commercial"@en ;
        skos:altLabel  "Ad"@en ;
        skos:definition   """A commercial video is a short-form type of advertisement ideally 30 seconds 
                long placed on TV, streaming services, social media platforms, and other digital channels. """ ;
        skos:inScheme    <https://metadata.amagi.tv/skos/amagi_ebu_AssetTypeCS> ;
        skos:broader    ast_type:_1.1 ;
        skos:changeNote "" ;
        skos:historyNote "2023-08-27" ;
        skos:note "Valid" .

ast_type:_1.1.5
        rdf:type        ebucore:AssetType ;
        skos:prefLabel  "Trailer"@en ;
        skos:altLabel  "Preview"@en ;
        skos:definition   """A trailer (also known as a preview, coming attraction or attraction video) is
                 a commercial advertisement, originally for a feature film that is going to be exhibited 
                 in the future at a movie theater/cinema.""" ;
        skos:inScheme    <https://metadata.amagi.tv/skos/amagi_ebu_AssetTypeCS> ;
        skos:broader    ast_type:_1.1 ;
        skos:changeNote "" ;
        skos:historyNote "2023-08-27" ;
        skos:note "Valid" .

ast_type:_1.1.6
        rdf:type        ebucore:AssetType ;
        skos:prefLabel  "Promo"@en ;
        skos:definition   """ Promo is a video used for the express purpose of promoting a specific marketing 
                        initiative, sale, or event. Promos are often similar in style and tone to a teaser video,
                         where you grab your audience’s attention and draw them in to learn more. Promos are
                          primarily used to increase the target audience’s trust in the brand. """ ;
        skos:inScheme    <https://metadata.amagi.tv/skos/amagi_ebu_AssetTypeCS> ;
        skos:broader    ast_type:_1.1 ;
        skos:changeNote "" ;
        skos:historyNote "2023-08-27" ;
        skos:note "Valid" .

ast_type:_1.1.7
        rdf:type        ebucore:AssetType ;
        skos:prefLabel  "Interstitial"@en ;
        skos:definition   """ Interstitial ads are interactive, full-screen ads that cover the interface of 
                        their host app or site. These ads appear between content, so they place at natural
                         transition points or breaks, such as in between activities or game levels. Their 
                         full-coverage is what differentiates them from other ad types, like pop-up, native,
                          and banner ads. """ ;
        skos:inScheme    <https://metadata.amagi.tv/skos/amagi_ebu_AssetTypeCS> ;
        skos:broader    ast_type:_1.1 ;
        skos:changeNote "" ;
        skos:historyNote "2023-08-27" ;
        skos:note "Valid" .

ast_type:_1.1.8
        rdf:type        ebucore:AssetType ;
        skos:prefLabel  "Bumper"@en ;
        skos:definition   """Little segments in shows that come between the show and the commercial break. 
                         Most common types of bump is the 5-second logo animation that pops up reminding you 
                         what show you are watching as you go to or come back from a commercial.""" ;
        skos:inScheme    <https://metadata.amagi.tv/skos/amagi_ebu_AssetTypeCS> ;
        skos:broader    ast_type:_1.1 ;
        skos:narrower    ast_type:_1.1.8.1 ;
        skos:narrower    ast_type:_1.1.8.2 ;
        skos:narrower    ast_type:_1.1.8.3 ;
        skos:changeNote "" ;
        skos:historyNote "2023-08-27" ;
        skos:note "Valid" .

ast_type:_1.1.8.1
        rdf:type        ebucore:AssetType ;
        skos:prefLabel  "BumperIn"@en ;
        skos:definition   "Bumper at beginning of show" ;
        skos:inScheme    <https://metadata.amagi.tv/skos/amagi_ebu_AssetTypeCS> ;
        skos:broader    ast_type:_1.1.8 ;
        skos:changeNote "" ;
        skos:historyNote "2023-08-27" ;
        skos:note "Valid" .

ast_type:_1.1.8.2
        rdf:type        ebucore:AssetType ;
        skos:prefLabel  "BumperOut"@en ;
        skos:definition   "Bumper at exit of show and at entry into ad break" ;
        skos:inScheme    <https://metadata.amagi.tv/skos/amagi_ebu_AssetTypeCS> ;
        skos:broader    ast_type:_1.1.8 ;
        skos:changeNote "" ;
        skos:historyNote "2023-08-27" ;
        skos:note "Valid" .

ast_type:_1.1.8.3
        rdf:type        ebucore:AssetType ;
        skos:prefLabel  "Bumper Sponsored"@en ;
        skos:definition   "Bumper with sponsorship" ;
        skos:inScheme    <https://metadata.amagi.tv/skos/amagi_ebu_AssetTypeCS> ;
        skos:broader    ast_type:_1.1.8 ;
        skos:changeNote "" ;
        skos:historyNote "2024-11-18" ;
        skos:note "Valid" .

ast_type:_1.1.9
        rdf:type        ebucore:AssetType ;
        skos:prefLabel  "Rescue"@en ;
        skos:definition   "Asset Type Rescue" ;
        skos:inScheme    <https://metadata.amagi.tv/skos/amagi_ebu_AssetTypeCS> ;
        skos:broader    ast_type:_1.1 ;
        skos:changeNote "" ;
        skos:historyNote "2023-08-27" ;
        skos:note "Valid" .

ast_type:_1.1.10 
        rdf:type        ebucore:AssetType ;
        skos:prefLabel  "Other"@en ;
        skos:definition   "Asset Type Other" ;
        skos:inScheme    <https://metadata.amagi.tv/skos/amagi_ebu_AssetTypeCS> ;
        skos:broader    ast_type:_1.1 ;
        skos:changeNote "" ;
        skos:historyNote "2023-08-27" ;
        skos:note "Valid" .

ast_type:_1.1.11
        rdf:type        ebucore:AssetType ;
        skos:prefLabel  "Teaser"@en ;
        skos:definition   """A teaser captures an intense clip from the movie without any relevant arrangement 
                        as against a trailer which captures the beginning, middle, and end of a particular movie 
                        in a three-act structure.""" ;
        skos:inScheme    <https://metadata.amagi.tv/skos/amagi_ebu_AssetTypeCS> ;
        skos:broader    ast_type:_1.1 ;
        skos:changeNote "" ;
        skos:historyNote "2023-08-27" ;
        skos:note "Valid" .

ast_type:_1.1.12
        rdf:type        ebucore:AssetType ;
        skos:prefLabel  "Live"@en ;
        skos:definition   "Any Live content streaming which later forms a regular TV show" ;
        skos:inScheme    <https://metadata.amagi.tv/skos/amagi_ebu_AssetTypeCS> ;
        skos:broader    ast_type:_1.1 ;
        skos:changeNote "" ;
        skos:historyNote "2023-08-27" ;
        skos:note "Valid" .

ast_type:_1.1.13
        rdf:type        ebucore:AssetType ;
        skos:prefLabel  "Sponsored"@en ;
        skos:definition   """Sponsored content is a long-form or otherwise in-depth asset whose production is
                          funded by a sponsor, but whose creation and distribution is handled by a partner, 
                          which in turn ensures that the asset closely resembles the non-ad content on its platform. """ ;
        skos:inScheme    <https://metadata.amagi.tv/skos/amagi_ebu_AssetTypeCS> ;
        skos:broader    ast_type:_1.1 ;
        skos:changeNote "" ;
        skos:historyNote "2023-08-27" ;
        skos:note "Valid" . 

ast_type:_1.1.14
        rdf:type        ebucore:AssetType ;
        skos:prefLabel  "Filler"@en ;
        skos:definition   """Filler is video of lower cost or quality that is used to fill a certain television time slot
                         or physical medium """ ;
        skos:inScheme    <https://metadata.amagi.tv/skos/amagi_ebu_AssetTypeCS> ;
        skos:broader    ast_type:_1.1 ;
        skos:changeNote "" ;
        skos:historyNote "2023-08-27" ;
        skos:note "Valid" . 

ast_type:_1.1.15
        rdf:type        ebucore:AssetType ;
        skos:prefLabel  "Wheeler"@en ;
        skos:definition   """These are contents that are designed to be played partially. 
                The content can be scheduled for a shorter duration than content duration. 
                These types of contents are used for filling the last of portion of the island, 
                for which a Filler content matching the duration is not available """ ;
        skos:inScheme    <https://metadata.amagi.tv/skos/amagi_ebu_AssetTypeCS> ;
        skos:broader    ast_type:_1.1 ;
        skos:changeNote "" ;
        skos:historyNote "2023-09-27" ;
        skos:note "Valid" . 

ast_type:_1.1.16
        rdf:type        ebucore:AssetType ;
        skos:prefLabel  "Ident"@en ;
        skos:definition   """An ident (short for identification) refers to a short piece of content that 
                                serves to identify the broadcaster or channel. It often features the channel's 
                                logo, branding elements, and sometimes a jingle or sound that reinforces the brand identity. """ ;
        skos:inScheme    <https://metadata.amagi.tv/skos/amagi_ebu_AssetTypeCS> ;
        skos:broader    ast_type:_1.1 ;
        skos:narrower    ast_type:_1.1.16.1 ;
        skos:changeNote "" ;
        skos:historyNote "2024-11-18" ;
        skos:note "Valid" . 

ast_type:_1.1.16.1
        rdf:type        ebucore:AssetType ;
        skos:prefLabel  "Ident Adjustable"@en ;
        skos:definition   """An ident that can have adjustable duration similiar to a filler or wheeler""" ;
        skos:inScheme    <https://metadata.amagi.tv/skos/amagi_ebu_AssetTypeCS> ;
        skos:broader    ast_type:_1.1.16 ;
        skos:changeNote "" ;
        skos:historyNote "2024-11-18" ;
        skos:note "Valid" . 

ast_type:_1.1.17
        rdf:type        ebucore:AssetType ;
        skos:prefLabel  "Warning"@en ;
        skos:definition   """A warning clip  """ ;
        skos:inScheme    <https://metadata.amagi.tv/skos/amagi_ebu_AssetTypeCS> ;
        skos:broader    ast_type:_1.1 ;
        skos:changeNote "" ;
        skos:historyNote "2024-11-18" ;
        skos:note "Valid" . 

ast_type:_1.2.1
        rdf:type        ebucore:AssetType ;
        skos:prefLabel  "Short Form"@en ;
        skos:definition   "Episode that is less than 10 minutes" ;
        skos:inScheme    <https://metadata.amagi.tv/skos/amagi_ebu_AssetTypeCS> ;
        skos:broader    ast_type:_1.2 ;
        skos:narrower    ast_type:_1.2.1.1 ;
        skos:changeNote "" ;
        skos:historyNote "2023-08-27" ;
        skos:note "Valid" .

ast_type:_1.2.1.1
        rdf:type        ebucore:AssetType ;
        skos:prefLabel  "Shorts Sponsored"@en ;
        skos:definition   "An episodic short form video that is sponsored" ;
        skos:inScheme    <https://metadata.amagi.tv/skos/amagi_ebu_AssetTypeCS> ;
        skos:broader    ast_type:_1.2.1 ;
        skos:changeNote "" ;
        skos:historyNote "2024-11-18" ;
        skos:note "Valid" .

ast_type:_1.2.2
        rdf:type        ebucore:AssetType ;
        skos:prefLabel  "Program"@en ;
        skos:definition   "Episode is a Program" ;
        skos:inScheme    <https://metadata.amagi.tv/skos/amagi_ebu_AssetTypeCS> ;
        skos:broader    ast_type:_1.2 ;
        skos:changeNote "" ;
        skos:historyNote "2023-08-27" ;
        skos:note "Valid" .

ast_type:_2
        rdf:type        ebucore:AssetType ;
        skos:prefLabel  "Audio"@en ;
        skos:definition   "Audio Only Asset Type Top Concept" ;
        skos:inScheme    <https://metadata.amagi.tv/skos/amagi_ebu_AssetTypeCS> ;
        skos:narrower    ast_type:_2.1 ;
        skos:changeNote "" ;
        skos:historyNote "2023-08-27" ;
        skos:note "Valid" . 

ast_type:_2.1
        rdf:type        ebucore:AssetType ;
        skos:prefLabel  "Podcast"@en ;
        skos:definition   "Audio Podacast" ;
        skos:inScheme    <https://metadata.amagi.tv/skos/amagi_ebu_AssetTypeCS> ;
        skos:broader    ast_type:_2 ;
        skos:changeNote "" ;
        skos:historyNote "2023-08-27" ;
        skos:note "Valid" .

ast_type:_3 
        rdf:type        ebucore:AssetType ;
        skos:prefLabel  "Image"@en ;
        skos:definition   "Image Asset Type Top Concept" ;
        skos:inScheme    <https://metadata.amagi.tv/skos/amagi_ebu_AssetTypeCS> ;
        skos:narrower    ast_type:_3.1 ;
        skos:narrower    ast_type:_3.2 ;
        skos:narrower    ast_type:_3.3 ;
        skos:narrower    ast_type:_3.4 ;
        skos:narrower    ast_type:_3.5 ;
        skos:narrower    ast_type:_3.6 ;
        skos:changeNote "" ;
        skos:historyNote "2025-02-19" ;
        skos:note "Valid" . 

ast_type:_3.1
        rdf:type        ebucore:AssetType ;
        skos:prefLabel  "Poster"@en ;
        skos:altLabel  "Banner"@en ;
        skos:definition   "Poster Image" ;
        skos:inScheme    <https://metadata.amagi.tv/skos/amagi_ebu_AssetTypeCS> ;
        skos:broader    ast_type:_3 ;
        skos:narrower    ast_type:_3.1.1 ;
        skos:narrower    ast_type:_3.1.2 ;
        skos:narrower    ast_type:_3.1.3 ;
        skos:narrower    ast_type:_3.1.4 ;
        skos:changeNote "" ;
        skos:historyNote "2023-08-27" ;
        skos:note "Valid" .

ast_type:_3.1.1
        rdf:type        ebucore:AssetType ;
        skos:prefLabel  "PosterTitledLight"@en ;
        skos:definition   "Poster with titled text in light theme" ;
        skos:inScheme    <https://metadata.amagi.tv/skos/amagi_ebu_AssetTypeCS> ;
        skos:broader    ast_type:_3.1 ;
        skos:changeNote "" ;
        skos:historyNote "2024-07-02" ;
        skos:note "Valid" .

ast_type:_3.1.2
        rdf:type        ebucore:AssetType ;
        skos:prefLabel  "PosterTitledDark"@en ;
        skos:definition   "Poster with titled text in dark theme" ;
        skos:inScheme    <https://metadata.amagi.tv/skos/amagi_ebu_AssetTypeCS> ;
        skos:broader    ast_type:_3.1 ;
        skos:changeNote "" ;
        skos:historyNote "2024-07-02" ;
        skos:note "Valid" .

ast_type:_3.1.3
        rdf:type        ebucore:AssetType ;
        skos:prefLabel  "PosterUntitledLight"@en ;
        skos:definition  "Poster without titled text in light theme" ;
        skos:inScheme    <https://metadata.amagi.tv/skos/amagi_ebu_AssetTypeCS> ;
        skos:broader    ast_type:_3.1 ;
        skos:changeNote "" ;
        skos:historyNote "2024-07-02" ;
        skos:note "Valid" .

ast_type:_3.1.4
        rdf:type        ebucore:AssetType ;
        skos:prefLabel  "PosterUntitledDark"@en ;
        skos:definition  "Poster without titled text in dark theme" ;
        skos:inScheme    <https://metadata.amagi.tv/skos/amagi_ebu_AssetTypeCS> ;
        skos:broader    ast_type:_3.1 ;
        skos:changeNote "" ;
        skos:historyNote "2024-07-02" ;
        skos:note "Valid" .

ast_type:_3.2
        rdf:type        ebucore:AssetType ;
        skos:prefLabel  "Logo"@en ;
        skos:definition   "Logo Image" ;
        skos:inScheme    <https://metadata.amagi.tv/skos/amagi_ebu_AssetTypeCS> ;
        skos:broader    ast_type:_3 ;
        skos:changeNote "" ;
        skos:historyNote "2023-08-27" ;
        skos:note "Valid" .

ast_type:_3.3
        rdf:type        ebucore:AssetType ;
        skos:prefLabel  "Thumbnail"@en ;
        skos:definition   "Thumbnail Image" ;
        skos:inScheme    <https://metadata.amagi.tv/skos/amagi_ebu_AssetTypeCS> ;
        skos:broader    ast_type:_3 ;
        skos:narrower    ast_type:_3.3.1 ;
        skos:narrower    ast_type:_3.3.2 ;
        skos:changeNote "" ;
        skos:historyNote "2023-08-27" ;
        skos:note "Valid" .

ast_type:_3.3.1
        rdf:type        ebucore:AssetType ;
        skos:prefLabel  "ThumbnailLight"@en ;
        skos:definition   "Light themed Thumbnail Image" ;
        skos:inScheme    <https://metadata.amagi.tv/skos/amagi_ebu_AssetTypeCS> ;
        skos:broader    ast_type:_3.3 ;
        skos:changeNote "" ;
        skos:historyNote "2023-08-27" ;
        skos:note "Valid" .

ast_type:_3.3.2
        rdf:type        ebucore:AssetType ;
        skos:prefLabel  "ThumbnailDark"@en ;
        skos:definition   "Dark themed Thumbnail Image" ;
        skos:inScheme    <https://metadata.amagi.tv/skos/amagi_ebu_AssetTypeCS> ;
        skos:broader    ast_type:_3.3 ;
        skos:changeNote "" ;
        skos:historyNote "2023-08-27" ;
        skos:note "Valid" .

ast_type:_3.4
        rdf:type        ebucore:AssetType ;
        skos:prefLabel  "Other"@en ;
        skos:definition   "Other Image" ;
        skos:inScheme    <https://metadata.amagi.tv/skos/amagi_ebu_AssetTypeCS> ;
        skos:broader    ast_type:_3 ;
        skos:changeNote "" ;
        skos:historyNote "2023-08-27" ;
        skos:note "Valid" .

ast_type:_3.5
        rdf:type        ebucore:AssetType ;
        skos:prefLabel  "Stillcut"@en ;
        skos:definition   "Stillcut Image" ;
        skos:inScheme    <https://metadata.amagi.tv/skos/amagi_ebu_AssetTypeCS> ;
        skos:broader    ast_type:_3 ;
        skos:narrower    ast_type:_3.5.1 ;
        skos:narrower    ast_type:_3.5.2 ;
        skos:narrower    ast_type:_3.5.3 ;
        skos:narrower    ast_type:_3.5.4 ;
        skos:changeNote "" ;
        skos:historyNote "2025-02-19" ;
        skos:note "Valid" .

ast_type:_3.5.1
        rdf:type        ebucore:AssetType ;
        skos:prefLabel  "StillcutTitledLight"@en ;
        skos:definition   "Stillcut with titled text in light theme" ;
        skos:inScheme    <https://metadata.amagi.tv/skos/amagi_ebu_AssetTypeCS> ;
        skos:broader    ast_type:_3.5 ;
        skos:changeNote "" ;
        skos:historyNote "2025-02-19" ;
        skos:note "Valid" .

ast_type:_3.5.2
        rdf:type        ebucore:AssetType ;
        skos:prefLabel  "StillcutTitledDark"@en ;
        skos:definition   "Stillcut with titled text in dark theme" ;
        skos:inScheme    <https://metadata.amagi.tv/skos/amagi_ebu_AssetTypeCS> ;
        skos:broader    ast_type:_3.5 ;
        skos:changeNote "" ;
        skos:historyNote "2025-02-19" ;
        skos:note "Valid" .

ast_type:_3.5.3
        rdf:type        ebucore:AssetType ;
        skos:prefLabel  "StillcutUntitledLight"@en ;
        skos:definition  "Stillcut without titled text in light theme" ;
        skos:inScheme    <https://metadata.amagi.tv/skos/amagi_ebu_AssetTypeCS> ;
        skos:broader    ast_type:_3.5 ;
        skos:changeNote "" ;
        skos:historyNote "2025-02-19" ;
        skos:note "Valid" .

ast_type:_3.5.4
        rdf:type        ebucore:AssetType ;
        skos:prefLabel  "StillcutUntitledDark"@en ;
        skos:definition  "Stillcut without titled text in dark theme" ;
        skos:inScheme    <https://metadata.amagi.tv/skos/amagi_ebu_AssetTypeCS> ;
        skos:broader    ast_type:_3.5 ;
        skos:changeNote "" ;
        skos:historyNote "2025-02-19" ;
        skos:note "Valid" .

ast_type:_3.6
        rdf:type        ebucore:AssetType ;
        skos:prefLabel  "Landscape"@en ;
        skos:definition   "Landscape Image" ;
        skos:inScheme    <https://metadata.amagi.tv/skos/amagi_ebu_AssetTypeCS> ;
        skos:broader    ast_type:_3 ;
        skos:narrower    ast_type:_3.6.1 ;
        skos:narrower    ast_type:_3.6.2 ;
        skos:narrower    ast_type:_3.6.3 ;
        skos:narrower    ast_type:_3.6.4 ;
        skos:changeNote "" ;
        skos:historyNote "2025-02-19" ;
        skos:note "Valid" .

ast_type:_3.6.1
        rdf:type        ebucore:AssetType ;
        skos:prefLabel  "LandscapeTitledLight"@en ;
        skos:definition   "Landscape with titled text in light theme" ;
        skos:inScheme    <https://metadata.amagi.tv/skos/amagi_ebu_AssetTypeCS> ;
        skos:broader    ast_type:_3.6 ;
        skos:changeNote "" ;
        skos:historyNote "2025-02-19" ;
        skos:note "Valid" .

ast_type:_3.6.2
        rdf:type        ebucore:AssetType ;
        skos:prefLabel  "LandscapeTitledDark"@en ;
        skos:definition   "Landscape with titled text in dark theme" ;
        skos:inScheme    <https://metadata.amagi.tv/skos/amagi_ebu_AssetTypeCS> ;
        skos:broader    ast_type:_3.6 ;
        skos:changeNote "" ;
        skos:historyNote "2025-02-19" ;
        skos:note "Valid" .

ast_type:_3.6.3
        rdf:type        ebucore:AssetType ;
        skos:prefLabel  "LandscapeUntitledLight"@en ;
        skos:definition  "Landscape without titled text in light theme" ;
        skos:inScheme    <https://metadata.amagi.tv/skos/amagi_ebu_AssetTypeCS> ;
        skos:broader    ast_type:_3.6 ;
        skos:changeNote "" ;
        skos:historyNote "2025-02-19" ;
        skos:note "Valid" .

ast_type:_3.6.4
        rdf:type        ebucore:AssetType ;
        skos:prefLabel  "LandscapeUntitledDark"@en ;
        skos:definition  "Landscape without titled text in dark theme" ;
        skos:inScheme    <https://metadata.amagi.tv/skos/amagi_ebu_AssetTypeCS> ;
        skos:broader    ast_type:_3.6 ;
        skos:changeNote "" ;
        skos:historyNote "2025-02-19" ;
        skos:note "Valid" .


ast_type:_4 
        rdf:type        ebucore:AssetType ;
        skos:prefLabel  "Graphic"@en ;
        skos:definition   "Graphic Asset Type Top Concept" ;
        skos:inScheme    <https://metadata.amagi.tv/skos/amagi_ebu_AssetTypeCS> ;
        skos:narrower    ast_type:_4.1 ;
        skos:narrower    ast_type:_4.2 ;
        skos:narrower    ast_type:_4.3 ;
        skos:narrower    ast_type:_4.4 ;
        skos:narrower    ast_type:_4.5 ;
        skos:narrower    ast_type:_4.6 ;
        skos:changeNote "" ;
        skos:historyNote "2023-10-16" ;
        skos:note "Valid" . 


ast_type:_4.1
        rdf:type        ebucore:AssetType ;
        skos:prefLabel  "Logo"@en ;
        skos:altLabel   "Bug"@en ;
        skos:definition   "A small graphic or logo placed in a corner of the screen, often used for branding" ;
        skos:inScheme    <https://metadata.amagi.tv/skos/amagi_ebu_AssetTypeCS> ;
        skos:broader    ast_type:_4 ;
        skos:changeNote "" ;
        skos:historyNote "2024-07-12" ;
        skos:note "Valid" .

ast_type:_4.2
        rdf:type        ebucore:AssetType ;
        skos:prefLabel  "AstonBand"@en ;
        skos:altLabel   "LowerThird"@en ;
        skos:definition   "Text or graphics displayed in the lower third of the screen, usually containing information such as names, titles, ads, or other contextual data" ;
        skos:inScheme    <https://metadata.amagi.tv/skos/amagi_ebu_AssetTypeCS> ;
        skos:broader    ast_type:_4 ;
        skos:changeNote "" ;
        skos:historyNote "2024-07-12" ;
        skos:note "Valid" .

ast_type:_4.3
        rdf:type        ebucore:AssetType ;
        skos:prefLabel  "L-Band"@en ;
        skos:definition   "L band ads are graphic overlays that appear in an L-shape on the screen, often during sports events or news broadcasts. These ads provide information without taking up the entire screen, allowing viewers to continue watching the main content." ;
        skos:inScheme    <https://metadata.amagi.tv/skos/amagi_ebu_AssetTypeCS> ;
        skos:broader    ast_type:_4 ;
        skos:changeNote "" ;
        skos:historyNote "2024-07-12" ;
        skos:note "Valid" .

ast_type:_4.4
        rdf:type        ebucore:AssetType ;
        skos:prefLabel  "FullScreenGraphic"@en ;
        skos:definition   "Graphics that take up the entire screen, used for things like title cards, charts, maps, or detailed information." ;
        skos:inScheme    <https://metadata.amagi.tv/skos/amagi_ebu_AssetTypeCS> ;
        skos:broader    ast_type:_4 ;
        skos:changeNote "" ;
        skos:historyNote "2024-07-12" ;
        skos:note "Valid" .

ast_type:_4.5
        rdf:type        ebucore:AssetType ;
        skos:prefLabel  "Ticker"@en ;
        skos:definition   "A scrolling line of text, typically at the bottom of the screen, used for continuous updates like news headlines, sports scores, or stock prices." ;
        skos:inScheme    <https://metadata.amagi.tv/skos/amagi_ebu_AssetTypeCS> ;
        skos:broader    ast_type:_4 ;
        skos:changeNote "" ;
        skos:historyNote "2024-07-12" ;
        skos:note "Valid" .

ast_type:_4.6
        rdf:type        ebucore:AssetType ;
        skos:prefLabel  "NowNextLater"@en ;
        skos:definition   "A side band or boottom overlay that shows the current program, the next program, and the program after that." ;
        skos:inScheme    <https://metadata.amagi.tv/skos/amagi_ebu_AssetTypeCS> ;
        skos:broader    ast_type:_4 ;
        skos:changeNote "" ;
        skos:historyNote "2024-07-12" ;
        skos:note "Valid" .
