@prefix rdf: <http://www.w3.org/1999/02/22-rdf-syntax-ns#> .
@prefix ebucore: <http://www.ebu.ch/metadata/ontologies/ebucore/ebucore#> .
@prefix skos: <http://www.w3.org/2004/02/skos/core#> .
@prefix owl: <http://www.w3.org/2002/07/owl#> .
@prefix dc: <http://purl.org/dc/elements/1.1/> .
@prefix dct: <http://purl.org/dc/terms/> .
@prefix rdfs: <http://www.w3.org/2000/01/rdf-schema#> .
@prefix part_type: <https://metadata.amagi.tv/skos/amagi_ebu_PartTypeCS#> .

<https://metadata.amagi.tv/skos/amagi_ebu_PartTypeCS.rdf>
        rdf:type         owl:Ontology ;
        dct:title        "EBU Based SKOS Classification Scheme for Part Types"@en ;
        dct:contributor  "Amagi metadata community" ;
        dct:description  "An RDF vocabulary defining the type of media resource fragment/part. E.g color-bars, content, start-credits etc"@en ;
        dct:creator      "Shashidhar, Amagi, shashidhar@amagi.com" ;
        dct:publisher    "EBU" ;
        dct:rights       "http://creativecommons.org/licenses/by-nc-sa/3.0/" .

<https://metadata.amagi.tv/skos/amagi_ebu_PartTypeCS>
        rdf:type            skos:ConceptScheme ;
        rdfs:label          "EBU SKOS Classification Scheme for Part Type"@en ;
        rdfs:isDefinedBy    <https://metadata.amagi.tv/skos/amagi_ebu_PartTypeCS> ;
        skos:hasTopConcept  part_type:_1 ;
        skos:hasTopConcept  part_type:_2 ;
        skos:hasTopConcept  part_type:_3 ;
        skos:hasTopConcept  part_type:_4 ;
        skos:hasTopConcept  part_type:_5 ;
        skos:hasTopConcept  part_type:_6 ;
        skos:hasTopConcept  part_type:_7 .

part_type:_1
        rdf:type        ebucore:Part_Type ;
        skos:prefLabel  "content"@en ;
        skos:definition   "Part type corresponding to program content in a media resource"@en ;
        skos:inScheme    <https://metadata.amagi.tv/skos/amagi_ebu_PartTypeCS> ;
        skos:changeNote "" ;
        skos:historyNote "2024-05-01" ;
        skos:note "Valid" . 

part_type:_2
        rdf:type        ebucore:Part_Type ;
        skos:prefLabel  "black"@en ;
        skos:definition   "Part type corresponding to black video that typically marks the scene boundaries"@en ;
        skos:inScheme    <https://metadata.amagi.tv/skos/amagi_ebu_PartTypeCS> ;
        skos:changeNote "" ;
        skos:historyNote "2024-05-01" ;
        skos:note "Valid" .

part_type:_3
        rdf:type        ebucore:Part_Type ;
        skos:prefLabel  "slate"@en ;
        skos:definition   "Part type corresponding to a title card listing important metadata of a television program, included before the first frame of the program"@en ;
        skos:inScheme    <https://metadata.amagi.tv/skos/amagi_ebu_PartTypeCS> ;
        skos:changeNote "" ;
        skos:historyNote "2024-05-01" ;
        skos:note "Valid" . 

part_type:_4
        rdf:type        ebucore:Part_Type ;
        skos:prefLabel  "credits"@en ;
        skos:definition   "Part type where list of cast and crew for the asset are listed"@en ;
        skos:inScheme    <https://metadata.amagi.tv/skos/amagi_ebu_PartTypeCS> ;
        skos:narrower    part_type:_4.1 ;
        skos:narrower    part_type:_4.2 ;
        skos:changeNote "" ;
        skos:historyNote "2024-05-01" ;
        skos:note "Valid" . 

part_type:_4.1
        rdf:type        ebucore:Part_Type ;
        skos:prefLabel  "opening-credits"@en ;
        skos:definition   "Part type that appears in the beginning, where list of cast and crew for the asset are listed"@en ;
        skos:inScheme    <https://metadata.amagi.tv/skos/amagi_ebu_PartTypeCS> ;
        skos:broader     part_type:_4 ;
        skos:changeNote "" ;
        skos:historyNote "2024-05-01" ;
        skos:note "Valid" . 

part_type:_4.2
        rdf:type        ebucore:Part_Type ;
        skos:prefLabel  "end-credits"@en ;
        skos:altLabel    "closing-credits"@en ;
        skos:definition   "Part type that appears at the end, where list of cast and crew for the asset are listed"@en ;
        skos:inScheme    <https://metadata.amagi.tv/skos/amagi_ebu_PartTypeCS> ;
        skos:broader     part_type:_4 ;
        skos:changeNote "" ;
        skos:historyNote "2024-05-01" ;
        skos:note "Valid" .

part_type:5
        rdf:type        ebucore:Part_Type ;
        skos:prefLabel  "color-bars"@en ;
        skos:definition   "Part type corresponding to color bars that are used to calibrate the video signal"@en ;
        skos:inScheme    <https://metadata.amagi.tv/skos/amagi_ebu_PartTypeCS> ;
        skos:changeNote "" ;
        skos:historyNote "2024-05-01" ;
        skos:note "Valid" .

part_type:6
        rdf:type        ebucore:Part_Type ;
        skos:prefLabel  "intro"@en ;
        skos:definition  "Part type corresponding to the introduction of a media resource"@en ;
        skos:inScheme    <https://metadata.amagi.tv/skos/amagi_ebu_PartTypeCS> ;
        skos:changeNote "" ;
        skos:historyNote "2024-05-01" ;
        skos:note "Valid" .

part_type:7
        rdf:type        ebucore:Part_Type ;
        skos:prefLabel  "recap"@en ;
        skos:definition  "Part type corresponding to a recap of the previous episode of a television program"@en ;
        skos:inScheme    <https://metadata.amagi.tv/skos/amagi_ebu_PartTypeCS> ;
        skos:changeNote "" ;
        skos:historyNote "2024-05-01" ;
        skos:note "Valid" .
