<rdf:RDF
    xmlns:dct="http://purl.org/dc/terms/"
    xmlns:rdf="http://www.w3.org/1999/02/22-rdf-syntax-ns#"
    xmlns:dc="http://purl.org/dc/elements/1.1/"
    xmlns:ebucore="http://www.ebu.ch/metadata/ontologies/ebucore/ebucore#"
    xmlns:owl="http://www.w3.org/2002/07/owl#"
    xmlns:skos="http://www.w3.org/2004/02/skos/core#"
    xmlns:rdfs="http://www.w3.org/2000/01/rdf-schema#" > 
  <rdf:Description rdf:about="https://metadata.amagi.tv/skos/amagi_ebu_IdentifierTypeCS#_tmsid">
    <skos:prefLabel xml:lang="en">TMSID</skos:prefLabel>
    <skos:note>Valid</skos:note>
    <skos:inScheme rdf:resource="https://metadata.amagi.tv/skos/amagi_ebu_IdentifierTypeCS"/>
    <skos:historyNote>2022-11-29</skos:historyNote>
    <skos:example>MV003331980000</skos:example>
    <skos:definition xml:lang="en">Gracenote TMSID. Check https://en.wikipedia.org/wiki/TMS_(entertainment_data) and https://www.gracenote.com/gracenote-id/</skos:definition>
    <skos:changeNote>First version</skos:changeNote>
    <rdf:type rdf:resource="http://www.ebu.ch/metadata/ontologies/ebucore/ebucore#IdentifierType"/>
  </rdf:Description>
  <rdf:Description rdf:about="https://metadata.amagi.tv/skos/amagi_ebu_IdentifierTypeCS">
    <rdfs:label xml:lang="en">EBU SKOS Classification Scheme for media IdentifierType</rdfs:label>
    <rdfs:isDefinedBy rdf:resource="https://metadata.amagi.tv/skos/amagi_ebu_IdentifierTypeCS"/>
    <rdf:type rdf:resource="http://www.w3.org/2004/02/skos/core#ConceptScheme"/>
  </rdf:Description>
  <rdf:Description rdf:about="https://metadata.amagi.tv/skos/amagi_ebu_IdentifierTypeCS#_amgastid">
    <skos:prefLabel xml:lang="en">AMAGI-ASSETID</skos:prefLabel>
    <skos:note>Valid</skos:note>
    <skos:inScheme rdf:resource="https://metadata.amagi.tv/skos/amagi_ebu_IdentifierTypeCS"/>
    <skos:historyNote>2023-11-03</skos:historyNote>
    <skos:example></skos:example>
    <skos:definition xml:lang="en">unique identifier for asset ingested using amagi</skos:definition>
    <skos:changeNote>First version</skos:changeNote>
    <rdf:type rdf:resource="http://www.ebu.ch/metadata/ontologies/ebucore/ebucore#IdentifierType"/>
  </rdf:Description>
  <rdf:Description rdf:about="https://metadata.amagi.tv/skos/amagi_ebu_IdentifierTypeCS#_wikidata">
    <skos:prefLabel xml:lang="en">WIKI</skos:prefLabel>
    <skos:note>Valid</skos:note>
    <skos:inScheme rdf:resource="https://metadata.amagi.tv/skos/amagi_ebu_IdentifierTypeCS"/>
    <skos:historyNote>2023-10-25</skos:historyNote>
    <skos:example></skos:example>
    <skos:definition xml:lang="en">Wikidata identifier. Check https://www.wikidata.org/</skos:definition>
    <skos:changeNote>First version</skos:changeNote>
    <rdf:type rdf:resource="http://www.ebu.ch/metadata/ontologies/ebucore/ebucore#IdentifierType"/>
  </rdf:Description>
  <rdf:Description rdf:about="https://metadata.amagi.tv/skos/amagi_ebu_IdentifierTypeCS#_gracenote">
    <skos:prefLabel xml:lang="en">gracenote</skos:prefLabel>
    <skos:note>Valid</skos:note>
    <skos:inScheme rdf:resource="https://metadata.amagi.tv/skos/amagi_ebu_IdentifierTypeCS"/>
    <skos:historyNote>2023-11-10</skos:historyNote>
    <skos:example>MV003331980000</skos:example>
    <skos:definition xml:lang="en">Gracenote TMSID. Check https://en.wikipedia.org/wiki/TMS_(entertainment_data) and https://www.gracenote.com/gracenote-id</skos:definition>
    <skos:changeNote>First version</skos:changeNote>
    <rdf:type rdf:resource="http://www.ebu.ch/metadata/ontologies/ebucore/ebucore#IdentifierType"/>
  </rdf:Description>
  <rdf:Description rdf:about="https://metadata.amagi.tv/skos/amagi_ebu_IdentifierTypeCS#_tastemade">
    <skos:prefLabel xml:lang="en">tastemade</skos:prefLabel>
    <skos:note>Valid</skos:note>
    <skos:inScheme rdf:resource="https://metadata.amagi.tv/skos/amagi_ebu_IdentifierTypeCS"/>
    <skos:historyNote>2023-11-10</skos:historyNote>
    <skos:example>37190</skos:example>
    <skos:definition xml:lang="en">external id provided from tastemade</skos:definition>
    <skos:changeNote>First version</skos:changeNote>
    <rdf:type rdf:resource="http://www.ebu.ch/metadata/ontologies/ebucore/ebucore#IdentifierType"/>
  </rdf:Description>
  <rdf:Description rdf:about="https://metadata.amagi.tv/skos/amagi_ebu_IdentifierTypeCS#_iab30">
    <skos:prefLabel xml:lang="en">IAB-3.0</skos:prefLabel>
    <skos:note>Valid</skos:note>
    <skos:inScheme rdf:resource="https://metadata.amagi.tv/skos/amagi_ebu_IdentifierTypeCS"/>
    <skos:historyNote>2023-11-10</skos:historyNote>
    <skos:example></skos:example>
    <skos:definition xml:lang="en">iab 3.0 content taxonomy. Check https://github.com/InteractiveAdvertisingBureau/Taxonomies/blob/main/Content%20Taxonomies/Content%20Taxonomy%203.0.tsv</skos:definition>
    <skos:changeNote>First version</skos:changeNote>
    <rdf:type rdf:resource="http://www.ebu.ch/metadata/ontologies/ebucore/ebucore#IdentifierType"/>
  </rdf:Description>
  <rdf:Description rdf:about="https://metadata.amagi.tv/skos/amagi_ebu_IdentifierTypeCS#_eidr">
    <skos:prefLabel xml:lang="en">EIDR</skos:prefLabel>
    <skos:note>Valid</skos:note>
    <skos:inScheme rdf:resource="https://metadata.amagi.tv/skos/amagi_ebu_IdentifierTypeCS"/>
    <skos:historyNote>2022-11-29</skos:historyNote>
    <skos:example></skos:example>
    <skos:definition xml:lang="en">The universal media identifier. Check https://www.eidr.org/</skos:definition>
    <skos:changeNote>First version</skos:changeNote>
    <rdf:type rdf:resource="http://www.ebu.ch/metadata/ontologies/ebucore/ebucore#IdentifierType"/>
  </rdf:Description>
  <rdf:Description rdf:about="https://metadata.amagi.tv/skos/amagi_ebu_IdentifierTypeCS#_iptcmediatopic">
    <skos:prefLabel xml:lang="en">IPTC-MEDIATOPIC</skos:prefLabel>
    <skos:note>Valid</skos:note>
    <skos:inScheme rdf:resource="https://metadata.amagi.tv/skos/amagi_ebu_IdentifierTypeCS"/>
    <skos:historyNote>2023-11-03</skos:historyNote>
    <skos:example></skos:example>
    <skos:definition xml:lang="en">iptc mediatopic identifier. Check http://cv.iptc.org/newscodes/mediatopic/</skos:definition>
    <skos:changeNote>First version</skos:changeNote>
    <rdf:type rdf:resource="http://www.ebu.ch/metadata/ontologies/ebucore/ebucore#IdentifierType"/>
  </rdf:Description>
  <rdf:Description rdf:about="https://metadata.amagi.tv/skos/amagi_ebu_IdentifierTypeCS#_amagi">
    <skos:prefLabel xml:lang="en">Amagi</skos:prefLabel>
    <skos:note>Valid</skos:note>
    <skos:inScheme rdf:resource="https://metadata.amagi.tv/skos/amagi_ebu_IdentifierTypeCS"/>
    <skos:historyNote>2023-11-10</skos:historyNote>
    <skos:example>ACm1io6d5z76aehcyESGbki</skos:example>
    <skos:definition xml:lang="en">external id provided by amagi</skos:definition>
    <skos:changeNote>First version</skos:changeNote>
    <rdf:type rdf:resource="http://www.ebu.ch/metadata/ontologies/ebucore/ebucore#IdentifierType"/>
  </rdf:Description>
  <rdf:Description rdf:about="https://metadata.amagi.tv/skos/amagi_ebu_IdentifierTypeCS#_provider_guid">
    <skos:prefLabel xml:lang="en">provider_guid</skos:prefLabel>
    <skos:note>Valid</skos:note>
    <skos:inScheme rdf:resource="https://metadata.amagi.tv/skos/amagi_ebu_IdentifierTypeCS"/>
    <skos:historyNote>2023-11-10</skos:historyNote>
    <skos:example>tmk-video-2779f930951347e0ad939b05f43a8ff8</skos:example>
    <skos:definition xml:lang="en">Unique id from the provider</skos:definition>
    <skos:changeNote>First version</skos:changeNote>
    <rdf:type rdf:resource="http://www.ebu.ch/metadata/ontologies/ebucore/ebucore#IdentifierType"/>
  </rdf:Description>
  <rdf:Description rdf:about="https://metadata.amagi.tv/skos/amagi_ebu_IdentifierTypeCS#_aichatctxid">
    <skos:prefLabel xml:lang="en">ai_chat_context_id</skos:prefLabel>
    <skos:note>Valid</skos:note>
    <skos:inScheme rdf:resource="https://metadata.amagi.tv/skos/amagi_ebu_IdentifierTypeCS"/>
    <skos:historyNote>2025-03-25</skos:historyNote>
    <skos:example>39ij490jk</skos:example>
    <skos:definition xml:lang="en">Chat-ID provided in response of AI metadata generation. This chat-id will be used in the UI to call chat interaction to fine tune the response</skos:definition>
    <skos:changeNote>First version</skos:changeNote>
    <rdf:type rdf:resource="http://www.ebu.ch/metadata/ontologies/ebucore/ebucore#IdentifierType"/>
  </rdf:Description>
  <rdf:Description rdf:about="https://metadata.amagi.tv/skos/amagi_ebu_IdentifierTypeCS#_imdb">
    <skos:prefLabel xml:lang="en">IMDB</skos:prefLabel>
    <skos:note>Valid</skos:note>
    <skos:inScheme rdf:resource="https://metadata.amagi.tv/skos/amagi_ebu_IdentifierTypeCS"/>
    <skos:historyNote>2022-11-29</skos:historyNote>
    <skos:example></skos:example>
    <skos:definition xml:lang="en">IMDB identifier. Check https://www.imdb.org/</skos:definition>
    <skos:changeNote>First version</skos:changeNote>
    <rdf:type rdf:resource="http://www.ebu.ch/metadata/ontologies/ebucore/ebucore#IdentifierType"/>
  </rdf:Description>
  <rdf:Description rdf:about="https://metadata.amagi.tv/skos/amagi_ebu_IdentifierTypeCS#_cpaltid">
    <skos:prefLabel xml:lang="en">ALTERNATE-ID</skos:prefLabel>
    <skos:note>Valid</skos:note>
    <skos:inScheme rdf:resource="https://metadata.amagi.tv/skos/amagi_ebu_IdentifierTypeCS"/>
    <skos:historyNote>2024-10-25</skos:historyNote>
    <skos:example>S0_A0_123</skos:example>
    <skos:definition xml:lang="en">Content partner alternate identifier. 
        Can be used to allow the content partner who is the amagi 
        account holder ingesting the assets to store an additional identifier. 
        This e.g. can be used to store additional identifiers for collections.</skos:definition>
    <skos:changeNote>First version</skos:changeNote>
    <rdf:type rdf:resource="http://www.ebu.ch/metadata/ontologies/ebucore/ebucore#IdentifierType"/>
  </rdf:Description>
</rdf:RDF>
