@prefix rdf: <http://www.w3.org/1999/02/22-rdf-syntax-ns#> .
@prefix ebucore: <http://www.ebu.ch/metadata/ontologies/ebucore/ebucore#> .
@prefix skos: <http://www.w3.org/2004/02/skos/core#> .
@prefix owl: <http://www.w3.org/2002/07/owl#> .
@prefix dc: <http://purl.org/dc/elements/1.1/> .
@prefix dct: <http://purl.org/dc/terms/> .
@prefix rdfs: <http://www.w3.org/2000/01/rdf-schema#> .
@prefix parentalguidance: <http://www.ebu.ch/metadata/ontologies/skos/ebu_ParentalGuidanceCodeCS#> .

<http://www.ebu.ch/metadata/ontologies/skos/ebu_ParentalGuidanceCodeCS.rdf>
        rdf:type         owl:Ontology ;
        dct:title        "EBU SKOS Classification Scheme for Parental Guidance"@en ;
        dct:contributor  "EBU metadata community experts" ;
        dct:description  "An RDF vocabulary defining television, radio and associated\n         pafental guidance codes"@en ;
        dct:creator      "Jean-Pierre Evain, EBU, metadata@ebu.ch" ;
        dct:publisher    "EBU" ;
        dct:rights       "http://creativecommons.org/licenses/by-nc-sa/3.0/" .

<http://www.ebu.ch/metadata/ontologies/skos/ebu_ParentalGuidanceCodeCS>
        rdf:type            skos:ConceptScheme ;
        rdfs:label          "EBU SKOS Classification Scheme for Parental Guidance"@en ;
        rdfs:isDefinedBy    <http://www.ebu.ch/metadata/ontologies/skos/ebu_ParentalGuidanceCodeCS> ;
        skos:hasTopConcept  parentalguidance:_1 ;
        skos:hasTopConcept  parentalguidance:_2 ;
        skos:hasTopConcept  parentalguidance:_3 ;
        skos:hasTopConcept  parentalguidance:_4 ;
        skos:hasTopConcept  parentalguidance:_5 ;
        skos:hasTopConcept  parentalguidance:_6 ;
        skos:hasTopConcept  parentalguidance:_7 ;
        skos:hasTopConcept  parentalguidance:_8 ;
        skos:hasTopConcept  parentalguidance:_9 ;
        skos:hasTopConcept  parentalguidance:_10 ;
        skos:hasTopConcept  parentalguidance:_11 ;
        skos:hasTopConcept  parentalguidance:_12 ;
        skos:hasTopConcept  parentalguidance:_13 ;
        skos:hasTopConcept  parentalguidance:_14 ;
        skos:hasTopConcept  parentalguidance:_15 ;
        skos:hasTopConcept  parentalguidance:_16 ;
        skos:hasTopConcept  parentalguidance:_17 ;
        skos:hasTopConcept  parentalguidance:_18 ;
        skos:hasTopConcept  parentalguidance:_19 ;
        skos:hasTopConcept  parentalguidance:_20 ;
        skos:hasTopConcept  parentalguidance:_21 ;
        skos:hasTopConcept  parentalguidance:_22 ;
        skos:hasTopConcept  parentalguidance:_23 ;
        skos:hasTopConcept  parentalguidance:_24 ;
        skos:hasTopConcept  parentalguidance:_25 ;
        skos:hasTopConcept  parentalguidance:_26 ;
        skos:hasTopConcept  parentalguidance:_27 ;
        skos:hasTopConcept  parentalguidance:_28 ;
        skos:hasTopConcept  parentalguidance:_29 ;
        skos:hasTopConcept  parentalguidance:_30 ;
        skos:hasTopConcept  parentalguidance:_31 ;
        skos:hasTopConcept  parentalguidance:_32 ;
        skos:hasTopConcept  parentalguidance:_33 ;
        skos:hasTopConcept  parentalguidance:_34 ;
        skos:hasTopConcept  parentalguidance:_35 ;
        skos:hasTopConcept  parentalguidance:_36 ;
        skos:hasTopConcept  parentalguidance:_37 ;
        skos:hasTopConcept  parentalguidance:_38 ;
        skos:hasTopConcept  parentalguidance:_39 ;
        skos:hasTopConcept  parentalguidance:_40 ;
        skos:hasTopConcept  parentalguidance:_41 ;
        skos:hasTopConcept  parentalguidance:_42 ;
        skos:hasTopConcept  parentalguidance:_43 ;
        skos:hasTopConcept  parentalguidance:_44 ;
        skos:hasTopConcept  parentalguidance:_45 ;
        skos:hasTopConcept  parentalguidance:_46 ;
        skos:hasTopConcept  parentalguidance:_47 ;
        skos:hasTopConcept  parentalguidance:_48 ;
        skos:hasTopConcept  parentalguidance:_49 ;
        skos:hasTopConcept  parentalguidance:_50 ;
        skos:hasTopConcept  parentalguidance:_51 ;
        skos:hasTopConcept  parentalguidance:_52 ;
        skos:hasTopConcept  parentalguidance:_53 ;
        skos:hasTopConcept  parentalguidance:_54 ;
        skos:hasTopConcept  parentalguidance:_55 ;
        skos:hasTopConcept  parentalguidance:_56 ;
        skos:hasTopConcept  parentalguidance:_57 ;
        skos:hasTopConcept  parentalguidance:_58 ;
        skos:hasTopConcept  parentalguidance:_59 ;
        skos:hasTopConcept  parentalguidance:_60 ;
        skos:hasTopConcept  parentalguidance:_61 ;
        skos:hasTopConcept  parentalguidance:_62 ;
        skos:hasTopConcept  parentalguidance:_63 ;
        skos:hasTopConcept  parentalguidance:_64 ;
        skos:hasTopConcept  parentalguidance:_65 ;
        skos:hasTopConcept  parentalguidance:_66 ;
        skos:hasTopConcept  parentalguidance:_67 ;
        skos:hasTopConcept  parentalguidance:_68 ; # Italy MBACT
        skos:hasTopConcept  parentalguidance:_69 ; # Italy AGCOM
        skos:hasTopConcept  parentalguidance:_70 ; # Japan EIRIN
        skos:hasTopConcept  parentalguidance:_71 ; # Russia MKRF
        skos:hasTopConcept  parentalguidance:_72 .

parentalguidance:_1  rdf:type  ebucore:TargetAudience ;
        skos:prefLabel    "AR-INCAA"@en ;
        skos:altLabel     "Instituto Nacional de Cine y Artes Audiovisuales"@es ;
        skos:scopeNote    "Region:Argentina"@en ;
        skos:definition   "Instituto Nacional de Cine y Artes Audiovisuales"@es ;
        skos:definition   "National Institute of Cinema and Audiovisual Arts"@en ;
        skos:inScheme     <http://www.ebu.ch/metadata/ontologies/skos/ebu_ParentalGuidanceCodeCS> ;
        skos:narrower     parentalguidance:_1.1 ;
        skos:narrower     parentalguidance:_1.2 ;
        skos:narrower     parentalguidance:_1.3 ;
        skos:narrower     parentalguidance:_1.4 ;
        skos:narrower     parentalguidance:_1.5 ;
        skos:narrower     parentalguidance:_1.6 ;
        skos:changeNote   "Update" ;
        skos:historyNote  "2009-07-27" ;
        skos:example      "" ;
        skos:note         "Valid" .

parentalguidance:_1.1
        rdf:type          ebucore:TargetAudience ;
        skos:prefLabel    "ATP"@en ;
        skos:prefLabel    "ATP"@es ;
        skos:definition   "Apta (para) Todo Público"@es ;
        skos:definition   "For all ages"@en ;
        skos:broader      parentalguidance:_1 ;
        skos:inScheme     <http://www.ebu.ch/metadata/ontologies/skos/ebu_ParentalGuidanceCodeCS> ;
        skos:changeNote   "" ;
        skos:historyNote  "" ;
        skos:example      "" .

parentalguidance:_1.2
        rdf:type          ebucore:TargetAudience ;
        skos:prefLabel    "13"@en ;
        skos:prefLabel    "13"@es ;
        skos:definition   "Not under 13"@en ;
        skos:definition   "Apto para mayores de 13 años"@es ;
        skos:broader      parentalguidance:_1 ;
        skos:inScheme     <http://www.ebu.ch/metadata/ontologies/skos/ebu_ParentalGuidanceCodeCS> ;
        skos:changeNote   "" ;
        skos:historyNote  "" ;
        skos:example      "" .

parentalguidance:_1.3
        rdf:type          ebucore:TargetAudience ;
        skos:prefLabel    "16"@en ;
        skos:prefLabel    "16"@es ;
        skos:definition   "Not under 16"@en ;
        skos:definition   "Apto para mayores de 16 años"@es ;
        skos:broader      parentalguidance:_1 ;
        skos:inScheme     <http://www.ebu.ch/metadata/ontologies/skos/ebu_ParentalGuidanceCodeCS> ;
        skos:changeNote   "" ;
        skos:historyNote  "" ;
        skos:example      "" .

parentalguidance:_1.4
        rdf:type          ebucore:TargetAudience ;
        skos:prefLabel    "18"@en ;
        skos:prefLabel    "18"@es ;
        skos:definition   "Not under 18"@en ;
        skos:definition   "Apto para mayores de 18 años"@es ;
        skos:broader      parentalguidance:_1 ;
        skos:inScheme     <http://www.ebu.ch/metadata/ontologies/skos/ebu_ParentalGuidanceCodeCS> ;
        skos:changeNote   "" ;
        skos:historyNote  "" ;
        skos:example      "" .

parentalguidance:_1.5
        rdf:type          ebucore:TargetAudience ;
        skos:prefLabel    "X"@en ;
        skos:definition   "Explicit"@en ;
        skos:broader      parentalguidance:_1 ;
        skos:inScheme     <http://www.ebu.ch/metadata/ontologies/skos/ebu_ParentalGuidanceCodeCS> ;
        skos:changeNote   "" ;
        skos:historyNote  "" ;
        skos:example      "" .

parentalguidance:_1.6
        rdf:type          ebucore:TargetAudience ;
        skos:prefLabel    "E"@en ;
        skos:definition   "Exempt: sports, music, etc."@en ;
        skos:broader      parentalguidance:_1 ;
        skos:inScheme     <http://www.ebu.ch/metadata/ontologies/skos/ebu_ParentalGuidanceCodeCS> ;
        skos:changeNote   "" ;
        skos:historyNote  "" ;
        skos:example      "" .

parentalguidance:_2  rdf:type  ebucore:TargetAudience ;
        skos:prefLabel    "AT-BMUKK"@en ;
        skos:scopeNote    "Region:Austria"@en ;
        skos:definition   "Federal Ministry for Education, the Arts and\n         Culture"@en ;
        skos:definition   "Bundesministerium für Unterricht, Kunst und\n         Kultur"@de ;
        skos:inScheme     <http://www.ebu.ch/metadata/ontologies/skos/ebu_ParentalGuidanceCodeCS> ;
        skos:narrower     parentalguidance:_2.1 ;
        skos:narrower     parentalguidance:_2.2 ;
        skos:narrower     parentalguidance:_2.3 ;
        skos:narrower     parentalguidance:_2.4 ;
        skos:narrower     parentalguidance:_2.5 ;
        skos:narrower     parentalguidance:_2.6 ;
        skos:changeNote   "Update" ;
        skos:historyNote  "2009-07-27" ;
        skos:example      "" ;
        skos:note         "Valid" .

parentalguidance:_2.1
        rdf:type          ebucore:TargetAudience ;
        skos:prefLabel    "None"@en ;
        skos:prefLabel    "Ohne"@de ;
        skos:definition   "For all ages"@en ;
        skos:definition   "Freigegeben fur alle Altersstufen"@de ;
        skos:broader      parentalguidance:_2 ;
        skos:inScheme     <http://www.ebu.ch/metadata/ontologies/skos/ebu_ParentalGuidanceCodeCS> ;
        skos:changeNote   "" ;
        skos:historyNote  "" ;
        skos:example      "" .

parentalguidance:_2.2
        rdf:type          ebucore:TargetAudience ;
        skos:prefLabel    "6"@en ;
        skos:definition   "6 years and above"@en ;
        skos:broader      parentalguidance:_2 ;
        skos:inScheme     <http://www.ebu.ch/metadata/ontologies/skos/ebu_ParentalGuidanceCodeCS> ;
        skos:changeNote   "" ;
        skos:historyNote  "" ;
        skos:example      "" .

parentalguidance:_2.3
        rdf:type          ebucore:TargetAudience ;
        skos:prefLabel    "10"@en ;
        skos:definition   "10 years and above"@en ;
        skos:broader      parentalguidance:_2 ;
        skos:inScheme     <http://www.ebu.ch/metadata/ontologies/skos/ebu_ParentalGuidanceCodeCS> ;
        skos:changeNote   "" ;
        skos:historyNote  "" ;
        skos:example      "" .

parentalguidance:_2.4
        rdf:type          ebucore:TargetAudience ;
        skos:prefLabel    "12"@en ;
        skos:definition   "12 years and above"@en ;
        skos:broader      parentalguidance:_2 ;
        skos:inScheme     <http://www.ebu.ch/metadata/ontologies/skos/ebu_ParentalGuidanceCodeCS> ;
        skos:changeNote   "" ;
        skos:historyNote  "" ;
        skos:example      "" .

parentalguidance:_2.5
        rdf:type          ebucore:TargetAudience ;
        skos:prefLabel    "14"@en ;
        skos:definition   "14 years and above"@en ;
        skos:broader      parentalguidance:_2 ;
        skos:inScheme     <http://www.ebu.ch/metadata/ontologies/skos/ebu_ParentalGuidanceCodeCS> ;
        skos:changeNote   "" ;
        skos:historyNote  "" ;
        skos:example      "" .

parentalguidance:_2.6
        rdf:type          ebucore:TargetAudience ;
        skos:prefLabel    "16"@en ;
        skos:definition   "16 years and above"@en ;
        skos:broader      parentalguidance:_2 ;
        skos:inScheme     <http://www.ebu.ch/metadata/ontologies/skos/ebu_ParentalGuidanceCodeCS> ;
        skos:changeNote   "" ;
        skos:historyNote  "" ;
        skos:example      "" .

parentalguidance:_3  rdf:type  ebucore:TargetAudience ;
        skos:prefLabel    "AU-OFLC"@en ;
        skos:altLabel     "AU-NCS"@en ;
        skos:altLabel     "Australian Classification Board"@en ;
        skos:scopeNote    "Region:Australia"@en ;
        skos:definition   "Office of Film and Literature Classification"@en ;
        skos:inScheme     <http://www.ebu.ch/metadata/ontologies/skos/ebu_ParentalGuidanceCodeCS> ;
        skos:narrower     parentalguidance:_3.1 ;
        skos:narrower     parentalguidance:_3.2 ;
        skos:narrower     parentalguidance:_3.3 ;
        skos:narrower     parentalguidance:_3.4 ;
        skos:narrower     parentalguidance:_3.5 ;
        skos:narrower     parentalguidance:_3.6 ;
        skos:changeNote   "Update" ;
        skos:historyNote  "2009-07-27" ;
        skos:example      "" ;
        skos:note         "Valid" .

parentalguidance:_3.1
        rdf:type          ebucore:TargetAudience ;
        skos:prefLabel    "G"@en ;
        skos:altLabel    "General"@en ;
        skos:definition   "G classified films and computer games are for general viewing.\n         Many of the films and computer games contain content that would be of no interest to\n         children. The impact of the content is very mild."@en ;
        skos:broader      parentalguidance:_3 ;
        skos:inScheme     <http://www.ebu.ch/metadata/ontologies/skos/ebu_ParentalGuidanceCodeCS> ;
        skos:changeNote   "" ;
        skos:historyNote  "" ;
        skos:example      "" .

parentalguidance:_3.2
        rdf:type          ebucore:TargetAudience ;
        skos:prefLabel     "PG"@en ;
        skos:altLabel    "Parental Guidance"@en ;
        skos:definition   "PG classified films and computer games may contain material\n         that needs to be explained to children therefore parental guidance is recommended. The\n         impact of the content is mild."@en ;
        skos:broader      parentalguidance:_3 ;
        skos:inScheme     <http://www.ebu.ch/metadata/ontologies/skos/ebu_ParentalGuidanceCodeCS> ;
        skos:changeNote   "" ;
        skos:historyNote  "" ;
        skos:example      "" .

parentalguidance:_3.3
        rdf:type          ebucore:TargetAudience ;
        skos:prefLabel    "M"@en ;
        skos:altLabel     "Mature"@en ;
        skos:definition   "The M category is recommended for mature audiences. A mature\n         perspective is required to view this material. The impact of the content is\n         moderate."@en ;
        skos:broader      parentalguidance:_3 ;
        skos:inScheme     <http://www.ebu.ch/metadata/ontologies/skos/ebu_ParentalGuidanceCodeCS> ;
        skos:changeNote   "" ;
        skos:historyNote  "" ;
        skos:example      "" .

parentalguidance:_3.4
        rdf:type          ebucore:TargetAudience ;
        skos:prefLabel    "MA15+"@en ;
        skos:definition   "The MA 15+ category is a legally restricted category. The\n         impact of the content is strong. A person under the age of 15 years must be accompanied by\n         a parent or adult guardian if viewing or buying a film or computer game classified MA\n         15+."@en ;
        skos:broader      parentalguidance:_3 ;
        skos:inScheme     <http://www.ebu.ch/metadata/ontologies/skos/ebu_ParentalGuidanceCodeCS> ;
        skos:changeNote   "" ;
        skos:historyNote  "" ;
        skos:example      "" .

parentalguidance:_3.5
        rdf:type          ebucore:TargetAudience ;
        skos:prefLabel    "R18+"@en ;
        skos:definition   "R 18+ classified films are legally restricted to persons 18\n         years and over because of the high impact content. Some material in this classification may\n         be offensive to some sections of the adult community. "@en ;
        skos:broader      parentalguidance:_3 ;
        skos:inScheme     <http://www.ebu.ch/metadata/ontologies/skos/ebu_ParentalGuidanceCodeCS> ;
        skos:changeNote   "" ;
        skos:historyNote  "" ;
        skos:example      "" .

parentalguidance:_3.6
        rdf:type          ebucore:TargetAudience ;
        skos:prefLabel    "X18+"@en ;
        skos:altLabel     "Restricted to 18 and over"@en ;
        skos:definition   "The X 18+ classification only applies to films that contain\n         sexually explicit material between consenting adults. It is restricted to persons aged 18\n         years and over and can only be sold or hired legally in the ACT and the Northern Territory.\n         The possession and supply of X 18+ films is prohibited in prescribed areas of the Northern\n         Territory."@en ;
        skos:broader      parentalguidance:_3 ;
        skos:inScheme     <http://www.ebu.ch/metadata/ontologies/skos/ebu_ParentalGuidanceCodeCS> ;
        skos:changeNote   "" ;
        skos:historyNote  "" ;
        skos:example      "" .

parentalguidance:_4  rdf:type  ebucore:TargetAudience ;
        skos:prefLabel    "AU-ACMA"@en ;
        skos:altLabel     "www.acma.gov.au"@en ;
        skos:scopeNote    "Region:Australia"@en ;
        skos:definition   "Australian Communications and Media Authority"@en ;
        skos:inScheme     <http://www.ebu.ch/metadata/ontologies/skos/ebu_ParentalGuidanceCodeCS> ;
        skos:narrower     parentalguidance:_4.1 ;
        skos:narrower     parentalguidance:_4.2 ;
        skos:changeNote   "Update" ;
        skos:historyNote  "2009-07-27" ;
        skos:example      "" ;
        skos:note         "Valid" .

parentalguidance:_4.1
        rdf:type          ebucore:TargetAudience ;
        skos:prefLabel    "Rating"@en ;
        skos:definition   ""@en ;
        skos:broader      parentalguidance:_4 ;
        skos:inScheme     <http://www.ebu.ch/metadata/ontologies/skos/ebu_ParentalGuidanceCodeCS> ;
        skos:narrower     parentalguidance:_4.1.1 ;
        skos:narrower     parentalguidance:_4.1.2 ;
        skos:narrower     parentalguidance:_4.1.3 ;
        skos:narrower     parentalguidance:_4.1.4 ;
        skos:narrower     parentalguidance:_4.1.5 ;
        skos:narrower     parentalguidance:_4.1.6 ;
        skos:narrower     parentalguidance:_4.1.7 ;
        skos:changeNote   "" ;
        skos:historyNote  "" ;
        skos:example      "" .

parentalguidance:_4.1.1
        rdf:type          ebucore:TargetAudience ;
        skos:prefLabel    "P"@en ;
        skos:definition   "Pre-school"@en ;
        skos:broader      parentalguidance:_4.1 ;
        skos:inScheme     <http://www.ebu.ch/metadata/ontologies/skos/ebu_ParentalGuidanceCodeCS> ;
        skos:changeNote   "" ;
        skos:historyNote  "" ;
        skos:example      "" .

parentalguidance:_4.1.2
        rdf:type          ebucore:TargetAudience ;
        skos:prefLabel    "C"@en ;
        skos:definition   "Children"@en ;
        skos:broader      parentalguidance:_4.1 ;
        skos:inScheme     <http://www.ebu.ch/metadata/ontologies/skos/ebu_ParentalGuidanceCodeCS> ;
        skos:changeNote   "" ;
        skos:historyNote  "" ;
        skos:example      "" .

parentalguidance:_4.1.3
        rdf:type          ebucore:TargetAudience ;
        skos:prefLabel    "G"@en ;
        skos:definition   "General"@en ;
        skos:broader      parentalguidance:_4.1 ;
        skos:inScheme     <http://www.ebu.ch/metadata/ontologies/skos/ebu_ParentalGuidanceCodeCS> ;
        skos:changeNote   "" ;
        skos:historyNote  "" ;
        skos:example      "" .

parentalguidance:_4.1.4
        rdf:type          ebucore:TargetAudience ;
        skos:prefLabel    "PG"@en ;
        skos:definition   "Parental Guidance"@en ;
        skos:broader      parentalguidance:_4.1 ;
        skos:inScheme     <http://www.ebu.ch/metadata/ontologies/skos/ebu_ParentalGuidanceCodeCS> ;
        skos:changeNote   "" ;
        skos:historyNote  "" ;
        skos:example      "" .

parentalguidance:_4.1.5
        rdf:type          ebucore:TargetAudience ;
        skos:prefLabel    "M"@en ;
        skos:definition   "Mature"@en ;
        skos:broader      parentalguidance:_4.1 ;
        skos:inScheme     <http://www.ebu.ch/metadata/ontologies/skos/ebu_ParentalGuidanceCodeCS> ;
        skos:changeNote   "" ;
        skos:historyNote  "" ;
        skos:example      "" .

parentalguidance:_4.1.6
        rdf:type          ebucore:TargetAudience ;
        skos:prefLabel    "MA15+"@en ;
        skos:definition   "15 or older"@en ;
        skos:broader      parentalguidance:_4.1 ;
        skos:inScheme     <http://www.ebu.ch/metadata/ontologies/skos/ebu_ParentalGuidanceCodeCS> ;
        skos:changeNote   "" ;
        skos:historyNote  "" ;
        skos:example      "" .

parentalguidance:_4.1.7
        rdf:type          ebucore:TargetAudience ;
        skos:prefLabel    "AV15+"@en ;
        skos:definition   "15 or older with violent content"@en ;
        skos:broader      parentalguidance:_4.1 ;
        skos:inScheme     <http://www.ebu.ch/metadata/ontologies/skos/ebu_ParentalGuidanceCodeCS> ;
        skos:changeNote   "" ;
        skos:historyNote  "" ;
        skos:example      "" .

parentalguidance:_4.2
        rdf:type          ebucore:TargetAudience ;
        skos:prefLabel    "Criteria"@en ;
        skos:definition   ""@en ;
        skos:broader      parentalguidance:_4 ;
        skos:inScheme     <http://www.ebu.ch/metadata/ontologies/skos/ebu_ParentalGuidanceCodeCS> ;
        skos:narrower     parentalguidance:_4.2.1 ;
        skos:narrower     parentalguidance:_4.2.2 ;
        skos:narrower     parentalguidance:_4.2.3 ;
        skos:narrower     parentalguidance:_4.2.4 ;
        skos:narrower     parentalguidance:_4.2.5 ;
        skos:narrower     parentalguidance:_4.2.6 ;
        skos:narrower     parentalguidance:_4.2.7 ;
        skos:narrower     parentalguidance:_4.2.8 ;
        skos:narrower     parentalguidance:_4.2.9 ;
        skos:narrower     parentalguidance:_4.2.10 ;
        skos:narrower     parentalguidance:_4.2.11 ;
        skos:changeNote   "" ;
        skos:historyNote  "" ;
        skos:example      "" .

parentalguidance:_4.2.1
        rdf:type          ebucore:TargetAudience ;
        skos:prefLabel    "A"@en ;
        skos:definition   "Adult"@en ;
        skos:broader      parentalguidance:_4.2 ;
        skos:inScheme     <http://www.ebu.ch/metadata/ontologies/skos/ebu_ParentalGuidanceCodeCS> ;
        skos:changeNote   "" ;
        skos:historyNote  "" ;
        skos:example      "" .

parentalguidance:_4.2.2
        rdf:type          ebucore:TargetAudience ;
        skos:prefLabel    "V"@en ;
        skos:definition   "Violence"@en ;
        skos:broader      parentalguidance:_4.2 ;
        skos:inScheme     <http://www.ebu.ch/metadata/ontologies/skos/ebu_ParentalGuidanceCodeCS> ;
        skos:changeNote   "" ;
        skos:historyNote  "" ;
        skos:example      "" .

parentalguidance:_4.2.3
        rdf:type          ebucore:TargetAudience ;
        skos:prefLabel    "L"@en ;
        skos:definition   "Language"@en ;
        skos:broader      parentalguidance:_4.2 ;
        skos:inScheme     <http://www.ebu.ch/metadata/ontologies/skos/ebu_ParentalGuidanceCodeCS> ;
        skos:changeNote   "" ;
        skos:historyNote  "" ;
        skos:example      "" .

parentalguidance:_4.2.4
        rdf:type          ebucore:TargetAudience ;
        skos:prefLabel    "S"@en ;
        skos:definition   "Sex"@en ;
        skos:broader      parentalguidance:_4.2 ;
        skos:inScheme     <http://www.ebu.ch/metadata/ontologies/skos/ebu_ParentalGuidanceCodeCS> ;
        skos:changeNote   "" ;
        skos:historyNote  "" ;
        skos:example      "" .

parentalguidance:_4.2.5
        rdf:type          ebucore:TargetAudience ;
        skos:prefLabel    "H"@en ;
        skos:definition   "Horror"@en ;
        skos:broader      parentalguidance:_4.2 ;
        skos:inScheme     <http://www.ebu.ch/metadata/ontologies/skos/ebu_ParentalGuidanceCodeCS> ;
        skos:changeNote   "" ;
        skos:historyNote  "" ;
        skos:example      "" .

parentalguidance:_4.2.6
        rdf:type          ebucore:TargetAudience ;
        skos:prefLabel    "D"@en ;
        skos:definition   "Drugs"@en ;
        skos:broader      parentalguidance:_4.2 ;
        skos:inScheme     <http://www.ebu.ch/metadata/ontologies/skos/ebu_ParentalGuidanceCodeCS> ;
        skos:changeNote   "" ;
        skos:historyNote  "" ;
        skos:example      "" .

parentalguidance:_4.2.7
        rdf:type          ebucore:TargetAudience ;
        skos:prefLabel    "N"@en ;
        skos:definition   "Nudity"@en ;
        skos:broader      parentalguidance:_4.2 ;
        skos:inScheme     <http://www.ebu.ch/metadata/ontologies/skos/ebu_ParentalGuidanceCodeCS> ;
        skos:changeNote   "" ;
        skos:historyNote  "" ;
        skos:example      "" .

parentalguidance:_4.2.8
        rdf:type          ebucore:TargetAudience ;
        skos:prefLabel    "SN"@en ;
        skos:definition   "Supernatural"@en ;
        skos:broader      parentalguidance:_4.2 ;
        skos:inScheme     <http://www.ebu.ch/metadata/ontologies/skos/ebu_ParentalGuidanceCodeCS> ;
        skos:changeNote   "" ;
        skos:historyNote  "" ;
        skos:example      "" .

parentalguidance:_4.2.9
        rdf:type          ebucore:TargetAudience ;
        skos:prefLabel    "M"@en ;
        skos:definition   "Medical"@en ;
        skos:broader      parentalguidance:_4.2 ;
        skos:inScheme     <http://www.ebu.ch/metadata/ontologies/skos/ebu_ParentalGuidanceCodeCS> ;
        skos:changeNote   "" ;
        skos:historyNote  "" ;
        skos:example      "" .

parentalguidance:_4.2.10
        rdf:type          ebucore:TargetAudience ;
        skos:prefLabel    "W"@en ;
        skos:definition   "War"@en ;
        skos:broader      parentalguidance:_4.2 ;
        skos:inScheme     <http://www.ebu.ch/metadata/ontologies/skos/ebu_ParentalGuidanceCodeCS> ;
        skos:changeNote   "" ;
        skos:historyNote  "" ;
        skos:example      "" .

parentalguidance:_4.2.11
        rdf:type          ebucore:TargetAudience ;
        skos:prefLabel    "B"@en ;
        skos:definition   "Colorful behaviour"@en ;
        skos:broader      parentalguidance:_4.2 ;
        skos:inScheme     <http://www.ebu.ch/metadata/ontologies/skos/ebu_ParentalGuidanceCodeCS> ;
        skos:changeNote   "" ;
        skos:historyNote  "" ;
        skos:example      "" .

parentalguidance:_5  rdf:type  ebucore:TargetAudience ;
        skos:prefLabel    "BE-CICF"@en ;
        skos:scopeNote    "Region:Belgium"@en ;
        skos:inScheme     <http://www.ebu.ch/metadata/ontologies/skos/ebu_ParentalGuidanceCodeCS> ;
        skos:narrower     parentalguidance:_5.1 ;
        skos:narrower     parentalguidance:_5.2 ;
        skos:changeNote   "" ;
        skos:historyNote  "" ;
        dct:description   "Movie labs ratings: https://www.movielabs.com/md/ratings/v2.0/html/BE_CICF_Ratings.html"@en ;
        skos:example      "" .

parentalguidance:_5.1
        rdf:type          ebucore:TargetAudience ;
        skos:prefLabel    "KT"@nl ;
        skos:prefLabel    "EA"@fr ;
        skos:prefLabel    "Children Allowed"@en ;
        skos:definition   "Kinderen Toegelaten"@nl ;
        skos:definition   "Enfants admis"@fr ;
        skos:definition   "Children admitted - Suitable for all"@en ;
        skos:broader      parentalguidance:_5 ;
        skos:inScheme     <http://www.ebu.ch/metadata/ontologies/skos/ebu_ParentalGuidanceCodeCS> ;
        skos:changeNote   "" ;
        skos:historyNote  "" ;
        skos:example      "" .

parentalguidance:_5.2
        rdf:type          ebucore:TargetAudience ;
        skos:prefLabel    "KNT"@nl ;
        skos:prefLabel    "ENA"@fr ;
        skos:prefLabel    "Children Not Allowed"@en ;
        skos:definition   "Kinderen Niet Toegelaten"@nl ;
        skos:definition   "Enfants Non admis"@fr ;
        skos:definition   "Children not admitted (below 16 years of age)"@en ;
        skos:broader      parentalguidance:_5 ;
        skos:inScheme     <http://www.ebu.ch/metadata/ontologies/skos/ebu_ParentalGuidanceCodeCS> ;
        skos:changeNote   "" ;
        skos:historyNote  "" ;
        skos:example      "" .

parentalguidance:_6  rdf:type  ebucore:TargetAudience ;
        skos:prefLabel    "BG-FIA"@en ;
        skos:altLabel     "BG-NFRC"@en ;
        skos:scopeNote    "Region:Bulgaria"@en ;
        skos:definition   "Film Industry Act"@en ;
        skos:definition   "National Film Rating Committee"@en ;
        skos:inScheme     <http://www.ebu.ch/metadata/ontologies/skos/ebu_ParentalGuidanceCodeCS> ;
        skos:narrower     parentalguidance:_6.1 ;
        skos:narrower     parentalguidance:_6.2 ;
        skos:narrower     parentalguidance:_6.3 ;
        skos:narrower     parentalguidance:_6.4 ;
        skos:narrower     parentalguidance:_6.5 ;
        skos:changeNote   "Update" ;
        skos:historyNote  "2009-07-27" ;
        skos:example      "" ;
        skos:note         "Valid" .

parentalguidance:_6.1
        rdf:type          ebucore:TargetAudience ;
        skos:prefLabel    "A"@po ;
        skos:prefLabel    "A"@en ;
        skos:definition   "When the film confirms the ideals of humanism or popularizes\n         the national and world cultures or contributes to upbringing children"@en ;
        skos:broader      parentalguidance:_6 ;
        skos:inScheme     <http://www.ebu.ch/metadata/ontologies/skos/ebu_ParentalGuidanceCodeCS> ;
        skos:changeNote   "" ;
        skos:historyNote  "" ;
        skos:example      "" .

parentalguidance:_6.2
        rdf:type          ebucore:TargetAudience ;
        skos:prefLabel    "B"@en ;
        skos:definition   "All ages - When the film is in no way contrary to the universal\n         rules of morality in this country, has no restrictive recommendations from the Committee\n         and does not fall in rating A"@en ;
        skos:broader      parentalguidance:_6 ;
        skos:inScheme     <http://www.ebu.ch/metadata/ontologies/skos/ebu_ParentalGuidanceCodeCS> ;
        skos:changeNote   "" ;
        skos:historyNote  "" ;
        skos:example      "" .

parentalguidance:_6.3
        rdf:type          ebucore:TargetAudience ;
        skos:prefLabel    "C"@en ;
        skos:definition   "For 12 and over - When the film contains certain erotic scenes\n         or scenes with drinking, taking drugs or stimulants or a few scenes of\n         violence"@en ;
        skos:broader      parentalguidance:_6 ;
        skos:inScheme     <http://www.ebu.ch/metadata/ontologies/skos/ebu_ParentalGuidanceCodeCS> ;
        skos:changeNote   "" ;
        skos:historyNote  "" ;
        skos:example      "" .

parentalguidance:_6.4
        rdf:type          ebucore:TargetAudience ;
        skos:prefLabel    "D"@po ;
        skos:prefLabel    "D"@en ;
        skos:definition   "For 16 and over - When the film contains quite a number of\n         erotic scenes or scenes with drinking, taking drugs or stimulants or a considerable number\n         of scenes showing violence"@en ;
        skos:broader      parentalguidance:_6 ;
        skos:inScheme     <http://www.ebu.ch/metadata/ontologies/skos/ebu_ParentalGuidanceCodeCS> ;
        skos:changeNote   "" ;
        skos:historyNote  "" ;
        skos:example      "" .

parentalguidance:_6.5
        rdf:type          ebucore:TargetAudience ;
        skos:prefLabel    "D"@po ;
        skos:prefLabel    "X"@en ;
        skos:definition   "When the film is naturalistically erotic or shows violence in\n         an ostentatious manner"@en ;
        skos:broader      parentalguidance:_6 ;
        skos:inScheme     <http://www.ebu.ch/metadata/ontologies/skos/ebu_ParentalGuidanceCodeCS> ;
        skos:changeNote   "" ;
        skos:historyNote  "" ;
        skos:example      "" .

parentalguidance:_7  rdf:type  ebucore:TargetAudience ;
        skos:prefLabel    "BR-DJCTQ"@en ;
        skos:altLabel     "Departamento de Justiça, Classificação, Títulos e Qualificação"@pt ;
        skos:scopeNote    "Region:Brazil"@en ;
        skos:definition   "Department of Justice, Rating, Titles and Qualification"@en ;
        skos:definition   "Departamento de Justiça, Classificação, Títulos e Qualificação"@pt ;
        skos:inScheme     <http://www.ebu.ch/metadata/ontologies/skos/ebu_ParentalGuidanceCodeCS> ;
        skos:narrower     parentalguidance:_7.1 ;
        skos:narrower     parentalguidance:_7.2 ;
        skos:narrower     parentalguidance:_7.3 ;
        skos:narrower     parentalguidance:_7.4 ;
        skos:narrower     parentalguidance:_7.5 ;
        skos:narrower     parentalguidance:_7.6 ;
        skos:narrower     parentalguidance:_7.7 ;
        skos:changeNote   "Update" ;
        skos:historyNote  "2009-07-27" ;
        skos:example      "" ;
        skos:note         "Valid" .

parentalguidance:_7.1
        rdf:type          ebucore:TargetAudience ;
        skos:prefLabel    "ER"@pt ;
        skos:prefLabel    "ER"@en ;
        skos:definition   "Especialmente Recomendado para Crianças e\n         Adolescentes"@pt ;
        skos:definition   "Especially Recommended for Children and Adolescents. This\n         rating means that the film is especially advised for children and adolescents. Contains\n         educational material, and doesn't have any inappropriate content. "@en ;
        skos:broader      parentalguidance:_7 ;
        skos:inScheme     <http://www.ebu.ch/metadata/ontologies/skos/ebu_ParentalGuidanceCodeCS> ;
        skos:changeNote   "" ;
        skos:historyNote  "" ;
        skos:example      "" .

parentalguidance:_7.2
        rdf:type          ebucore:TargetAudience ;
        skos:prefLabel    "L"@pt ;
        skos:prefLabel    "L"@en ;
        skos:definition   "Livre para Todos os Públicos"@pt ;
        skos:definition   "This rating means that the film/game can be watched/played by\n         anyone and doesn't have any inappropriate content"@en ;
        skos:broader      parentalguidance:_7 ;
        skos:inScheme     <http://www.ebu.ch/metadata/ontologies/skos/ebu_ParentalGuidanceCodeCS> ;
        skos:changeNote   "" ;
        skos:historyNote  "" ;
        skos:example      "" .

parentalguidance:_7.3
        rdf:type          ebucore:TargetAudience ;
        skos:prefLabel    "10"@pt ;
        skos:prefLabel    "10"@en ;
        skos:definition   "This film/game is recommended for persons with or over 10 years\n         of age. May contain a little inappropriate language, sexual innuendo, or mild\n         violence."@en ;
        skos:definition   "Não Recomendando para Menores de 10 Anos"@pt ;
        skos:broader      parentalguidance:_7 ;
        skos:inScheme     <http://www.ebu.ch/metadata/ontologies/skos/ebu_ParentalGuidanceCodeCS> ;
        skos:changeNote   "" ;
        skos:historyNote  "" ;
        skos:example      "" .

parentalguidance:_7.4
        rdf:type          ebucore:TargetAudience ;
        skos:prefLabel    "12"@pt ;
        skos:prefLabel    "12"@en ;
        skos:definition   "This film/game is recommended for persons with or over 12 years\n         of age. May contain a little inappropriate language, sexual innuendo, or mild\n         violence."@en ;
        skos:definition   "Não Recomendando para Menores de 12 Anos"@pt ;
        skos:broader      parentalguidance:_7 ;
        skos:inScheme     <http://www.ebu.ch/metadata/ontologies/skos/ebu_ParentalGuidanceCodeCS> ;
        skos:changeNote   "" ;
        skos:historyNote  "" ;
        skos:example      "" .

parentalguidance:_7.5
        rdf:type          ebucore:TargetAudience ;
        skos:prefLabel    "14"@pt ;
        skos:prefLabel    "14"@en ;
        skos:definition   "This film/game is recommended for persons with or over 14 years\n         of age. May contain inappropriate language, sexual innuendo and/or mild sex with no nudity\n         or the act being explicit shown, violence, mention to drug use."@en ;
        skos:definition   "Não Recomendando para Menores de 14 Anos"@pt ;
        skos:broader      parentalguidance:_7 ;
        skos:inScheme     <http://www.ebu.ch/metadata/ontologies/skos/ebu_ParentalGuidanceCodeCS> ;
        skos:changeNote   "" ;
        skos:historyNote  "" ;
        skos:example      "" .

parentalguidance:_7.6
        rdf:type          ebucore:TargetAudience ;
        skos:prefLabel    "16"@pt ;
        skos:prefLabel    "16"@en ;
        skos:definition   "This film/game is recommended for persons with or over 16 years\n         of age. May contain strong language, sexual innuendo and/or mild sex with or without mild\n         nudity, strong violence, drug use."@en ;
        skos:definition   "Não Recomendando para Menores de 16 Anos"@pt ;
        skos:broader      parentalguidance:_7 ;
        skos:inScheme     <http://www.ebu.ch/metadata/ontologies/skos/ebu_ParentalGuidanceCodeCS> ;
        skos:changeNote   "" ;
        skos:historyNote  "" ;
        skos:example      "" .

parentalguidance:_7.7
        rdf:type          ebucore:TargetAudience ;
        skos:prefLabel    "18"@pt ;
        skos:prefLabel    "18"@en ;
        skos:definition   "This film/game is forbidden for people under 18 years of age.\n         It may contain strong language, intense sex, strong nudity, strong violence, intense drug\n         use. It is also used to rate pornographic films.."@en ;
        skos:definition   "Não Recomendando para Menores de 18 Anos"@pt ;
        skos:broader      parentalguidance:_7 ;
        skos:inScheme     <http://www.ebu.ch/metadata/ontologies/skos/ebu_ParentalGuidanceCodeCS> ;
        skos:changeNote   "" ;
        skos:historyNote  "" ;
        skos:example      "" .

parentalguidance:_8  rdf:type  ebucore:TargetAudience ;
        skos:prefLabel    "CA-CHVRS"@en ;
        skos:altLabel     "Canadian Parental Rating"@en ;
        skos:scopeNote    "Region:Canada"@en ;
        skos:definition   "Canadian Home Video Rating System"@en ;
        skos:inScheme     <http://www.ebu.ch/metadata/ontologies/skos/ebu_ParentalGuidanceCodeCS> ;
        skos:narrower     parentalguidance:_8.1 ;
        skos:narrower     parentalguidance:_8.2 ;
        skos:narrower     parentalguidance:_8.3 ;
        skos:narrower     parentalguidance:_8.4 ;
        skos:narrower     parentalguidance:_8.5 ;
        skos:narrower     parentalguidance:_8.6 ;
        skos:changeNote   "Update" ;
        skos:historyNote  "2009-07-27" ;
        skos:example      "" ;
        skos:note         "Valid" .

parentalguidance:_8.1
        rdf:type          ebucore:TargetAudience ;
        skos:prefLabel    "G - General"@en ;
        skos:definition   "Suitable for viewing by all ages"@en ;
        skos:broader      parentalguidance:_8 ;
        skos:inScheme     <http://www.ebu.ch/metadata/ontologies/skos/ebu_ParentalGuidanceCodeCS> ;
        skos:changeNote   "" ;
        skos:historyNote  "" ;
        skos:example      "" .

parentalguidance:_8.2
        rdf:type          ebucore:TargetAudience ;
        skos:prefLabel    "PG"@en ;
        skos:altLabel     "Parental Guidance"@en ;
        skos:definition   "Parental guidance advised. Theme or content may not be suitable\n         for all children."@en ;
        skos:broader      parentalguidance:_8 ;
        skos:inScheme     <http://www.ebu.ch/metadata/ontologies/skos/ebu_ParentalGuidanceCodeCS> ;
        skos:changeNote   "" ;
        skos:historyNote  "" ;
        skos:example      "" .

parentalguidance:_8.3
        rdf:type          ebucore:TargetAudience ;
        skos:prefLabel    "14A"@en ;
        skos:definition   "Suitable for people 14 years of age or older. Those under 14\n         should view with an adult. No rental or purchase by those under 14 where prohibited by law.\n         Parents cautioned. May contain violence, coarse language and/or sexually suggestive\n         scenes."@en ;
        skos:broader      parentalguidance:_8 ;
        skos:inScheme     <http://www.ebu.ch/metadata/ontologies/skos/ebu_ParentalGuidanceCodeCS> ;
        skos:changeNote   "" ;
        skos:historyNote  "" ;
        skos:example      "" .

parentalguidance:_8.4
        rdf:type          ebucore:TargetAudience ;
        skos:prefLabel    "18A"@en ;
        skos:definition   "Suitable for people 18 years of age or older. Persons under 18\n         should view with an adult. No rental or purchase by those under 18. Parents strongly\n         cautioned. Will likely contain explicit violence, frequent coarse language, sexual activity\n         and/or horror."@en ;
        skos:broader      parentalguidance:_8 ;
        skos:inScheme     <http://www.ebu.ch/metadata/ontologies/skos/ebu_ParentalGuidanceCodeCS> ;
        skos:changeNote   "" ;
        skos:historyNote  "" ;
        skos:example      "" .

parentalguidance:_8.5
        rdf:type          ebucore:TargetAudience ;
        skos:prefLabel    "R - Restricted"@en ;
        skos:definition   "Restricted to 18 years and older. No rental or purchase by\n         those under 18. Contents not suitable for minors. Contains frequent sexual activity,\n         brutality/graphic violence, intense horror, and/or other disturbing content. "@en ;
        skos:broader      parentalguidance:_8 ;
        skos:inScheme     <http://www.ebu.ch/metadata/ontologies/skos/ebu_ParentalGuidanceCodeCS> ;
        skos:changeNote   "" ;
        skos:historyNote  "" ;
        skos:example      "" .

parentalguidance:_8.6
        rdf:type          ebucore:TargetAudience ;
        skos:prefLabel    "E - Exempt"@en ;
        skos:definition   "Contains material not subject to classification, such as\n         documentaries, nature, travel, music, arts and culture, sports and leisure, educational and\n         instructional information."@en ;
        skos:broader      parentalguidance:_8 ;
        skos:inScheme     <http://www.ebu.ch/metadata/ontologies/skos/ebu_ParentalGuidanceCodeCS> ;
        skos:changeNote   "" ;
        skos:historyNote  "" ;
        skos:example      "" .

parentalguidance:_9  rdf:type  ebucore:TargetAudience ;
        skos:prefLabel    "CA-AFR"@en ;
        skos:altLabel     "Alberta's Film Classification Board"@en ;
        skos:scopeNote    "Region:Canada"@en ;
        skos:definition   "Alberta Film rating"@en ;
        skos:inScheme     <http://www.ebu.ch/metadata/ontologies/skos/ebu_ParentalGuidanceCodeCS> ;
        skos:narrower     parentalguidance:_9.1 ;
        skos:narrower     parentalguidance:_9.2 ;
        skos:narrower     parentalguidance:_9.3 ;
        skos:narrower     parentalguidance:_9.4 ;
        skos:narrower     parentalguidance:_9.5 ;
        skos:narrower     parentalguidance:_9.6 ;
        skos:changeNote   "Update" ;
        skos:historyNote  "2009-07-27" ;
        skos:example      "" ;
        skos:note         "Valid" .

parentalguidance:_9.1
        rdf:type          ebucore:TargetAudience ;
        skos:prefLabel    "G"@en ;
        skos:altLabel    "General"@en ;
        skos:definition   "Suitable for viewing by all ages"@en ;
        skos:broader      parentalguidance:_9 ;
        skos:inScheme     <http://www.ebu.ch/metadata/ontologies/skos/ebu_ParentalGuidanceCodeCS> ;
        skos:changeNote   "" ;
        skos:historyNote  "" ;
        skos:example      "" .

parentalguidance:_9.2
        rdf:type          ebucore:TargetAudience ;
        skos:prefLabel     "PG"@en ;
        skos:altLabel    "Parental Guidance"@en ;
        skos:definition   "Parental guidance advised. Theme or content may not be suitable\n         for all children."@en ;
        skos:broader      parentalguidance:_9 ;
        skos:inScheme     <http://www.ebu.ch/metadata/ontologies/skos/ebu_ParentalGuidanceCodeCS> ;
        skos:changeNote   "" ;
        skos:historyNote  "" ;
        skos:example      "" .

parentalguidance:_9.3
        rdf:type          ebucore:TargetAudience ;
        skos:prefLabel    "14A"@en ;
        skos:definition   "Suitable for people 14 years of age or older. Those under 14\n         should view with an adult. No rental or purchase by those under 14 where prohibited by law.\n         Parents cautioned. May contain violence, coarse language and/or sexually suggestive\n         scenes."@en ;
        skos:broader      parentalguidance:_9 ;
        skos:inScheme     <http://www.ebu.ch/metadata/ontologies/skos/ebu_ParentalGuidanceCodeCS> ;
        skos:changeNote   "" ;
        skos:historyNote  "" ;
        skos:example      "" .

parentalguidance:_9.4
        rdf:type          ebucore:TargetAudience ;
        skos:prefLabel    "18A"@en ;
        skos:definition   "Suitable for people 18 years of age or older. Persons under 18\n         should view with an adult. No rental or purchase by those under 18. Parents strongly\n         cautioned. Will likely contain explicit violence, frequent coarse language, sexual activity\n         and/or horror."@en ;
        skos:broader      parentalguidance:_9 ;
        skos:inScheme     <http://www.ebu.ch/metadata/ontologies/skos/ebu_ParentalGuidanceCodeCS> ;
        skos:changeNote   "" ;
        skos:historyNote  "" ;
        skos:example      "" .

parentalguidance:_9.5
        rdf:type          ebucore:TargetAudience ;
        skos:prefLabel    "R"@en ;
        skos:altLabel     "Restricted"@en ;
        skos:definition   "Restricted to 18 years and older. No rental or purchase by\n         those under 18. Contents not suitable for minors. Contains frequent sexual activity,\n         brutality/graphic violence, intense horror, and/or other disturbing content. "@en ;
        skos:broader      parentalguidance:_9 ;
        skos:inScheme     <http://www.ebu.ch/metadata/ontologies/skos/ebu_ParentalGuidanceCodeCS> ;
        skos:changeNote   "" ;
        skos:historyNote  "" ;
        skos:example      "" .

parentalguidance:_9.6
        rdf:type          ebucore:TargetAudience ;
        skos:prefLabel    "A"@en ;
        skos:altLabel     "Adult"@en ;
        skos:definition   "Admittance restricted to persons 18 years of age or older.\n         Content not suitable for minors. Contains predominantly sexually explicit activity. "@en ;
        skos:broader      parentalguidance:_9 ;
        skos:inScheme     <http://www.ebu.ch/metadata/ontologies/skos/ebu_ParentalGuidanceCodeCS> ;
        skos:changeNote   "" ;
        skos:historyNote  "" ;
        skos:example      "" .

parentalguidance:_10  rdf:type  ebucore:TargetAudience ;
        skos:prefLabel    "CA-OFRB"@en ;
        skos:altLabel     "Ontario Film Authority"@en ;
        skos:scopeNote    "Region:Canada"@en ;
        skos:definition   "Ontario Film Review Board"@en ;
        skos:inScheme     <http://www.ebu.ch/metadata/ontologies/skos/ebu_ParentalGuidanceCodeCS> ;
        skos:narrower     parentalguidance:_10.1 ;
        skos:narrower     parentalguidance:_10.2 ;
        skos:narrower     parentalguidance:_10.3 ;
        skos:narrower     parentalguidance:_10.4 ;
        skos:narrower     parentalguidance:_10.5 ;
        skos:changeNote   "Update" ;
        skos:historyNote  "2009-07-27" ;
        skos:example      "" ;
        skos:note         "Valid" .

parentalguidance:_10.1
        rdf:type          ebucore:TargetAudience ;
        skos:prefLabel    "G"@en ;
        skos:altLabel     "General"@en ;
        skos:definition   "Suitable for viewing by all ages"@en ;
        skos:broader      parentalguidance:_10 ;
        skos:inScheme     <http://www.ebu.ch/metadata/ontologies/skos/ebu_ParentalGuidanceCodeCS> ;
        skos:changeNote   "" ;
        skos:historyNote  "" ;
        skos:example      "" .

parentalguidance:_10.2
        rdf:type          ebucore:TargetAudience ;
        skos:prefLabel     "PG"@en ;
        skos:altLabel    "Parental Guidance"@en ;
        skos:definition   "Parental guidance advised. Theme or content may not be suitable\n         for all children."@en ;
        skos:broader      parentalguidance:_10 ;
        skos:inScheme     <http://www.ebu.ch/metadata/ontologies/skos/ebu_ParentalGuidanceCodeCS> ;
        skos:changeNote   "" ;
        skos:historyNote  "" ;
        skos:example      "" .

parentalguidance:_10.3
        rdf:type          ebucore:TargetAudience ;
        skos:prefLabel    "14A"@en ;
        skos:definition   "Suitable for people 14 years of age or older. Those under 14\n         should view with an adult. No rental or purchase by those under 14 where prohibited by law.\n         Parents cautioned. May contain violence, coarse language and/or sexually suggestive\n         scenes."@en ;
        skos:broader      parentalguidance:_10 ;
        skos:inScheme     <http://www.ebu.ch/metadata/ontologies/skos/ebu_ParentalGuidanceCodeCS> ;
        skos:changeNote   "" ;
        skos:historyNote  "" ;
        skos:example      "" .

parentalguidance:_10.4
        rdf:type          ebucore:TargetAudience ;
        skos:prefLabel    "18A"@en ;
        skos:definition   "Suitable for people 18 years of age or older. Persons under 18\n         should view with an adult. No rental or purchase by those under 18. Parents strongly\n         cautioned. Will likely contain explicit violence, frequent coarse language, sexual activity\n         and/or horror."@en ;
        skos:broader      parentalguidance:_10 ;
        skos:inScheme     <http://www.ebu.ch/metadata/ontologies/skos/ebu_ParentalGuidanceCodeCS> ;
        skos:changeNote   "" ;
        skos:historyNote  "" ;
        skos:example      "" .

parentalguidance:_10.5
        rdf:type          ebucore:TargetAudience ;
        skos:prefLabel    "R"@en ;
        skos:altLabel     "Restricted"@en ;
        skos:definition   "Restricted to 18 years and older. No rental or purchase by\n         those under 18. Contents not suitable for minors. Contains frequent sexual activity,\n         brutality/graphic violence, intense horror, and/or other disturbing content. "@en ;
        skos:broader      parentalguidance:_10 ;
        skos:inScheme     <http://www.ebu.ch/metadata/ontologies/skos/ebu_ParentalGuidanceCodeCS> ;
        skos:changeNote   "" ;
        skos:historyNote  "" ;
        skos:example      "" .

parentalguidance:_11  rdf:type  ebucore:TargetAudience ;
        skos:prefLabel    "CA-RCQ"@en ;
        skos:scopeNote    "Region:Canada"@en ;
        skos:definition   "Regie du cinema du Quebec"@fr ;
        skos:inScheme     <http://www.ebu.ch/metadata/ontologies/skos/ebu_ParentalGuidanceCodeCS> ;
        skos:narrower     parentalguidance:_11.1 ;
        skos:narrower     parentalguidance:_11.2 ;
        skos:narrower     parentalguidance:_11.3 ;
        skos:narrower     parentalguidance:_11.4 ;
        skos:changeNote   "Update" ;
        skos:historyNote  "2009-07-27" ;
        skos:example      "" ;
        skos:note         "Valid" .

parentalguidance:_11.1
        rdf:type          ebucore:TargetAudience ;
        skos:prefLabel    "G"@en ;
        skos:prefLabel    "G"@fr ;
        skos:definition   "General"@fr ;
        skos:definition   "Le film peut être vu, loué ou acheté sans risque par des\n         personnes de tout âge"@fr ;
        skos:definition   "For all ages"@en ;
        skos:broader      parentalguidance:_11 ;
        skos:inScheme     <http://www.ebu.ch/metadata/ontologies/skos/ebu_ParentalGuidanceCodeCS> ;
        skos:changeNote   "" ;
        skos:historyNote  "" ;
        skos:example      "" .

parentalguidance:_11.2
        rdf:type          ebucore:TargetAudience ;
        skos:prefLabel    "13+"@en ;
        skos:prefLabel    "13+"@fr ;
        skos:definition   "Le film ne peut être vu, acheté ou loué que par des personnes\n         de 13 ans et plus. Les enfants de moins de 13 ans peuvent y avoir accès s’ils sont\n         accompagnés par un adulte."@fr ;
        skos:definition   "For 13 and older in presence of an adult"@en ;
        skos:broader      parentalguidance:_11 ;
        skos:inScheme     <http://www.ebu.ch/metadata/ontologies/skos/ebu_ParentalGuidanceCodeCS> ;
        skos:changeNote   "" ;
        skos:historyNote  "" ;
        skos:example      "" .

parentalguidance:_11.3
        rdf:type          ebucore:TargetAudience ;
        skos:prefLabel    "16+"@en ;
        skos:prefLabel    "16+"@fr ;
        skos:definition   "Le film ne peut être vu, acheté ou loué que par des personnes\n         de 16 ans et plus."@fr ;
        skos:definition   "Only for 16 and older"@en ;
        skos:broader      parentalguidance:_11 ;
        skos:inScheme     <http://www.ebu.ch/metadata/ontologies/skos/ebu_ParentalGuidanceCodeCS> ;
        skos:changeNote   "" ;
        skos:historyNote  "" ;
        skos:example      "" .

parentalguidance:_11.4
        rdf:type          ebucore:TargetAudience ;
        skos:prefLabel    "18+"@en ;
        skos:prefLabel    "18+"@fr ;
        skos:definition   "Le film ne peut être vu, acheté ou loué que par des personnes\n         de 18 ans et plus."@fr ;
        skos:definition   "Only for 18 and older"@en ;
        skos:broader      parentalguidance:_11 ;
        skos:inScheme     <http://www.ebu.ch/metadata/ontologies/skos/ebu_ParentalGuidanceCodeCS> ;
        skos:changeNote   "" ;
        skos:historyNote  "" ;
        skos:example      "" .

parentalguidance:_12  rdf:type  ebucore:TargetAudience ;
        skos:prefLabel    "CA-CBSC-CCNR-English and third-languages"@en ;
        skos:altLabel     "www.cbsc.ca"@en ;
        skos:scopeNote    "Region:Canada"@en ;
        skos:definition   "Ratings Classification for Canadian English-Language and\n         Third-Language Broadcasters"@en ;
        skos:inScheme     <http://www.ebu.ch/metadata/ontologies/skos/ebu_ParentalGuidanceCodeCS> ;
        skos:narrower     parentalguidance:_12.1 ;
        skos:narrower     parentalguidance:_12.2 ;
        skos:narrower     parentalguidance:_12.3 ;
        skos:narrower     parentalguidance:_12.4 ;
        skos:narrower     parentalguidance:_12.5 ;
        skos:narrower     parentalguidance:_12.6 ;
        skos:changeNote   "Update" ;
        skos:historyNote  "2009-07-27" ;
        skos:example      "" ;
        skos:note         "Valid" .

parentalguidance:_12.1
        rdf:type          ebucore:TargetAudience ;
        skos:prefLabel    "C"@en ;
        skos:definition   "Children"@en ;
        skos:broader      parentalguidance:_12 ;
        skos:inScheme     <http://www.ebu.ch/metadata/ontologies/skos/ebu_ParentalGuidanceCodeCS> ;
        skos:changeNote   "" ;
        skos:historyNote  "" ;
        skos:example      "" .

parentalguidance:_12.2
        rdf:type          ebucore:TargetAudience ;
        skos:prefLabel    "C8"@en ;
        skos:definition   "Children over 8 years"@en ;
        skos:broader      parentalguidance:_12 ;
        skos:inScheme     <http://www.ebu.ch/metadata/ontologies/skos/ebu_ParentalGuidanceCodeCS> ;
        skos:changeNote   "" ;
        skos:historyNote  "" ;
        skos:example      "" .

parentalguidance:_12.3
        rdf:type          ebucore:TargetAudience ;
        skos:prefLabel    "G"@en ;
        skos:altLabel     "General"@en ;
        skos:definition   "Considered acceptable for all age groups. Appropriate viewing\n         for the entire family."@en ;
        skos:broader      parentalguidance:_12 ;
        skos:inScheme     <http://www.ebu.ch/metadata/ontologies/skos/ebu_ParentalGuidanceCodeCS> ;
        skos:changeNote   "" ;
        skos:historyNote  "" ;
        skos:example      "" .

parentalguidance:_12.4
        rdf:type          ebucore:TargetAudience ;
        skos:prefLabel     "PG"@en ;
        skos:altLabel    "Parental Guidance"@en ;
        skos:definition   "This programming, while intended for a general audience, may\n         not be suitable for younger children (under the age of 8). Parents/guardians should be\n         aware that there might be content elements which some could consider inappropriate for\n         unsupervised viewing by children in the 8-13 age range."@en ;
        skos:broader      parentalguidance:_12 ;
        skos:inScheme     <http://www.ebu.ch/metadata/ontologies/skos/ebu_ParentalGuidanceCodeCS> ;
        skos:changeNote   "" ;
        skos:historyNote  "" ;
        skos:example      "" .

parentalguidance:_12.5
        rdf:type          ebucore:TargetAudience ;
        skos:prefLabel    "14+"@en ;
        skos:definition   "Over 14 Years"@en ;
        skos:broader      parentalguidance:_12 ;
        skos:inScheme     <http://www.ebu.ch/metadata/ontologies/skos/ebu_ParentalGuidanceCodeCS> ;
        skos:changeNote   "" ;
        skos:historyNote  "" ;
        skos:example      "" .

parentalguidance:_12.6
        rdf:type          ebucore:TargetAudience ;
        skos:prefLabel    "18+"@en ;
        skos:definition   "Over 18 Years"@en ;
        skos:broader      parentalguidance:_12 ;
        skos:inScheme     <http://www.ebu.ch/metadata/ontologies/skos/ebu_ParentalGuidanceCodeCS> ;
        skos:changeNote   "" ;
        skos:historyNote  "" ;
        skos:example      "" .

parentalguidance:_13  rdf:type  ebucore:TargetAudience ;
        skos:prefLabel    "CA-CBSC-CCNR-French"@en ;
        skos:scopeNote    "Region:Canada"@en ;
        skos:definition   "Ratings Classification for Canadian French-Language\n         Broadcasters"@en ;
        skos:inScheme     <http://www.ebu.ch/metadata/ontologies/skos/ebu_ParentalGuidanceCodeCS> ;
        skos:narrower     parentalguidance:_13.1 ;
        skos:narrower     parentalguidance:_13.2 ;
        skos:narrower     parentalguidance:_13.3 ;
        skos:narrower     parentalguidance:_13.4 ;
        skos:narrower     parentalguidance:_13.5 ;
        skos:changeNote   "Update" ;
        skos:historyNote  "2009-07-27" ;
        skos:example      "" ;
        skos:note         "Valid" .

parentalguidance:_13.1
        rdf:type          ebucore:TargetAudience ;
        skos:prefLabel    "G"@en ;
        skos:prefLabel    "G"@fr ;
        skos:definition   "General"@fr ;
        skos:definition   "Le film peut être vu, loué ou acheté sans risque par des\n         personnes de tout âge"@fr ;
        skos:definition   "For all ages"@en ;
        skos:broader      parentalguidance:_13 ;
        skos:inScheme     <http://www.ebu.ch/metadata/ontologies/skos/ebu_ParentalGuidanceCodeCS> ;
        skos:changeNote   "" ;
        skos:historyNote  "" ;
        skos:example      "" .

parentalguidance:_13.2
        rdf:type          ebucore:TargetAudience ;
        skos:prefLabel    "8+"@en ;
        skos:prefLabel    "8+"@fr ;
        skos:definition   "General, non approprié pour jeunes enfants de moins e 8\n         ans"@fr ;
        skos:definition   "General – Not Suitable for Young Children"@en ;
        skos:broader      parentalguidance:_13 ;
        skos:inScheme     <http://www.ebu.ch/metadata/ontologies/skos/ebu_ParentalGuidanceCodeCS> ;
        skos:changeNote   "" ;
        skos:historyNote  "" ;
        skos:example      "" .

parentalguidance:_13.3
        rdf:type          ebucore:TargetAudience ;
        skos:prefLabel    "13+"@en ;
        skos:prefLabel    "13+"@fr ;
        skos:definition   "Le film ne peut être vu, acheté ou loué que par des personnes\n         de 13 ans et plus. Les enfants de moins de 13 ans peuvent y avoir accès s’ils sont\n         accompagnés par un adulte."@fr ;
        skos:definition   "For 13 and older in presence of an adult"@en ;
        skos:broader      parentalguidance:_13 ;
        skos:inScheme     <http://www.ebu.ch/metadata/ontologies/skos/ebu_ParentalGuidanceCodeCS> ;
        skos:changeNote   "" ;
        skos:historyNote  "" ;
        skos:example      "" .

parentalguidance:_13.4
        rdf:type          ebucore:TargetAudience ;
        skos:prefLabel    "16+"@en ;
        skos:prefLabel    "16+"@fr ;
        skos:definition   "Le film ne peut être vu, acheté ou loué que par des personnes\n         de 16 ans et plus."@fr ;
        skos:definition   "Only for 16 and older"@en ;
        skos:broader      parentalguidance:_13 ;
        skos:inScheme     <http://www.ebu.ch/metadata/ontologies/skos/ebu_ParentalGuidanceCodeCS> ;
        skos:changeNote   "" ;
        skos:historyNote  "" ;
        skos:example      "" .

parentalguidance:_13.5
        rdf:type          ebucore:TargetAudience ;
        skos:prefLabel    "18+"@en ;
        skos:prefLabel    "18+"@fr ;
        skos:definition   "Le film ne peut être vu, acheté ou loué que par des personnes\n         de 18 ans et plus."@fr ;
        skos:definition   "Only for 18 and older"@en ;
        skos:broader      parentalguidance:_13 ;
        skos:inScheme     <http://www.ebu.ch/metadata/ontologies/skos/ebu_ParentalGuidanceCodeCS> ;
        skos:changeNote   "" ;
        skos:historyNote  "" ;
        skos:example      "" .

parentalguidance:_14  rdf:type  ebucore:TargetAudience ;
        skos:prefLabel    "CL-ANATEL"@es ;
        skos:prefLabel    "CL-ANATEL"@en ;
        skos:altLabel    "Chilean National Television Association"@en ;
        skos:altLabel    "Consejo Nacional de Televisión"@es ;
        skos:scopeNote    "Region:Chile"@en ;
        skos:definition   "Asociación Nacional de Televisión"@es ;
        skos:definition   "National Broadcasting Association rating\n         system"@en ;
        skos:inScheme     <http://www.ebu.ch/metadata/ontologies/skos/ebu_ParentalGuidanceCodeCS> ;
        skos:narrower     parentalguidance:_14.1 ;
        skos:narrower     parentalguidance:_14.2 ;
        skos:narrower     parentalguidance:_14.3 ;
        skos:narrower     parentalguidance:_14.4 ;
        skos:narrower     parentalguidance:_14.5 ;
        skos:narrower     parentalguidance:_14.6 ;
        skos:changeNote   "Update" ;
        skos:historyNote  "2009-07-27" ;
        skos:example      "" ;
        skos:note         "Valid" .

parentalguidance:_14.1
        rdf:type          ebucore:TargetAudience ;
        skos:prefLabel    "I"@en ;
        skos:definition   "Infantil"@es ;
        skos:definition   "For all ages"@en ;
        skos:broader      parentalguidance:_14 ;
        skos:inScheme     <http://www.ebu.ch/metadata/ontologies/skos/ebu_ParentalGuidanceCodeCS> ;
        skos:changeNote   "" ;
        skos:historyNote  "" ;
        skos:example      "" .

parentalguidance:_14.2
        rdf:type          ebucore:TargetAudience ;
        skos:prefLabel    "I7"@en ;
        skos:definition   "Infantil para mayores de 7 años"@es ;
        skos:definition   "For ages 7 and older"@en ;
        skos:broader      parentalguidance:_14 ;
        skos:inScheme     <http://www.ebu.ch/metadata/ontologies/skos/ebu_ParentalGuidanceCodeCS> ;
        skos:changeNote   "" ;
        skos:historyNote  "" ;
        skos:example      "" .

parentalguidance:_14.3
        rdf:type          ebucore:TargetAudience ;
        skos:prefLabel    "I12"@en ;
        skos:definition   "Infantil para mayores de 12 años"@es ;
        skos:definition   "For ages 12 and older"@en ;
        skos:broader      parentalguidance:_14 ;
        skos:inScheme     <http://www.ebu.ch/metadata/ontologies/skos/ebu_ParentalGuidanceCodeCS> ;
        skos:changeNote   "" ;
        skos:historyNote  "" ;
        skos:example      "" .

parentalguidance:_14.4
        rdf:type          ebucore:TargetAudience ;
        skos:prefLabel    "F"@en ;
        skos:definition   "Familiar"@es ;
        skos:definition   "Shows suitable for all ages, regardless of specific\n         content."@en ;
        skos:broader      parentalguidance:_14 ;
        skos:inScheme     <http://www.ebu.ch/metadata/ontologies/skos/ebu_ParentalGuidanceCodeCS> ;
        skos:changeNote   "" ;
        skos:historyNote  "" ;
        skos:example      "" .

parentalguidance:_14.5
        rdf:type          ebucore:TargetAudience ;
        skos:prefLabel    "R"@en ;
        skos:definition   "Responsabilidad compartida"@es ;
        skos:definition   "Shared responsibility - Children accompanied by an\n         adult."@en ;
        skos:broader      parentalguidance:_14 ;
        skos:inScheme     <http://www.ebu.ch/metadata/ontologies/skos/ebu_ParentalGuidanceCodeCS> ;
        skos:changeNote   "" ;
        skos:historyNote  "" ;
        skos:example      "" .

parentalguidance:_14.6
        rdf:type          ebucore:TargetAudience ;
        skos:prefLabel    "A"@en ;
        skos:definition   "Adulto"@es ;
        skos:definition   "For adult audiences only (ages 18 or older). Shows that contain\n         explicit language, sex scenes, explicit situations"@en ;
        skos:broader      parentalguidance:_14 ;
        skos:inScheme     <http://www.ebu.ch/metadata/ontologies/skos/ebu_ParentalGuidanceCodeCS> ;
        skos:changeNote   "" ;
        skos:historyNote  "" ;
        skos:example      "" .

parentalguidance:_15  rdf:type  ebucore:TargetAudience ;
        skos:prefLabel    "CL-CCC"@en ;
        skos:prefLabel    "CL-CCC"@es ;
        skos:altLabel     "Consejo de Calificacion Cinematografica"@es ;
        skos:altLabel     "Chilean Council of Cinematographic Classification"@en ;
        skos:scopeNote    "Region:Chile"@en ;
        skos:definition   "Movie ratings as defined by the Chilean Council of\n         Cinematographic Classification"@en ;
        skos:definition   "Consejo de Calificacion Cinematografica"@es ;
        skos:inScheme     <http://www.ebu.ch/metadata/ontologies/skos/ebu_ParentalGuidanceCodeCS> ;
        skos:narrower     parentalguidance:_15.1 ;
        skos:narrower     parentalguidance:_15.2 ;
        skos:narrower     parentalguidance:_15.3 ;
        skos:narrower     parentalguidance:_15.4 ;
        skos:narrower     parentalguidance:_15.5 ;
        skos:changeNote   "Update" ;
        skos:historyNote  "2009-07-27" ;
        skos:example      "" ;
        skos:note         "Valid" .

parentalguidance:_15.1
        rdf:type          ebucore:TargetAudience ;
        skos:prefLabel    "TE"@en ;
        skos:definition   "Todo expectador"@es ;
        skos:definition   "All Audiences"@en ;
        skos:broader      parentalguidance:_15 ;
        skos:inScheme     <http://www.ebu.ch/metadata/ontologies/skos/ebu_ParentalGuidanceCodeCS> ;
        skos:changeNote   "" ;
        skos:historyNote  "" ;
        skos:example      "" .

parentalguidance:_15.2
        rdf:type          ebucore:TargetAudience ;
        skos:prefLabel    "14"@en ;
        skos:definition   "Mayor de 14 anos"@es ;
        skos:definition   "Inappropriate for children under 14"@en ;
        skos:broader      parentalguidance:_15 ;
        skos:inScheme     <http://www.ebu.ch/metadata/ontologies/skos/ebu_ParentalGuidanceCodeCS> ;
        skos:changeNote   "" ;
        skos:historyNote  "" ;
        skos:example      "" .

parentalguidance:_15.3
        rdf:type          ebucore:TargetAudience ;
        skos:prefLabel    "18"@en ;
        skos:definition   "Mayor de 18 anos"@es ;
        skos:definition   "Suitable for people aged 18 and over"@en ;
        skos:broader      parentalguidance:_15 ;
        skos:inScheme     <http://www.ebu.ch/metadata/ontologies/skos/ebu_ParentalGuidanceCodeCS> ;
        skos:changeNote   "" ;
        skos:historyNote  "" ;
        skos:example      "" .

parentalguidance:_15.4
        rdf:type          ebucore:TargetAudience ;
        skos:prefLabel    "18/S"@en ;
        skos:definition   "Suitable for people aged 18 and over with sexually explicit\n         content"@en ;
        skos:broader      parentalguidance:_15 ;
        skos:inScheme     <http://www.ebu.ch/metadata/ontologies/skos/ebu_ParentalGuidanceCodeCS> ;
        skos:changeNote   "" ;
        skos:historyNote  "" ;
        skos:example      "" .

parentalguidance:_15.5
        rdf:type          ebucore:TargetAudience ;
        skos:prefLabel    "18/V"@en ;
        skos:definition   "Suitable for people aged 18 and over with extreme violence\n         content"@en ;
        skos:broader      parentalguidance:_15 ;
        skos:inScheme     <http://www.ebu.ch/metadata/ontologies/skos/ebu_ParentalGuidanceCodeCS> ;
        skos:changeNote   "" ;
        skos:historyNote  "" ;
        skos:example      "" .

parentalguidance:_16  rdf:type  ebucore:TargetAudience ;
        skos:prefLabel    "CN-HK-HKBA"@en ;
        skos:definition   "Hong-Kong Broadcasting Authority"@en ;
        skos:scopeNote    "Region:Hong-Kong"@en ;
        skos:inScheme     <http://www.ebu.ch/metadata/ontologies/skos/ebu_ParentalGuidanceCodeCS> ;
        skos:narrower     parentalguidance:_16.1 ;
        skos:narrower     parentalguidance:_16.2 ;
        skos:changeNote   "Update" ;
        skos:historyNote  "2009-07-28" ;
        skos:example      "" ;
        skos:note         "Valid" .

parentalguidance:_16.1
        rdf:type          ebucore:TargetAudience ;
        skos:prefLabel    "Rating"@en ;
        skos:broader      parentalguidance:_16 ;
        skos:inScheme     <http://www.ebu.ch/metadata/ontologies/skos/ebu_ParentalGuidanceCodeCS> ;
        skos:narrower     parentalguidance:_16.1.1 ;
        skos:narrower     parentalguidance:_16.1.2 ;
        skos:changeNote   "" ;
        skos:historyNote  "" ;
        skos:example      "" .

parentalguidance:_16.1.1
        rdf:type          ebucore:TargetAudience ;
        skos:prefLabel     "PG"@en ;
        skos:altLabel    "Parental Guidance"@en ;
        skos:definition   "Programmes classified \"PG\" may contain adult themes or concepts\n         but must remain suitable for children to watch under the guidance of a parent or\n         guardian."@en ;
        skos:broader      parentalguidance:_16.1 ;
        skos:inScheme     <http://www.ebu.ch/metadata/ontologies/skos/ebu_ParentalGuidanceCodeCS> ;
        skos:changeNote   "" ;
        skos:historyNote  "" ;
        skos:example      "" .

parentalguidance:_16.1.2
        rdf:type          ebucore:TargetAudience ;
        skos:prefLabel    "M"@en ;
        skos:altLabel     "Mature"@en ;
        skos:definition   "Programmes classified \"M\" are recommended for viewing by\n         grown-up members of the family only."@en ;
        skos:broader      parentalguidance:_16.1 ;
        skos:inScheme     <http://www.ebu.ch/metadata/ontologies/skos/ebu_ParentalGuidanceCodeCS> ;
        skos:changeNote   "" ;
        skos:historyNote  "" ;
        skos:example      "" .

parentalguidance:_16.2
        rdf:type          ebucore:TargetAudience ;
        skos:prefLabel    "Criteria"@en ;
        skos:broader      parentalguidance:_16 ;
        skos:inScheme     <http://www.ebu.ch/metadata/ontologies/skos/ebu_ParentalGuidanceCodeCS> ;
        skos:narrower     parentalguidance:_16.2.1 ;
        skos:narrower     parentalguidance:_16.2.2 ;
        skos:narrower     parentalguidance:_16.2.3 ;
        skos:narrower     parentalguidance:_16.2.4 ;
        skos:narrower     parentalguidance:_16.2.5 ;
        skos:narrower     parentalguidance:_16.2.6 ;
        skos:narrower     parentalguidance:_16.2.7 ;
        skos:narrower     parentalguidance:_16.2.8 ;
        skos:narrower     parentalguidance:_16.2.9 ;
        skos:narrower     parentalguidance:_16.2.10 ;
        skos:narrower     parentalguidance:_16.2.11 ;
        skos:changeNote   "" ;
        skos:historyNote  "" ;
        skos:example      "" .

parentalguidance:_16.2.1
        rdf:type          ebucore:TargetAudience ;
        skos:prefLabel    "Violence"@en ;
        skos:broader      parentalguidance:_16.2 ;
        skos:inScheme     <http://www.ebu.ch/metadata/ontologies/skos/ebu_ParentalGuidanceCodeCS> ;
        skos:changeNote   "" ;
        skos:historyNote  "" ;
        skos:example      "" .

parentalguidance:_16.2.2
        rdf:type          ebucore:TargetAudience ;
        skos:prefLabel    "Language"@en ;
        skos:broader      parentalguidance:_16.2 ;
        skos:inScheme     <http://www.ebu.ch/metadata/ontologies/skos/ebu_ParentalGuidanceCodeCS> ;
        skos:changeNote   "" ;
        skos:historyNote  "" ;
        skos:example      "" .

parentalguidance:_16.2.3
        rdf:type          ebucore:TargetAudience ;
        skos:prefLabel    "Sex and nudity"@en ;
        skos:broader      parentalguidance:_16.2 ;
        skos:inScheme     <http://www.ebu.ch/metadata/ontologies/skos/ebu_ParentalGuidanceCodeCS> ;
        skos:changeNote   "" ;
        skos:historyNote  "" ;
        skos:example      "" .

parentalguidance:_16.2.4
        rdf:type          ebucore:TargetAudience ;
        skos:prefLabel    "Sexual Violence"@en ;
        skos:broader      parentalguidance:_16.2 ;
        skos:inScheme     <http://www.ebu.ch/metadata/ontologies/skos/ebu_ParentalGuidanceCodeCS> ;
        skos:changeNote   "" ;
        skos:historyNote  "" ;
        skos:example      "" .

parentalguidance:_16.2.5
        rdf:type          ebucore:TargetAudience ;
        skos:prefLabel    "Drugs and alcohol"@en ;
        skos:broader      parentalguidance:_16.2 ;
        skos:inScheme     <http://www.ebu.ch/metadata/ontologies/skos/ebu_ParentalGuidanceCodeCS> ;
        skos:changeNote   "" ;
        skos:historyNote  "" ;
        skos:example      "" .

parentalguidance:_16.2.6
        rdf:type          ebucore:TargetAudience ;
        skos:prefLabel    "Dangerous behaviour"@en ;
        skos:broader      parentalguidance:_16.2 ;
        skos:inScheme     <http://www.ebu.ch/metadata/ontologies/skos/ebu_ParentalGuidanceCodeCS> ;
        skos:changeNote   "" ;
        skos:historyNote  "" ;
        skos:example      "" .

parentalguidance:_16.2.7
        rdf:type          ebucore:TargetAudience ;
        skos:prefLabel    "Hanging scenes"@en ;
        skos:broader      parentalguidance:_16.2 ;
        skos:inScheme     <http://www.ebu.ch/metadata/ontologies/skos/ebu_ParentalGuidanceCodeCS> ;
        skos:changeNote   "" ;
        skos:historyNote  "" ;
        skos:example      "" .

parentalguidance:_16.2.8
        rdf:type          ebucore:TargetAudience ;
        skos:prefLabel    "Bad taste and indecency"@en ;
        skos:broader      parentalguidance:_16.2 ;
        skos:inScheme     <http://www.ebu.ch/metadata/ontologies/skos/ebu_ParentalGuidanceCodeCS> ;
        skos:changeNote   "" ;
        skos:historyNote  "" ;
        skos:example      "" .

parentalguidance:_16.2.9
        rdf:type          ebucore:TargetAudience ;
        skos:prefLabel    "Scenes of extreme suffering and distress"@en ;
        skos:broader      parentalguidance:_16.2 ;
        skos:inScheme     <http://www.ebu.ch/metadata/ontologies/skos/ebu_ParentalGuidanceCodeCS> ;
        skos:changeNote   "" ;
        skos:historyNote  "" ;
        skos:example      "" .

parentalguidance:_16.2.10
        rdf:type          ebucore:TargetAudience ;
        skos:prefLabel    "Exorcism, psychic or occultic practice and depiction of the\n         supernatural"@en ;
        skos:broader      parentalguidance:_16.2 ;
        skos:inScheme     <http://www.ebu.ch/metadata/ontologies/skos/ebu_ParentalGuidanceCodeCS> ;
        skos:changeNote   "" ;
        skos:historyNote  "" ;
        skos:example      "" .

parentalguidance:_16.2.11
        rdf:type          ebucore:TargetAudience ;
        skos:prefLabel    "Triad expressions and ceremonies"@en ;
        skos:broader      parentalguidance:_16.2 ;
        skos:inScheme     <http://www.ebu.ch/metadata/ontologies/skos/ebu_ParentalGuidanceCodeCS> ;
        skos:changeNote   "" ;
        skos:historyNote  "" ;
        skos:example      "" .

parentalguidance:_17  rdf:type  ebucore:TargetAudience ;
        skos:prefLabel    "CO-MOC"@en ;
        skos:scopeNote    "Region:Columbia"@en ;
        skos:definition   "Movie ratings as defined by the Colombian Ministry of\n         Culture"@en ;
        skos:inScheme     <http://www.ebu.ch/metadata/ontologies/skos/ebu_ParentalGuidanceCodeCS> ;
        skos:narrower     parentalguidance:_17.1 ;
        skos:narrower     parentalguidance:_17.2 ;
        skos:narrower     parentalguidance:_17.3 ;
        skos:narrower     parentalguidance:_17.4 ;
        skos:narrower     parentalguidance:_17.5 ;
        skos:narrower     parentalguidance:_17.6 ;
        skos:changeNote   "Update" ;
        skos:historyNote  "2009-07-27" ;
        skos:example      "" ;
        dct:description   "Movie labs ratings: https://www.movielabs.com/md/ratings/v2.0/html/CO_MOC_Ratings.html"@en ;
        skos:note         "Valid" .


parentalguidance:_17.1
        rdf:type          ebucore:TargetAudience ;
        skos:prefLabel    "T"@en ;
        skos:prefLabel    "T"@es ;
        skos:definition   "Todos"@es ;
        skos:definition   "All Audiences"@en ;
        skos:broader      parentalguidance:_17 ;
        skos:inScheme     <http://www.ebu.ch/metadata/ontologies/skos/ebu_ParentalGuidanceCodeCS> ;
        skos:changeNote   "" ;
        skos:historyNote  "" ;
        skos:example      "" .

parentalguidance:_17.2
        rdf:type          ebucore:TargetAudience ;
        skos:prefLabel    "7"@en ;
        skos:definition   "Suitable for people aged 7 and over"@en ;
        skos:broader      parentalguidance:_17 ;
        skos:inScheme     <http://www.ebu.ch/metadata/ontologies/skos/ebu_ParentalGuidanceCodeCS> ;
        skos:changeNote   "" ;
        skos:historyNote  "" ;
        skos:example      "" .

parentalguidance:_17.3
        rdf:type          ebucore:TargetAudience ;
        skos:prefLabel    "12"@en ;
        skos:definition   "Suitable for people aged 12 and over"@en ;
        skos:broader      parentalguidance:_17 ;
        skos:inScheme     <http://www.ebu.ch/metadata/ontologies/skos/ebu_ParentalGuidanceCodeCS> ;
        skos:changeNote   "" ;
        skos:historyNote  "" ;
        skos:example      "" .

parentalguidance:_17.4
        rdf:type          ebucore:TargetAudience ;
        skos:prefLabel    "15"@en ;
        skos:definition   "Suitable for people aged 15 and over"@en ;
        skos:broader      parentalguidance:_17 ;
        skos:inScheme     <http://www.ebu.ch/metadata/ontologies/skos/ebu_ParentalGuidanceCodeCS> ;
        skos:changeNote   "" ;
        skos:historyNote  "" ;
        skos:example      "" .

parentalguidance:_17.5
        rdf:type          ebucore:TargetAudience ;
        skos:prefLabel    "18"@en ;
        skos:definition   "Suitable for people aged 18 and over"@en ;
        skos:broader      parentalguidance:_17 ;
        skos:inScheme     <http://www.ebu.ch/metadata/ontologies/skos/ebu_ParentalGuidanceCodeCS> ;
        skos:changeNote   "" ;
        skos:historyNote  "" ;
        skos:example      "" .

parentalguidance:_17.6
        rdf:type          ebucore:TargetAudience ;
        skos:prefLabel    "X"@en ;
        skos:definition   "Adulto"@es ;
        skos:definition   "Adult - Pornographic Content"@en ;
        skos:broader      parentalguidance:_17 ;
        skos:inScheme     <http://www.ebu.ch/metadata/ontologies/skos/ebu_ParentalGuidanceCodeCS> ;
        skos:changeNote   "" ;
        skos:historyNote  "" ;
        skos:example      "" .

parentalguidance:_18  rdf:type  ebucore:TargetAudience ;
        skos:prefLabel    "DE-FSF"@en ;
        skos:altLabel     "Freiwillige Selbstkontrolle Fernsehen"@de ;
        skos:definition   "Freiwillige Selbskontrolle Fernsehen Altersfreigabe"@de ;
        skos:scopeNote    "Region:Germany"@en ;
        skos:definition   "German TV content classification"@en ;
        skos:inScheme     <http://www.ebu.ch/metadata/ontologies/skos/ebu_ParentalGuidanceCodeCS> ;
        skos:narrower     parentalguidance:_18.1 ;
        skos:narrower     parentalguidance:_18.2 ;
        skos:narrower     parentalguidance:_18.3 ;
        skos:narrower     parentalguidance:_18.4 ;
        skos:narrower     parentalguidance:_18.5 ;
        skos:changeNote   "Update" ;
        skos:historyNote  "2009-07-28" ;
        skos:example      "" ;
        skos:note         "Valid" .

parentalguidance:_18.1
        rdf:type          ebucore:TargetAudience ;
        skos:prefLabel    "0"@en ;
        skos:prefLabel    "0"@de ;
        skos:definition   "For all ages"@en ;
        skos:definition   "Ohne Altersbeschränkung"@de ;
        skos:broader      parentalguidance:_18 ;
        skos:inScheme     <http://www.ebu.ch/metadata/ontologies/skos/ebu_ParentalGuidanceCodeCS> ;
        skos:changeNote   "" ;
        skos:historyNote  "" ;
        skos:example      "" .

parentalguidance:_18.2
        rdf:type          ebucore:TargetAudience ;
        skos:prefLabel    "6"@en ;
        skos:prefLabel    "6"@de ;
        skos:definition   "No one under 6 years admitted"@en ;
        skos:definition   "Freigegeben ab 6 Jahren"@de ;
        skos:broader      parentalguidance:_18 ;
        skos:inScheme     <http://www.ebu.ch/metadata/ontologies/skos/ebu_ParentalGuidanceCodeCS> ;
        skos:changeNote   "" ;
        skos:historyNote  "" ;
        skos:example      "" .

parentalguidance:_18.3
        rdf:type          ebucore:TargetAudience ;
        skos:prefLabel    "12"@en ;
        skos:prefLabel    "12"@de ;
        skos:definition   "People 12 or older admitted, children between 6 and 11 only\n         when accompanied by parent or legal guardian"@en ;
        skos:definition   "Freigegeben ab 12 Jahren"@de ;
        skos:broader      parentalguidance:_18 ;
        skos:inScheme     <http://www.ebu.ch/metadata/ontologies/skos/ebu_ParentalGuidanceCodeCS> ;
        skos:changeNote   "" ;
        skos:historyNote  "" ;
        skos:example      "" .

parentalguidance:_18.4
        rdf:type          ebucore:TargetAudience ;
        skos:prefLabel    "16"@en ;
        skos:prefLabel    "16"@de ;
        skos:definition   "People 16 or older admitted"@en ;
        skos:definition   "Freigegeben ab 16 Jahren"@de ;
        skos:broader      parentalguidance:_18 ;
        skos:inScheme     <http://www.ebu.ch/metadata/ontologies/skos/ebu_ParentalGuidanceCodeCS> ;
        skos:changeNote   "" ;
        skos:historyNote  "" ;
        skos:example      "" .

parentalguidance:_18.5
        rdf:type          ebucore:TargetAudience ;
        skos:prefLabel    "18"@en ;
        skos:prefLabel    "18"@de ;
        skos:definition   "\"No youth admitted\", only adults"@en ;
        skos:definition   "Keine Jugendfreigabe"@de ;
        skos:broader      parentalguidance:_18 ;
        skos:inScheme     <http://www.ebu.ch/metadata/ontologies/skos/ebu_ParentalGuidanceCodeCS> ;
        skos:changeNote   "" ;
        skos:historyNote  "" ;
        skos:example      "" .

parentalguidance:_19  rdf:type  ebucore:TargetAudience ;
        skos:prefLabel    "DE-FSK"@en ;
        skos:altLabel     "www.fsk.de"@en ;
        skos:altLabel     "Freiwillige Selbstkontrolle der Filmwirtschaft"@de ;
        skos:scopeNote    "Region:Germany"@en ;
        skos:definition   "Voluntary Self-Control of the Film Business' rating"@en ;
        skos:definition   "Freiwillige Selbstkontrolle der Filmwirtschaft Altersfreigabe"@en ;
        skos:inScheme     <http://www.ebu.ch/metadata/ontologies/skos/ebu_ParentalGuidanceCodeCS> ;
        skos:narrower     parentalguidance:_19.1 ;
        skos:narrower     parentalguidance:_19.2 ;
        skos:narrower     parentalguidance:_19.3 ;
        skos:narrower     parentalguidance:_19.4 ;
        skos:narrower     parentalguidance:_19.5 ;
        skos:changeNote   "Update" ;
        skos:historyNote  "2009-07-28" ;
        skos:example      "" ;
        skos:note         "Valid" .

parentalguidance:_19.1
        rdf:type          ebucore:TargetAudience ;
        skos:prefLabel    "FSK 0"@en ;
        skos:prefLabel    "FSK 0"@de ;
        skos:definition   "For all ages"@en ;
        skos:definition   "Ohne Altersbeschränkung"@de ;
        skos:broader      parentalguidance:_19 ;
        skos:inScheme     <http://www.ebu.ch/metadata/ontologies/skos/ebu_ParentalGuidanceCodeCS> ;
        skos:changeNote   "" ;
        skos:historyNote  "" ;
        skos:example      "" .

parentalguidance:_19.2
        rdf:type          ebucore:TargetAudience ;
        skos:prefLabel    "FSK 6"@en ;
        skos:prefLabel    "FSK 6"@de ;
        skos:definition   "No one under 6 years admitted"@en ;
        skos:definition   "Freigegeben ab 6 Jahren"@de ;
        skos:broader      parentalguidance:_19 ;
        skos:inScheme     <http://www.ebu.ch/metadata/ontologies/skos/ebu_ParentalGuidanceCodeCS> ;
        skos:changeNote   "" ;
        skos:historyNote  "" ;
        skos:example      "" .

parentalguidance:_19.3
        rdf:type          ebucore:TargetAudience ;
        skos:prefLabel    "FSK 12"@en ;
        skos:prefLabel    "FSK 12"@de ;
        skos:definition   "People 12 or older admitted, children between 6 and 11 only\n         when accompanied by parent or legal guardian"@en ;
        skos:definition   "Freigegeben ab 12 Jahren"@de ;
        skos:broader      parentalguidance:_19 ;
        skos:inScheme     <http://www.ebu.ch/metadata/ontologies/skos/ebu_ParentalGuidanceCodeCS> ;
        skos:changeNote   "" ;
        skos:historyNote  "" ;
        skos:example      "" ;
        skos:hiddenLabel  "12"@en .

parentalguidance:_19.4
        rdf:type          ebucore:TargetAudience ;
        skos:prefLabel    "FSK 16"@en ;
        skos:prefLabel    "FSK 16"@de ;
        skos:definition   "People 16 or older admitted"@en ;
        skos:definition   "Freigegeben ab 16 Jahren"@de ;
        skos:broader      parentalguidance:_19 ;
        skos:inScheme     <http://www.ebu.ch/metadata/ontologies/skos/ebu_ParentalGuidanceCodeCS> ;
        skos:changeNote   "" ;
        skos:historyNote  "" ;
        skos:example      "" ;
        skos:hiddenLabel  "16"@en .

parentalguidance:_19.5
        rdf:type          ebucore:TargetAudience ;
        skos:prefLabel    "FSK 18"@en ;
        skos:prefLabel    "FSK 18"@de ;
        skos:definition   "\"No youth admitted\", only adults"@en ;
        skos:definition   "Keine Jugendfreigabe"@de ;
        skos:broader      parentalguidance:_19 ;
        skos:inScheme     <http://www.ebu.ch/metadata/ontologies/skos/ebu_ParentalGuidanceCodeCS> ;
        skos:changeNote   "" ;
        skos:historyNote  "" ;
        skos:example      "" .

parentalguidance:_20  rdf:type  ebucore:TargetAudience ;
        skos:prefLabel    "DK-MBU"@en ;
        skos:scopeNote    "Region:Denmark"@en ;
        skos:definition   "Medieradet for barn och unga - Media Advice for Children and\n         Youths (Denmark)"@en ;
        skos:definition   "Scheme as defined by the Danish Media Council for Children and\n         Young People"@en ;
        skos:inScheme     <http://www.ebu.ch/metadata/ontologies/skos/ebu_ParentalGuidanceCodeCS> ;
        skos:narrower     parentalguidance:_20.1 ;
        skos:narrower     parentalguidance:_20.2 ;
        skos:narrower     parentalguidance:_20.3 ;
        skos:narrower     parentalguidance:_20.4 ;
        skos:changeNote   "Update" ;
        skos:historyNote  "2009-07-28" ;
        skos:example      "" ;
        skos:note         "Valid" .

parentalguidance:_20.1
        rdf:type          ebucore:TargetAudience ;
        skos:prefLabel    "A"@en ;
        skos:definition   "Approval of the film for general admittance"@en ;
        skos:broader      parentalguidance:_20 ;
        skos:inScheme     <http://www.ebu.ch/metadata/ontologies/skos/ebu_ParentalGuidanceCodeCS> ;
        skos:changeNote   "" ;
        skos:historyNote  "" ;
        skos:example      "" .

parentalguidance:_20.2
        rdf:type          ebucore:TargetAudience ;
        skos:prefLabel    "7"@en ;
        skos:definition   "Approval of the film for general admittance, but not\n         recommended for children under the age of 7"@en ;
        skos:broader      parentalguidance:_20 ;
        skos:inScheme     <http://www.ebu.ch/metadata/ontologies/skos/ebu_ParentalGuidanceCodeCS> ;
        skos:changeNote   "" ;
        skos:historyNote  "" ;
        skos:example      "" .

parentalguidance:_20.3
        rdf:type          ebucore:TargetAudience ;
        skos:prefLabel    "11"@en ;
        skos:definition   "Approval of the film for admittance of children from the age of\n         11"@en ;
        skos:broader      parentalguidance:_20 ;
        skos:inScheme     <http://www.ebu.ch/metadata/ontologies/skos/ebu_ParentalGuidanceCodeCS> ;
        skos:changeNote   "" ;
        skos:historyNote  "" ;
        skos:example      "" .

parentalguidance:_20.4
        rdf:type          ebucore:TargetAudience ;
        skos:prefLabel    "15"@en ;
        skos:definition   "Approval of the film for admittance of children from the age of\n         15"@en ;
        skos:broader      parentalguidance:_20 ;
        skos:inScheme     <http://www.ebu.ch/metadata/ontologies/skos/ebu_ParentalGuidanceCodeCS> ;
        skos:changeNote   "" ;
        skos:historyNote  "" ;
        skos:example      "" .

parentalguidance:_21  rdf:type  ebucore:TargetAudience ;
        skos:prefLabel    "DK-DR"@en ;
        skos:scopeNote    "Region:Denmark"@en ;
        skos:definition   "Denmark Radio"@en ;
        skos:inScheme     <http://www.ebu.ch/metadata/ontologies/skos/ebu_ParentalGuidanceCodeCS> ;
        skos:narrower     parentalguidance:_21.1 ;
        skos:narrower     parentalguidance:_21.2 ;
        skos:narrower     parentalguidance:_21.3 ;
        skos:changeNote   "Update Update" ;
        skos:historyNote  "2009-07-28 2009-07-28" ;
        skos:example      "" ;
        skos:note         "Valid" .

parentalguidance:_21.1
        rdf:type          ebucore:TargetAudience ;
        skos:prefLabel    "Green"@en ;
        skos:definition   "All ages"@en ;
        skos:broader      parentalguidance:_21 ;
        skos:inScheme     <http://www.ebu.ch/metadata/ontologies/skos/ebu_ParentalGuidanceCodeCS> ;
        skos:changeNote   "" ;
        skos:historyNote  "" ;
        skos:example      "" .

parentalguidance:_21.2
        rdf:type          ebucore:TargetAudience ;
        skos:prefLabel    "Yellow"@en ;
        skos:definition   "Adult supervision"@en ;
        skos:broader      parentalguidance:_21 ;
        skos:inScheme     <http://www.ebu.ch/metadata/ontologies/skos/ebu_ParentalGuidanceCodeCS> ;
        skos:changeNote   "" ;
        skos:historyNote  "" ;
        skos:example      "" .

parentalguidance:_21.3
        rdf:type          ebucore:TargetAudience ;
        skos:prefLabel    "Red"@en ;
        skos:definition   "Adult"@en ;
        skos:broader      parentalguidance:_21 ;
        skos:inScheme     <http://www.ebu.ch/metadata/ontologies/skos/ebu_ParentalGuidanceCodeCS> ;
        skos:changeNote   "" ;
        skos:historyNote  "" ;
        skos:example      "" .

parentalguidance:_22  rdf:type  ebucore:TargetAudience ;
        skos:prefLabel    "ES"@en ;
        skos:altLabel     "ES-ICAA"@en ;
        skos:altLabel     "Instiuto de la Cinematografía y de las Artes Audiovisuales (ICAA)"@es ;
        skos:scopeNote    "Region:Spain"@en ;
        skos:inScheme     <http://www.ebu.ch/metadata/ontologies/skos/ebu_ParentalGuidanceCodeCS> ;
        skos:narrower     parentalguidance:_22.1 ;
        skos:narrower     parentalguidance:_22.2 ;
        skos:narrower     parentalguidance:_22.3 ;
        skos:narrower     parentalguidance:_22.4 ;
        skos:narrower     parentalguidance:_22.5 ;
        skos:changeNote   "Update" ;
        skos:historyNote  "2009-07-28" ;
        skos:example      "" ;
        skos:note         "Valid" .

parentalguidance:_22.1
        rdf:type          ebucore:TargetAudience ;
        skos:prefLabel    "ERI"@en ;
        skos:definition   "Especial recomendado para la infancia"@es ;
        skos:definition   "Specially recommended for children under 7"@en ;
        skos:broader      parentalguidance:_22 ;
        skos:inScheme     <http://www.ebu.ch/metadata/ontologies/skos/ebu_ParentalGuidanceCodeCS> ;
        skos:changeNote   "" ;
        skos:historyNote  "" ;
        skos:example      "" .

parentalguidance:_22.2
        rdf:type          ebucore:TargetAudience ;
        skos:prefLabel    "TP"@en ;
        skos:definition   "Todos los publicos"@en ;
        skos:definition   "Suitable for the general public"@en ;
        skos:broader      parentalguidance:_22 ;
        skos:inScheme     <http://www.ebu.ch/metadata/ontologies/skos/ebu_ParentalGuidanceCodeCS> ;
        skos:changeNote   "" ;
        skos:historyNote  "" ;
        skos:example      "" .

parentalguidance:_22.3
        rdf:type          ebucore:TargetAudience ;
        skos:prefLabel    "7"@en ;
        skos:definition   "For 7 and older"@en ;
        skos:broader      parentalguidance:_22 ;
        skos:inScheme     <http://www.ebu.ch/metadata/ontologies/skos/ebu_ParentalGuidanceCodeCS> ;
        skos:changeNote   "" ;
        skos:historyNote  "" ;
        skos:example      "" .

parentalguidance:_22.4
        rdf:type          ebucore:TargetAudience ;
        skos:prefLabel    "13"@en ;
        skos:definition   "For 13 and older"@en ;
        skos:broader      parentalguidance:_22 ;
        skos:inScheme     <http://www.ebu.ch/metadata/ontologies/skos/ebu_ParentalGuidanceCodeCS> ;
        skos:changeNote   "" ;
        skos:historyNote  "" ;
        skos:example      "" .

parentalguidance:_22.5
        rdf:type          ebucore:TargetAudience ;
        skos:prefLabel    "18"@en ;
        skos:definition   "For 18 and older"@en ;
        skos:broader      parentalguidance:_22 ;
        skos:inScheme     <http://www.ebu.ch/metadata/ontologies/skos/ebu_ParentalGuidanceCodeCS> ;
        skos:changeNote   "" ;
        skos:historyNote  "" ;
        skos:example      "" .

parentalguidance:_23  rdf:type  ebucore:TargetAudience ;
        skos:prefLabel    "EU-PEGI"@en ;
        skos:scopeNote    "Region:Europe"@en ;
        skos:definition   "Pan European Game Information"@en ;
        skos:inScheme     <http://www.ebu.ch/metadata/ontologies/skos/ebu_ParentalGuidanceCodeCS> ;
        skos:narrower     parentalguidance:_23.1 ;
        skos:narrower     parentalguidance:_23.2 ;
        skos:changeNote   "Update" ;
        skos:historyNote  "2009-07-28" ;
        skos:example      "" ;
        skos:note         "Valid" .

parentalguidance:_23.1
        rdf:type          ebucore:TargetAudience ;
        skos:prefLabel    "Rating"@en ;
        skos:broader      parentalguidance:_23 ;
        skos:inScheme     <http://www.ebu.ch/metadata/ontologies/skos/ebu_ParentalGuidanceCodeCS> ;
        skos:narrower     parentalguidance:_23.1.1 ;
        skos:narrower     parentalguidance:_23.1.2 ;
        skos:narrower     parentalguidance:_23.1.3 ;
        skos:narrower     parentalguidance:_23.1.4 ;
        skos:narrower     parentalguidance:_23.1.5 ;
        skos:changeNote   "" ;
        skos:historyNote  "" ;
        skos:example      "" .

parentalguidance:_23.1.1
        rdf:type          ebucore:TargetAudience ;
        skos:prefLabel    "3+"@en ;
        skos:definition   "Suitable for ages 3 and over. Contains very mild violence or\n         suggestive themes."@en ;
        skos:broader      parentalguidance:_23.1 ;
        skos:inScheme     <http://www.ebu.ch/metadata/ontologies/skos/ebu_ParentalGuidanceCodeCS> ;
        skos:changeNote   "" ;
        skos:historyNote  "" ;
        skos:example      "" .

parentalguidance:_23.1.2
        rdf:type          ebucore:TargetAudience ;
        skos:prefLabel    "7+"@en ;
        skos:definition   "These games are the same as Early Childhood ratings but may\n         include content descriptors like mild violence and in a rare case, very mild action\n         violence."@en ;
        skos:broader      parentalguidance:_23.1 ;
        skos:inScheme     <http://www.ebu.ch/metadata/ontologies/skos/ebu_ParentalGuidanceCodeCS> ;
        skos:changeNote   "" ;
        skos:historyNote  "" ;
        skos:example      "" .

parentalguidance:_23.1.3
        rdf:type          ebucore:TargetAudience ;
        skos:prefLabel    "12+"@en ;
        skos:definition   "Suitable only for persons of over ages 12 and older. This\n         rating contains mild action violence or suggestive themes and mildly suggestive song\n         lyrics."@en ;
        skos:broader      parentalguidance:_23.1 ;
        skos:inScheme     <http://www.ebu.ch/metadata/ontologies/skos/ebu_ParentalGuidanceCodeCS> ;
        skos:changeNote   "" ;
        skos:historyNote  "" ;
        skos:example      "" .

parentalguidance:_23.1.4
        rdf:type          ebucore:TargetAudience ;
        skos:prefLabel    "16+"@en ;
        skos:definition   "This rating is suitable only for persons of 16 years of age or\n         older. Some situations include strong action violence, mild references to gambling, and\n         rude humor."@en ;
        skos:broader      parentalguidance:_23.1 ;
        skos:inScheme     <http://www.ebu.ch/metadata/ontologies/skos/ebu_ParentalGuidanceCodeCS> ;
        skos:changeNote   "" ;
        skos:historyNote  "" ;
        skos:example      "" .

parentalguidance:_23.1.5
        rdf:type          ebucore:TargetAudience ;
        skos:prefLabel    "18+"@en ;
        skos:definition   "This rating is suitable only for persons 18 years of age and\n         older with graphic violence, strong sexual content, explicit references to gambling, and\n         vulgar language (spoken and used in song lyrics)"@en ;
        skos:broader      parentalguidance:_23.1 ;
        skos:inScheme     <http://www.ebu.ch/metadata/ontologies/skos/ebu_ParentalGuidanceCodeCS> ;
        skos:changeNote   "" ;
        skos:historyNote  "" ;
        skos:example      "" .

parentalguidance:_23.2
        rdf:type          ebucore:TargetAudience ;
        skos:prefLabel    "Criteria"@en ;
        skos:broader      parentalguidance:_23 ;
        skos:inScheme     <http://www.ebu.ch/metadata/ontologies/skos/ebu_ParentalGuidanceCodeCS> ;
        skos:narrower     parentalguidance:_23.2.1 ;
        skos:narrower     parentalguidance:_23.2.2 ;
        skos:narrower     parentalguidance:_23.2.3 ;
        skos:narrower     parentalguidance:_23.2.4 ;
        skos:narrower     parentalguidance:_23.2.5 ;
        skos:narrower     parentalguidance:_23.2.6 ;
        skos:narrower     parentalguidance:_23.2.7 ;
        skos:changeNote   "" ;
        skos:historyNote  "" ;
        skos:example      "" .

parentalguidance:_23.2.1
        rdf:type          ebucore:TargetAudience ;
        skos:prefLabel    "Profanity"@en ;
        skos:broader      parentalguidance:_23.2 ;
        skos:inScheme     <http://www.ebu.ch/metadata/ontologies/skos/ebu_ParentalGuidanceCodeCS> ;
        skos:changeNote   "" ;
        skos:historyNote  "" ;
        skos:example      "" .

parentalguidance:_23.2.2
        rdf:type          ebucore:TargetAudience ;
        skos:prefLabel    "Discrimination"@en ;
        skos:broader      parentalguidance:_23.2 ;
        skos:inScheme     <http://www.ebu.ch/metadata/ontologies/skos/ebu_ParentalGuidanceCodeCS> ;
        skos:changeNote   "" ;
        skos:historyNote  "" ;
        skos:example      "" .

parentalguidance:_23.2.3
        rdf:type          ebucore:TargetAudience ;
        skos:prefLabel    "Drugs"@en ;
        skos:broader      parentalguidance:_23.2 ;
        skos:inScheme     <http://www.ebu.ch/metadata/ontologies/skos/ebu_ParentalGuidanceCodeCS> ;
        skos:changeNote   "" ;
        skos:historyNote  "" ;
        skos:example      "" .

parentalguidance:_23.2.4
        rdf:type          ebucore:TargetAudience ;
        skos:prefLabel    "Fear"@en ;
        skos:broader      parentalguidance:_23.2 ;
        skos:inScheme     <http://www.ebu.ch/metadata/ontologies/skos/ebu_ParentalGuidanceCodeCS> ;
        skos:changeNote   "" ;
        skos:historyNote  "" ;
        skos:example      "" .

parentalguidance:_23.2.5
        rdf:type          ebucore:TargetAudience ;
        skos:prefLabel    "Sex"@en ;
        skos:broader      parentalguidance:_23.2 ;
        skos:inScheme     <http://www.ebu.ch/metadata/ontologies/skos/ebu_ParentalGuidanceCodeCS> ;
        skos:changeNote   "" ;
        skos:historyNote  "" ;
        skos:example      "" .

parentalguidance:_23.2.6
        rdf:type          ebucore:TargetAudience ;
        skos:prefLabel    "Violence"@en ;
        skos:broader      parentalguidance:_23.2 ;
        skos:inScheme     <http://www.ebu.ch/metadata/ontologies/skos/ebu_ParentalGuidanceCodeCS> ;
        skos:changeNote   "" ;
        skos:historyNote  "" ;
        skos:example      "" .

parentalguidance:_23.2.7
        rdf:type          ebucore:TargetAudience ;
        skos:prefLabel    "Gambling"@en ;
        skos:broader      parentalguidance:_23.2 ;
        skos:inScheme     <http://www.ebu.ch/metadata/ontologies/skos/ebu_ParentalGuidanceCodeCS> ;
        skos:changeNote   "" ;
        skos:historyNote  "" ;
        skos:example      "" .

parentalguidance:_24  rdf:type  ebucore:TargetAudience ;
        skos:prefLabel    "FI-VET"@en ;
        skos:altLabel     "FI_MEKU"@en ;
        skos:altLabel     "Mediakasvatus- ja kuvaohjelmakeskus"@fi ; #https://en.wikipedia.org/wiki/Finnish_Board_of_Film_Classification
        skos:scopeNote    "Region:Finland"@fi ;
        skos:definition   "Valtion elokuvatarkastamo"@fi ;
        skos:definition   "Finnish Board of Film Classification"@en ;
        skos:inScheme     <http://www.ebu.ch/metadata/ontologies/skos/ebu_ParentalGuidanceCodeCS> ;
        skos:narrower     parentalguidance:_24.1 ;
        skos:narrower     parentalguidance:_24.2 ;
        skos:narrower     parentalguidance:_24.3 ;
        skos:narrower     parentalguidance:_24.4 ;
        skos:narrower     parentalguidance:_24.5 ;
        skos:narrower     parentalguidance:_24.6 ;
        skos:changeNote   "Update" ;
        skos:historyNote  "2009-07-28" ;
        skos:example      "" ;
        skos:note         "Valid" .

parentalguidance:_24.1
        rdf:type          ebucore:TargetAudience ;
        skos:prefLabel    "S"@en ;
        skos:definition   "For all ages"@en ;
        skos:broader      parentalguidance:_24 ;
        skos:inScheme     <http://www.ebu.ch/metadata/ontologies/skos/ebu_ParentalGuidanceCodeCS> ;
        skos:changeNote   "" ;
        skos:historyNote  "" ;
        skos:example      "" .

parentalguidance:_24.2
        rdf:type          ebucore:TargetAudience ;
        skos:prefLabel    "K-3"@en ;
        skos:definition   "For all ages"@en ;
        skos:broader      parentalguidance:_24 ;
        skos:inScheme     <http://www.ebu.ch/metadata/ontologies/skos/ebu_ParentalGuidanceCodeCS> ;
        skos:changeNote   "" ;
        skos:historyNote  "" ;
        skos:example      "" .

parentalguidance:_24.3
        rdf:type          ebucore:TargetAudience ;
        skos:prefLabel    "K-7"@en ;
        skos:definition   "For people aged 7 years and above"@en ;
        skos:broader      parentalguidance:_24 ;
        skos:inScheme     <http://www.ebu.ch/metadata/ontologies/skos/ebu_ParentalGuidanceCodeCS> ;
        skos:changeNote   "" ;
        skos:historyNote  "" ;
        skos:example      "" .


parentalguidance:_24.4
        rdf:type          ebucore:TargetAudience ;
        skos:prefLabel    "K-12"@en ;
        skos:definition   "For people aged 12 years and above"@en ;
        skos:broader      parentalguidance:_24 ;
        skos:inScheme     <http://www.ebu.ch/metadata/ontologies/skos/ebu_ParentalGuidanceCodeCS> ;
        skos:changeNote   "" ;
        skos:historyNote  "" ;
        skos:example      "" .

parentalguidance:_24.5
        rdf:type          ebucore:TargetAudience ;
        skos:prefLabel    "K-16"@en ;
        skos:definition   "For people aged 16 years and above"@en ;
        skos:broader      parentalguidance:_24 ;
        skos:inScheme     <http://www.ebu.ch/metadata/ontologies/skos/ebu_ParentalGuidanceCodeCS> ;
        skos:changeNote   "" ;
        skos:historyNote  "" ;
        skos:example      "" .

parentalguidance:_24.6
        rdf:type          ebucore:TargetAudience ;
        skos:prefLabel    "K-18"@en ;
        skos:definition   "For people aged 18 years and above"@en ;
        skos:broader      parentalguidance:_24 ;
        skos:inScheme     <http://www.ebu.ch/metadata/ontologies/skos/ebu_ParentalGuidanceCodeCS> ;
        skos:changeNote   "" ;
        skos:historyNote  "" ;
        skos:example      "" .


parentalguidance:_25  rdf:type  ebucore:TargetAudience ;
        skos:prefLabel    "FR-CNC"@en ;
        skos:altLabel     "Centre national du cinéma et de l'image animée"@fr ;
        skos:scopeNote    "Region:France" ;
        skos:definition   "Centre National de Cinematographie"@en ;
        skos:inScheme     <http://www.ebu.ch/metadata/ontologies/skos/ebu_ParentalGuidanceCodeCS> ;
        skos:narrower     parentalguidance:_25.1 ;
        skos:narrower     parentalguidance:_25.2 ;
        skos:narrower     parentalguidance:_25.3 ;
        skos:narrower     parentalguidance:_25.4 ;
        skos:narrower     parentalguidance:_25.5 ;
        skos:changeNote   "Update" ;
        skos:historyNote  "2009-07-28" ;
        skos:example      "" ;
        skos:note         "Valid" .

parentalguidance:_25.1
        rdf:type          ebucore:TargetAudience ;
        skos:prefLabel    "Tout public"@fr ;
        skos:prefLabel    "For all audiences"@en ;
        skos:definition   "For all audiences"@en ;
        skos:broader      parentalguidance:_25 ;
        skos:inScheme     <http://www.ebu.ch/metadata/ontologies/skos/ebu_ParentalGuidanceCodeCS> ;
        skos:changeNote   "" ;
        skos:historyNote  "" ;
        skos:example      "" .

parentalguidance:_25.2
        rdf:type          ebucore:TargetAudience ;
        skos:prefLabel    "-12"@en ;
        skos:definition   "Interdiction de représentation aux moins de douze\n         ans"@fr ;
        skos:definition   "Unsuitable for minors under 12"@en ;
        skos:broader      parentalguidance:_25 ;
        skos:inScheme     <http://www.ebu.ch/metadata/ontologies/skos/ebu_ParentalGuidanceCodeCS> ;
        skos:changeNote   "" ;
        skos:historyNote  "" ;
        skos:example      "" .

parentalguidance:_25.3
        rdf:type          ebucore:TargetAudience ;
        skos:prefLabel    "-16"@en ;
        skos:definition   "Interdiction de représentation aux moins de seize\n         ans"@fr ;
        skos:definition   "Unsuitable for minors under 16"@en ;
        skos:broader      parentalguidance:_25 ;
        skos:inScheme     <http://www.ebu.ch/metadata/ontologies/skos/ebu_ParentalGuidanceCodeCS> ;
        skos:changeNote   "" ;
        skos:historyNote  "" ;
        skos:example      "" .

parentalguidance:_25.4
        rdf:type          ebucore:TargetAudience ;
        skos:prefLabel    "-18"@en ;
        skos:definition   "Interdiction de représentation aux moins de dix-huit ans,\n         prévoit que cette restriction peut concerner les œuvres qui comportent « des scènes de sexe\n         non simulées ou de très grande violence mais qui, par la manière dont elles sont filmées et\n         la nature du thème traité ne justifient pas » d’un classement X"@fr ;
        skos:definition   "Unsuitable for minors under 18, may apply to works with\n         non-simulated sexual acts or extreme violence, but do not apply to X rating due to the\n         nature of the theme being treated or the way it has been filmed"@en ;
        skos:broader      parentalguidance:_25 ;
        skos:inScheme     <http://www.ebu.ch/metadata/ontologies/skos/ebu_ParentalGuidanceCodeCS> ;
        skos:changeNote   "" ;
        skos:historyNote  "" ;
        skos:example      "" .

parentalguidance:_25.5
        rdf:type          ebucore:TargetAudience ;
        skos:prefLabel    "X"@en ;
        skos:definition   "Programme pour adultes - Contenu de nature\n         pornographie"@fr ;
        skos:definition   "Adult only, pornographic content"@en ;
        skos:broader      parentalguidance:_25 ;
        skos:inScheme     <http://www.ebu.ch/metadata/ontologies/skos/ebu_ParentalGuidanceCodeCS> ;
        skos:changeNote   "" ;
        skos:historyNote  "" ;
        skos:example      "" .

parentalguidance:_26  rdf:type  ebucore:TargetAudience ;
        skos:prefLabel    "FR-CSA"@en ;
        skos:altLabel     "Conseil Superieur de l'Audiovisuel"@fr ;
        skos:scopeNote    "Region:France" ;
        skos:definition   "Conseil Superieur de l'Audiovisuel"@en ;
        skos:inScheme     <http://www.ebu.ch/metadata/ontologies/skos/ebu_ParentalGuidanceCodeCS> ;
        skos:narrower     parentalguidance:_26.1 ;
        skos:narrower     parentalguidance:_26.2 ;
        skos:narrower     parentalguidance:_26.3 ;
        skos:narrower     parentalguidance:_26.4 ;
        skos:narrower     parentalguidance:_26.5 ;
        skos:changeNote   "Update" ;
        skos:historyNote  "2009-07-28" ;
        skos:example      "" ;
        skos:note         "Valid" .

parentalguidance:_26.1
        rdf:type          ebucore:TargetAudience ;
        skos:prefLabel    "-10"@en ;
        skos:definition   "Pas pour les moins de dix ans"@fr ;
        skos:definition   "Not Recommended for children under 10"@en ;
        skos:broader      parentalguidance:_26 ;
        skos:inScheme     <http://www.ebu.ch/metadata/ontologies/skos/ebu_ParentalGuidanceCodeCS> ;
        skos:changeNote   "" ;
        skos:historyNote  "" ;
        skos:example      "" .

parentalguidance:_26.2
        rdf:type          ebucore:TargetAudience ;
        skos:prefLabel    "-12"@en ;
        skos:definition   "Pas pour les moins de douze ans"@fr ;
        skos:definition   "Not Recommended for children under 12"@en ;
        skos:broader      parentalguidance:_26 ;
        skos:inScheme     <http://www.ebu.ch/metadata/ontologies/skos/ebu_ParentalGuidanceCodeCS> ;
        skos:changeNote   "" ;
        skos:historyNote  "" ;
        skos:example      "" .

parentalguidance:_26.3
        rdf:type          ebucore:TargetAudience ;
        skos:prefLabel    "-16"@en ;
        skos:definition   "Pas pour les moins de seize ans"@fr ;
        skos:definition   "Not Recommended for children under 16"@en ;
        skos:broader      parentalguidance:_26 ;
        skos:inScheme     <http://www.ebu.ch/metadata/ontologies/skos/ebu_ParentalGuidanceCodeCS> ;
        skos:changeNote   "" ;
        skos:historyNote  "" ;
        skos:example      "" .

parentalguidance:_26.4
        rdf:type          ebucore:TargetAudience ;
        skos:prefLabel    "-18"@en ;
        skos:definition   "Pas pour les moins de dix-huit ans, prévoit que cette\n         restriction peut concerner les œuvres qui comportent « des scènes de sexe non simulées ou\n         de très grande violence mais qui, par la manière dont elles sont filmées et la nature du\n         thème traité ne justifient pas » d’un classement X"@fr ;
        skos:definition   "Unsuitable for minors under 18, may apply to works with\n         non-simulated sexual acts or extreme violence, but do not apply to X rating due to the\n         nature of the theme being treated or the way it has been filmed"@en ;
        skos:broader      parentalguidance:_26 ;
        skos:inScheme     <http://www.ebu.ch/metadata/ontologies/skos/ebu_ParentalGuidanceCodeCS> ;
        skos:changeNote   "" ;
        skos:historyNote  "" ;
        skos:example      "" .

parentalguidance:_26.5
        rdf:type          ebucore:TargetAudience ;
        skos:prefLabel    "X"@en ;
        skos:definition   "Adulte - Contenu de nature pornographie"@fr ;
        skos:definition   "Adult, pornographic content"@en ;
        skos:broader      parentalguidance:_26 ;
        skos:inScheme     <http://www.ebu.ch/metadata/ontologies/skos/ebu_ParentalGuidanceCodeCS> ;
        skos:changeNote   "" ;
        skos:historyNote  "" ;
        skos:example      "" .

parentalguidance:_27  rdf:type  ebucore:TargetAudience ;
        skos:prefLabel    "GB-BBFC"@en ;
        skos:altLabel     "British Board of Film Classification"@en ;
        skos:altLabel     "UK Content Provider"@en ;
        skos:altLabel     "www.bbfc.co.uk"@en ;
        skos:scopeNote    "Region:Britain" ;
        skos:definition   "British Board of Film Classification"@en ;
        skos:inScheme     <http://www.ebu.ch/metadata/ontologies/skos/ebu_ParentalGuidanceCodeCS> ;
        skos:narrower     parentalguidance:_27.1 ;
        skos:narrower     parentalguidance:_27.2 ;
        skos:narrower     parentalguidance:_27.3 ;
        skos:narrower     parentalguidance:_27.4 ;
        skos:narrower     parentalguidance:_27.5 ;
        skos:narrower     parentalguidance:_27.6 ;
        skos:changeNote   "Update" ;
        skos:historyNote  "2009-07-28" ;
        skos:example      "" ;
        skos:note         "Valid" .

parentalguidance:_27.1
        rdf:type          ebucore:TargetAudience ;
        skos:prefLabel    "U"@en ;
        skos:definition   "Suitable for all"@en ;
        skos:broader      parentalguidance:_27 ;
        skos:inScheme     <http://www.ebu.ch/metadata/ontologies/skos/ebu_ParentalGuidanceCodeCS> ;
        skos:changeNote   "" ;
        skos:historyNote  "" ;
        skos:example      "" .

parentalguidance:_27.2
        rdf:type          ebucore:TargetAudience ;
        skos:prefLabel    "PG"@en ;
        skos:definition   "General viewing but some scenes may be unsuitable for young\n         children"@en ;
        skos:broader      parentalguidance:_27 ;
        skos:inScheme     <http://www.ebu.ch/metadata/ontologies/skos/ebu_ParentalGuidanceCodeCS> ;
        skos:changeNote   "" ;
        skos:historyNote  "" ;
        skos:example      "" .

parentalguidance:_27.3
        rdf:type          ebucore:TargetAudience ;
        skos:prefLabel    "12A/12"@en ;
        skos:definition   "Suitable for 12 years and older. No 12 year old child may see a\n         12A film without the presence of an accompanying adult."@en ;
        skos:broader      parentalguidance:_27 ;
        skos:inScheme     <http://www.ebu.ch/metadata/ontologies/skos/ebu_ParentalGuidanceCodeCS> ;
        skos:changeNote   "" ;
        skos:historyNote  "" ;
        skos:example      "" ;
        skos:hiddenLabel  "12"@en .

parentalguidance:_27.4
        rdf:type          ebucore:TargetAudience ;
        skos:prefLabel    "15"@en ;
        skos:definition   "No one under 15 years of age may see a \"15\" film or rent or buy\n         a \"15\" video"@en ;
        skos:broader      parentalguidance:_27 ;
        skos:inScheme     <http://www.ebu.ch/metadata/ontologies/skos/ebu_ParentalGuidanceCodeCS> ;
        skos:changeNote   "" ;
        skos:historyNote  "" ;
        skos:example      "" .

parentalguidance:_27.5
        rdf:type          ebucore:TargetAudience ;
        skos:prefLabel    "18"@en ;
        skos:definition   "Suitable only for adults"@en ;
        skos:broader      parentalguidance:_27 ;
        skos:inScheme     <http://www.ebu.ch/metadata/ontologies/skos/ebu_ParentalGuidanceCodeCS> ;
        skos:changeNote   "" ;
        skos:historyNote  "" ;
        skos:example      "" .

parentalguidance:_27.6
        rdf:type          ebucore:TargetAudience ;
        skos:prefLabel    "R18"@en ;
        skos:definition   "To be supplied only in licensed sex shops or cinemas to adults\n         of not less than 18 years of age"@en ;
        skos:broader      parentalguidance:_27 ;
        skos:inScheme     <http://www.ebu.ch/metadata/ontologies/skos/ebu_ParentalGuidanceCodeCS> ;
        skos:changeNote   "" ;
        skos:historyNote  "" ;
        skos:example      "" .

parentalguidance:_28  rdf:type  ebucore:TargetAudience ;
        skos:prefLabel    "IE-IFCO"@en ;
        skos:altLabel    "Irish Film Classification Office"@en ;
        skos:scopeNote    "Region:Ireland"@en ;
        skos:definition   "Irish Film Classification Office"@en ;
        skos:inScheme     <http://www.ebu.ch/metadata/ontologies/skos/ebu_ParentalGuidanceCodeCS> ;
        skos:narrower     parentalguidance:_28.1 ;
        skos:narrower     parentalguidance:_28.2 ;
        skos:narrower     parentalguidance:_28.3 ;
        skos:narrower     parentalguidance:_28.4 ;
        skos:narrower     parentalguidance:_28.5 ;
        skos:narrower     parentalguidance:_28.6 ;
        skos:changeNote   "Update" ;
        skos:historyNote  "2009-07-28" ;
        skos:example      "" ;
        skos:note         "Valid" .

parentalguidance:_28.1
        rdf:type          ebucore:TargetAudience ;
        skos:prefLabel    "G"@en ;
        skos:definition   "'A film classified as 'General' should be suitable for children\n         of school going age."@en ;
        skos:broader      parentalguidance:_28 ;
        skos:inScheme     <http://www.ebu.ch/metadata/ontologies/skos/ebu_ParentalGuidanceCodeCS> ;
        skos:changeNote   "" ;
        skos:historyNote  "" ;
        skos:example      "" .

parentalguidance:_28.2
        rdf:type          ebucore:TargetAudience ;
        skos:prefLabel    "PG"@en ;
        skos:definition   "A film with a 'PG' cert may be watched by unaccompanied\n         children of any age."@en ;
        skos:broader      parentalguidance:_28 ;
        skos:inScheme     <http://www.ebu.ch/metadata/ontologies/skos/ebu_ParentalGuidanceCodeCS> ;
        skos:changeNote   "" ;
        skos:historyNote  "" ;
        skos:example      "" .

parentalguidance:_28.3
        rdf:type          ebucore:TargetAudience ;
        skos:prefLabel    "12A"@en ;
        skos:definition   "Films classified in this category are considered to be suitable\n         for those of twelve and upwards. They may also be seen by younger children provided a\n         parent or adult guardian accompanies them."@en ;
        skos:broader      parentalguidance:_28 ;
        skos:inScheme     <http://www.ebu.ch/metadata/ontologies/skos/ebu_ParentalGuidanceCodeCS> ;
        skos:changeNote   "" ;
        skos:historyNote  "" ;
        skos:example      "" .

parentalguidance:_28.4
        rdf:type          ebucore:TargetAudience ;
        skos:prefLabel    "15A"@en ;
        skos:definition   "Films classified in this category are considered to be suitable\n         for those of fifteen and upwards. They may also be seen by younger children provided a\n         parent or adult guardian accompanies them."@en ;
        skos:broader      parentalguidance:_28 ;
        skos:inScheme     <http://www.ebu.ch/metadata/ontologies/skos/ebu_ParentalGuidanceCodeCS> ;
        skos:changeNote   "" ;
        skos:historyNote  "" ;
        skos:example      "" .

parentalguidance:_28.5
        rdf:type          ebucore:TargetAudience ;
        skos:prefLabel    "16"@en ;
        skos:definition   "Films classified in this category are considered to be suitable\n         for persons of sixteen or over. Children under this age cannot be admitted to\n         cinemas."@en ;
        skos:broader      parentalguidance:_28 ;
        skos:inScheme     <http://www.ebu.ch/metadata/ontologies/skos/ebu_ParentalGuidanceCodeCS> ;
        skos:changeNote   "" ;
        skos:historyNote  "" ;
        skos:example      "" .

parentalguidance:_28.6
        rdf:type          ebucore:TargetAudience ;
        skos:prefLabel    "18"@en ;
        skos:definition   "Adults only"@en ;
        skos:broader      parentalguidance:_28 ;
        skos:inScheme     <http://www.ebu.ch/metadata/ontologies/skos/ebu_ParentalGuidanceCodeCS> ;
        skos:changeNote   "" ;
        skos:historyNote  "" ;
        skos:example      "" .

parentalguidance:_29  rdf:type  ebucore:TargetAudience ;
        skos:prefLabel    "IE-RTE"@en ;
        skos:scopeNote    "Region:Ireland"@en ;
        skos:definition   "Irish Film Classification Office"@en ;
        skos:inScheme     <http://www.ebu.ch/metadata/ontologies/skos/ebu_ParentalGuidanceCodeCS> ;
        skos:narrower     parentalguidance:_29.1 ;
        skos:narrower     parentalguidance:_29.2 ;
        skos:narrower     parentalguidance:_29.3 ;
        skos:narrower     parentalguidance:_29.4 ;
        skos:narrower     parentalguidance:_29.5 ;
        skos:changeNote   "Update" ;
        skos:historyNote  "2009-07-28" ;
        skos:example      "" ;
        skos:note         "Valid" .

parentalguidance:_29.1
        rdf:type          ebucore:TargetAudience ;
        skos:prefLabel    "GA"@en ;
        skos:altLabel     "General Audience"@en ;
        skos:prefLabel    "Lucht Féachana Ginearálta"@ga ;
        skos:definition   "A programme that would be acceptable to all ages and\n         tastes."@en ;
        skos:broader      parentalguidance:_29 ;
        skos:inScheme     <http://www.ebu.ch/metadata/ontologies/skos/ebu_ParentalGuidanceCodeCS> ;
        skos:changeNote   "" ;
        skos:historyNote  "" ;
        skos:example      "" .

parentalguidance:_29.2
        rdf:type          ebucore:TargetAudience ;
        skos:prefLabel    "CH"@en ;
        skos:altLabel     "Children"@en ;
        skos:prefLabel    "Páistí"@ga ;
        skos:definition   "a programme aimed specifically at children ages 5–10. May\n         contain mild cartoon or fantasy violence."@en ;
        skos:broader      parentalguidance:_29 ;
        skos:inScheme     <http://www.ebu.ch/metadata/ontologies/skos/ebu_ParentalGuidanceCodeCS> ;
        skos:changeNote   "" ;
        skos:historyNote  "" ;
        skos:example      "" .

parentalguidance:_29.3
        rdf:type          ebucore:TargetAudience ;
        skos:prefLabel    "YA"@en ;
        skos:altLabel     "Young Adult"@en ;
        skos:prefLabel    "Ógra"@ga ;
        skos:definition   "a programme aimed at an adolescent audience. That is to say it\n         would not be of great interest to an adult. However, it might deal with issues which affect\n         the teenage and late preteen audience, e.g. relationships, sexual activity, sexuality, soft\n         drugs. Parents and guardians could expect that \"YA\" programmes might contain such material\n         and may choose to limit their children's access."@en ;
        skos:broader      parentalguidance:_29 ;
        skos:inScheme     <http://www.ebu.ch/metadata/ontologies/skos/ebu_ParentalGuidanceCodeCS> ;
        skos:changeNote   "" ;
        skos:historyNote  "" ;
        skos:example      "" .

parentalguidance:_29.4
        rdf:type          ebucore:TargetAudience ;
        skos:prefLabel    "PS"@en ;
        skos:altLabel     "Parental Supervision"@en ;
        skos:prefLabel    "Treoir Tuismitheora"@ga ;
        skos:definition   "a programme aimed at a mature audience (i.e. It might deal with\n         adult themes, be moderately violent, frightening or contain an occasional swear word.) and\n         the classification label invites parents or guardians to consider restricting children's\n         access."@en ;
        skos:broader      parentalguidance:_29 ;
        skos:inScheme     <http://www.ebu.ch/metadata/ontologies/skos/ebu_ParentalGuidanceCodeCS> ;
        skos:changeNote   "" ;
        skos:historyNote  "" ;
        skos:example      "" .

parentalguidance:_29.5
        rdf:type          ebucore:TargetAudience ;
        skos:prefLabel    "MA"@en ;
        skos:altLabel     "Mature Audience"@en ;
        skos:prefLabel    "Lucht Féachana Lánfhásta Amháin"@ga ;
        skos:definition   "a typical \"post-watershed\" program which might contain scenes\n         of strong sexual activity and heavy violence, or the dialogue might be\n         profane."@en ;
        skos:broader      parentalguidance:_29 ;
        skos:inScheme     <http://www.ebu.ch/metadata/ontologies/skos/ebu_ParentalGuidanceCodeCS> ;
        skos:changeNote   "" ;
        skos:historyNote  "" ;
        skos:example      "" .

parentalguidance:_30  rdf:type  ebucore:TargetAudience ;
        skos:prefLabel    "IT-RAI"@en ;
        skos:scopeNote    "Region:Italy"@en ;
        skos:definition   "Rating used by Radio Televisione Italiana"@en ;
        skos:inScheme     <http://www.ebu.ch/metadata/ontologies/skos/ebu_ParentalGuidanceCodeCS> ;
        skos:narrower     parentalguidance:_30.1 ;
        skos:narrower     parentalguidance:_30.2 ;
        skos:narrower     parentalguidance:_30.3 ;
        skos:changeNote   "Update" ;
        skos:historyNote  "2009-07-27" ;
        skos:example      "" ;
        skos:note         "Valid" .

parentalguidance:_30.1
        rdf:type          ebucore:TargetAudience ;
        skos:prefLabel    "Green"@en ;
        skos:definition   "All audiences allowed"@en ;
        skos:broader      parentalguidance:_30 ;
        skos:inScheme     <http://www.ebu.ch/metadata/ontologies/skos/ebu_ParentalGuidanceCodeCS> ;
        skos:changeNote   "" ;
        skos:historyNote  "" ;
        skos:example      "" .

parentalguidance:_30.2
        rdf:type          ebucore:TargetAudience ;
        skos:prefLabel    "Yellow"@en ;
        skos:definition   "Children allowed, but parental guidance is strongly\n         advised."@en ;
        skos:broader      parentalguidance:_30 ;
        skos:inScheme     <http://www.ebu.ch/metadata/ontologies/skos/ebu_ParentalGuidanceCodeCS> ;
        skos:changeNote   "" ;
        skos:historyNote  "" ;
        skos:example      "" .

parentalguidance:_30.3
        rdf:type          ebucore:TargetAudience ;
        skos:prefLabel    "Red"@en ;
        skos:definition   "adults only."@en ;
        skos:broader      parentalguidance:_30 ;
        skos:inScheme     <http://www.ebu.ch/metadata/ontologies/skos/ebu_ParentalGuidanceCodeCS> ;
        skos:narrower     parentalguidance:_30.3.1 ;
        skos:changeNote   "" ;
        skos:historyNote  "" ;
        skos:example      "" .

parentalguidance:_30.3.1
        rdf:type          ebucore:TargetAudience ;
        skos:prefLabel    "VM14"@en ;
        skos:definition   "No one under the age of 14 admitted"@en ;
        skos:broader      parentalguidance:_30.3 ;
        skos:inScheme     <http://www.ebu.ch/metadata/ontologies/skos/ebu_ParentalGuidanceCodeCS> ;
        skos:changeNote   "" ;
        skos:historyNote  "" ;
        skos:example      "" .

parentalguidance:_31  rdf:type  ebucore:TargetAudience ;
        skos:prefLabel    "JA-CERO"@en ;
        skos:scopeNote    "Region:Japan"@en ;
        skos:definition   "Computer Entertainment Rating Organization"@en ;
        skos:definition   "Tokutei Hieiri Katsudō Hōjin Konpyūta Entāteinmento Rētingu\n         Kikō - 特定非営利活動法人 コンピュータエンターテインメントレーティング機構"@ja ;
        skos:inScheme     <http://www.ebu.ch/metadata/ontologies/skos/ebu_ParentalGuidanceCodeCS> ;
        skos:narrower     parentalguidance:_31.1 ;
        skos:narrower     parentalguidance:_31.2 ;
        skos:changeNote   "Update" ;
        skos:historyNote  "2009-07-27" ;
        skos:example      "" ;
        skos:note         "Valid" .

parentalguidance:_31.1
        rdf:type          ebucore:TargetAudience ;
        skos:prefLabel    "Rating"@en ;
        skos:prefLabel    "レーティングマーク"@ja ;
        skos:broader      parentalguidance:_31 ;
        skos:inScheme     <http://www.ebu.ch/metadata/ontologies/skos/ebu_ParentalGuidanceCodeCS> ;
        skos:narrower     parentalguidance:_31.1.1 ;
        skos:narrower     parentalguidance:_31.1.2 ;
        skos:narrower     parentalguidance:_31.1.3 ;
        skos:narrower     parentalguidance:_31.1.4 ;
        skos:narrower     parentalguidance:_31.1.5 ;
        skos:changeNote   "" ;
        skos:historyNote  "" ;
        skos:example      "" .

parentalguidance:_31.1.1
        rdf:type          ebucore:TargetAudience ;
        skos:prefLabel    "A"@en ;
        skos:prefLabel    "黒"@ja ;
        skos:altLabel     "Black"@en ;
        skos:definition   ""@ja ;
        skos:definition   "All ages"@en ;
        skos:broader      parentalguidance:_31.1 ;
        skos:inScheme     <http://www.ebu.ch/metadata/ontologies/skos/ebu_ParentalGuidanceCodeCS> ;
        skos:changeNote   "" ;
        skos:historyNote  "" ;
        skos:example      "" .

parentalguidance:_31.1.2
        rdf:type          ebucore:TargetAudience ;
        skos:prefLabel    "B"@en ;
        skos:prefLabel    "緑"@ja ;
        skos:prefLabel    "Green"@en ;
        skos:definition   "12歳以上のみ"@ja ;
        skos:definition   "12 and over"@en ;
        skos:broader      parentalguidance:_31.1 ;
        skos:inScheme     <http://www.ebu.ch/metadata/ontologies/skos/ebu_ParentalGuidanceCodeCS> ;
        skos:changeNote   "" ;
        skos:historyNote  "" ;
        skos:example      "" .

parentalguidance:_31.1.3
        rdf:type          ebucore:TargetAudience ;
        skos:prefLabel    "C"@en ;
        skos:prefLabel    "青"@ja ;
        skos:altLabel     "Blue"@en ;
        skos:definition   "15歳以上のみ"@ja ;
        skos:definition   "15 and over"@en ;
        skos:broader      parentalguidance:_31.1 ;
        skos:inScheme     <http://www.ebu.ch/metadata/ontologies/skos/ebu_ParentalGuidanceCodeCS> ;
        skos:changeNote   "" ;
        skos:historyNote  "" ;
        skos:example      "" .

parentalguidance:_31.1.4
        rdf:type          ebucore:TargetAudience ;
        skos:prefLabel    "D"@en ;
        skos:prefLabel     "橙"@ja ;
        skos:altLabel     "Orange"@en ;
        skos:definition   "17歳以上のみ"@ja ;
        skos:definition   "17 and over"@en ;
        skos:broader      parentalguidance:_31.1 ;
        skos:inScheme     <http://www.ebu.ch/metadata/ontologies/skos/ebu_ParentalGuidanceCodeCS> ;
        skos:changeNote   "" ;
        skos:historyNote  "" ;
        skos:example      "" .

parentalguidance:_31.1.5
        rdf:type          ebucore:TargetAudience ;
        skos:prefLabel    "Z"@en ;
        skos:prefLabel    "赤"@ja ;
        skos:altLabel    "Red"@en ;
        skos:definition   "18歳以上のみ"@ja ;
        skos:definition   "18 and over"@en ;
        skos:broader      parentalguidance:_31.1 ;
        skos:inScheme     <http://www.ebu.ch/metadata/ontologies/skos/ebu_ParentalGuidanceCodeCS> ;
        skos:changeNote   "" ;
        skos:historyNote  "" ;
        skos:example      "" .

parentalguidance:_31.2
        rdf:type          ebucore:TargetAudience ;
        skos:prefLabel    "Criteria"@en ;
        skos:prefLabel    "コンテンツアイコン"@ja ;
        skos:broader      parentalguidance:_31 ;
        skos:inScheme     <http://www.ebu.ch/metadata/ontologies/skos/ebu_ParentalGuidanceCodeCS> ;
        skos:narrower     parentalguidance:_31.2.1 ;
        skos:narrower     parentalguidance:_31.2.2 ;
        skos:narrower     parentalguidance:_31.2.3 ;
        skos:narrower     parentalguidance:_31.2.4 ;
        skos:narrower     parentalguidance:_31.2.5 ;
        skos:narrower     parentalguidance:_31.2.6 ;
        skos:narrower     parentalguidance:_31.2.7 ;
        skos:narrower     parentalguidance:_31.2.8 ;
        skos:narrower     parentalguidance:_31.2.9 ;
        skos:changeNote   "" ;
        skos:historyNote  "" ;
        skos:example      "" .

parentalguidance:_31.2.1
        rdf:type          ebucore:TargetAudience ;
        skos:prefLabel    "恋愛"@ja ;
        skos:prefLabel    "Love"@en ;
        skos:broader      parentalguidance:_31.2 ;
        skos:inScheme     <http://www.ebu.ch/metadata/ontologies/skos/ebu_ParentalGuidanceCodeCS> ;
        skos:changeNote   "" ;
        skos:historyNote  "" ;
        skos:example      "" .

parentalguidance:_31.2.2
        rdf:type          ebucore:TargetAudience ;
        skos:prefLabel    "セクシャル"@ja ;
        skos:prefLabel    "Sex"@en ;
        skos:broader      parentalguidance:_31.2 ;
        skos:inScheme     <http://www.ebu.ch/metadata/ontologies/skos/ebu_ParentalGuidanceCodeCS> ;
        skos:changeNote   "" ;
        skos:historyNote  "" ;
        skos:example      "" .

parentalguidance:_31.2.3
        rdf:type          ebucore:TargetAudience ;
        skos:prefLabel    "暴力"@ja ;
        skos:prefLabel    "Violence"@en ;
        skos:broader      parentalguidance:_31.2 ;
        skos:inScheme     <http://www.ebu.ch/metadata/ontologies/skos/ebu_ParentalGuidanceCodeCS> ;
        skos:changeNote   "" ;
        skos:historyNote  "" ;
        skos:example      "" .

parentalguidance:_31.2.4
        rdf:type          ebucore:TargetAudience ;
        skos:prefLabel    "恐怖"@ja ;
        skos:prefLabel    "Surnatural"@en ;
        skos:broader      parentalguidance:_31.2 ;
        skos:inScheme     <http://www.ebu.ch/metadata/ontologies/skos/ebu_ParentalGuidanceCodeCS> ;
        skos:changeNote   "" ;
        skos:historyNote  "" ;
        skos:example      "" .

parentalguidance:_31.2.5
        rdf:type          ebucore:TargetAudience ;
        skos:prefLabel    "飲酒・喫煙"@ja ;
        skos:prefLabel    "Alcohol & Tobacco"@en ;
        skos:broader      parentalguidance:_31.2 ;
        skos:inScheme     <http://www.ebu.ch/metadata/ontologies/skos/ebu_ParentalGuidanceCodeCS> ;
        skos:changeNote   "" ;
        skos:historyNote  "" ;
        skos:example      "" .

parentalguidance:_31.2.6
        rdf:type          ebucore:TargetAudience ;
        skos:prefLabel    "ギャンブル"@ja ;
        skos:prefLabel    "Gambling"@en ;
        skos:broader      parentalguidance:_31.2 ;
        skos:inScheme     <http://www.ebu.ch/metadata/ontologies/skos/ebu_ParentalGuidanceCodeCS> ;
        skos:changeNote   "" ;
        skos:historyNote  "" ;
        skos:example      "" .

parentalguidance:_31.2.7
        rdf:type          ebucore:TargetAudience ;
        skos:prefLabel    "犯罪"@ja ;
        skos:prefLabel    "Murder"@en ;
        skos:broader      parentalguidance:_31.2 ;
        skos:inScheme     <http://www.ebu.ch/metadata/ontologies/skos/ebu_ParentalGuidanceCodeCS> ;
        skos:changeNote   "" ;
        skos:historyNote  "" ;
        skos:example      "" .

parentalguidance:_31.2.8
        rdf:type          ebucore:TargetAudience ;
        skos:prefLabel    "麻薬"@ja ;
        skos:prefLabel    "Drugs"@en ;
        skos:broader      parentalguidance:_31.2 ;
        skos:inScheme     <http://www.ebu.ch/metadata/ontologies/skos/ebu_ParentalGuidanceCodeCS> ;
        skos:changeNote   "" ;
        skos:historyNote  "" ;
        skos:example      "" .

parentalguidance:_31.2.9
        rdf:type          ebucore:TargetAudience ;
        skos:prefLabel    "言葉・その他"@ja ;
        skos:prefLabel    "Strong vocabulary"@en ;
        skos:broader      parentalguidance:_31.2 ;
        skos:inScheme     <http://www.ebu.ch/metadata/ontologies/skos/ebu_ParentalGuidanceCodeCS> ;
        skos:changeNote   "" ;
        skos:historyNote  "" ;
        skos:example      "" .

parentalguidance:_32  rdf:type  ebucore:TargetAudience ;
        skos:prefLabel    "KR-KBS"@en ;
        skos:scopeNote    "Region:South Korea"@en ;
        skos:definition   "Scheme as defined by the Korea Broadcasting\n         Station"@en ;
        skos:inScheme     <http://www.ebu.ch/metadata/ontologies/skos/ebu_ParentalGuidanceCodeCS> ;
        skos:narrower     parentalguidance:_32.1 ;
        skos:narrower     parentalguidance:_32.2 ;
        skos:narrower     parentalguidance:_32.3 ;
        skos:narrower     parentalguidance:_32.4 ;
        skos:narrower     parentalguidance:_32.5 ;
        skos:changeNote   "" ;
        skos:historyNote  "" ;
        skos:example      "" .

parentalguidance:_32.1
        rdf:type          ebucore:TargetAudience ;
        skos:prefLabel    "All"@en ;
        skos:definition   "Suitable for all ages"@en ;
        skos:broader      parentalguidance:_32 ;
        skos:inScheme     <http://www.ebu.ch/metadata/ontologies/skos/ebu_ParentalGuidanceCodeCS> ;
        skos:changeNote   "" ;
        skos:historyNote  "" ;
        skos:example      "" .

parentalguidance:_32.2
        rdf:type          ebucore:TargetAudience ;
        skos:prefLabel    "7"@en ;
        skos:definition   "This rating is for programming that may contain material\n         inappropriate for children younger than 7, and parental discretion should be\n         used."@en ;
        skos:broader      parentalguidance:_32 ;
        skos:inScheme     <http://www.ebu.ch/metadata/ontologies/skos/ebu_ParentalGuidanceCodeCS> ;
        skos:changeNote   "" ;
        skos:historyNote  "" ;
        skos:example      "" .

parentalguidance:_32.3
        rdf:type          ebucore:TargetAudience ;
        skos:prefLabel    "12"@en ;
        skos:definition   "This rating is for programs that may contain material\n         inappropriate for those younger than 12, and parental discretion should be used. Usually\n         used for animations that have stronger themes or violence then those designed for\n         childrens, or for reality variety programs that have mild violence, theme, or\n         language."@en ;
        skos:broader      parentalguidance:_32 ;
        skos:inScheme     <http://www.ebu.ch/metadata/ontologies/skos/ebu_ParentalGuidanceCodeCS> ;
        skos:changeNote   "" ;
        skos:historyNote  "" ;
        skos:example      "" .

parentalguidance:_32.4
        rdf:type          ebucore:TargetAudience ;
        skos:prefLabel    "15"@en ;
        skos:definition   "This rating is for programs that contain material that may be\n         inappropriate for children under 15, and that parental discretion should be\n         used."@en ;
        skos:broader      parentalguidance:_32 ;
        skos:inScheme     <http://www.ebu.ch/metadata/ontologies/skos/ebu_ParentalGuidanceCodeCS> ;
        skos:changeNote   "" ;
        skos:historyNote  "" ;
        skos:example      "" .

parentalguidance:_32.5
        rdf:type          ebucore:TargetAudience ;
        skos:prefLabel    "19"@en ;
        skos:definition   "This rating is for programs that are not recommended to those\n         younger than 19."@en ;
        skos:broader      parentalguidance:_32 ;
        skos:inScheme     <http://www.ebu.ch/metadata/ontologies/skos/ebu_ParentalGuidanceCodeCS> ;
        skos:changeNote   "" ;
        skos:historyNote  "" ;
        skos:example      "" .

parentalguidance:_33  rdf:type  ebucore:TargetAudience ;
        skos:prefLabel    "KR-KMRB"@en ;
        skos:scopeNote    "Region:South Korea"@en ;
        skos:definition   "Scheme as defined by the Korea Media Rating\n         Board"@en ;
        skos:inScheme     <http://www.ebu.ch/metadata/ontologies/skos/ebu_ParentalGuidanceCodeCS> ;
        skos:narrower     parentalguidance:_33.1 ;
        skos:narrower     parentalguidance:_33.2 ;
        skos:narrower     parentalguidance:_33.3 ;
        skos:narrower     parentalguidance:_33.4 ;
        skos:narrower     parentalguidance:_33.5 ;
        skos:changeNote   "" ;
        skos:historyNote  "" ;
        skos:example      "" .

parentalguidance:_33.1
        rdf:type          ebucore:TargetAudience ;
        skos:prefLabel    "All"@en ;
        skos:definition   "Suitable for all ages"@en ;
        skos:broader      parentalguidance:_33 ;
        skos:inScheme     <http://www.ebu.ch/metadata/ontologies/skos/ebu_ParentalGuidanceCodeCS> ;
        skos:changeNote   "" ;
        skos:historyNote  "" ;
        skos:example      "" .

parentalguidance:_33.2
        rdf:type          ebucore:TargetAudience ;
        skos:prefLabel    "12+"@en ;
        skos:definition   "Suitable for those aged 12 and over"@en ;
        skos:broader      parentalguidance:_33 ;
        skos:inScheme     <http://www.ebu.ch/metadata/ontologies/skos/ebu_ParentalGuidanceCodeCS> ;
        skos:changeNote   "" ;
        skos:historyNote  "" ;
        skos:example      "" .

parentalguidance:_33.3
        rdf:type          ebucore:TargetAudience ;
        skos:prefLabel    "15+"@en ;
        skos:definition   "Suitable for those aged 15 and over"@en ;
        skos:broader      parentalguidance:_33 ;
        skos:inScheme     <http://www.ebu.ch/metadata/ontologies/skos/ebu_ParentalGuidanceCodeCS> ;
        skos:changeNote   "" ;
        skos:historyNote  "" ;
        skos:example      "" .

parentalguidance:_33.4
        rdf:type          ebucore:TargetAudience ;
        skos:prefLabel    "Teenager Restricted"@en ;
        skos:definition   "Unsuitable for those aged under 18"@en ;
        skos:broader      parentalguidance:_33 ;
        skos:inScheme     <http://www.ebu.ch/metadata/ontologies/skos/ebu_ParentalGuidanceCodeCS> ;
        skos:changeNote   "" ;
        skos:historyNote  "" ;
        skos:example      "" .

parentalguidance:_33.5
        rdf:type          ebucore:TargetAudience ;
        skos:prefLabel    "Restricted"@en ;
        skos:definition   "Suitable for those aged 18 and over"@en ;
        skos:broader      parentalguidance:_33 ;
        skos:inScheme     <http://www.ebu.ch/metadata/ontologies/skos/ebu_ParentalGuidanceCodeCS> ;
        skos:changeNote   "" ;
        skos:historyNote  "" ;
        skos:example      "" .

parentalguidance:_34  rdf:type  ebucore:TargetAudience ;
        skos:prefLabel    "MV-NBC"@en ;
        skos:scopeNote    "Region:Maldives"@en ;
        skos:definition   "National Bureau of Classification"@en ;
        skos:inScheme     <http://www.ebu.ch/metadata/ontologies/skos/ebu_ParentalGuidanceCodeCS> ;
        skos:narrower     parentalguidance:_34.1 ;
        skos:narrower     parentalguidance:_34.2 ;
        skos:changeNote   "Update" ;
        skos:historyNote  "2009-07-28" ;
        skos:example      "" ;
        skos:note         "Valid" .

parentalguidance:_34.1
        rdf:type          ebucore:TargetAudience ;
        skos:prefLabel    "Rating"@en ;
        skos:broader      parentalguidance:_34 ;
        skos:inScheme     <http://www.ebu.ch/metadata/ontologies/skos/ebu_ParentalGuidanceCodeCS> ;
        skos:narrower     parentalguidance:_34.1.1 ;
        skos:narrower     parentalguidance:_34.1.2 ;
        skos:narrower     parentalguidance:_34.1.3 ;
        skos:narrower     parentalguidance:_34.1.4 ;
        skos:narrower     parentalguidance:_34.1.5 ;
        skos:changeNote   "" ;
        skos:historyNote  "" ;
        skos:example      "" .

parentalguidance:_34.1.1
        rdf:type          ebucore:TargetAudience ;
        skos:prefLabel    "G"@en ;
        skos:altLabel     "General"@en ;
        skos:altLabel     "Green"@en ;
        skos:definition   "Suitable for all ages"@en ;
        skos:broader      parentalguidance:_34.1 ;
        skos:inScheme     <http://www.ebu.ch/metadata/ontologies/skos/ebu_ParentalGuidanceCodeCS> ;
        skos:changeNote   "" ;
        skos:historyNote  "" ;
        skos:example      "" .

parentalguidance:_34.1.2
        rdf:type          ebucore:TargetAudience ;
        skos:prefLabel    "12+"@en ;
        skos:definition   "Ages 12 and above"@en ;
        skos:broader      parentalguidance:_34.1 ;
        skos:inScheme     <http://www.ebu.ch/metadata/ontologies/skos/ebu_ParentalGuidanceCodeCS> ;
        skos:changeNote   "" ;
        skos:historyNote  "" ;
        skos:example      "" .

parentalguidance:_34.1.3
        rdf:type          ebucore:TargetAudience ;
        skos:prefLabel    "15+"@en ;
        skos:definition   "Suitable for ages 15 and above"@en ;
        skos:broader      parentalguidance:_34.1 ;
        skos:inScheme     <http://www.ebu.ch/metadata/ontologies/skos/ebu_ParentalGuidanceCodeCS> ;
        skos:changeNote   "" ;
        skos:historyNote  "" ;
        skos:example      "" .

parentalguidance:_34.1.4
        rdf:type          ebucore:TargetAudience ;
        skos:prefLabel    "18+"@en ;
        skos:definition   "Suitable for ages 18 and above"@en ;
        skos:broader      parentalguidance:_34.1 ;
        skos:inScheme     <http://www.ebu.ch/metadata/ontologies/skos/ebu_ParentalGuidanceCodeCS> ;
        skos:changeNote   "" ;
        skos:historyNote  "" ;
        skos:example      "" .

parentalguidance:_34.1.5
        rdf:type          ebucore:TargetAudience ;
        skos:prefLabel    "PU"@en ;
        skos:definition   "For Professional Use Only"@en ;
        skos:broader      parentalguidance:_34.1 ;
        skos:inScheme     <http://www.ebu.ch/metadata/ontologies/skos/ebu_ParentalGuidanceCodeCS> ;
        skos:changeNote   "" ;
        skos:historyNote  "" ;
        skos:example      "" .

parentalguidance:_34.2
        rdf:type          ebucore:TargetAudience ;
        skos:prefLabel    "Criteria"@en ;
        skos:broader      parentalguidance:_34 ;
        skos:inScheme     <http://www.ebu.ch/metadata/ontologies/skos/ebu_ParentalGuidanceCodeCS> ;
        skos:narrower     parentalguidance:_34.2.1 ;
        skos:narrower     parentalguidance:_34.2.2 ;
        skos:narrower     parentalguidance:_34.2.3 ;
        skos:narrower     parentalguidance:_34.2.4 ;
        skos:narrower     parentalguidance:_34.2.5 ;
        skos:narrower     parentalguidance:_34.2.6 ;
        skos:narrower     parentalguidance:_34.2.7 ;
        skos:changeNote   "" ;
        skos:historyNote  "" ;
        skos:example      "" .

parentalguidance:_34.2.1
        rdf:type          ebucore:TargetAudience ;
        skos:prefLabel    "Violence"@en ;
        skos:broader      parentalguidance:_34.2 ;
        skos:inScheme     <http://www.ebu.ch/metadata/ontologies/skos/ebu_ParentalGuidanceCodeCS> ;
        skos:changeNote   "" ;
        skos:historyNote  "" ;
        skos:example      "" .

parentalguidance:_34.2.2
        rdf:type          ebucore:TargetAudience ;
        skos:prefLabel    "Sexual acts"@en ;
        skos:broader      parentalguidance:_34.2 ;
        skos:inScheme     <http://www.ebu.ch/metadata/ontologies/skos/ebu_ParentalGuidanceCodeCS> ;
        skos:changeNote   "" ;
        skos:historyNote  "" ;
        skos:example      "" .

parentalguidance:_34.2.3
        rdf:type          ebucore:TargetAudience ;
        skos:prefLabel    "Scary"@en ;
        skos:prefLabel    "Angst"@nl ;
        skos:broader      parentalguidance:_34.2 ;
        skos:inScheme     <http://www.ebu.ch/metadata/ontologies/skos/ebu_ParentalGuidanceCodeCS> ;
        skos:changeNote   "" ;
        skos:historyNote  "" ;
        skos:example      "" .

parentalguidance:_34.2.4
        rdf:type          ebucore:TargetAudience ;
        skos:prefLabel    "Nudity"@en ;
        skos:broader      parentalguidance:_34.2 ;
        skos:inScheme     <http://www.ebu.ch/metadata/ontologies/skos/ebu_ParentalGuidanceCodeCS> ;
        skos:changeNote   "" ;
        skos:historyNote  "" ;
        skos:example      "" .

parentalguidance:_34.2.5
        rdf:type          ebucore:TargetAudience ;
        skos:prefLabel    "Drugs abuse"@en ;
        skos:broader      parentalguidance:_34.2 ;
        skos:inScheme     <http://www.ebu.ch/metadata/ontologies/skos/ebu_ParentalGuidanceCodeCS> ;
        skos:changeNote   "" ;
        skos:historyNote  "" ;
        skos:example      "" .

parentalguidance:_34.2.6
        rdf:type          ebucore:TargetAudience ;
        skos:prefLabel    "Harshness of language"@en ;
        skos:broader      parentalguidance:_34.2 ;
        skos:inScheme     <http://www.ebu.ch/metadata/ontologies/skos/ebu_ParentalGuidanceCodeCS> ;
        skos:changeNote   "" ;
        skos:historyNote  "" ;
        skos:example      "" .

parentalguidance:_34.2.7
        rdf:type          ebucore:TargetAudience ;
        skos:prefLabel    "Religion"@en ;
        skos:broader      parentalguidance:_34.2 ;
        skos:inScheme     <http://www.ebu.ch/metadata/ontologies/skos/ebu_ParentalGuidanceCodeCS> ;
        skos:changeNote   "" ;
        skos:historyNote  "" ;
        skos:example      "" .

parentalguidance:_35  rdf:type  ebucore:TargetAudience ;
        skos:prefLabel    "MX-RTC"@en ;
        skos:scopeNote    "Region:Mexico"@en ;
        skos:definition   "Dirección General de Radio, Televisión y\n         Cinematografía"@en ;
        skos:inScheme     <http://www.ebu.ch/metadata/ontologies/skos/ebu_ParentalGuidanceCodeCS> ;
        skos:narrower     parentalguidance:_35.1 ;
        skos:narrower     parentalguidance:_35.2 ;
        skos:changeNote   "Update" ;
        skos:historyNote  "2009-07-28" ;
        skos:example      "" ;
        skos:note         "Valid" .

parentalguidance:_35.1
        rdf:type          ebucore:TargetAudience ;
        skos:prefLabel    "Rating"@en ;
        skos:broader      parentalguidance:_35 ;
        skos:inScheme     <http://www.ebu.ch/metadata/ontologies/skos/ebu_ParentalGuidanceCodeCS> ;
        skos:narrower     parentalguidance:_35.1.1 ;
        skos:narrower     parentalguidance:_35.1.2 ;
        skos:narrower     parentalguidance:_35.1.3 ;
        skos:narrower     parentalguidance:_35.1.4 ;
        skos:narrower     parentalguidance:_35.1.5 ;
        skos:narrower     parentalguidance:_35.1.6 ;
        skos:changeNote   "" ;
        skos:historyNote  "" ;
        skos:example      "" .

parentalguidance:_35.1.1
        rdf:type          ebucore:TargetAudience ;
        skos:prefLabel    "AA"@en ;
        skos:definition   "Particularly recommended for children under 7" ;
        skos:definition   "Comprensible para niños menores de 7 años"@es ;
        skos:broader      parentalguidance:_35.1 ;
        skos:inScheme     <http://www.ebu.ch/metadata/ontologies/skos/ebu_ParentalGuidanceCodeCS> ;
        skos:changeNote   "" ;
        skos:historyNote  "" ;
        skos:example      "" .

parentalguidance:_35.1.2
        rdf:type          ebucore:TargetAudience ;
        skos:prefLabel    "A"@en ;
        skos:definition   "For all audiences containing no content requiring parent\n         supervision" ;
        skos:definition   "Para todo público. Todos los programas bajo esta clasificación\n         son aptos para todo público y no deben contener elementos inadecuados para que los niños\n         los vean sin la supervisión de personas adultas."@es ;
        skos:broader      parentalguidance:_35.1 ;
        skos:inScheme     <http://www.ebu.ch/metadata/ontologies/skos/ebu_ParentalGuidanceCodeCS> ;
        skos:changeNote   "" ;
        skos:historyNote  "" ;
        skos:example      "" .

parentalguidance:_35.1.3
        rdf:type          ebucore:TargetAudience ;
        skos:prefLabel    "B"@en ;
        skos:definition   "For teenagers (ages 12 and older) and adults"@en ;
        skos:definition   "Para adolescentes de 12 años en adelante. Son programas aptos\n         para adolescentes y adultos. El material contiene temas o conceptos para adultos, sin\n         embargo es adecuado para que lo vean adolescentes mayores de 12 años."@es ;
        skos:broader      parentalguidance:_35.1 ;
        skos:inScheme     <http://www.ebu.ch/metadata/ontologies/skos/ebu_ParentalGuidanceCodeCS> ;
        skos:changeNote   "" ;
        skos:historyNote  "" ;
        skos:example      "" .

parentalguidance:_35.1.4
        rdf:type          ebucore:TargetAudience ;
        skos:prefLabel    "B15"@en ;
        skos:definition   "For ages 15 and older preferably in presence of supervising\n         adults"@en ;
        skos:definition   "No recomendada para menores de 15 años. Aptos para mayores de\n         15 años. El material clasificado contiene temas o conceptos para adultos, pero sigue siendo\n         adecuado para ser visto por adolescentes, preferentemente con la guía de personas\n         adultas."@es ;
        skos:broader      parentalguidance:_35.1 ;
        skos:inScheme     <http://www.ebu.ch/metadata/ontologies/skos/ebu_ParentalGuidanceCodeCS> ;
        skos:changeNote   "" ;
        skos:historyNote  "" ;
        skos:example      "" .

parentalguidance:_35.1.5
        rdf:type          ebucore:TargetAudience ;
        skos:prefLabel    "C"@en ;
        skos:definition   "For ages 18 and above"@en ;
        skos:definition   "Para adultos de 18 años en adelante. Programas aptos para\n         mayores de 18 años."@es ;
        skos:broader      parentalguidance:_35.1 ;
        skos:inScheme     <http://www.ebu.ch/metadata/ontologies/skos/ebu_ParentalGuidanceCodeCS> ;
        skos:changeNote   "" ;
        skos:historyNote  "" ;
        skos:example      "" .

parentalguidance:_35.1.6
        rdf:type          ebucore:TargetAudience ;
        skos:prefLabel    "D"@en ;
        skos:definition   "For ages 18 and above, strictly"@en ;
        skos:definition   "Para Adultos. Programas exclusivamente para mayores de 18\n         años"@es ;
        skos:broader      parentalguidance:_35.1 ;
        skos:inScheme     <http://www.ebu.ch/metadata/ontologies/skos/ebu_ParentalGuidanceCodeCS> ;
        skos:changeNote   "" ;
        skos:historyNote  "" ;
        skos:example      "" .

parentalguidance:_35.2
        rdf:type          ebucore:TargetAudience ;
        skos:prefLabel    "Criteria"@en ;
        skos:broader      parentalguidance:_35 ;
        skos:inScheme     <http://www.ebu.ch/metadata/ontologies/skos/ebu_ParentalGuidanceCodeCS> ;
        skos:narrower     parentalguidance:_35.2.1 ;
        skos:narrower     parentalguidance:_35.2.2 ;
        skos:narrower     parentalguidance:_35.2.3 ;
        skos:narrower     parentalguidance:_35.2.4 ;
        skos:changeNote   "" ;
        skos:historyNote  "" ;
        skos:example      "" .

parentalguidance:_35.2.1
        rdf:type          ebucore:TargetAudience ;
        skos:prefLabel    "Violence"@en ;
        skos:prefLabel    "Violencia"@es ;
        skos:broader      parentalguidance:_35.2 ;
        skos:inScheme     <http://www.ebu.ch/metadata/ontologies/skos/ebu_ParentalGuidanceCodeCS> ;
        skos:changeNote   "" ;
        skos:historyNote  "" ;
        skos:example      "" .

parentalguidance:_35.2.2
        rdf:type          ebucore:TargetAudience ;
        skos:prefLabel    "Sexuality"@en ;
        skos:prefLabel    "Sexualidad"@es ;
        skos:broader      parentalguidance:_35.2 ;
        skos:inScheme     <http://www.ebu.ch/metadata/ontologies/skos/ebu_ParentalGuidanceCodeCS> ;
        skos:changeNote   "" ;
        skos:historyNote  "" ;
        skos:example      "" .

parentalguidance:_35.2.3
        rdf:type          ebucore:TargetAudience ;
        skos:prefLabel    "Language"@en ;
        skos:prefLabel    "Lenguaje"@es ;
        skos:broader      parentalguidance:_35.2 ;
        skos:inScheme     <http://www.ebu.ch/metadata/ontologies/skos/ebu_ParentalGuidanceCodeCS> ;
        skos:changeNote   "" ;
        skos:historyNote  "" ;
        skos:example      "" .

parentalguidance:_35.2.4
        rdf:type          ebucore:TargetAudience ;
        skos:prefLabel    "Adicciones"@es ;
        skos:prefLabel    "Drugs and aclohol"@en ;
        skos:broader      parentalguidance:_35.2 ;
        skos:inScheme     <http://www.ebu.ch/metadata/ontologies/skos/ebu_ParentalGuidanceCodeCS> ;
        skos:changeNote   "" ;
        skos:historyNote  "" ;
        skos:example      "" .

parentalguidance:_36  rdf:type  ebucore:TargetAudience ;
        skos:prefLabel    "NG-NFVCB"@en ;
        skos:scopeNote    "Region:Nigeria"@en ;
        skos:definition   "Natioanl Film and Video Censor Board"@en ;
        skos:inScheme     <http://www.ebu.ch/metadata/ontologies/skos/ebu_ParentalGuidanceCodeCS> ;
        skos:narrower     parentalguidance:_36.1 ;
        skos:narrower     parentalguidance:_36.2 ;
        skos:changeNote   "Update" ;
        skos:historyNote  "2009-07-28" ;
        skos:example      "" ;
        skos:note         "Valid" .

parentalguidance:_36.1
        rdf:type          ebucore:TargetAudience ;
        skos:prefLabel    "Rating"@en ;
        skos:broader      parentalguidance:_36 ;
        skos:inScheme     <http://www.ebu.ch/metadata/ontologies/skos/ebu_ParentalGuidanceCodeCS> ;
        skos:narrower     parentalguidance:_36.1.1 ;
        skos:narrower     parentalguidance:_36.1.2 ;
        skos:narrower     parentalguidance:_36.1.3 ;
        skos:narrower     parentalguidance:_36.1.4 ;
        skos:narrower     parentalguidance:_36.1.5 ;
        skos:narrower     parentalguidance:_36.1.6 ;
        skos:changeNote   "" ;
        skos:historyNote  "" ;
        skos:example      "" .

parentalguidance:_36.1.1
        rdf:type          ebucore:TargetAudience ;
        skos:prefLabel    "G"@en ;
        skos:altLabel     "General"@en ;
        skos:definition   "The content is considered by the board to be suitable for\n         viewing by persons of all ages."@en ;
        skos:broader      parentalguidance:_36.1 ;
        skos:inScheme     <http://www.ebu.ch/metadata/ontologies/skos/ebu_ParentalGuidanceCodeCS> ;
        skos:changeNote   "" ;
        skos:historyNote  "" ;
        skos:example      "" .

parentalguidance:_36.1.2
        rdf:type          ebucore:TargetAudience ;
        skos:prefLabel     "PG"@en ;
        skos:altLabel    "Parental Guidance"@en ;
        skos:definition   "the themes or content of the film may not, in the opinion of\n         the board, be suitable for all children."@en ;
        skos:broader      parentalguidance:_36.1 ;
        skos:inScheme     <http://www.ebu.ch/metadata/ontologies/skos/ebu_ParentalGuidanceCodeCS> ;
        skos:changeNote   "" ;
        skos:historyNote  "" ;
        skos:example      "" .

parentalguidance:_36.1.3
        rdf:type          ebucore:TargetAudience ;
        skos:prefLabel    "12A/12"@en ;
        skos:definition   "Suitable for viewing by persons 12 years of age or older but\n         not for children under 12 years of age unless accompanied by an adult"@en ;
        skos:broader      parentalguidance:_36.1 ;
        skos:inScheme     <http://www.ebu.ch/metadata/ontologies/skos/ebu_ParentalGuidanceCodeCS> ;
        skos:changeNote   "" ;
        skos:historyNote  "" ;
        skos:example      "" .

parentalguidance:_36.1.4
        rdf:type          ebucore:TargetAudience ;
        skos:prefLabel    "15"@en ;
        skos:definition   "Suitable for viewing by persons over 15 years of\n         age"@en ;
        skos:broader      parentalguidance:_36.1 ;
        skos:inScheme     <http://www.ebu.ch/metadata/ontologies/skos/ebu_ParentalGuidanceCodeCS> ;
        skos:changeNote   "" ;
        skos:historyNote  "" ;
        skos:example      "" .

parentalguidance:_36.1.5
        rdf:type          ebucore:TargetAudience ;
        skos:prefLabel    "18"@en ;
        skos:definition   "Suitable for viewing by persons over 18 years of\n         ages"@en ;
        skos:broader      parentalguidance:_36.1 ;
        skos:inScheme     <http://www.ebu.ch/metadata/ontologies/skos/ebu_ParentalGuidanceCodeCS> ;
        skos:changeNote   "" ;
        skos:historyNote  "" ;
        skos:example      "" .

parentalguidance:_36.1.6
        rdf:type          ebucore:TargetAudience ;
        skos:prefLabel    "RE"@en ;
        skos:definition   "not suitable for viewing by persons under 18 years of age with\n         certain sensitvities to classification criteria"@en ;
        skos:broader      parentalguidance:_36.1 ;
        skos:inScheme     <http://www.ebu.ch/metadata/ontologies/skos/ebu_ParentalGuidanceCodeCS> ;
        skos:changeNote   "" ;
        skos:historyNote  "" ;
        skos:example      "" .

parentalguidance:_36.2
        rdf:type          ebucore:TargetAudience ;
        skos:prefLabel    "Criteria"@en ;
        skos:broader      parentalguidance:_36 ;
        skos:inScheme     <http://www.ebu.ch/metadata/ontologies/skos/ebu_ParentalGuidanceCodeCS> ;
        skos:narrower     parentalguidance:_36.2.1 ;
        skos:narrower     parentalguidance:_36.2.2 ;
        skos:narrower     parentalguidance:_36.2.3 ;
        skos:narrower     parentalguidance:_36.2.4 ;
        skos:narrower     parentalguidance:_36.2.5 ;
        skos:changeNote   "" ;
        skos:historyNote  "" ;
        skos:example      "" .

parentalguidance:_36.2.1
        rdf:type          ebucore:TargetAudience ;
        skos:prefLabel    "Violence"@en ;
        skos:broader      parentalguidance:_36.2 ;
        skos:inScheme     <http://www.ebu.ch/metadata/ontologies/skos/ebu_ParentalGuidanceCodeCS> ;
        skos:changeNote   "" ;
        skos:historyNote  "" ;
        skos:example      "" .

parentalguidance:_36.2.2
        rdf:type          ebucore:TargetAudience ;
        skos:prefLabel    "Sex"@en ;
        skos:broader      parentalguidance:_36.2 ;
        skos:inScheme     <http://www.ebu.ch/metadata/ontologies/skos/ebu_ParentalGuidanceCodeCS> ;
        skos:changeNote   "" ;
        skos:historyNote  "" ;
        skos:example      "" .

parentalguidance:_36.2.3
        rdf:type          ebucore:TargetAudience ;
        skos:prefLabel    "Coarse language"@en ;
        skos:broader      parentalguidance:_36.2 ;
        skos:inScheme     <http://www.ebu.ch/metadata/ontologies/skos/ebu_ParentalGuidanceCodeCS> ;
        skos:changeNote   "" ;
        skos:historyNote  "" ;
        skos:example      "" .

parentalguidance:_36.2.4
        rdf:type          ebucore:TargetAudience ;
        skos:prefLabel    "Strong themes"@en ;
        skos:broader      parentalguidance:_36.2 ;
        skos:inScheme     <http://www.ebu.ch/metadata/ontologies/skos/ebu_ParentalGuidanceCodeCS> ;
        skos:changeNote   "" ;
        skos:historyNote  "" ;
        skos:example      "" .

parentalguidance:_36.2.5
        rdf:type          ebucore:TargetAudience ;
        skos:prefLabel    "Horror or ritual scenes"@en ;
        skos:broader      parentalguidance:_36.2 ;
        skos:inScheme     <http://www.ebu.ch/metadata/ontologies/skos/ebu_ParentalGuidanceCodeCS> ;
        skos:changeNote   "" ;
        skos:historyNote  "" ;
        skos:example      "" .

parentalguidance:_37  rdf:type  ebucore:TargetAudience ;
        skos:prefLabel    "NL-NICAM"@en ;
        skos:altLabel     "Kijkwijzer"@nl ;
        skos:scopeNote    "Region:Netherlands"@en ;
        skos:definition   "Nederlands Institute for the Classification of Audio-visual\n         Media"@en ;
        skos:inScheme     <http://www.ebu.ch/metadata/ontologies/skos/ebu_ParentalGuidanceCodeCS> ;
        skos:narrower     parentalguidance:_37.1 ;
        skos:narrower     parentalguidance:_37.2 ;
        skos:changeNote   "Update" ;
        skos:historyNote  "2009-07-28" ;
        skos:example      "" ;
        skos:note         "Valid" .

parentalguidance:_37.1
        rdf:type          ebucore:TargetAudience ;
        skos:prefLabel    "Rating"@en ;
        skos:broader      parentalguidance:_37 ;
        skos:inScheme     <http://www.ebu.ch/metadata/ontologies/skos/ebu_ParentalGuidanceCodeCS> ;
        skos:narrower     parentalguidance:_37.1.1 ;
        skos:narrower     parentalguidance:_37.1.2 ;
        skos:narrower     parentalguidance:_37.1.3 ;
        skos:narrower     parentalguidance:_37.1.4 ;
        skos:narrower     parentalguidance:_37.1.5 ;
        skos:changeNote   "" ;
        skos:historyNote  "" ;
        skos:example      "" .

parentalguidance:_37.1.1
        rdf:type          ebucore:TargetAudience ;
        skos:prefLabel    "AL"@en ;
        skos:definition   "Suitable for all ages"@en ;
        skos:definition   "Alle leeftijden"@nl ;
        skos:broader      parentalguidance:_37.1 ;
        skos:inScheme     <http://www.ebu.ch/metadata/ontologies/skos/ebu_ParentalGuidanceCodeCS> ;
        skos:changeNote   "" ;
        skos:historyNote  "" ;
        skos:example      "" .

parentalguidance:_37.1.2
        rdf:type          ebucore:TargetAudience ;
        skos:prefLabel    "6"@en ;
        skos:definition   "Not recommended for viewers younger than 6\n         years"@en ;
        skos:definition   "Let op met kinderen tot 6 jaar"@nl ;
        skos:broader      parentalguidance:_37.1 ;
        skos:inScheme     <http://www.ebu.ch/metadata/ontologies/skos/ebu_ParentalGuidanceCodeCS> ;
        skos:changeNote   "" ;
        skos:historyNote  "" ;
        skos:example      "" .

parentalguidance:_37.1.3
        rdf:type          ebucore:TargetAudience ;
        skos:prefLabel    "9"@en ;
        skos:definition   "Not recommended for viewers younger than 9\n         years"@en ;
        skos:definition   "Let op met kinderen tot 9 jaar"@nl ;
        skos:broader      parentalguidance:_37.1 ;
        skos:inScheme     <http://www.ebu.ch/metadata/ontologies/skos/ebu_ParentalGuidanceCodeCS> ;
        skos:changeNote   "" ;
        skos:historyNote  "" ;
        skos:example      "" .

parentalguidance:_37.1.4
        rdf:type          ebucore:TargetAudience ;
        skos:prefLabel    "12"@en ;
        skos:definition   "Not recommended for viewers younger than 12\n         years"@en ;
        skos:definition   "Let op met kinderen tot 12 jaar"@nl ;
        skos:broader      parentalguidance:_37.1 ;
        skos:inScheme     <http://www.ebu.ch/metadata/ontologies/skos/ebu_ParentalGuidanceCodeCS> ;
        skos:changeNote   "" ;
        skos:historyNote  "" ;
        skos:example      "" .

parentalguidance:_37.1.5
        rdf:type          ebucore:TargetAudience ;
        skos:prefLabel    "16"@en ;
        skos:definition   "Movie shops/cinemas aren't allowed to show these movies to\n         people younger than 16 years"@en ;
        skos:definition   "Let op met kinderen tot 16 jaar"@nl ;
        skos:broader      parentalguidance:_37.1 ;
        skos:inScheme     <http://www.ebu.ch/metadata/ontologies/skos/ebu_ParentalGuidanceCodeCS> ;
        skos:changeNote   "" ;
        skos:historyNote  "" ;
        skos:example      "" .

parentalguidance:_37.2
        rdf:type          ebucore:TargetAudience ;
        skos:prefLabel    "Criteria"@en ;
        skos:broader      parentalguidance:_37 ;
        skos:inScheme     <http://www.ebu.ch/metadata/ontologies/skos/ebu_ParentalGuidanceCodeCS> ;
        skos:narrower     parentalguidance:_37.2.1 ;
        skos:narrower     parentalguidance:_37.2.2 ;
        skos:narrower     parentalguidance:_37.2.3 ;
        skos:narrower     parentalguidance:_37.2.4 ;
        skos:narrower     parentalguidance:_37.2.5 ;
        skos:narrower     parentalguidance:_37.2.6 ;
        skos:changeNote   "" ;
        skos:historyNote  "" ;
        skos:example      "" .

parentalguidance:_37.2.1
        rdf:type          ebucore:TargetAudience ;
        skos:prefLabel    "Violence"@en ;
        skos:prefLabel    "Geweld"@nl ;
        skos:broader      parentalguidance:_37.2 ;
        skos:inScheme     <http://www.ebu.ch/metadata/ontologies/skos/ebu_ParentalGuidanceCodeCS> ;
        skos:changeNote   "" ;
        skos:historyNote  "" ;
        skos:example      "" .

parentalguidance:_37.2.2
        rdf:type          ebucore:TargetAudience ;
        skos:prefLabel    "Sex"@en ;
        skos:prefLabel    "Seks"@nl ;
        skos:broader      parentalguidance:_37.2 ;
        skos:inScheme     <http://www.ebu.ch/metadata/ontologies/skos/ebu_ParentalGuidanceCodeCS> ;
        skos:changeNote   "" ;
        skos:historyNote  "" ;
        skos:example      "" .

parentalguidance:_37.2.3
        rdf:type          ebucore:TargetAudience ;
        skos:prefLabel    "Scary"@en ;
        skos:prefLabel    "Angst"@nl ;
        skos:broader      parentalguidance:_37.2 ;
        skos:inScheme     <http://www.ebu.ch/metadata/ontologies/skos/ebu_ParentalGuidanceCodeCS> ;
        skos:changeNote   "" ;
        skos:historyNote  "" ;
        skos:example      "" .

parentalguidance:_37.2.4
        rdf:type          ebucore:TargetAudience ;
        skos:prefLabel    "Discrimination"@en ;
        skos:prefLabel    "Discriminatie"@nl ;
        skos:broader      parentalguidance:_37.2 ;
        skos:inScheme     <http://www.ebu.ch/metadata/ontologies/skos/ebu_ParentalGuidanceCodeCS> ;
        skos:changeNote   "" ;
        skos:historyNote  "" ;
        skos:example      "" .

parentalguidance:_37.2.5
        rdf:type          ebucore:TargetAudience ;
        skos:prefLabel    "Drugs & alcohol"@en ;
        skos:prefLabel    "Drugs- en alcoholmisbruik"@nl ;
        skos:broader      parentalguidance:_37.2 ;
        skos:inScheme     <http://www.ebu.ch/metadata/ontologies/skos/ebu_ParentalGuidanceCodeCS> ;
        skos:changeNote   "" ;
        skos:historyNote  "" ;
        skos:example      "" .

parentalguidance:_37.2.6
        rdf:type          ebucore:TargetAudience ;
        skos:prefLabel    "Bad language"@en ;
        skos:prefLabel    "Grof taalgebruik"@nl ;
        skos:broader      parentalguidance:_37.2 ;
        skos:inScheme     <http://www.ebu.ch/metadata/ontologies/skos/ebu_ParentalGuidanceCodeCS> ;
        skos:changeNote   "" ;
        skos:historyNote  "" ;
        skos:example      "" .

parentalguidance:_38  rdf:type  ebucore:TargetAudience ;
        skos:prefLabel    "NO-Medietilsynet-Om_aldersgrenser"@en ;
        skos:altLabel     "Medietilsynet"@no ;
        skos:scopeNote    "Region:Norway"@en ;
        skos:definition   "Scheme as defined by the Medietilsynet"@en ;
        skos:inScheme     <http://www.ebu.ch/metadata/ontologies/skos/ebu_ParentalGuidanceCodeCS> ;
        skos:narrower     parentalguidance:_38.1 ;
        skos:narrower     parentalguidance:_38.2 ;
        skos:narrower     parentalguidance:_38.3 ;
        skos:narrower     parentalguidance:_38.4 ;
        skos:narrower     parentalguidance:_38.5 ;
        skos:changeNote   "Update" ;
        skos:historyNote  "2009-07-28" ;
        skos:example      "" ;
        skos:note         "Valid" .

parentalguidance:_38.1
        rdf:type          ebucore:TargetAudience ;
        skos:prefLabel    "All"@en ;
        skos:prefLabel    "Alle"@no ;
        skos:definition   "Tillaten for alle"@no ;
        skos:definition   "For all"@en ;
        skos:broader      parentalguidance:_38 ;
        skos:inScheme     <http://www.ebu.ch/metadata/ontologies/skos/ebu_ParentalGuidanceCodeCS> ;
        skos:changeNote   "" ;
        skos:historyNote  "" ;
        skos:example      "" .

parentalguidance:_38.2
        rdf:type          ebucore:TargetAudience ;
        skos:prefLabel    "7"@en ;
        skos:definition   "7 år (barn ned til 4 år i følgje med\n         føresette)"@no ;
        skos:definition   "7 and older or from 4 in presence of an accompanying\n         adult"@en ;
        skos:broader      parentalguidance:_38 ;
        skos:inScheme     <http://www.ebu.ch/metadata/ontologies/skos/ebu_ParentalGuidanceCodeCS> ;
        skos:changeNote   "" ;
        skos:historyNote  "" ;
        skos:example      "" .

parentalguidance:_38.3
        rdf:type          ebucore:TargetAudience ;
        skos:prefLabel    "11"@en ;
        skos:definition   "11 år (barn ned til 8 år i følgje med\n         føresette)"@no ;
        skos:definition   "11 and older or from 8 in presence of an accompanying\n         adult"@en ;
        skos:broader      parentalguidance:_38 ;
        skos:inScheme     <http://www.ebu.ch/metadata/ontologies/skos/ebu_ParentalGuidanceCodeCS> ;
        skos:changeNote   "" ;
        skos:historyNote  "" ;
        skos:example      "" .

parentalguidance:_38.4
        rdf:type          ebucore:TargetAudience ;
        skos:prefLabel    "15"@en ;
        skos:definition   "15 år (unge ned til 12 år i følgje med\n         føresette)"@no ;
        skos:definition   "15 and older, not under 12, above 12 in presence of an\n         accompanying adult"@en ;
        skos:broader      parentalguidance:_38 ;
        skos:inScheme     <http://www.ebu.ch/metadata/ontologies/skos/ebu_ParentalGuidanceCodeCS> ;
        skos:changeNote   "" ;
        skos:historyNote  "" ;
        skos:example      "" .

parentalguidance:_38.5
        rdf:type          ebucore:TargetAudience ;
        skos:prefLabel    "18"@en ;
        skos:definition   "18 år (absolutt nedre grense)"@no ;
        skos:definition   "Not under 18"@en ;
        skos:broader      parentalguidance:_38 ;
        skos:inScheme     <http://www.ebu.ch/metadata/ontologies/skos/ebu_ParentalGuidanceCodeCS> ;
        skos:changeNote   "" ;
        skos:historyNote  "" ;
        skos:example      "" .

parentalguidance:_39  rdf:type  ebucore:TargetAudience ;
        skos:prefLabel    "NZ-OFLC"@en ;
        skos:altLabel     "NZ Office of Film and Literature Classification"@en ;
        skos:scopeNote    "Region:New Zealand"@en ;
        skos:definition   "Office of Film and Literature Classification"@en ;
        skos:inScheme     <http://www.ebu.ch/metadata/ontologies/skos/ebu_ParentalGuidanceCodeCS> ;
        skos:narrower     parentalguidance:_39.1 ;
        skos:narrower     parentalguidance:_39.2 ;
        skos:narrower     parentalguidance:_39.3 ;
        skos:narrower     parentalguidance:_39.4 ;
        skos:narrower     parentalguidance:_39.5 ;
        skos:narrower     parentalguidance:_39.6 ;
        skos:narrower     parentalguidance:_39.7 ;
        skos:narrower     parentalguidance:_39.8 ;
        skos:changeNote   "Update" ;
        skos:historyNote  "2009-07-27" ;
        skos:example      "" ;
        skos:note         "Valid" .

parentalguidance:_39.1
        rdf:type          ebucore:TargetAudience ;
        skos:prefLabel    "G"@en ;
        skos:altLabel     "General"@en ;
        skos:definition   "Suitable for general audiences (awarded by the Film and Video\n         Labelling Body and the Office of Film and Literature Classification)"@en ;
        skos:broader      parentalguidance:_39 ;
        skos:inScheme     <http://www.ebu.ch/metadata/ontologies/skos/ebu_ParentalGuidanceCodeCS> ;
        skos:changeNote   "" ;
        skos:historyNote  "" ;
        skos:example      "" .

parentalguidance:_39.2
        rdf:type          ebucore:TargetAudience ;
        skos:prefLabel     "PG"@en ;
        skos:altLabel    "Parental Guidance"@en ;
        skos:definition   "Parental guidance recommended for younger viewers (awarded by\n         the Film and Video Labelling Body and the Office of Film and Literature\n         Classification)"@en ;
        skos:broader      parentalguidance:_39 ;
        skos:inScheme     <http://www.ebu.ch/metadata/ontologies/skos/ebu_ParentalGuidanceCodeCS> ;
        skos:changeNote   "" ;
        skos:historyNote  "" ;
        skos:example      "" .

parentalguidance:_39.3
        rdf:type          ebucore:TargetAudience ;
        skos:prefLabel    "M"@en ;
        skos:altLabel     "Mature"@en ;
        skos:definition   "Suitable for (but not restricted to) mature audiences 16 years\n         and over (awarded by the Film and Video Labelling Body and the Office of Film and\n         Literature Classification)"@en ;
        skos:broader      parentalguidance:_39 ;
        skos:inScheme     <http://www.ebu.ch/metadata/ontologies/skos/ebu_ParentalGuidanceCodeCS> ;
        skos:changeNote   "" ;
        skos:historyNote  "" ;
        skos:example      "" .

parentalguidance:_39.4
        rdf:type          ebucore:TargetAudience ;
        skos:prefLabel    "R13"@en ;
        skos:definition   "Suitable to persons 13 years of age and over (awarded by the\n         Office of Film and Literature Classification only)"@en ;
        skos:broader      parentalguidance:_39 ;
        skos:inScheme     <http://www.ebu.ch/metadata/ontologies/skos/ebu_ParentalGuidanceCodeCS> ;
        skos:changeNote   "" ;
        skos:historyNote  "" ;
        skos:example      "" .

parentalguidance:_39.5
        rdf:type          ebucore:TargetAudience ;
        skos:prefLabel    "R15"@en ;
        skos:definition   "Suitable to persons 15 years of age and over (awarded by the\n         Office of Film and Literature Classification only)"@en ;
        skos:broader      parentalguidance:_39 ;
        skos:inScheme     <http://www.ebu.ch/metadata/ontologies/skos/ebu_ParentalGuidanceCodeCS> ;
        skos:changeNote   "" ;
        skos:historyNote  "" ;
        skos:example      "" .

parentalguidance:_39.6
        rdf:type          ebucore:TargetAudience ;
        skos:prefLabel    "R16"@en ;
        skos:definition   "Suitable to persons 16 years of age and over (awarded by the\n         Office of Film and Literature Classification only)"@en ;
        skos:broader      parentalguidance:_39 ;
        skos:inScheme     <http://www.ebu.ch/metadata/ontologies/skos/ebu_ParentalGuidanceCodeCS> ;
        skos:changeNote   "" ;
        skos:historyNote  "" ;
        skos:example      "" .

parentalguidance:_39.7
        rdf:type          ebucore:TargetAudience ;
        skos:prefLabel    "R18"@en ;
        skos:definition   "Suitable to persons 18 years of age and over (awarded by the\n         Office of Film and Literature Classification only)"@en ;
        skos:broader      parentalguidance:_39 ;
        skos:inScheme     <http://www.ebu.ch/metadata/ontologies/skos/ebu_ParentalGuidanceCodeCS> ;
        skos:changeNote   "" ;
        skos:historyNote  "" ;
        skos:example      "" .

parentalguidance:_39.8
        rdf:type          ebucore:TargetAudience ;
        skos:prefLabel    "R"@en ;
        skos:altLabel     "Restricted"@en ;
        skos:definition   "Restricted to a particular class of persons, or for particular\n         purposes, or both, specified by the Office of Film and Literature\n         Classification"@en ;
        skos:broader      parentalguidance:_39 ;
        skos:inScheme     <http://www.ebu.ch/metadata/ontologies/skos/ebu_ParentalGuidanceCodeCS> ;
        skos:changeNote   "" ;
        skos:historyNote  "" ;
        skos:example      "" .

parentalguidance:_40  rdf:type  ebucore:TargetAudience ;
        skos:prefLabel    "PH-MTRCB"@en ;
        skos:altLabel     "The Movie and Television Review and Classification Board"@en ;
        skos:scopeNote    "Region:Philippines"@en ;
        skos:definition   "Movie and Television Review and Classification Board"@en ;
        skos:definition   "Lupon sa Pagrerepaso at Pag-uuri ng Sine at Telebisyon" ;
        skos:inScheme     <http://www.ebu.ch/metadata/ontologies/skos/ebu_ParentalGuidanceCodeCS> ;
        skos:narrower     parentalguidance:_40.1 ;
        skos:narrower     parentalguidance:_40.2 ;
        skos:narrower     parentalguidance:_40.3 ;
        skos:narrower     parentalguidance:_40.4 ;
        skos:changeNote   "Update" ;
        skos:historyNote  "2009-07-28" ;
        skos:example      "" ;
        skos:note         "Valid" .

parentalguidance:_40.1
        rdf:type          ebucore:TargetAudience ;
        skos:prefLabel    "G"@en ;
        skos:definition   "General Patronage. All ages admitted."@en ;
        skos:broader      parentalguidance:_40 ;
        skos:inScheme     <http://www.ebu.ch/metadata/ontologies/skos/ebu_ParentalGuidanceCodeCS> ;
        skos:changeNote   "" ;
        skos:historyNote  "" ;
        skos:example      "" .

parentalguidance:_40.2
        rdf:type          ebucore:TargetAudience ;
        skos:prefLabel    "PG-13"@en ;
        skos:definition   "Viewers below 13 years old must be accompanied by a parent or\n         an adult."@en ;
        skos:broader      parentalguidance:_40 ;
        skos:inScheme     <http://www.ebu.ch/metadata/ontologies/skos/ebu_ParentalGuidanceCodeCS> ;
        skos:changeNote   "" ;
        skos:historyNote  "" ;
        skos:example      "" .

parentalguidance:_40.3
        rdf:type          ebucore:TargetAudience ;
        skos:prefLabel    "R-13"@en ;
        skos:definition   "Only those who are 13 and above may view an “R-13”\n         film."@en ;
        skos:broader      parentalguidance:_40 ;
        skos:inScheme     <http://www.ebu.ch/metadata/ontologies/skos/ebu_ParentalGuidanceCodeCS> ;
        skos:changeNote   "" ;
        skos:historyNote  "" ;
        skos:example      "" .

parentalguidance:_40.4
        rdf:type          ebucore:TargetAudience ;
        skos:prefLabel    "R-18"@en ;
        skos:definition   "Only those who are 13 and above may view an “R-13”\n         film."@en ;
        skos:broader      parentalguidance:_40 ;
        skos:inScheme     <http://www.ebu.ch/metadata/ontologies/skos/ebu_ParentalGuidanceCodeCS> ;
        skos:changeNote   "" ;
        skos:historyNote  "" ;
        skos:example      "" .

parentalguidance:_41  rdf:type  ebucore:TargetAudience ;
        skos:prefLabel    "PL-RTP"@en ;
        skos:altLabel     "Krajowa Rada Radiofonii i Telewizji"@pl ;
        skos:scopeNote    "Region:Portugal"@en ;
        skos:definition   "Scheme as used by the Radio Telewisja Polska"@en ;
        skos:inScheme     <http://www.ebu.ch/metadata/ontologies/skos/ebu_ParentalGuidanceCodeCS> ;
        skos:narrower     parentalguidance:_41.1 ;
        skos:narrower     parentalguidance:_41.2 ;
        skos:narrower     parentalguidance:_41.3 ;
        skos:narrower     parentalguidance:_41.4 ;
        skos:narrower     parentalguidance:_41.5 ;
        skos:changeNote   "Update" ;
        skos:historyNote  "2009-07-28" ;
        skos:example      "" ;
        skos:note         "Valid" .

parentalguidance:_41.1
        rdf:type          ebucore:TargetAudience ;
        skos:prefLabel    "G"@en ;
        skos:definition   "For all audiences"@en ;
        skos:broader      parentalguidance:_41 ;
        skos:inScheme     <http://www.ebu.ch/metadata/ontologies/skos/ebu_ParentalGuidanceCodeCS> ;
        skos:changeNote   "" ;
        skos:historyNote  "" ;
        skos:example      "" .

parentalguidance:_41.2
        rdf:type          ebucore:TargetAudience ;
        skos:prefLabel    "7"@en ;
        skos:definition   "For persons of age 10 and above. Parental Guidance is\n         suggested."@en ;
        skos:broader      parentalguidance:_41 ;
        skos:inScheme     <http://www.ebu.ch/metadata/ontologies/skos/ebu_ParentalGuidanceCodeCS> ;
        skos:changeNote   "" ;
        skos:historyNote  "" ;
        skos:example      "" .

parentalguidance:_41.3
        rdf:type          ebucore:TargetAudience ;
        skos:prefLabel    "12"@en ;
        skos:definition   "For persons of age 12 and above. Parental Guidance is\n         suggested."@en ;
        skos:broader      parentalguidance:_41 ;
        skos:inScheme     <http://www.ebu.ch/metadata/ontologies/skos/ebu_ParentalGuidanceCodeCS> ;
        skos:changeNote   "" ;
        skos:historyNote  "" ;
        skos:example      "" .

parentalguidance:_41.4
        rdf:type          ebucore:TargetAudience ;
        skos:prefLabel    "16"@en ;
        skos:definition   "For persons of age 16 and above."@en ;
        skos:broader      parentalguidance:_41 ;
        skos:inScheme     <http://www.ebu.ch/metadata/ontologies/skos/ebu_ParentalGuidanceCodeCS> ;
        skos:changeNote   "" ;
        skos:historyNote  "" ;
        skos:example      "" .

parentalguidance:_41.5
        rdf:type          ebucore:TargetAudience ;
        skos:prefLabel    "R"@en ;
        skos:definition   "Adults only (18 and over)"@en ;
        skos:broader      parentalguidance:_41 ;
        skos:inScheme     <http://www.ebu.ch/metadata/ontologies/skos/ebu_ParentalGuidanceCodeCS> ;
        skos:changeNote   "" ;
        skos:historyNote  "" ;
        skos:example      "" .

parentalguidance:_42  rdf:type  ebucore:TargetAudience ;
        skos:prefLabel    "PT-CCE"@en ;
        skos:altLabel     "Comissão de Classificação de Espectáculos"@pt ;
        skos:scopeNote    "Region:Portugal"@en ;
        skos:definition   "Scheme as defined by the Comissão de Classificação de Espectáculos"@en ;
        skos:inScheme     <http://www.ebu.ch/metadata/ontologies/skos/ebu_ParentalGuidanceCodeCS> ;
        skos:narrower     parentalguidance:_42.1 ;
        skos:narrower     parentalguidance:_42.2 ;
        skos:narrower     parentalguidance:_42.3 ;
        skos:narrower     parentalguidance:_42.4 ;
        skos:narrower     parentalguidance:_42.5 ;
        skos:narrower     parentalguidance:_42.6 ;
        skos:narrower     parentalguidance:_42.7 ;
        skos:changeNote   "Update" ;
        skos:historyNote  "2009-07-28" ;
        skos:example      "" ;
        skos:note         "Valid" .

parentalguidance:_42.1
        rdf:type          ebucore:TargetAudience ;
        skos:prefLabel    "M/4"@en ;
        skos:definition   "For persons of age 4 and above"@en ;
        skos:definition   "os espectáculos de curta duração e de fácil compreensão que não\n         provoquem reacções de pavor e que não colidam com a fantasia e com o sentido lúdico deste\n         nível etário."@pt ;
        skos:broader      parentalguidance:_42 ;
        skos:inScheme     <http://www.ebu.ch/metadata/ontologies/skos/ebu_ParentalGuidanceCodeCS> ;
        skos:changeNote   "" ;
        skos:historyNote  "" ;
        skos:example      "" .

parentalguidance:_42.2
        rdf:type          ebucore:TargetAudience ;
        skos:prefLabel    "M/6"@en ;
        skos:definition   "For persons of age 6 and above"@en ;
        skos:definition   "os espectáculos que, pela sua temática ou extensão, não sejam\n         abrangidos pelos critérios fixados para os níveis etários superiores."@pt ;
        skos:broader      parentalguidance:_42 ;
        skos:inScheme     <http://www.ebu.ch/metadata/ontologies/skos/ebu_ParentalGuidanceCodeCS> ;
        skos:changeNote   "" ;
        skos:historyNote  "" ;
        skos:example      "" .

parentalguidance:_42.3
        rdf:type          ebucore:TargetAudience ;
        skos:prefLabel    "M/12"@en ;
        skos:definition   "For persons of age 12 and above"@en ;
        skos:definition   "os espectáculos que, pela sua extensão e complexidade, possam\n         provocar nos espectadores de nível etário inferior fadiga excessiva e ou traumatismo\n         psíquico."@pt ;
        skos:broader      parentalguidance:_42 ;
        skos:inScheme     <http://www.ebu.ch/metadata/ontologies/skos/ebu_ParentalGuidanceCodeCS> ;
        skos:changeNote   "" ;
        skos:historyNote  "" ;
        skos:example      "" .

parentalguidance:_42.4
        rdf:type          ebucore:TargetAudience ;
        skos:prefLabel    "M/16"@en ;
        skos:definition   "For persons of age 16 and above"@en ;
        skos:definition   "os espectáculos que explorem, em termos excessivos, aspectos da\n         sexualidade e da violência física e psíquica."@pt ;
        skos:broader      parentalguidance:_42 ;
        skos:inScheme     <http://www.ebu.ch/metadata/ontologies/skos/ebu_ParentalGuidanceCodeCS> ;
        skos:changeNote   "" ;
        skos:historyNote  "" ;
        skos:example      "" .

parentalguidance:_42.5
        rdf:type          ebucore:TargetAudience ;
        skos:prefLabel    "M/18"@en ;
        skos:definition   "For persons of age 18 and above"@en ;
        skos:definition   "os espectáculos pornográficos e os que explorem formas\n         patológicas de violência física e psíquica."@pt ;
        skos:broader      parentalguidance:_42 ;
        skos:inScheme     <http://www.ebu.ch/metadata/ontologies/skos/ebu_ParentalGuidanceCodeCS> ;
        skos:changeNote   "" ;
        skos:historyNote  "" ;
        skos:example      "" .

parentalguidance:_42.6
        rdf:type          ebucore:TargetAudience ;
        skos:prefLabel    "Pornográficos"@en ;
        skos:definition   "For persons of age 18 and above, sexual\n         content"@en ;
        skos:definition   "Serão classificados no 1º escalão (hard-core) os espectáculos\n         que apresentem uma descrição ostensiva e insistente de actos sexuais realmente praticados\n         com exibição dos órgãos genitais; Serão classificados no 2º escalão (soft-core) os\n         espectáculos que apresentem uma descrição ostensiva e insistente de actos sexuais\n         simulados."@pt ;
        skos:broader      parentalguidance:_42 ;
        skos:inScheme     <http://www.ebu.ch/metadata/ontologies/skos/ebu_ParentalGuidanceCodeCS> ;
        skos:changeNote   "" ;
        skos:historyNote  "" ;
        skos:example      "" .

parentalguidance:_42.7
        rdf:type          ebucore:TargetAudience ;
        skos:prefLabel    "De Qualidade"@en ;
        skos:definition   "Of quality from an artistic, thematic, pedagogic or technical\n         realisation perspective"@en ;
        skos:definition   "Os espectáculos que, pelos seus aspectos artístico, temático,\n         pedagógico e técnico mereçam esse atributo."@pt ;
        skos:broader      parentalguidance:_42 ;
        skos:inScheme     <http://www.ebu.ch/metadata/ontologies/skos/ebu_ParentalGuidanceCodeCS> ;
        skos:changeNote   "" ;
        skos:historyNote  "" ;
        skos:example      "" .

parentalguidance:_43  rdf:type  ebucore:TargetAudience ;
        skos:prefLabel    "PT-RTP"@en ;
        skos:scopeNote    "Region:Portugal"@en ;
        skos:definition   "Scheme as defined by the Radio Televisão\n         Portugal"@en ;
        skos:inScheme     <http://www.ebu.ch/metadata/ontologies/skos/ebu_ParentalGuidanceCodeCS> ;
        skos:narrower     parentalguidance:_43.1 ;
        skos:narrower     parentalguidance:_43.2 ;
        skos:narrower     parentalguidance:_43.3 ;
        skos:narrower     parentalguidance:_43.4 ;
        skos:changeNote   "Update" ;
        skos:historyNote  "2009-07-28" ;
        skos:example      "" ;
        skos:note         "Valid" .

parentalguidance:_43.1
        rdf:type          ebucore:TargetAudience ;
        skos:prefLabel    "T"@en ;
        skos:definition   "For all audiences"@en ;
        skos:definition   "Todos"@pt ;
        skos:broader      parentalguidance:_43 ;
        skos:inScheme     <http://www.ebu.ch/metadata/ontologies/skos/ebu_ParentalGuidanceCodeCS> ;
        skos:changeNote   "" ;
        skos:historyNote  "" ;
        skos:example      "" .

parentalguidance:_43.2
        rdf:type          ebucore:TargetAudience ;
        skos:prefLabel    "10"@en ;
        skos:definition   "For persons of age 10 and above. Parental Guidance is\n         suggested."@en ;
        skos:broader      parentalguidance:_43 ;
        skos:inScheme     <http://www.ebu.ch/metadata/ontologies/skos/ebu_ParentalGuidanceCodeCS> ;
        skos:changeNote   "" ;
        skos:historyNote  "" ;
        skos:example      "" .

parentalguidance:_43.3
        rdf:type          ebucore:TargetAudience ;
        skos:prefLabel    "12"@en ;
        skos:definition   "For persons of age 12 and above. Parental Guidance is\n         suggested."@en ;
        skos:broader      parentalguidance:_43 ;
        skos:inScheme     <http://www.ebu.ch/metadata/ontologies/skos/ebu_ParentalGuidanceCodeCS> ;
        skos:changeNote   "" ;
        skos:historyNote  "" ;
        skos:example      "" .

parentalguidance:_43.4
        rdf:type          ebucore:TargetAudience ;
        skos:prefLabel    "16"@en ;
        skos:definition   "For persons of age 16 and above."@en ;
        skos:broader      parentalguidance:_43 ;
        skos:inScheme     <http://www.ebu.ch/metadata/ontologies/skos/ebu_ParentalGuidanceCodeCS> ;
        skos:changeNote   "" ;
        skos:historyNote  "" ;
        skos:example      "" .

parentalguidance:_44  rdf:type  ebucore:TargetAudience ;
        skos:prefLabel    "SE-SB"@en ;
        skos:scopeNote    "Region:Sweden" ;
        skos:definition   "Swedish National Board of Film Censors"@en ;
        skos:definition   "Statens biografbyrå"@sv ;
        skos:inScheme     <http://www.ebu.ch/metadata/ontologies/skos/ebu_ParentalGuidanceCodeCS> ;
        skos:narrower     parentalguidance:_44.1 ;
        skos:narrower     parentalguidance:_44.2 ;
        skos:narrower     parentalguidance:_44.3 ;
        skos:narrower     parentalguidance:_44.4 ;
        skos:narrower     parentalguidance:_44.5 ;
        skos:changeNote   "Update" ;
        skos:historyNote  "2009-07-28" ;
        skos:example      "" ;
        skos:note         "Valid" .

parentalguidance:_44.1
        rdf:type          ebucore:TargetAudience ;
        skos:prefLabel    "Btl"@en ;
        skos:definition   "Barntillåten"@sv ;
        skos:definition   "Suitable for all ages"@en ;
        skos:broader      parentalguidance:_44 ;
        skos:inScheme     <http://www.ebu.ch/metadata/ontologies/skos/ebu_ParentalGuidanceCodeCS> ;
        skos:changeNote   "" ;
        skos:historyNote  "" ;
        skos:example      "" .

parentalguidance:_44.2
        rdf:type          ebucore:TargetAudience ;
        skos:prefLabel    "7"@en ;
        skos:definition   "Suitable for children of at least 7 years of\n         age"@en ;
        skos:broader      parentalguidance:_44 ;
        skos:inScheme     <http://www.ebu.ch/metadata/ontologies/skos/ebu_ParentalGuidanceCodeCS> ;
        skos:changeNote   "" ;
        skos:historyNote  "" ;
        skos:example      "" .

parentalguidance:_44.3
        rdf:type          ebucore:TargetAudience ;
        skos:prefLabel    "11"@en ;
        skos:definition   "Suitable for children of at least 11 years of\n         age"@en ;
        skos:broader      parentalguidance:_44 ;
        skos:inScheme     <http://www.ebu.ch/metadata/ontologies/skos/ebu_ParentalGuidanceCodeCS> ;
        skos:changeNote   "" ;
        skos:historyNote  "" ;
        skos:example      "" .

parentalguidance:_44.4
        rdf:type          ebucore:TargetAudience ;
        skos:prefLabel    "15"@en ;
        skos:definition   "No one under 15 years of age admitted"@en ;
        skos:broader      parentalguidance:_44 ;
        skos:inScheme     <http://www.ebu.ch/metadata/ontologies/skos/ebu_ParentalGuidanceCodeCS> ;
        skos:changeNote   "" ;
        skos:historyNote  "" ;
        skos:example      "" .

parentalguidance:_44.5
        rdf:type          ebucore:TargetAudience ;
        skos:prefLabel    "18"@en ;
        skos:definition   "No one under 18 years of age admitted"@en ;
        skos:broader      parentalguidance:_44 ;
        skos:inScheme     <http://www.ebu.ch/metadata/ontologies/skos/ebu_ParentalGuidanceCodeCS> ;
        skos:changeNote   "" ;
        skos:historyNote  "" ;
        skos:example      "" .

parentalguidance:_45  rdf:type  ebucore:TargetAudience ;
        skos:prefLabel    "SG-MDA"@en ;
        skos:scopeNote    "Region:Singapore" ;
        skos:definition   "Media Development Authority"@en ;
        skos:inScheme     <http://www.ebu.ch/metadata/ontologies/skos/ebu_ParentalGuidanceCodeCS> ;
        skos:narrower     parentalguidance:_45.1 ;
        skos:narrower     parentalguidance:_45.2 ;
        skos:narrower     parentalguidance:_45.3 ;
        skos:narrower     parentalguidance:_45.4 ;
        skos:narrower     parentalguidance:_45.5 ;
        skos:changeNote   "Update" ;
        skos:historyNote  "2009-07-28" ;
        skos:example      "" ;
        skos:note         "Valid" .

parentalguidance:_45.1
        rdf:type          ebucore:TargetAudience ;
        skos:prefLabel    "G"@en ;
        skos:altLabel     "General"@en ;
        skos:definition   "Suitable for all ages and audiences"@en ;
        skos:broader      parentalguidance:_45 ;
        skos:inScheme     <http://www.ebu.ch/metadata/ontologies/skos/ebu_ParentalGuidanceCodeCS> ;
        skos:changeNote   "" ;
        skos:historyNote  "" ;
        skos:example      "" .

parentalguidance:_45.2
        rdf:type          ebucore:TargetAudience ;
        skos:prefLabel     "PG"@en ;
        skos:altLabel    "Parental Guidance"@en ;
        skos:definition   "Parental supervision is advised"@en ;
        skos:broader      parentalguidance:_45 ;
        skos:inScheme     <http://www.ebu.ch/metadata/ontologies/skos/ebu_ParentalGuidanceCodeCS> ;
        skos:changeNote   "" ;
        skos:historyNote  "" ;
        skos:example      "" .

parentalguidance:_45.3
        rdf:type          ebucore:TargetAudience ;
        skos:prefLabel    "NC16"@en ;
        skos:definition   "No children below 16 years old"@en ;
        skos:broader      parentalguidance:_45 ;
        skos:inScheme     <http://www.ebu.ch/metadata/ontologies/skos/ebu_ParentalGuidanceCodeCS> ;
        skos:changeNote   "" ;
        skos:historyNote  "" ;
        skos:example      "" .

parentalguidance:_45.4
        rdf:type          ebucore:TargetAudience ;
        skos:prefLabel    "M18"@en ;
        skos:definition   "Mature 18 for persons 18 years and above"@en ;
        skos:broader      parentalguidance:_45 ;
        skos:inScheme     <http://www.ebu.ch/metadata/ontologies/skos/ebu_ParentalGuidanceCodeCS> ;
        skos:changeNote   "" ;
        skos:historyNote  "" ;
        skos:example      "" .

parentalguidance:_45.5
        rdf:type          ebucore:TargetAudience ;
        skos:prefLabel    "R21"@en ;
        skos:definition   "Restricted to persons 21 years and above"@en ;
        skos:broader      parentalguidance:_45 ;
        skos:inScheme     <http://www.ebu.ch/metadata/ontologies/skos/ebu_ParentalGuidanceCodeCS> ;
        skos:changeNote   "" ;
        skos:historyNote  "" ;
        skos:example      "" .

parentalguidance:_46  rdf:type  ebucore:TargetAudience ;
        skos:prefLabel    "TR-AISS"@en ;
        skos:scopeNote    "Region:Turkey" ;
        skos:definition   "Symbol system for content rating"@en ;
        skos:definition   "Akıllı İşaretler Sembol Sistemi"@tr ;
        skos:inScheme     <http://www.ebu.ch/metadata/ontologies/skos/ebu_ParentalGuidanceCodeCS> ;
        skos:narrower     parentalguidance:_46.1 ;
        skos:narrower     parentalguidance:_46.2 ;
        skos:changeNote   "Update" ;
        skos:historyNote  "2009-07-28" ;
        skos:example      "" ;
        skos:note         "Valid" .

parentalguidance:_46.1
        rdf:type          ebucore:TargetAudience ;
        skos:prefLabel    "Rating"@en ;
        skos:broader      parentalguidance:_46 ;
        skos:inScheme     <http://www.ebu.ch/metadata/ontologies/skos/ebu_ParentalGuidanceCodeCS> ;
        skos:narrower     parentalguidance:_46.1.1 ;
        skos:narrower     parentalguidance:_46.1.2 ;
        skos:narrower     parentalguidance:_46.1.3 ;
        skos:narrower     parentalguidance:_46.1.4 ;
        skos:changeNote   "" ;
        skos:historyNote  "" ;
        skos:example      "" .

parentalguidance:_46.1.1
        rdf:type          ebucore:TargetAudience ;
        skos:prefLabel    "All"@en ;
        skos:definition   "Genel izleyici kitlesi"@tr ;
        skos:definition   "Suitable for all ages"@en ;
        skos:broader      parentalguidance:_46.1 ;
        skos:inScheme     <http://www.ebu.ch/metadata/ontologies/skos/ebu_ParentalGuidanceCodeCS> ;
        skos:changeNote   "" ;
        skos:historyNote  "" ;
        skos:example      "" .

parentalguidance:_46.1.2
        rdf:type          ebucore:TargetAudience ;
        skos:prefLabel    "7+"@en ;
        skos:definition   "7 yaş ve üzeri için uygun"@tr ;
        skos:definition   "Suitable for children of at least 7 years of\n         age"@en ;
        skos:broader      parentalguidance:_46.1 ;
        skos:inScheme     <http://www.ebu.ch/metadata/ontologies/skos/ebu_ParentalGuidanceCodeCS> ;
        skos:changeNote   "" ;
        skos:historyNote  "" ;
        skos:example      "" .

parentalguidance:_46.1.3
        rdf:type          ebucore:TargetAudience ;
        skos:prefLabel    "13+"@en ;
        skos:definition   "13 yaş ve üzeri için uygun"@tr ;
        skos:definition   "Suitable for children of at least 11 years of\n         age"@en ;
        skos:broader      parentalguidance:_46.1 ;
        skos:inScheme     <http://www.ebu.ch/metadata/ontologies/skos/ebu_ParentalGuidanceCodeCS> ;
        skos:changeNote   "" ;
        skos:historyNote  "" ;
        skos:example      "" .

parentalguidance:_46.1.4
        rdf:type          ebucore:TargetAudience ;
        skos:prefLabel    "18+"@en ;
        skos:definition   "18 yaş ve üzeri için uygun"@tr ;
        skos:definition   "No one under 15 years of age admitted"@en ;
        skos:broader      parentalguidance:_46.1 ;
        skos:inScheme     <http://www.ebu.ch/metadata/ontologies/skos/ebu_ParentalGuidanceCodeCS> ;
        skos:changeNote   "" ;
        skos:historyNote  "" ;
        skos:example      "" .

parentalguidance:_46.2
        rdf:type          ebucore:TargetAudience ;
        skos:prefLabel    "Criteria"@en ;
        skos:broader      parentalguidance:_46 ;
        skos:inScheme     <http://www.ebu.ch/metadata/ontologies/skos/ebu_ParentalGuidanceCodeCS> ;
        skos:narrower     parentalguidance:_46.2.1 ;
        skos:narrower     parentalguidance:_46.2.2 ;
        skos:narrower     parentalguidance:_46.2.3 ;
        skos:changeNote   "" ;
        skos:historyNote  "" ;
        skos:example      "" .

parentalguidance:_46.2.1
        rdf:type          ebucore:TargetAudience ;
        skos:prefLabel    "Cinsellik içerir"@tr ;
        skos:prefLabel    "Sexual content"@en ;
        skos:broader      parentalguidance:_46.2 ;
        skos:inScheme     <http://www.ebu.ch/metadata/ontologies/skos/ebu_ParentalGuidanceCodeCS> ;
        skos:changeNote   "" ;
        skos:historyNote  "" ;
        skos:example      "" .

parentalguidance:_46.2.2
        rdf:type          ebucore:TargetAudience ;
        skos:prefLabel    "Şiddet ya da korku içerir"@tr ;
        skos:prefLabel    "Violence"@en ;
        skos:broader      parentalguidance:_46.2 ;
        skos:inScheme     <http://www.ebu.ch/metadata/ontologies/skos/ebu_ParentalGuidanceCodeCS> ;
        skos:changeNote   "" ;
        skos:historyNote  "" ;
        skos:example      "" .

parentalguidance:_46.2.3
        rdf:type          ebucore:TargetAudience ;
        skos:prefLabel    "Olumsuz örnek oluşturabilecek davranışlar içerir"@tr ;
        skos:prefLabel    "Negative behaviour"@en ;
        skos:broader      parentalguidance:_46.2 ;
        skos:inScheme     <http://www.ebu.ch/metadata/ontologies/skos/ebu_ParentalGuidanceCodeCS> ;
        skos:changeNote   "" ;
        skos:historyNote  "" ;
        skos:example      "" .

parentalguidance:_47  rdf:type  ebucore:TargetAudience ;
        skos:prefLabel    "US-ESRB"@en ;
        skos:scopeNote    "Region:United States"@en ;
        skos:definition   "Entertainment Software Rating Board scheme"@en ;
        skos:inScheme     <http://www.ebu.ch/metadata/ontologies/skos/ebu_ParentalGuidanceCodeCS> ;
        skos:narrower     parentalguidance:_47.1 ;
        skos:narrower     parentalguidance:_47.2 ;
        skos:changeNote   "Update" ;
        skos:historyNote  "2009-07-28" ;
        skos:example      "" ;
        skos:note         "Valid" .

parentalguidance:_47.1
        rdf:type          ebucore:TargetAudience ;
        skos:prefLabel    "Rating"@en ;
        skos:broader      parentalguidance:_47 ;
        skos:inScheme     <http://www.ebu.ch/metadata/ontologies/skos/ebu_ParentalGuidanceCodeCS> ;
        skos:narrower     parentalguidance:_47.1.1 ;
        skos:narrower     parentalguidance:_47.1.2 ;
        skos:narrower     parentalguidance:_47.1.3 ;
        skos:narrower     parentalguidance:_47.1.4 ;
        skos:narrower     parentalguidance:_47.1.5 ;
        skos:narrower     parentalguidance:_47.1.6 ;
        skos:narrower     parentalguidance:_47.1.7 ;
        skos:changeNote   "" ;
        skos:historyNote  "" ;
        skos:example      "" .

parentalguidance:_47.1.1
        rdf:type          ebucore:TargetAudience ;
        skos:prefLabel    "EC"@en ;
        skos:definition   "Titles rated EC (Early Childhood) have content that may be\n         suitable for ages 3 and older. Contains no material that parents would find\n         inappropriate" ;
        skos:broader      parentalguidance:_47.1 ;
        skos:inScheme     <http://www.ebu.ch/metadata/ontologies/skos/ebu_ParentalGuidanceCodeCS> ;
        skos:changeNote   "" ;
        skos:historyNote  "" ;
        skos:example      "" .

parentalguidance:_47.1.2
        rdf:type          ebucore:TargetAudience ;
        skos:prefLabel    "E"@en ;
        skos:definition   "Titles rated E (Everyone) have content that may be suitable for\n         ages 6 and older. Titles in this category may contain minimal cartoon, fantasy or mild\n         violence and/or infrequent use of mild language" ;
        skos:broader      parentalguidance:_47.1 ;
        skos:inScheme     <http://www.ebu.ch/metadata/ontologies/skos/ebu_ParentalGuidanceCodeCS> ;
        skos:changeNote   "" ;
        skos:historyNote  "" ;
        skos:example      "" .

parentalguidance:_47.1.3
        rdf:type          ebucore:TargetAudience ;
        skos:prefLabel    "E10+"@en ;
        skos:definition   "Titles rated E10+ (Everyone 10 and older) have content that may\n         be suitable for ages 10 and older. Titles in this category may contain more cartoon,\n         fantasy or mild violence, mild language and/or minimal suggestive themes" ;
        skos:broader      parentalguidance:_47.1 ;
        skos:inScheme     <http://www.ebu.ch/metadata/ontologies/skos/ebu_ParentalGuidanceCodeCS> ;
        skos:changeNote   "" ;
        skos:historyNote  "" ;
        skos:example      "" .

parentalguidance:_47.1.4
        rdf:type          ebucore:TargetAudience ;
        skos:prefLabel    "T"@en ;
        skos:definition   "Titles rated T (Teen) have content that may be suitable for ages\n         13 and older. Titles in this category may contain violence, suggestive themes, crude\n         humour, minimal blood, simulated gambling, and/or infrequent use of strong\n         language" ;
        skos:broader      parentalguidance:_47.1 ;
        skos:inScheme     <http://www.ebu.ch/metadata/ontologies/skos/ebu_ParentalGuidanceCodeCS> ;
        skos:changeNote   "" ;
        skos:historyNote  "" ;
        skos:example      "" .

parentalguidance:_47.1.5
        rdf:type          ebucore:TargetAudience ;
        skos:prefLabel    "M"@en ;
        skos:definition   "Titles rated M (Mature) have content that may be suitable for\n         persons ages 17 and older. Titles in this category may contain intense violence, blood and\n         gore, sexual content and/or strong language" ;
        skos:broader      parentalguidance:_47.1 ;
        skos:inScheme     <http://www.ebu.ch/metadata/ontologies/skos/ebu_ParentalGuidanceCodeCS> ;
        skos:changeNote   "" ;
        skos:historyNote  "" ;
        skos:example      "" .

parentalguidance:_47.1.6
        rdf:type          ebucore:TargetAudience ;
        skos:prefLabel    "AO"@en ;
        skos:definition   "Titles rated AO (Adults Only) have content that should only be\n         played by persons 18 years and older. Titles in this category may include prolonged scenes\n         of intense violence and/or graphic sexual content and nudity" ;
        skos:broader      parentalguidance:_47.1 ;
        skos:inScheme     <http://www.ebu.ch/metadata/ontologies/skos/ebu_ParentalGuidanceCodeCS> ;
        skos:changeNote   "" ;
        skos:historyNote  "" ;
        skos:example      "" .

parentalguidance:_47.1.7
        rdf:type          ebucore:TargetAudience ;
        skos:prefLabel    "RP"@en ;
        skos:definition   "Titles listed as RP (Rating Pending) have been submitted to the\n         ESRB and are awaiting final rating. (This symbol appears only in advertising prior to a\n         game's release)" ;
        skos:broader      parentalguidance:_47.1 ;
        skos:inScheme     <http://www.ebu.ch/metadata/ontologies/skos/ebu_ParentalGuidanceCodeCS> ;
        skos:changeNote   "" ;
        skos:historyNote  "" ;
        skos:example      "" .

parentalguidance:_47.2
        rdf:type          ebucore:TargetAudience ;
        skos:prefLabel    "Criteria"@en ;
        skos:broader      parentalguidance:_47 ;
        skos:inScheme     <http://www.ebu.ch/metadata/ontologies/skos/ebu_ParentalGuidanceCodeCS> ;
        skos:narrower     parentalguidance:_47.2.1 ;
        skos:narrower     parentalguidance:_47.2.2 ;
        skos:narrower     parentalguidance:_47.2.3 ;
        skos:narrower     parentalguidance:_47.2.4 ;
        skos:narrower     parentalguidance:_47.2.5 ;
        skos:narrower     parentalguidance:_47.2.6 ;
        skos:narrower     parentalguidance:_47.2.7 ;
        skos:narrower     parentalguidance:_47.2.8 ;
        skos:narrower     parentalguidance:_47.2.9 ;
        skos:narrower     parentalguidance:_47.2.10 ;
        skos:narrower     parentalguidance:_47.2.11 ;
        skos:narrower     parentalguidance:_47.2.12 ;
        skos:narrower     parentalguidance:_47.2.13 ;
        skos:narrower     parentalguidance:_47.2.14 ;
        skos:narrower     parentalguidance:_47.2.15 ;
        skos:narrower     parentalguidance:_47.2.16 ;
        skos:narrower     parentalguidance:_47.2.17 ;
        skos:narrower     parentalguidance:_47.2.18 ;
        skos:narrower     parentalguidance:_47.2.19 ;
        skos:narrower     parentalguidance:_47.2.20 ;
        skos:narrower     parentalguidance:_47.2.21 ;
        skos:narrower     parentalguidance:_47.2.22 ;
        skos:narrower     parentalguidance:_47.2.23 ;
        skos:narrower     parentalguidance:_47.2.24 ;
        skos:narrower     parentalguidance:_47.2.25 ;
        skos:narrower     parentalguidance:_47.2.26 ;
        skos:narrower     parentalguidance:_47.2.27 ;
        skos:narrower     parentalguidance:_47.2.28 ;
        skos:narrower     parentalguidance:_47.2.29 ;
        skos:narrower     parentalguidance:_47.2.30 ;
        skos:narrower     parentalguidance:_47.2.31 ;
        skos:narrower     parentalguidance:_47.2.32 ;
        skos:changeNote   "" ;
        skos:historyNote  "" ;
        skos:example      "" .

parentalguidance:_47.2.1
        rdf:type          ebucore:TargetAudience ;
        skos:prefLabel    "Alcohol Reference"@en ;
        skos:definition   "Reference to and/or images of alcoholic\n         beverages" ;
        skos:broader      parentalguidance:_47.2 ;
        skos:inScheme     <http://www.ebu.ch/metadata/ontologies/skos/ebu_ParentalGuidanceCodeCS> ;
        skos:changeNote   "" ;
        skos:historyNote  "" ;
        skos:example      "" .

parentalguidance:_47.2.2
        rdf:type          ebucore:TargetAudience ;
        skos:prefLabel    "Animated Blood"@en ;
        skos:definition   "Discoloured and/or unrealistic depictions of\n         blood" ;
        skos:broader      parentalguidance:_47.2 ;
        skos:inScheme     <http://www.ebu.ch/metadata/ontologies/skos/ebu_ParentalGuidanceCodeCS> ;
        skos:changeNote   "" ;
        skos:historyNote  "" ;
        skos:example      "" .

parentalguidance:_47.2.3
        rdf:type          ebucore:TargetAudience ;
        skos:prefLabel    "Blood"@en ;
        skos:definition   "Depictions of blood" ;
        skos:broader      parentalguidance:_47.2 ;
        skos:inScheme     <http://www.ebu.ch/metadata/ontologies/skos/ebu_ParentalGuidanceCodeCS> ;
        skos:changeNote   "" ;
        skos:historyNote  "" ;
        skos:example      "" .

parentalguidance:_47.2.4
        rdf:type          ebucore:TargetAudience ;
        skos:prefLabel    "Blood and Gore"@en ;
        skos:definition   "Depictions of blood or the mutilation of body\n         parts" ;
        skos:broader      parentalguidance:_47.2 ;
        skos:inScheme     <http://www.ebu.ch/metadata/ontologies/skos/ebu_ParentalGuidanceCodeCS> ;
        skos:changeNote   "" ;
        skos:historyNote  "" ;
        skos:example      "" .

parentalguidance:_47.2.5
        rdf:type          ebucore:TargetAudience ;
        skos:prefLabel    "Cartoon Violence"@en ;
        skos:definition   "Violent actions involving cartoon-like situations and characters.\n         May include violence where a character is unharmed after the action has been\n         inflicted" ;
        skos:broader      parentalguidance:_47.2 ;
        skos:inScheme     <http://www.ebu.ch/metadata/ontologies/skos/ebu_ParentalGuidanceCodeCS> ;
        skos:changeNote   "" ;
        skos:historyNote  "" ;
        skos:example      "" .

parentalguidance:_47.2.6
        rdf:type          ebucore:TargetAudience ;
        skos:prefLabel    "Comic Mischief"@en ;
        skos:definition   "Depictions or dialogue involving slapstick or suggestive\n         humour" ;
        skos:broader      parentalguidance:_47.2 ;
        skos:inScheme     <http://www.ebu.ch/metadata/ontologies/skos/ebu_ParentalGuidanceCodeCS> ;
        skos:changeNote   "" ;
        skos:historyNote  "" ;
        skos:example      "" .

parentalguidance:_47.2.7
        rdf:type          ebucore:TargetAudience ;
        skos:prefLabel    "Crude Humour"@en ;
        skos:definition   "Depictions or dialogue involving vulgar antics, including\n         'bathroom\" humour" ;
        skos:broader      parentalguidance:_47.2 ;
        skos:inScheme     <http://www.ebu.ch/metadata/ontologies/skos/ebu_ParentalGuidanceCodeCS> ;
        skos:changeNote   "" ;
        skos:historyNote  "" ;
        skos:example      "" .

parentalguidance:_47.2.8
        rdf:type          ebucore:TargetAudience ;
        skos:prefLabel    "Drug Reference"@en ;
        skos:definition   "Reference to and/or images of illegal drugs" ;
        skos:broader      parentalguidance:_47.2 ;
        skos:inScheme     <http://www.ebu.ch/metadata/ontologies/skos/ebu_ParentalGuidanceCodeCS> ;
        skos:changeNote   "" ;
        skos:historyNote  "" ;
        skos:example      "" .

parentalguidance:_47.2.9
        rdf:type          ebucore:TargetAudience ;
        skos:prefLabel    "Edutainment"@en ;
        skos:definition   "Content of product provides user with specific skills development\n         or reinforcement learning within an entertainment setting. Skill development is an integral\n         part of product" ;
        skos:broader      parentalguidance:_47.2 ;
        skos:inScheme     <http://www.ebu.ch/metadata/ontologies/skos/ebu_ParentalGuidanceCodeCS> ;
        skos:changeNote   "" ;
        skos:historyNote  "" ;
        skos:example      "" .

parentalguidance:_47.2.10
        rdf:type          ebucore:TargetAudience ;
        skos:prefLabel    "Fantasy Violence"@en ;
        skos:definition   "Violent actions of a fantasy nature, involving human or non-human\n         characters in situations easily distinguishable from real life" ;
        skos:broader      parentalguidance:_47.2 ;
        skos:inScheme     <http://www.ebu.ch/metadata/ontologies/skos/ebu_ParentalGuidanceCodeCS> ;
        skos:changeNote   "" ;
        skos:historyNote  "" ;
        skos:example      "" .

parentalguidance:_47.2.11
        rdf:type          ebucore:TargetAudience ;
        skos:prefLabel    "Informational"@en ;
        skos:definition   "Overall content of product contains data, facts, resource\n         information, reference materials or instructional text" ;
        skos:broader      parentalguidance:_47.2 ;
        skos:inScheme     <http://www.ebu.ch/metadata/ontologies/skos/ebu_ParentalGuidanceCodeCS> ;
        skos:changeNote   "" ;
        skos:historyNote  "" ;
        skos:example      "" .

parentalguidance:_47.2.12
        rdf:type          ebucore:TargetAudience ;
        skos:prefLabel    "Intense Violence"@en ;
        skos:definition   "Graphic and realistic-looking depictions of physical conflict.\n         May involve extreme and/or realistic blood, gore, weapons and depictions of human injury\n         and death" ;
        skos:broader      parentalguidance:_47.2 ;
        skos:inScheme     <http://www.ebu.ch/metadata/ontologies/skos/ebu_ParentalGuidanceCodeCS> ;
        skos:changeNote   "" ;
        skos:historyNote  "" ;
        skos:example      "" .

parentalguidance:_47.2.13
        rdf:type          ebucore:TargetAudience ;
        skos:prefLabel    "Language"@en ;
        skos:definition   "Mild to moderate use of profanity" ;
        skos:broader      parentalguidance:_47.2 ;
        skos:inScheme     <http://www.ebu.ch/metadata/ontologies/skos/ebu_ParentalGuidanceCodeCS> ;
        skos:changeNote   "" ;
        skos:historyNote  "" ;
        skos:example      "" .

parentalguidance:_47.2.14
        rdf:type          ebucore:TargetAudience ;
        skos:prefLabel    "Lyrics"@en ;
        skos:definition   "Mild references to profanity, sexuality, violence, alcohol or\n         drug use in music" ;
        skos:broader      parentalguidance:_47.2 ;
        skos:inScheme     <http://www.ebu.ch/metadata/ontologies/skos/ebu_ParentalGuidanceCodeCS> ;
        skos:changeNote   "" ;
        skos:historyNote  "" ;
        skos:example      "" .

parentalguidance:_47.2.15
        rdf:type          ebucore:TargetAudience ;
        skos:prefLabel    "Mature Humour"@en ;
        skos:definition   "Depictions or dialogue involving \"adult\" humour, including sexual\n         references" ;
        skos:broader      parentalguidance:_47.2 ;
        skos:inScheme     <http://www.ebu.ch/metadata/ontologies/skos/ebu_ParentalGuidanceCodeCS> ;
        skos:changeNote   "" ;
        skos:historyNote  "" ;
        skos:example      "" .

parentalguidance:_47.2.16
        rdf:type          ebucore:TargetAudience ;
        skos:prefLabel    "Mild Violence"@en ;
        skos:definition   "Mild scenes depicting characters in unsafe and/or violent\n         situations" ;
        skos:broader      parentalguidance:_47.2 ;
        skos:inScheme     <http://www.ebu.ch/metadata/ontologies/skos/ebu_ParentalGuidanceCodeCS> ;
        skos:changeNote   "" ;
        skos:historyNote  "" ;
        skos:example      "" .

parentalguidance:_47.2.17
        rdf:type          ebucore:TargetAudience ;
        skos:prefLabel    "Nudity"@en ;
        skos:definition   "Graphic or prolonged depictions of nudity" ;
        skos:broader      parentalguidance:_47.2 ;
        skos:inScheme     <http://www.ebu.ch/metadata/ontologies/skos/ebu_ParentalGuidanceCodeCS> ;
        skos:changeNote   "" ;
        skos:historyNote  "" ;
        skos:example      "" .

parentalguidance:_47.2.18
        rdf:type          ebucore:TargetAudience ;
        skos:prefLabel    "Partial Nudity"@en ;
        skos:definition   "Brief and/or mild depictions of nudity" ;
        skos:broader      parentalguidance:_47.2 ;
        skos:inScheme     <http://www.ebu.ch/metadata/ontologies/skos/ebu_ParentalGuidanceCodeCS> ;
        skos:changeNote   "" ;
        skos:historyNote  "" ;
        skos:example      "" .

parentalguidance:_47.2.19
        rdf:type          ebucore:TargetAudience ;
        skos:prefLabel    "Real Gambling"@en ;
        skos:definition   "Player can gamble, including betting or wagering real cash or\n         currency" ;
        skos:broader      parentalguidance:_47.2 ;
        skos:inScheme     <http://www.ebu.ch/metadata/ontologies/skos/ebu_ParentalGuidanceCodeCS> ;
        skos:changeNote   "" ;
        skos:historyNote  "" ;
        skos:example      "" .

parentalguidance:_47.2.20
        rdf:type          ebucore:TargetAudience ;
        skos:prefLabel    "Sexual Themes"@en ;
        skos:definition   "Mild to moderate sexual references and/or depictions. May include\n         partial nudity" ;
        skos:broader      parentalguidance:_47.2 ;
        skos:inScheme     <http://www.ebu.ch/metadata/ontologies/skos/ebu_ParentalGuidanceCodeCS> ;
        skos:changeNote   "" ;
        skos:historyNote  "" ;
        skos:example      "" .

parentalguidance:_47.2.21
        rdf:type          ebucore:TargetAudience ;
        skos:prefLabel    "Sexual Violence"@en ;
        skos:definition   "Depictions of rape or other violent sexual acts" ;
        skos:broader      parentalguidance:_47.2 ;
        skos:inScheme     <http://www.ebu.ch/metadata/ontologies/skos/ebu_ParentalGuidanceCodeCS> ;
        skos:changeNote   "" ;
        skos:historyNote  "" ;
        skos:example      "" .

parentalguidance:_47.2.22
        rdf:type          ebucore:TargetAudience ;
        skos:prefLabel    "Simulated Gambling"@en ;
        skos:definition   "Player can gamble without betting or wagering real cash or\n         currency" ;
        skos:broader      parentalguidance:_47.2 ;
        skos:inScheme     <http://www.ebu.ch/metadata/ontologies/skos/ebu_ParentalGuidanceCodeCS> ;
        skos:changeNote   "" ;
        skos:historyNote  "" ;
        skos:example      "" .

parentalguidance:_47.2.23
        rdf:type          ebucore:TargetAudience ;
        skos:prefLabel    "Some Adult Assistance May Be Needed"@en ;
        skos:definition   "Intended for very young ages" ;
        skos:broader      parentalguidance:_47.2 ;
        skos:inScheme     <http://www.ebu.ch/metadata/ontologies/skos/ebu_ParentalGuidanceCodeCS> ;
        skos:changeNote   "" ;
        skos:historyNote  "" ;
        skos:example      "" .

parentalguidance:_47.2.24
        rdf:type          ebucore:TargetAudience ;
        skos:prefLabel    "Strong Language"@en ;
        skos:definition   "Explicit and/or frequent use of profanity" ;
        skos:broader      parentalguidance:_47.2 ;
        skos:inScheme     <http://www.ebu.ch/metadata/ontologies/skos/ebu_ParentalGuidanceCodeCS> ;
        skos:changeNote   "" ;
        skos:historyNote  "" ;
        skos:example      "" .

parentalguidance:_47.2.25
        rdf:type          ebucore:TargetAudience ;
        skos:prefLabel    "Strong Lyrics"@en ;
        skos:definition   "Explicit and/or frequent references to profanity, sex, violence,\n         alcohol or drug use in music" ;
        skos:broader      parentalguidance:_47.2 ;
        skos:inScheme     <http://www.ebu.ch/metadata/ontologies/skos/ebu_ParentalGuidanceCodeCS> ;
        skos:changeNote   "" ;
        skos:historyNote  "" ;
        skos:example      "" .

parentalguidance:_47.2.26
        rdf:type          ebucore:TargetAudience ;
        skos:prefLabel    "Strong Sexual Content"@en ;
        skos:definition   "Graphic references to and/or depictions of sexual behaviour,\n         possibly including nudity" ;
        skos:broader      parentalguidance:_47.2 ;
        skos:inScheme     <http://www.ebu.ch/metadata/ontologies/skos/ebu_ParentalGuidanceCodeCS> ;
        skos:changeNote   "" ;
        skos:historyNote  "" ;
        skos:example      "" .

parentalguidance:_47.2.27
        rdf:type          ebucore:TargetAudience ;
        skos:prefLabel    "Suggestive Themes"@en ;
        skos:definition   "Mild provocative references or materials" ;
        skos:broader      parentalguidance:_47.2 ;
        skos:inScheme     <http://www.ebu.ch/metadata/ontologies/skos/ebu_ParentalGuidanceCodeCS> ;
        skos:changeNote   "" ;
        skos:historyNote  "" ;
        skos:example      "" .

parentalguidance:_47.2.28
        rdf:type          ebucore:TargetAudience ;
        skos:prefLabel    "Tobacco Reference"@en ;
        skos:definition   "Reference to and/or images of tobacco products" ;
        skos:broader      parentalguidance:_47.2 ;
        skos:inScheme     <http://www.ebu.ch/metadata/ontologies/skos/ebu_ParentalGuidanceCodeCS> ;
        skos:changeNote   "" ;
        skos:historyNote  "" ;
        skos:example      "" .

parentalguidance:_47.2.29
        rdf:type          ebucore:TargetAudience ;
        skos:prefLabel    "Use of Drugs"@en ;
        skos:definition   "The consumption or use of illegal drugs" ;
        skos:broader      parentalguidance:_47.2 ;
        skos:inScheme     <http://www.ebu.ch/metadata/ontologies/skos/ebu_ParentalGuidanceCodeCS> ;
        skos:changeNote   "" ;
        skos:historyNote  "" ;
        skos:example      "" .

parentalguidance:_47.2.30
        rdf:type          ebucore:TargetAudience ;
        skos:prefLabel    "Use of Alcohol"@en ;
        skos:definition   "The consumption of alcoholic beverages" ;
        skos:broader      parentalguidance:_47.2 ;
        skos:inScheme     <http://www.ebu.ch/metadata/ontologies/skos/ebu_ParentalGuidanceCodeCS> ;
        skos:changeNote   "" ;
        skos:historyNote  "" ;
        skos:example      "" .

parentalguidance:_47.2.31
        rdf:type          ebucore:TargetAudience ;
        skos:prefLabel    "Use of Tobacco"@en ;
        skos:definition   "The consumption of tobacco products" ;
        skos:broader      parentalguidance:_47.2 ;
        skos:inScheme     <http://www.ebu.ch/metadata/ontologies/skos/ebu_ParentalGuidanceCodeCS> ;
        skos:changeNote   "" ;
        skos:historyNote  "" ;
        skos:example      "" .

parentalguidance:_47.2.32
        rdf:type          ebucore:TargetAudience ;
        skos:prefLabel    "Violence"@en ;
        skos:definition   "Scenes involving aggressive conflict" ;
        skos:broader      parentalguidance:_47.2 ;
        skos:inScheme     <http://www.ebu.ch/metadata/ontologies/skos/ebu_ParentalGuidanceCodeCS> ;
        skos:changeNote   "" ;
        skos:historyNote  "" ;
        skos:example      "" .

parentalguidance:_48  rdf:type  ebucore:TargetAudience ;
        skos:prefLabel    "US-MPAA"@en ;
        skos:altLabel     "Motion Picture Association"@en ;
        skos:scopeNote    "Region:United States"@en ;
        skos:definition   "Motion Picture Association of America movie rating scheme"@en ;
        skos:inScheme     <http://www.ebu.ch/metadata/ontologies/skos/ebu_ParentalGuidanceCodeCS> ;
        skos:narrower     parentalguidance:_48.1 ;
        skos:narrower     parentalguidance:_48.2 ;
        skos:narrower     parentalguidance:_48.3 ;
        skos:narrower     parentalguidance:_48.4 ;
        skos:narrower     parentalguidance:_48.5 ;
        skos:narrower     parentalguidance:_48.6 ;
        skos:changeNote   "Update" ;
        skos:historyNote  "2009-07-27" ;
        skos:example      "" ;
        skos:note         "Valid" .

parentalguidance:_48.1
        rdf:type          ebucore:TargetAudience ;
        skos:prefLabel    "G"@en ;
        skos:altLabel    "General"@en ;
        skos:definition   "General audiences. All ages admitted."@en ;
        skos:broader      parentalguidance:_48 ;
        skos:inScheme     <http://www.ebu.ch/metadata/ontologies/skos/ebu_ParentalGuidanceCodeCS> ;
        skos:changeNote   "" ;
        skos:historyNote  "" ;
        skos:example      "" .

parentalguidance:_48.2
        rdf:type          ebucore:TargetAudience ;
        skos:prefLabel     "PG"@en ;
        skos:altLabel    "Parental Guidance"@en ;
        skos:definition   "Parental guidance suggested. Theme or content may not be\n         suitable for children."@en ;
        skos:broader      parentalguidance:_48 ;
        skos:inScheme     <http://www.ebu.ch/metadata/ontologies/skos/ebu_ParentalGuidanceCodeCS> ;
        skos:changeNote   "" ;
        skos:historyNote  "" ;
        skos:example      "" .

parentalguidance:_48.3
        rdf:type          ebucore:TargetAudience ;
        skos:prefLabel    "PG-13"@en ;
        skos:definition   "Parents strongly cautioned"@en ;
        skos:definition   "Some material may be inappropriate for children under 13. "@en ;
        skos:broader      parentalguidance:_48 ;
        skos:inScheme     <http://www.ebu.ch/metadata/ontologies/skos/ebu_ParentalGuidanceCodeCS> ;
        skos:changeNote   "" ;
        skos:historyNote  "" ;
        skos:example      "" .

parentalguidance:_48.4
        rdf:type          ebucore:TargetAudience ;
        skos:prefLabel    "R"@en ;
        skos:altLabel    "Restricted"@en ;
        skos:definition   "Under 17 requires accompyning parent or adult guardian. "@en ;
        skos:broader      parentalguidance:_48 ;
        skos:inScheme     <http://www.ebu.ch/metadata/ontologies/skos/ebu_ParentalGuidanceCodeCS> ;
        skos:changeNote   "" ;
        skos:historyNote  "" ;
        skos:example      "" .

parentalguidance:_48.5
        rdf:type          ebucore:TargetAudience ;
        skos:prefLabel    "NC-17"@en ;
        skos:definition   "Not one 17 and under admitted."@en ;
        skos:broader      parentalguidance:_48 ;
        skos:inScheme     <http://www.ebu.ch/metadata/ontologies/skos/ebu_ParentalGuidanceCodeCS> ;
        skos:changeNote   "" ;
        skos:historyNote  "" ;
        skos:example      "" ;
        skos:hiddenLabel  "adult"@en .

parentalguidance:_48.6
        rdf:type          ebucore:TargetAudience ;
        skos:prefLabel    "NR"@en ;
        skos:altLabel     "UR"@en ;
        skos:definition   "Not rated or Unrated"@en ;
        skos:broader      parentalguidance:_48 ;
        skos:inScheme     <http://www.ebu.ch/metadata/ontologies/skos/ebu_ParentalGuidanceCodeCS> ;
        skos:changeNote   "" ;
        skos:historyNote  "" ;
        skos:example      "" .

parentalguidance:_48.7
        rdf:type          ebucore:TargetAudience ;
        skos:prefLabel    "TV-14"@en ;
        skos:definition   "Parents strongly cautioned"@en ;
        skos:broader      parentalguidance:_48 ;
        skos:inScheme     <http://www.ebu.ch/metadata/ontologies/skos/ebu_ParentalGuidanceCodeCS> ;
        skos:changeNote   "" ;
        skos:historyNote  "" ;
        skos:example      "" .

parentalguidance:_49  rdf:type  ebucore:TargetAudience ;
        skos:prefLabel    "US-RIAA"@en ;
        skos:scopeNote    "Region:United States"@en ;
        skos:definition   "Recording Industry Association of America scheme. Scheme for\n         music rating as defined by the Recording Industry Association of America"@en ;
        skos:inScheme     <http://www.ebu.ch/metadata/ontologies/skos/ebu_ParentalGuidanceCodeCS> ;
        skos:narrower     parentalguidance:_49.1 ;
        skos:changeNote   "Update" ;
        skos:historyNote  "2009-07-28" ;
        skos:example      "" ;
        skos:note         "Valid" .

parentalguidance:_49.1
        rdf:type          ebucore:TargetAudience ;
        skos:prefLabel    "Parental Advisory"@en ;
        skos:definition   "The Parental Advisory is a notice to consumers that recordings\n         identified by this value may contain strong language or depiction of violence, sex or\n         substance abuse. Parental discretion is advised" ;
        skos:broader      parentalguidance:_49 ;
        skos:inScheme     <http://www.ebu.ch/metadata/ontologies/skos/ebu_ParentalGuidanceCodeCS> ;
        skos:changeNote   "" ;
        skos:historyNote  "" ;
        skos:example      "" .

parentalguidance:_50  rdf:type ebucore:TargetAudience ;
        skos:prefLabel "US-TVPG"@en ;
        skos:altLabel "US-V-Chip"@en ;
        skos:altLabel "USA Parental Rating"@en ;
        skos:altLabel "USA_PR"@en ;
        skos:scopeNote "Region: United States"@en ;
        skos:definition "The US TV Parental Guidelines system (V-Chip)"@en ;
        skos:inScheme <http://www.ebu.ch/metadata/ontologies/skos/ebu_ParentalGuidanceCodeCS> ;
        skos:narrower parentalguidance:_50.1 ;
        skos:narrower parentalguidance:_50.2 .

parentalguidance:_50.1 rdf:type ebucore:TargetAudience ;
        skos:prefLabel "Ratings"@en ;
        skos:broader parentalguidance:_50 ;
        skos:inScheme <http://www.ebu.ch/metadata/ontologies/skos/ebu_ParentalGuidanceCodeCS> ;
        skos:narrower parentalguidance:_50.1.1 ;
        skos:narrower parentalguidance:_50.1.2 ;
        skos:narrower parentalguidance:_50.1.3 ;
        skos:narrower parentalguidance:_50.1.4 ;
        skos:narrower parentalguidance:_50.1.5 ;
        skos:narrower parentalguidance:_50.1.6 .

parentalguidance:_50.1.1 rdf:type ebucore:TargetAudience ;
        skos:prefLabel "TV-Y"@en ;
        skos:definition "All Children"@en ;
        skos:broader parentalguidance:_50.1 ;
        skos:inScheme <http://www.ebu.ch/metadata/ontologies/skos/ebu_ParentalGuidanceCodeCS> .

parentalguidance:_50.1.2 rdf:type ebucore:TargetAudience ;
        skos:prefLabel "TV-Y7"@en ;
        skos:definition "Directed to Older Children"@en ;
        skos:broader parentalguidance:_50.1 ;
        skos:inScheme <http://www.ebu.ch/metadata/ontologies/skos/ebu_ParentalGuidanceCodeCS> ;
        skos:narrower parentalguidance:_50.1.2.1 .

parentalguidance:_50.1.2.1 rdf:type ebucore:TargetAudience ;
        skos:prefLabel "TV-Y7-FV"@en ;
        skos:definition "Directed to Older Children - Fantasy Violence"@en ;
        skos:broader parentalguidance:_50.1.2 ;
        skos:inScheme <http://www.ebu.ch/metadata/ontologies/skos/ebu_ParentalGuidanceCodeCS> .

parentalguidance:_50.1.3 rdf:type ebucore:TargetAudience ;
        skos:prefLabel "TV-G"@en ;
        skos:definition "General Audience"@en ;
        skos:broader parentalguidance:_50.1 ;
        skos:inScheme <http://www.ebu.ch/metadata/ontologies/skos/ebu_ParentalGuidanceCodeCS> .

parentalguidance:_50.1.4 rdf:type ebucore:TargetAudience ;
        skos:prefLabel "TV-PG"@en ;
        skos:definition "Parental Guidance Suggested"@en ;
        skos:broader parentalguidance:_50.1 ;
        skos:inScheme <http://www.ebu.ch/metadata/ontologies/skos/ebu_ParentalGuidanceCodeCS> .

parentalguidance:_50.1.5 rdf:type ebucore:TargetAudience ;
        skos:prefLabel "TV-14"@en ;
        skos:definition "Parents Strongly Cautioned"@en ;
        skos:broader parentalguidance:_50.1 ;
        skos:inScheme <http://www.ebu.ch/metadata/ontologies/skos/ebu_ParentalGuidanceCodeCS> .

parentalguidance:_50.1.6 rdf:type ebucore:TargetAudience ;
        skos:prefLabel "TV-MA"@en ;
        skos:definition "Mature Audience Only"@en ;
        skos:broader parentalguidance:_50.1 ;
        skos:inScheme <http://www.ebu.ch/metadata/ontologies/skos/ebu_ParentalGuidanceCodeCS> .

parentalguidance:_50.2 rdf:type ebucore:TargetAudience ;
        skos:prefLabel "Criteria"@en ;
        skos:broader parentalguidance:_50 ;
        skos:inScheme <http://www.ebu.ch/metadata/ontologies/skos/ebu_ParentalGuidanceCodeCS> ;
        skos:narrower parentalguidance:_50.2.1 ;
        skos:narrower parentalguidance:_50.2.2 ;
        skos:narrower parentalguidance:_50.2.3 ;
        skos:narrower parentalguidance:_50.2.4 .

parentalguidance:_50.2.1 rdf:type ebucore:TargetAudience ;
        skos:prefLabel "V"@en ;
        skos:definition "Violence"@en ;
        skos:broader parentalguidance:_50.2 ;
        skos:inScheme <http://www.ebu.ch/metadata/ontologies/skos/ebu_ParentalGuidanceCodeCS> .

parentalguidance:_50.2.2 rdf:type ebucore:TargetAudience ;
        skos:prefLabel "L"@en ;
        skos:definition "Coarse Language"@en ;
        skos:broader parentalguidance:_50.2 ;
        skos:inScheme <http://www.ebu.ch/metadata/ontologies/skos/ebu_ParentalGuidanceCodeCS> .

parentalguidance:_50.2.3 rdf:type ebucore:TargetAudience ;
        skos:prefLabel "S"@en ;
        skos:definition "Sexual Content"@en ;
        skos:broader parentalguidance:_50.2 ;
        skos:inScheme <http://www.ebu.ch/metadata/ontologies/skos/ebu_ParentalGuidanceCodeCS> .

parentalguidance:_50.2.4 rdf:type ebucore:TargetAudience ;
        skos:prefLabel "D"@en ;
        skos:definition "Suggestive Dialogue"@en ;
        skos:broader parentalguidance:_50.2 ;
        skos:inScheme <http://www.ebu.ch/metadata/ontologies/skos/ebu_ParentalGuidanceCodeCS> .

parentalguidance:_51  rdf:type  ebucore:TargetAudience ;
        skos:prefLabel    "ZA-FPB"@en ;
        skos:definition   "Film and Publication Board"@en ;
        skos:scopeNote    "Region:South Africa"@en ;
        skos:inScheme     <http://www.ebu.ch/metadata/ontologies/skos/ebu_ParentalGuidanceCodeCS> ;
        skos:narrower     parentalguidance:_51.1 ;
        skos:narrower     parentalguidance:_51.2 ;
        skos:changeNote   "Update" ;
        skos:historyNote  "2009-07-28" ;
        skos:example      "" ;
        skos:note         "Valid" .

parentalguidance:_51.1
        rdf:type          ebucore:TargetAudience ;
        skos:prefLabel    "Rating"@en ;
        skos:broader      parentalguidance:_51 ;
        skos:inScheme     <http://www.ebu.ch/metadata/ontologies/skos/ebu_ParentalGuidanceCodeCS> ;
        skos:narrower     parentalguidance:_51.1.1 ;
        skos:narrower     parentalguidance:_51.1.2 ;
        skos:narrower     parentalguidance:_51.1.3 ;
        skos:narrower     parentalguidance:_51.1.4 ;
        skos:narrower     parentalguidance:_51.1.5 ;
        skos:narrower     parentalguidance:_51.1.6 ;
        skos:narrower     parentalguidance:_51.1.7 ;
        skos:changeNote   "" ;
        skos:historyNote  "" ;
        skos:example      "" .

parentalguidance:_51.1.1
        rdf:type          ebucore:TargetAudience ;
        skos:prefLabel    "A"@en ;
        skos:definition   "All ages"@en ;
        skos:broader      parentalguidance:_51.1 ;
        skos:inScheme     <http://www.ebu.ch/metadata/ontologies/skos/ebu_ParentalGuidanceCodeCS> ;
        skos:changeNote   "" ;
        skos:historyNote  "" ;
        skos:example      "" .

parentalguidance:_51.1.2
        rdf:type          ebucore:TargetAudience ;
        skos:prefLabel    "PG"@en ;
        skos:definition   "A category with content that may be disturbing to or\n         inappropriate for children"@en ;
        skos:broader      parentalguidance:_51.1 ;
        skos:inScheme     <http://www.ebu.ch/metadata/ontologies/skos/ebu_ParentalGuidanceCodeCS> ;
        skos:changeNote   "" ;
        skos:historyNote  "" ;
        skos:example      "" .

parentalguidance:_51.1.3
        rdf:type          ebucore:TargetAudience ;
        skos:prefLabel    "10M"@en ;
        skos:definition   "Children under the age of 10 years must be accompanied by an\n         adult"@en ;
        skos:broader      parentalguidance:_51.1 ;
        skos:inScheme     <http://www.ebu.ch/metadata/ontologies/skos/ebu_ParentalGuidanceCodeCS> ;
        skos:changeNote   "" ;
        skos:historyNote  "" ;
        skos:example      "" .

parentalguidance:_51.1.4
        rdf:type          ebucore:TargetAudience ;
        skos:prefLabel    "10M-13PG"@en ;
        skos:definition   "Persons under the age of 13 must be accompanied by an adult to\n         any filem classfied 13M, while a DVB or VHS or an interactive computer game classfied 13 PG\n         requires Parental Guidance for persons under the age of 13"@en ;
        skos:broader      parentalguidance:_51.1 ;
        skos:inScheme     <http://www.ebu.ch/metadata/ontologies/skos/ebu_ParentalGuidanceCodeCS> ;
        skos:changeNote   "" ;
        skos:historyNote  "" ;
        skos:example      "" .

parentalguidance:_51.1.5
        rdf:type          ebucore:TargetAudience ;
        skos:prefLabel    "10"@en ;
        skos:definition   "10 years and older only"@en ;
        skos:broader      parentalguidance:_51.1 ;
        skos:inScheme     <http://www.ebu.ch/metadata/ontologies/skos/ebu_ParentalGuidanceCodeCS> ;
        skos:changeNote   "" ;
        skos:historyNote  "" ;
        skos:example      "" .

parentalguidance:_51.1.6
        rdf:type          ebucore:TargetAudience ;
        skos:prefLabel    "16"@en ;
        skos:definition   "16 years and older only"@en ;
        skos:broader      parentalguidance:_51.1 ;
        skos:inScheme     <http://www.ebu.ch/metadata/ontologies/skos/ebu_ParentalGuidanceCodeCS> ;
        skos:changeNote   "" ;
        skos:historyNote  "" ;
        skos:example      "" .

parentalguidance:_51.1.7
        rdf:type          ebucore:TargetAudience ;
        skos:prefLabel    "18"@en ;
        skos:definition   "Adults only"@en ;
        skos:broader      parentalguidance:_51.1 ;
        skos:inScheme     <http://www.ebu.ch/metadata/ontologies/skos/ebu_ParentalGuidanceCodeCS> ;
        skos:changeNote   "" ;
        skos:historyNote  "" ;
        skos:example      "" .

parentalguidance:_51.2
        rdf:type          ebucore:TargetAudience ;
        skos:prefLabel    "Criteria"@en ;
        skos:broader      parentalguidance:_51 ;
        skos:inScheme     <http://www.ebu.ch/metadata/ontologies/skos/ebu_ParentalGuidanceCodeCS> ;
        skos:narrower     parentalguidance:_51.2.1 ;
        skos:narrower     parentalguidance:_51.2.2 ;
        skos:narrower     parentalguidance:_51.2.3 ;
        skos:narrower     parentalguidance:_51.2.4 ;
        skos:narrower     parentalguidance:_51.2.5 ;
        skos:narrower     parentalguidance:_51.2.6 ;
        skos:changeNote   "" ;
        skos:historyNote  "" ;
        skos:example      "" .

parentalguidance:_51.2.1
        rdf:type          ebucore:TargetAudience ;
        skos:prefLabel    "D"@en ;
        skos:definition   "Drug and alocohol abuse"@en ;
        skos:broader      parentalguidance:_51.2 ;
        skos:inScheme     <http://www.ebu.ch/metadata/ontologies/skos/ebu_ParentalGuidanceCodeCS> ;
        skos:changeNote   "" ;
        skos:historyNote  "" ;
        skos:example      "" .

parentalguidance:_51.2.2
        rdf:type          ebucore:TargetAudience ;
        skos:prefLabel    "L"@en ;
        skos:definition   "Strong language"@en ;
        skos:broader      parentalguidance:_51.2 ;
        skos:inScheme     <http://www.ebu.ch/metadata/ontologies/skos/ebu_ParentalGuidanceCodeCS> ;
        skos:changeNote   "" ;
        skos:historyNote  "" ;
        skos:example      "" .

parentalguidance:_51.2.3
        rdf:type          ebucore:TargetAudience ;
        skos:prefLabel    "N"@en ;
        skos:definition   "Nudity"@en ;
        skos:broader      parentalguidance:_51.2 ;
        skos:inScheme     <http://www.ebu.ch/metadata/ontologies/skos/ebu_ParentalGuidanceCodeCS> ;
        skos:changeNote   "" ;
        skos:historyNote  "" ;
        skos:example      "" .

parentalguidance:_51.2.4
        rdf:type          ebucore:TargetAudience ;
        skos:prefLabel    "P"@en ;
        skos:definition   "Biased or prejudiced with regard to race, ethnicity, gender,\n         religion, or other group identifiable characteristics"@en ;
        skos:broader      parentalguidance:_51.2 ;
        skos:inScheme     <http://www.ebu.ch/metadata/ontologies/skos/ebu_ParentalGuidanceCodeCS> ;
        skos:changeNote   "" ;
        skos:historyNote  "" ;
        skos:example      "" .

parentalguidance:_51.2.5
        rdf:type          ebucore:TargetAudience ;
        skos:prefLabel    "S"@en ;
        skos:definition   "Sex"@en ;
        skos:broader      parentalguidance:_51.2 ;
        skos:inScheme     <http://www.ebu.ch/metadata/ontologies/skos/ebu_ParentalGuidanceCodeCS> ;
        skos:changeNote   "" ;
        skos:historyNote  "" ;
        skos:example      "" .

parentalguidance:_51.2.6
        rdf:type          ebucore:TargetAudience ;
        skos:prefLabel    "V"@en ;
        skos:definition   "Violence"@en ;
        skos:broader      parentalguidance:_51.2 ;
        skos:inScheme     <http://www.ebu.ch/metadata/ontologies/skos/ebu_ParentalGuidanceCodeCS> ;
        skos:changeNote   "" ;
        skos:historyNote  "" ;
        skos:example      "" .

parentalguidance:_52  rdf:type  ebucore:TargetAudience ;
        skos:prefLabel    "DE-USK"@en ;
        skos:scopeNote    "Region:Germany" ;
        skos:definition   "UnterhaltungSoftware SebstKontrolle"@de ;
        skos:definition   "Entertianment and software self control"@en ;
        skos:inScheme     <http://www.ebu.ch/metadata/ontologies/skos/ebu_ParentalGuidanceCodeCS> ;
        skos:narrower     parentalguidance:_52.1 ;
        skos:narrower     parentalguidance:_52.2 ;
        skos:narrower     parentalguidance:_52.3 ;
        skos:narrower     parentalguidance:_52.4 ;
        skos:narrower     parentalguidance:_52.5 ;
        skos:changeNote   "Change subterm termId from 18.x to 52.x" ;
        skos:historyNote  "2019-06-24" ;
        skos:example      "" ;
        skos:note         "Valid" .

parentalguidance:_52.1
        rdf:type          ebucore:TargetAudience ;
        skos:prefLabel    "ALL"@en ;
        skos:prefLabel    "ALL AGES"@de ;
        skos:definition   "For all ages"@en ;
        skos:definition   "Ohne Altersbeschränkung"@de ;
        skos:broader      parentalguidance:_52 ;
        skos:inScheme     <http://www.ebu.ch/metadata/ontologies/skos/ebu_ParentalGuidanceCodeCS> ;
        skos:changeNote   "Change termId from 18.x to 52.x" ;
        skos:historyNote  "2019-06-24" ;
        skos:example      "" .

parentalguidance:_52.2
        rdf:type          ebucore:TargetAudience ;
        skos:prefLabel    "6+"@en ;
        skos:prefLabel    "6+"@de ;
        skos:definition   "No one under 6 years admitted"@en ;
        skos:definition   "Freigegeben ab 6 Jahren"@de ;
        skos:broader      parentalguidance:_52 ;
        skos:inScheme     <http://www.ebu.ch/metadata/ontologies/skos/ebu_ParentalGuidanceCodeCS> ;
        skos:changeNote   "Change termId from 18.x to 52.x" ;
        skos:historyNote  "2019-06-24" ;
        skos:example      "" .

parentalguidance:_52.3
        rdf:type          ebucore:TargetAudience ;
        skos:prefLabel    "12+"@en ;
        skos:prefLabel    "12+"@de ;
        skos:definition   "People 12 or older admitted, children between 6 and 11 only\n         when accompanied by parent or legal guardian"@en ;
        skos:definition   "Freigegeben ab 12 Jahren"@de ;
        skos:broader      parentalguidance:_52 ;
        skos:inScheme     <http://www.ebu.ch/metadata/ontologies/skos/ebu_ParentalGuidanceCodeCS> ;
        skos:changeNote   "Change termId from 18.x to 52.x" ;
        skos:historyNote  "2019-06-24" ;
        skos:example      "" .

parentalguidance:_52.4
        rdf:type          ebucore:TargetAudience ;
        skos:prefLabel    "16+"@en ;
        skos:prefLabel    "16+"@de ;
        skos:definition   "People 16 or older admitted"@en ;
        skos:definition   "Freigegeben ab 16 Jahren"@de ;
        skos:broader      parentalguidance:_52 ;
        skos:inScheme     <http://www.ebu.ch/metadata/ontologies/skos/ebu_ParentalGuidanceCodeCS> ;
        skos:changeNote   "Change termId from 18.x to 52.x" ;
        skos:historyNote  "2019-06-24" ;
        skos:example      "" .

parentalguidance:_52.5
        rdf:type          ebucore:TargetAudience ;
        skos:prefLabel    "18+"@en ;
        skos:prefLabel    "18+"@de ;
        skos:definition   "\"No youth admitted\", only adults"@en ;
        skos:definition   "Keine Jugendfreigabe"@de ;
        skos:broader      parentalguidance:_52 ;
        skos:inScheme     <http://www.ebu.ch/metadata/ontologies/skos/ebu_ParentalGuidanceCodeCS> ;
        skos:changeNote   "Change termId from 18.x to 52.x" ;
        skos:historyNote  "2019-06-24" ;
        skos:example      "" .

parentalguidance:_53  rdf:type  ebucore:TargetAudience ;
        skos:prefLabel    "CZ-Film"@en ;
        skos:definition   ""@en ;
        skos:scopeNote    "Region:Czech republic"@en ;
        skos:inScheme     <http://www.ebu.ch/metadata/ontologies/skos/ebu_ParentalGuidanceCodeCS> ;
        skos:narrower     parentalguidance:_53.1 ;
        skos:changeNote   "Update" ;
        skos:historyNote  "2010-08-03" ;
        skos:example      "" ;
        skos:note         "Valid" .

parentalguidance:_53.1
        rdf:type          ebucore:TargetAudience ;
        skos:prefLabel    "Rating"@en ;
        skos:broader      parentalguidance:_53 ;
        skos:inScheme     <http://www.ebu.ch/metadata/ontologies/skos/ebu_ParentalGuidanceCodeCS> ;
        skos:narrower     parentalguidance:_53.1.1 ;
        skos:narrower     parentalguidance:_53.1.2 ;
        skos:narrower     parentalguidance:_53.1.3 ;
        skos:narrower     parentalguidance:_53.1.4 ;
        skos:narrower     parentalguidance:_53.1.5 ;
        skos:changeNote   "" ;
        skos:historyNote  "" ;
        skos:example      "" .

parentalguidance:_53.1.1
        rdf:type          ebucore:TargetAudience ;
        skos:prefLabel    "U"@en ;
        skos:definition   "Suitable for all audiences "@en ;
        skos:broader      parentalguidance:_53.1 ;
        skos:inScheme     <http://www.ebu.ch/metadata/ontologies/skos/ebu_ParentalGuidanceCodeCS> ;
        skos:changeNote   "" ;
        skos:historyNote  "" ;
        skos:example      "" .

parentalguidance:_53.1.2
        rdf:type          ebucore:TargetAudience ;
        skos:prefLabel    "12"@en ;
        skos:definition   ""@en ;
        skos:broader      parentalguidance:_53.1 ;
        skos:inScheme     <http://www.ebu.ch/metadata/ontologies/skos/ebu_ParentalGuidanceCodeCS> ;
        skos:changeNote   "" ;
        skos:historyNote  "" ;
        skos:example      "" .

parentalguidance:_53.1.3
        rdf:type          ebucore:TargetAudience ;
        skos:prefLabel    "15"@en ;
        skos:definition   ""@en ;
        skos:broader      parentalguidance:_53.1 ;
        skos:inScheme     <http://www.ebu.ch/metadata/ontologies/skos/ebu_ParentalGuidanceCodeCS> ;
        skos:changeNote   "" ;
        skos:historyNote  "" ;
        skos:example      "" .

parentalguidance:_53.1.4
        rdf:type          ebucore:TargetAudience ;
        skos:prefLabel    "18"@en ;
        skos:definition   ""@en ;
        skos:broader      parentalguidance:_53.1 ;
        skos:inScheme     <http://www.ebu.ch/metadata/ontologies/skos/ebu_ParentalGuidanceCodeCS> ;
        skos:changeNote   "" ;
        skos:historyNote  "" ;
        skos:example      "" .

parentalguidance:_53.1.5
        rdf:type          ebucore:TargetAudience ;
        skos:prefLabel    "E"@en ;
        skos:definition   "Exempt from classification"@en ;
        skos:broader      parentalguidance:_53.1 ;
        skos:inScheme     <http://www.ebu.ch/metadata/ontologies/skos/ebu_ParentalGuidanceCodeCS> ;
        skos:changeNote   "" ;
        skos:historyNote  "" ;
        skos:example      "" .

parentalguidance:_54  rdf:type  ebucore:TargetAudience ;
        skos:prefLabel    "HU-Film"@en ;
        skos:scopeNote    "Region:Hungary"@en ;
        skos:definition   "National Film Office"@en ;
        skos:inScheme     <http://www.ebu.ch/metadata/ontologies/skos/ebu_ParentalGuidanceCodeCS> ;
        skos:narrower     parentalguidance:_54.1 ;
        skos:changeNote   "Update" ;
        skos:historyNote  "2010-08-03" ;
        skos:example      "" ;
        skos:note         "Valid" .

parentalguidance:_54.1
        rdf:type          ebucore:TargetAudience ;
        skos:prefLabel    "Rating"@en ;
        skos:broader      parentalguidance:_54 ;
        skos:inScheme     <http://www.ebu.ch/metadata/ontologies/skos/ebu_ParentalGuidanceCodeCS> ;
        skos:narrower     parentalguidance:_54.1.1 ;
        skos:narrower     parentalguidance:_54.1.2 ;
        skos:narrower     parentalguidance:_54.1.3 ;
        skos:narrower     parentalguidance:_54.1.4 ;
        skos:narrower     parentalguidance:_54.1.5 ;
        skos:changeNote   "" ;
        skos:historyNote  "" ;
        skos:example      "" .

parentalguidance:_54.1.1
        rdf:type          ebucore:TargetAudience ;
        skos:prefLabel    "KN"@en ;
        skos:definition   "suitable for all (category I.) "@en ;
        skos:broader      parentalguidance:_54.1 ;
        skos:inScheme     <http://www.ebu.ch/metadata/ontologies/skos/ebu_ParentalGuidanceCodeCS> ;
        skos:changeNote   "" ;
        skos:historyNote  "" ;
        skos:example      "" .

parentalguidance:_54.1.2
        rdf:type          ebucore:TargetAudience ;
        skos:prefLabel    "12"@en ;
        skos:definition   "parental guidance suggested for children under 12. (category\n         II.) "@en ;
        skos:broader      parentalguidance:_54.1 ;
        skos:inScheme     <http://www.ebu.ch/metadata/ontologies/skos/ebu_ParentalGuidanceCodeCS> ;
        skos:changeNote   "" ;
        skos:historyNote  "" ;
        skos:example      "" .

parentalguidance:_54.1.3
        rdf:type          ebucore:TargetAudience ;
        skos:prefLabel    "16"@en ;
        skos:definition   "not suitable for children under 16. (category III.) "@en ;
        skos:broader      parentalguidance:_54.1 ;
        skos:inScheme     <http://www.ebu.ch/metadata/ontologies/skos/ebu_ParentalGuidanceCodeCS> ;
        skos:changeNote   "" ;
        skos:historyNote  "" ;
        skos:example      "" .

parentalguidance:_54.1.4
        rdf:type          ebucore:TargetAudience ;
        skos:prefLabel    "18"@en ;
        skos:definition   "not suitable for people under 18. (category IV.) "@en ;
        skos:broader      parentalguidance:_54.1 ;
        skos:inScheme     <http://www.ebu.ch/metadata/ontologies/skos/ebu_ParentalGuidanceCodeCS> ;
        skos:changeNote   "" ;
        skos:historyNote  "" ;
        skos:example      "" .

parentalguidance:_54.1.5
        rdf:type          ebucore:TargetAudience ;
        skos:prefLabel    "X"@en ;
        skos:definition   "only for adults (category V.) "@en ;
        skos:broader      parentalguidance:_54.1 ;
        skos:inScheme     <http://www.ebu.ch/metadata/ontologies/skos/ebu_ParentalGuidanceCodeCS> ;
        skos:changeNote   "" ;
        skos:historyNote  "" ;
        skos:example      "" .

parentalguidance:_55  rdf:type  ebucore:TargetAudience ;
        skos:prefLabel    "IS-Smais"@en ;
        skos:scopeNote    "Region:Iceland"@en ;
        skos:definition   "National Film Office"@en ;
        skos:inScheme     <http://www.ebu.ch/metadata/ontologies/skos/ebu_ParentalGuidanceCodeCS> ;
        skos:narrower     parentalguidance:_55.1 ;
        skos:changeNote   "Correct subterm termId 54.1.5 into 55.1.5" ;
        skos:historyNote  "2019-06-24" ;
        skos:example      "" ;
        skos:note         "Valid" .

parentalguidance:_55.1
        rdf:type          ebucore:TargetAudience ;
        skos:prefLabel    "Rating"@en ;
        skos:broader      parentalguidance:_55 ;
        skos:inScheme     <http://www.ebu.ch/metadata/ontologies/skos/ebu_ParentalGuidanceCodeCS> ;
        skos:narrower     parentalguidance:_55.1.1 ;
        skos:narrower     parentalguidance:_55.1.2 ;
        skos:narrower     parentalguidance:_55.1.3 ;
        skos:narrower     parentalguidance:_55.1.4 ;
        skos:narrower     parentalguidance:_55.1.5 ;
        skos:narrower     parentalguidance:_55.1.6 ;
        skos:changeNote   "" ;
        skos:historyNote  "" ;
        skos:example      "" .

parentalguidance:_55.1.1
        rdf:type          ebucore:TargetAudience ;
        skos:prefLabel    "L"@en ;
        skos:definition   "Suitable for all "@en ;
        skos:broader      parentalguidance:_55.1 ;
        skos:inScheme     <http://www.ebu.ch/metadata/ontologies/skos/ebu_ParentalGuidanceCodeCS> ;
        skos:changeNote   "" ;
        skos:historyNote  "" ;
        skos:example      "" .

parentalguidance:_55.1.2
        rdf:type          ebucore:TargetAudience ;
        skos:prefLabel    "7"@en ;
        skos:definition   "Passed only for 7 and older "@en ;
        skos:broader      parentalguidance:_55.1 ;
        skos:inScheme     <http://www.ebu.ch/metadata/ontologies/skos/ebu_ParentalGuidanceCodeCS> ;
        skos:changeNote   "" ;
        skos:historyNote  "" ;
        skos:example      "" .

parentalguidance:_55.1.3
        rdf:type          ebucore:TargetAudience ;
        skos:prefLabel    "12"@en ;
        skos:definition   "Passed only for 12 and older "@en ;
        skos:broader      parentalguidance:_55.1 ;
        skos:inScheme     <http://www.ebu.ch/metadata/ontologies/skos/ebu_ParentalGuidanceCodeCS> ;
        skos:changeNote   "" ;
        skos:historyNote  "" ;
        skos:example      "" .

parentalguidance:_55.1.4
        rdf:type          ebucore:TargetAudience ;
        skos:prefLabel    "14"@en ;
        skos:definition   "Passed only for 14 and older "@en ;
        skos:broader      parentalguidance:_55.1 ;
        skos:inScheme     <http://www.ebu.ch/metadata/ontologies/skos/ebu_ParentalGuidanceCodeCS> ;
        skos:changeNote   "" ;
        skos:historyNote  "" ;
        skos:example      "" .

parentalguidance:_55.1.5
        rdf:type          ebucore:TargetAudience ;
        skos:prefLabel    "16"@en ;
        skos:definition   "Passed only for 16 and older "@en ;
        skos:broader      parentalguidance:_55.1 ;
        skos:inScheme     <http://www.ebu.ch/metadata/ontologies/skos/ebu_ParentalGuidanceCodeCS> ;
        skos:changeNote   "" ;
        skos:historyNote  "" ;
        skos:example      "" .

parentalguidance:_55.1.6
        rdf:type          ebucore:TargetAudience ;
        skos:prefLabel    "18"@en ;
        skos:definition   "Passed only for 18 and older "@en ;
        skos:broader      parentalguidance:_55.1 ;
        skos:inScheme     <http://www.ebu.ch/metadata/ontologies/skos/ebu_ParentalGuidanceCodeCS> ;
        skos:changeNote   "" ;
        skos:historyNote  "" ;
        skos:example      "" .

parentalguidance:_56  rdf:type  ebucore:TargetAudience ;
        skos:prefLabel    "IN-CBFC"@en ;
        skos:altLabel     "Central Board of Film Certification"@en ;
        skos:altLabel     "India Content Provider"@en ;
        skos:scopeNote    "Region:India"@en ;
        skos:definition   "Film Board"@en ;
        skos:inScheme     <http://www.ebu.ch/metadata/ontologies/skos/ebu_ParentalGuidanceCodeCS> ;
        skos:narrower     parentalguidance:_56.1 ;
        skos:changeNote   "Update" ;
        skos:historyNote  "2010-08-03" ;
        skos:example      "" ;
        skos:note         "Valid" .

parentalguidance:_56.1
        rdf:type          ebucore:TargetAudience ;
        skos:prefLabel    "Rating"@en ;
        skos:broader      parentalguidance:_56 ;
        skos:inScheme     <http://www.ebu.ch/metadata/ontologies/skos/ebu_ParentalGuidanceCodeCS> ;
        skos:narrower     parentalguidance:_56.1.1 ;
        skos:narrower     parentalguidance:_56.1.2 ;
        skos:narrower     parentalguidance:_56.1.3 ;
        skos:narrower     parentalguidance:_56.1.4 ;
        skos:narrower     parentalguidance:_56.1.5 ;
        skos:narrower     parentalguidance:_56.1.6 ;
        skos:changeNote   "" ;
        skos:historyNote  "" ;
        skos:example      "" .

parentalguidance:_56.1.1
        rdf:type          ebucore:TargetAudience ;
        skos:prefLabel    "U"@en ;
        skos:definition   "Unrestricted Public Exhibition throughout India"@en ;
        skos:broader      parentalguidance:_56.1 ;
        skos:inScheme     <http://www.ebu.ch/metadata/ontologies/skos/ebu_ParentalGuidanceCodeCS> ;
        skos:changeNote   "" ;
        skos:historyNote  "" ;
        skos:example      "" .

parentalguidance:_56.1.2
        rdf:type          ebucore:TargetAudience ;
        skos:prefLabel    "U/A 7+"@en ;
        skos:definition   "Suitable for children aged 7 and above with parental guidance"@en ;
        skos:broader      parentalguidance:_56.1 ;
        skos:inScheme     <http://www.ebu.ch/metadata/ontologies/skos/ebu_ParentalGuidanceCodeCS> ;
        skos:changeNote   "" ;
        skos:historyNote  "" ;
        skos:example      "" .

parentalguidance:_56.1.3
        rdf:type          ebucore:TargetAudience ;
        skos:prefLabel    "U/A 13+"@en ;
        skos:definition   "Suitable for children aged 13 and above with parental guidance"@en ;
        skos:broader      parentalguidance:_56.1 ;
        skos:inScheme     <http://www.ebu.ch/metadata/ontologies/skos/ebu_ParentalGuidanceCodeCS> ;
        skos:changeNote   "" ;
        skos:historyNote  "" ;
        skos:example      "" .

parentalguidance:_56.1.4
        rdf:type          ebucore:TargetAudience ;
        skos:prefLabel    "U/A 16+"@en ;
        skos:definition   "Suitable for children aged 16 and above with parental guidance"@en ;
        skos:broader      parentalguidance:_56.1 ;
        skos:inScheme     <http://www.ebu.ch/metadata/ontologies/skos/ebu_ParentalGuidanceCodeCS> ;
        skos:changeNote   "" ;
        skos:historyNote  "" ;
        skos:example      "" .

parentalguidance:_56.1.5
        rdf:type          ebucore:TargetAudience ;
        skos:prefLabel    "A"@en ;
        skos:definition   "Public exhibition restricted to adults above 18 years only"@en ;
        skos:broader      parentalguidance:_56.1 ;
        skos:inScheme     <http://www.ebu.ch/metadata/ontologies/skos/ebu_ParentalGuidanceCodeCS> ;
        skos:changeNote   "" ;
        skos:historyNote  "" ;
        skos:example      "" .

parentalguidance:_56.1.6
        rdf:type          ebucore:TargetAudience ;
        skos:prefLabel    "S"@en ;
        skos:definition   "Exhibition to restricted audience such as doctors etc."@en ;
        skos:broader      parentalguidance:_56.1 ;
        skos:inScheme     <http://www.ebu.ch/metadata/ontologies/skos/ebu_ParentalGuidanceCodeCS> ;
        skos:changeNote   "" ;
        skos:historyNote  "" ;
        skos:example      "" .

parentalguidance:_57  rdf:type  ebucore:TargetAudience ;
        skos:prefLabel    "EG-Film"@en ;
        skos:scopeNote    "Region:Egypt"@en ;
        skos:definition   "Film Board"@en ;
        skos:inScheme     <http://www.ebu.ch/metadata/ontologies/skos/ebu_ParentalGuidanceCodeCS> ;
        skos:narrower     parentalguidance:_57.1 ;
        skos:changeNote   "Update" ;
        skos:historyNote  "2010-08-03" ;
        skos:example      "" ;
        skos:note         "Valid" .

parentalguidance:_57.1
        rdf:type          ebucore:TargetAudience ;
        skos:prefLabel    "Rating"@en ;
        skos:broader      parentalguidance:_57 ;
        skos:inScheme     <http://www.ebu.ch/metadata/ontologies/skos/ebu_ParentalGuidanceCodeCS> ;
        skos:narrower     parentalguidance:_57.1.1 ;
        skos:narrower     parentalguidance:_57.1.2 ;
        skos:narrower     parentalguidance:_57.1.3 ;
        skos:changeNote   "" ;
        skos:historyNote  "" ;
        skos:example      "" .

parentalguidance:_57.1.1
        rdf:type          ebucore:TargetAudience ;
        skos:prefLabel    "General Audience"@en ;
        skos:definition   "Everyone is admitted"@en ;
        skos:broader      parentalguidance:_57.1 ;
        skos:inScheme     <http://www.ebu.ch/metadata/ontologies/skos/ebu_ParentalGuidanceCodeCS> ;
        skos:changeNote   "" ;
        skos:historyNote  "" ;
        skos:example      "" .

parentalguidance:_57.1.2
        rdf:type          ebucore:TargetAudience ;
        skos:prefLabel    "Adults Only"@en ;
        skos:definition   "Restricted to audiences aged 18 and above"@en ;
        skos:broader      parentalguidance:_57.1 ;
        skos:inScheme     <http://www.ebu.ch/metadata/ontologies/skos/ebu_ParentalGuidanceCodeCS> ;
        skos:changeNote   "" ;
        skos:historyNote  "" ;
        skos:example      "" .

parentalguidance:_57.1.3
        rdf:type          ebucore:TargetAudience ;
        skos:prefLabel    "Exempt from classification"@en ;
        skos:definition   ""@en ;
        skos:broader      parentalguidance:_57.1 ;
        skos:inScheme     <http://www.ebu.ch/metadata/ontologies/skos/ebu_ParentalGuidanceCodeCS> ;
        skos:changeNote   "" ;
        skos:historyNote  "" ;
        skos:example      "" .

parentalguidance:_58  rdf:type  ebucore:TargetAudience ;
        skos:prefLabel    "ES-Film"@en ;
        skos:scopeNote    "Region:Estonia"@en ;
        skos:definition   "Film Board"@en ;
        skos:inScheme     <http://www.ebu.ch/metadata/ontologies/skos/ebu_ParentalGuidanceCodeCS> ;
        skos:narrower     parentalguidance:_58.1 ;
        skos:changeNote   "Update" ;
        skos:historyNote  "2010-08-03" ;
        skos:example      "" ;
        skos:note         "Valid" .

parentalguidance:_58.1
        rdf:type          ebucore:TargetAudience ;
        skos:prefLabel    "Rating"@en ;
        skos:broader      parentalguidance:_58 ;
        skos:inScheme     <http://www.ebu.ch/metadata/ontologies/skos/ebu_ParentalGuidanceCodeCS> ;
        skos:narrower     parentalguidance:_58.1.1 ;
        skos:narrower     parentalguidance:_58.1.2 ;
        skos:narrower     parentalguidance:_58.1.3 ;
        skos:narrower     parentalguidance:_58.1.4 ;
        skos:narrower     parentalguidance:_58.1.5 ;
        skos:narrower     parentalguidance:_58.1.6 ;
        skos:narrower     parentalguidance:_58.1.7 ;
        skos:narrower     parentalguidance:_58.1.8 ;
        skos:changeNote   "" ;
        skos:historyNote  "" ;
        skos:example      "" .

parentalguidance:_58.1.1
        rdf:type          ebucore:TargetAudience ;
        skos:prefLabel    "Pere"@en ;
        skos:definition   "Family film"@en ;
        skos:broader      parentalguidance:_58.1 ;
        skos:inScheme     <http://www.ebu.ch/metadata/ontologies/skos/ebu_ParentalGuidanceCodeCS> ;
        skos:changeNote   "" ;
        skos:historyNote  "" ;
        skos:example      "" .

parentalguidance:_58.1.2
        rdf:type          ebucore:TargetAudience ;
        skos:prefLabel    "L"@en ;
        skos:definition   "For all audiences"@en ;
        skos:broader      parentalguidance:_58.1 ;
        skos:inScheme     <http://www.ebu.ch/metadata/ontologies/skos/ebu_ParentalGuidanceCodeCS> ;
        skos:changeNote   "" ;
        skos:historyNote  "" ;
        skos:example      "" .

parentalguidance:_58.1.3
        rdf:type          ebucore:TargetAudience ;
        skos:prefLabel    "MS-6"@en ;
        skos:definition   "Younger than 6 Not Recommended "@en ;
        skos:broader      parentalguidance:_58.1 ;
        skos:inScheme     <http://www.ebu.ch/metadata/ontologies/skos/ebu_ParentalGuidanceCodeCS> ;
        skos:changeNote   "" ;
        skos:historyNote  "" ;
        skos:example      "" .

parentalguidance:_58.1.4
        rdf:type          ebucore:TargetAudience ;
        skos:prefLabel    "MS-12"@en ;
        skos:definition   "Younger than 12 Not Recommended "@en ;
        skos:broader      parentalguidance:_58.1 ;
        skos:inScheme     <http://www.ebu.ch/metadata/ontologies/skos/ebu_ParentalGuidanceCodeCS> ;
        skos:changeNote   "" ;
        skos:historyNote  "" ;
        skos:example      "" .

parentalguidance:_58.1.5
        rdf:type          ebucore:TargetAudience ;
        skos:prefLabel    "K-12"@en ;
        skos:definition   "Younger than 12 Prohibited"@en ;
        skos:broader      parentalguidance:_58.1 ;
        skos:inScheme     <http://www.ebu.ch/metadata/ontologies/skos/ebu_ParentalGuidanceCodeCS> ;
        skos:changeNote   "" ;
        skos:historyNote  "" ;
        skos:example      "" .

parentalguidance:_58.1.6
        rdf:type          ebucore:TargetAudience ;
        skos:prefLabel    "K-14"@en ;
        skos:definition   "Younger than 14 Prohibited"@en ;
        skos:broader      parentalguidance:_58.1 ;
        skos:inScheme     <http://www.ebu.ch/metadata/ontologies/skos/ebu_ParentalGuidanceCodeCS> ;
        skos:changeNote   "" ;
        skos:historyNote  "" ;
        skos:example      "" .

parentalguidance:_58.1.7
        rdf:type          ebucore:TargetAudience ;
        skos:prefLabel    "K-16"@en ;
        skos:definition   "Younger than 16 Prohibited"@en ;
        skos:broader      parentalguidance:_58.1 ;
        skos:inScheme     <http://www.ebu.ch/metadata/ontologies/skos/ebu_ParentalGuidanceCodeCS> ;
        skos:changeNote   "" ;
        skos:historyNote  "" ;
        skos:example      "" .

parentalguidance:_58.1.8
        rdf:type          ebucore:TargetAudience ;
        skos:prefLabel    "K-6"@en ;
        skos:definition   "Younger than 6 Prohibited. Commonly know as\n         K-E"@en ;
        skos:broader      parentalguidance:_58.1 ;
        skos:inScheme     <http://www.ebu.ch/metadata/ontologies/skos/ebu_ParentalGuidanceCodeCS> ;
        skos:changeNote   "" ;
        skos:historyNote  "" ;
        skos:example      "" .

parentalguidance:_59  rdf:type  ebucore:TargetAudience ;
        skos:prefLabel    "GR-Film"@en ;
        skos:scopeNote    "Region:Greece"@en ;
        skos:definition   "Film Board"@en ;
        skos:inScheme     <http://www.ebu.ch/metadata/ontologies/skos/ebu_ParentalGuidanceCodeCS> ;
        skos:narrower     parentalguidance:_59.1 ;
        skos:changeNote   "Update" ;
        skos:historyNote  "2010-08-03" ;
        skos:example      "" ;
        skos:note         "Valid" .

parentalguidance:_59.1
        rdf:type          ebucore:TargetAudience ;
        skos:prefLabel    "Rating"@en ;
        skos:broader      parentalguidance:_59 ;
        skos:inScheme     <http://www.ebu.ch/metadata/ontologies/skos/ebu_ParentalGuidanceCodeCS> ;
        skos:narrower     parentalguidance:_59.1.1 ;
        skos:narrower     parentalguidance:_59.1.2 ;
        skos:narrower     parentalguidance:_59.1.3 ;
        skos:narrower     parentalguidance:_59.1.4 ;
        skos:changeNote   "" ;
        skos:historyNote  "" ;
        skos:example      "" .

parentalguidance:_59.1.1
        rdf:type          ebucore:TargetAudience ;
        skos:prefLabel    "K"@en ;
        skos:definition   "Suitable film for everyone, including children. The film does\n         not contain violence, drug abuse, or sexual content."@en ;
        skos:broader      parentalguidance:_59.1 ;
        skos:inScheme     <http://www.ebu.ch/metadata/ontologies/skos/ebu_ParentalGuidanceCodeCS> ;
        skos:changeNote   "" ;
        skos:historyNote  "" ;
        skos:example      "" .

parentalguidance:_59.1.2
        rdf:type          ebucore:TargetAudience ;
        skos:prefLabel    "K-13"@en ;
        skos:definition   "Suitable film for children over the age of 13. The film may\n         contain mild violence and adult themes. "@en ;
        skos:broader      parentalguidance:_59.1 ;
        skos:inScheme     <http://www.ebu.ch/metadata/ontologies/skos/ebu_ParentalGuidanceCodeCS> ;
        skos:changeNote   "" ;
        skos:historyNote  "" ;
        skos:example      "" .

parentalguidance:_59.1.3
        rdf:type          ebucore:TargetAudience ;
        skos:prefLabel    "K-17"@en ;
        skos:definition   "Suitable film for adults over the age of 17. The film may\n         contain violence, drug abuse, and mild pornographic scenes. An ID card certifying the age\n         is required in all Greek cinemas and DVD rental shops in order to get a cinema ticket or\n         rent a DVD of a \"K-17\" rated film. This category is legally restricted. "@en ;
        skos:broader      parentalguidance:_59.1 ;
        skos:inScheme     <http://www.ebu.ch/metadata/ontologies/skos/ebu_ParentalGuidanceCodeCS> ;
        skos:changeNote   "" ;
        skos:historyNote  "" ;
        skos:example      "" .

parentalguidance:_59.1.4
        rdf:type          ebucore:TargetAudience ;
        skos:prefLabel    "E"@en ;
        skos:definition   "Exempt from classification "@en ;
        skos:broader      parentalguidance:_59.1 ;
        skos:inScheme     <http://www.ebu.ch/metadata/ontologies/skos/ebu_ParentalGuidanceCodeCS> ;
        skos:changeNote   "" ;
        skos:historyNote  "" ;
        skos:example      "" .

parentalguidance:_60  rdf:type  ebucore:TargetAudience ;
        skos:prefLabel    "ID-LSF"@en ;
        skos:altLabel     "Lembaga Sensor Film"@en ;
        skos:scopeNote    "Region:Indonesia"@en ;
        skos:definition   "Lembaga Sensor Film"@en ;
        skos:inScheme     <http://www.ebu.ch/metadata/ontologies/skos/ebu_ParentalGuidanceCodeCS> ;
        skos:narrower     parentalguidance:_60.1 ;
        skos:changeNote   "Update" ;
        skos:historyNote  "2010-08-03" ;
        skos:example      "" ;
        skos:note         "Valid" .

parentalguidance:_60.1
        rdf:type          ebucore:TargetAudience ;
        skos:prefLabel    "Rating"@en ;
        skos:broader      parentalguidance:_60 ;
        skos:inScheme     <http://www.ebu.ch/metadata/ontologies/skos/ebu_ParentalGuidanceCodeCS> ;
        skos:narrower     parentalguidance:_60.1.1 ;
        skos:narrower     parentalguidance:_60.1.2 ;
        skos:narrower     parentalguidance:_60.1.3 ;
        skos:narrower     parentalguidance:_60.1.4 ;
        skos:narrower     parentalguidance:_60.1.5 ;
        skos:changeNote   "" ;
        skos:historyNote  "" ;
        skos:example      "" .

parentalguidance:_60.1.1
        rdf:type          ebucore:TargetAudience ;
        skos:prefLabel    "SU"@en ;
        skos:definition   "(Semua Umur): All ages "@en ;
        skos:broader      parentalguidance:_60.1 ;
        skos:inScheme     <http://www.ebu.ch/metadata/ontologies/skos/ebu_ParentalGuidanceCodeCS> ;
        skos:changeNote   "" ;
        skos:historyNote  "" ;
        skos:example      "" .

parentalguidance:_60.1.2
        rdf:type          ebucore:TargetAudience ;
        skos:prefLabel    "A"@en ;
        skos:definition   "(Anak-anak): Children (3–12 years) "@en ;
        skos:broader      parentalguidance:_60.1 ;
        skos:inScheme     <http://www.ebu.ch/metadata/ontologies/skos/ebu_ParentalGuidanceCodeCS> ;
        skos:changeNote   "" ;
        skos:historyNote  "" ;
        skos:example      "" .

parentalguidance:_60.1.3
        rdf:type          ebucore:TargetAudience ;
        skos:prefLabel    "BO"@en ;
        skos:definition   "BO (Bimbingan Orangtua): Parental Guidance (parental\n         supervision is recommended for persons under 13 years) "@en ;
        skos:broader      parentalguidance:_60.1 ;
        skos:inScheme     <http://www.ebu.ch/metadata/ontologies/skos/ebu_ParentalGuidanceCodeCS> ;
        skos:changeNote   "" ;
        skos:historyNote  "" ;
        skos:example      "" .

parentalguidance:_60.1.4
        rdf:type          ebucore:TargetAudience ;
        skos:prefLabel    "R"@en ;
        skos:definition   "Remaja): Teen (13–15 years and over) "@en ;
        skos:broader      parentalguidance:_60.1 ;
        skos:inScheme     <http://www.ebu.ch/metadata/ontologies/skos/ebu_ParentalGuidanceCodeCS> ;
        skos:changeNote   "" ;
        skos:historyNote  "" ;
        skos:example      "" .

parentalguidance:_60.1.5
        rdf:type          ebucore:TargetAudience ;
        skos:prefLabel    "D"@en ;
        skos:definition   "(Dewasa): Mature (17 years and over) "@en ;
        skos:broader      parentalguidance:_60.1 ;
        skos:inScheme     <http://www.ebu.ch/metadata/ontologies/skos/ebu_ParentalGuidanceCodeCS> ;
        skos:changeNote   "" ;
        skos:historyNote  "" ;
        skos:example      "" .

parentalguidance:_61  rdf:type  ebucore:TargetAudience ;
        skos:prefLabel    "LV-NCC"@en ;
        skos:scopeNote    "Region:Latvia"@en ;
        skos:definition   "Nacionālais Kino Centrs"@lv ;
        skos:definition   "National Cinema Center"@en ;
        skos:inScheme     <http://www.ebu.ch/metadata/ontologies/skos/ebu_ParentalGuidanceCodeCS> ;
        skos:narrower     parentalguidance:_61.1 ;
        skos:changeNote   "Update" ;
        skos:historyNote  "2010-08-03" ;
        skos:example      "" ;
        skos:note         "Valid" .

parentalguidance:_61.1
        rdf:type          ebucore:TargetAudience ;
        skos:prefLabel    "Rating"@en ;
        skos:broader      parentalguidance:_61 ;
        skos:inScheme     <http://www.ebu.ch/metadata/ontologies/skos/ebu_ParentalGuidanceCodeCS> ;
        skos:narrower     parentalguidance:_61.1.1 ;
        skos:narrower     parentalguidance:_61.1.2 ;
        skos:narrower     parentalguidance:_61.1.3 ;
        skos:narrower     parentalguidance:_61.1.4 ;
        skos:narrower     parentalguidance:_61.1.5 ;
        skos:narrower     parentalguidance:_61.1.6 ;
        skos:changeNote   "" ;
        skos:historyNote  "" ;
        skos:example      "" .

parentalguidance:_61.1.1
        rdf:type          ebucore:TargetAudience ;
        skos:prefLabel    "U"@en ;
        skos:definition   "rated for all ages (added in July 2007)."@en ;
        skos:broader      parentalguidance:_61.1 ;
        skos:inScheme     <http://www.ebu.ch/metadata/ontologies/skos/ebu_ParentalGuidanceCodeCS> ;
        skos:changeNote   "" ;
        skos:historyNote  "" ;
        skos:example      "" .

parentalguidance:_61.1.2
        rdf:type          ebucore:TargetAudience ;
        skos:prefLabel    "7+"@en ;
        skos:definition   "Not recommended until 7 "@en ;
        skos:broader      parentalguidance:_61.1 ;
        skos:inScheme     <http://www.ebu.ch/metadata/ontologies/skos/ebu_ParentalGuidanceCodeCS> ;
        skos:changeNote   "" ;
        skos:historyNote  "" ;
        skos:example      "" .

parentalguidance:_61.1.3
        rdf:type          ebucore:TargetAudience ;
        skos:prefLabel    "12+"@en ;
        skos:definition   "Not recommended until 12 "@en ;
        skos:broader      parentalguidance:_61.1 ;
        skos:inScheme     <http://www.ebu.ch/metadata/ontologies/skos/ebu_ParentalGuidanceCodeCS> ;
        skos:changeNote   "" ;
        skos:historyNote  "" ;
        skos:example      "" .

parentalguidance:_61.1.4
        rdf:type          ebucore:TargetAudience ;
        skos:prefLabel    "16+"@en ;
        skos:definition   "Not recommended until 16 "@en ;
        skos:broader      parentalguidance:_61.1 ;
        skos:inScheme     <http://www.ebu.ch/metadata/ontologies/skos/ebu_ParentalGuidanceCodeCS> ;
        skos:changeNote   "" ;
        skos:historyNote  "" ;
        skos:example      "" .

parentalguidance:_61.1.5
        rdf:type          ebucore:TargetAudience ;
        skos:prefLabel    "18+ (blue)"@en ;
        skos:definition   "Not recommended until 18 "@en ;
        skos:broader      parentalguidance:_61.1 ;
        skos:inScheme     <http://www.ebu.ch/metadata/ontologies/skos/ebu_ParentalGuidanceCodeCS> ;
        skos:changeNote   "" ;
        skos:historyNote  "" ;
        skos:example      "" .

parentalguidance:_61.1.6
        rdf:type          ebucore:TargetAudience ;
        skos:prefLabel    "18+ (red)"@en ;
        skos:definition   "Prohibited for minors "@en ;
        skos:broader      parentalguidance:_61.1 ;
        skos:inScheme     <http://www.ebu.ch/metadata/ontologies/skos/ebu_ParentalGuidanceCodeCS> ;
        skos:changeNote   "" ;
        skos:historyNote  "" ;
        skos:example      "" .

parentalguidance:_62  rdf:type  ebucore:TargetAudience ;
        skos:prefLabel    "MA-FCB"@en ;
        skos:scopeNote    "Region:Malaysia"@en ;
        skos:definition   "Film Censorship Board"@en ;
        skos:inScheme     <http://www.ebu.ch/metadata/ontologies/skos/ebu_ParentalGuidanceCodeCS> ;
        skos:narrower     parentalguidance:_62.1 ;
        skos:changeNote   "Update" ;
        skos:historyNote  "2010-08-03" ;
        skos:example      "" ;
        skos:note         "Valid" .

parentalguidance:_62.1
        rdf:type          ebucore:TargetAudience ;
        skos:prefLabel    "Rating"@en ;
        skos:broader      parentalguidance:_62 ;
        skos:inScheme     <http://www.ebu.ch/metadata/ontologies/skos/ebu_ParentalGuidanceCodeCS> ;
        skos:narrower     parentalguidance:_62.1.1 ;
        skos:narrower     parentalguidance:_62.1.2 ;
        skos:narrower     parentalguidance:_62.1.3 ;
        skos:changeNote   "" ;
        skos:historyNote  "" ;
        skos:example      "" .

parentalguidance:_62.1.1
        rdf:type          ebucore:TargetAudience ;
        skos:prefLabel    "U"@en ;
        skos:definition   "General viewing for all ages."@en ;
        skos:broader      parentalguidance:_62.1 ;
        skos:inScheme     <http://www.ebu.ch/metadata/ontologies/skos/ebu_ParentalGuidanceCodeCS> ;
        skos:changeNote   "" ;
        skos:historyNote  "" ;
        skos:example      "" .

parentalguidance:_62.1.2
        rdf:type          ebucore:TargetAudience ;
        skos:prefLabel    "PG13"@en ;
        skos:definition   "Parental guidance is suggested for viewers under\n         13"@en ;
        skos:broader      parentalguidance:_62.1 ;
        skos:inScheme     <http://www.ebu.ch/metadata/ontologies/skos/ebu_ParentalGuidanceCodeCS> ;
        skos:changeNote   "" ;
        skos:historyNote  "" ;
        skos:example      "" .

parentalguidance:_62.1.3
        rdf:type          ebucore:TargetAudience ;
        skos:prefLabel    "18"@en ;
        skos:definition   "For aged 18 and above only"@en ;
        skos:broader      parentalguidance:_62.1 ;
        skos:inScheme     <http://www.ebu.ch/metadata/ontologies/skos/ebu_ParentalGuidanceCodeCS> ;
        skos:changeNote   "" ;
        skos:historyNote  "" ;
        skos:example      "" .

parentalguidance:_63  rdf:type  ebucore:TargetAudience ;
        skos:prefLabel    "MT-MCCAA"@en ;
        skos:scopeNote    "Region:Malta"@en ;
        skos:definition   ""@en ;
        skos:inScheme     <http://www.ebu.ch/metadata/ontologies/skos/ebu_ParentalGuidanceCodeCS> ;
        skos:narrower     parentalguidance:_63.1 ;
        skos:changeNote   "Update" ;
        skos:historyNote  "2010-08-03" ;
        skos:example      "" ;
        skos:note         "Valid" .

parentalguidance:_63.1
        rdf:type          ebucore:TargetAudience ;
        skos:prefLabel    "Rating"@en ;
        skos:broader      parentalguidance:_63 ;
        skos:inScheme     <http://www.ebu.ch/metadata/ontologies/skos/ebu_ParentalGuidanceCodeCS> ;
        skos:narrower     parentalguidance:_63.1.1 ;
        skos:narrower     parentalguidance:_63.1.2 ;
        skos:narrower     parentalguidance:_63.1.3 ;
        skos:narrower     parentalguidance:_63.1.4 ;
        skos:narrower     parentalguidance:_63.1.5 ;
        skos:narrower     parentalguidance:_63.1.6 ;
        skos:narrower     parentalguidance:_63.1.7 ;
        skos:changeNote   "" ;
        skos:historyNote  "" ;
        skos:example      "" .

parentalguidance:_63.1.1
        rdf:type          ebucore:TargetAudience ;
        skos:prefLabel    "U /Universal)"@en ;
        skos:definition   "General viewing for all ages."@en ;
        skos:broader      parentalguidance:_63.1 ;
        skos:inScheme     <http://www.ebu.ch/metadata/ontologies/skos/ebu_ParentalGuidanceCodeCS> ;
        skos:changeNote   "" ;
        skos:historyNote  "" ;
        skos:example      "" .

parentalguidance:_63.1.2
        rdf:type          ebucore:TargetAudience ;
        skos:altLabel    "Parental Guidance"@en ;
        skos:prefLabel    "PG"@en ;
        skos:definition   "Some material may be unsuitable for younger children. Children\n         under the age of 12 are to be accompanied by an adult. "@en ;
        skos:broader      parentalguidance:_63.1 ;
        skos:inScheme     <http://www.ebu.ch/metadata/ontologies/skos/ebu_ParentalGuidanceCodeCS> ;
        skos:changeNote   "" ;
        skos:historyNote  "" ;
        skos:example      "" .

parentalguidance:_63.1.3
        rdf:type          ebucore:TargetAudience ;
        skos:prefLabel    "12"@en ;
        skos:definition   "Suitable only for persons 12 years and older. No one under this\n         age is admitted. "@en ;
        skos:broader      parentalguidance:_63.1 ;
        skos:inScheme     <http://www.ebu.ch/metadata/ontologies/skos/ebu_ParentalGuidanceCodeCS> ;
        skos:changeNote   "" ;
        skos:historyNote  "" ;
        skos:example      "" .

parentalguidance:_63.1.4
        rdf:type          ebucore:TargetAudience ;
        skos:prefLabel    "14"@en ;
        skos:definition   "Suitable only for persons 14 years and older. No one under this\n         age is admitted. "@en ;
        skos:broader      parentalguidance:_63.1 ;
        skos:inScheme     <http://www.ebu.ch/metadata/ontologies/skos/ebu_ParentalGuidanceCodeCS> ;
        skos:changeNote   "" ;
        skos:historyNote  "" ;
        skos:example      "" .

parentalguidance:_63.1.5
        rdf:type          ebucore:TargetAudience ;
        skos:prefLabel    "15"@en ;
        skos:definition   "Suitable only for persons 15 years and older. No one under this\n         age is admitted. "@en ;
        skos:broader      parentalguidance:_63.1 ;
        skos:inScheme     <http://www.ebu.ch/metadata/ontologies/skos/ebu_ParentalGuidanceCodeCS> ;
        skos:changeNote   "" ;
        skos:historyNote  "" ;
        skos:example      "" .

parentalguidance:_63.1.6
        rdf:type          ebucore:TargetAudience ;
        skos:prefLabel    "16"@en ;
        skos:definition   "Suitable only for persons 16 years and older. No one under this\n         age is admitted. "@en ;
        skos:broader      parentalguidance:_63.1 ;
        skos:inScheme     <http://www.ebu.ch/metadata/ontologies/skos/ebu_ParentalGuidanceCodeCS> ;
        skos:changeNote   "" ;
        skos:historyNote  "" ;
        skos:example      "" .

parentalguidance:_63.1.7
        rdf:type          ebucore:TargetAudience ;
        skos:prefLabel    "18"@en ;
        skos:definition   "Suitable only for persons 18 years and older. No one under this\n         age is admitted. "@en ;
        skos:broader      parentalguidance:_63.1 ;
        skos:inScheme     <http://www.ebu.ch/metadata/ontologies/skos/ebu_ParentalGuidanceCodeCS> ;
        skos:changeNote   "" ;
        skos:historyNote  "" ;
        skos:example      "" .

parentalguidance:_64  rdf:type  ebucore:TargetAudience ;
        skos:prefLabel    "CH-Film"@en ;
        skos:scopeNote    "Region:Switzerland"@en ;
        skos:definition   ""@en ;
        skos:inScheme     <http://www.ebu.ch/metadata/ontologies/skos/ebu_ParentalGuidanceCodeCS> ;
        skos:narrower     parentalguidance:_64.1 ;
        skos:changeNote   "Update" ;
        skos:historyNote  "2010-08-03" ;
        skos:example      "" ;
        dct:description   "Movie labs ratings: https://www.movielabs.com/md/ratings/v2.0/html/CH_Film_Ratings.html"@en ;
        skos:note         "Valid" .

parentalguidance:_64.1
        rdf:type          ebucore:TargetAudience ;
        skos:prefLabel    "Rating"@en ;
        skos:broader      parentalguidance:_64 ;
        skos:inScheme     <http://www.ebu.ch/metadata/ontologies/skos/ebu_ParentalGuidanceCodeCS> ;
        skos:narrower     parentalguidance:_64.1.1 ;
        skos:narrower     parentalguidance:_64.1.2 ;
        skos:narrower     parentalguidance:_64.1.3 ;
        skos:narrower     parentalguidance:_64.1.4 ;
        skos:narrower     parentalguidance:_64.1.5 ;
        skos:narrower     parentalguidance:_64.1.6 ;
        skos:narrower     parentalguidance:_64.1.7 ;
        skos:changeNote   "" ;
        skos:historyNote  "" ;
        skos:example      "" .

parentalguidance:_64.1.1
        rdf:type          ebucore:TargetAudience ;
        skos:prefLabel    "0"@en ;
        skos:definition   "General viewing for all ages."@en ;
        skos:broader      parentalguidance:_64.1 ;
        skos:inScheme     <http://www.ebu.ch/metadata/ontologies/skos/ebu_ParentalGuidanceCodeCS> ;
        skos:changeNote   "" ;
        skos:historyNote  "" ;
        skos:example      "" .

parentalguidance:_64.1.2
        rdf:type          ebucore:TargetAudience ;
        skos:prefLabel    "7"@en ;
        skos:definition   "No one under the age of 7 admitted "@en ;
        skos:broader      parentalguidance:_64.1 ;
        skos:inScheme     <http://www.ebu.ch/metadata/ontologies/skos/ebu_ParentalGuidanceCodeCS> ;
        skos:changeNote   "" ;
        skos:historyNote  "" ;
        skos:example      "" .

parentalguidance:_64.1.3
        rdf:type          ebucore:TargetAudience ;
        skos:prefLabel    "10"@en ;
        skos:definition   "No one under the age of 10 admitted "@en ;
        skos:broader      parentalguidance:_64.1 ;
        skos:inScheme     <http://www.ebu.ch/metadata/ontologies/skos/ebu_ParentalGuidanceCodeCS> ;
        skos:changeNote   "" ;
        skos:historyNote  "" ;
        skos:example      "" .

parentalguidance:_64.1.4
        rdf:type          ebucore:TargetAudience ;
        skos:prefLabel    "12"@en ;
        skos:definition   "No one under the age of 12 admitted "@en ;
        skos:broader      parentalguidance:_64.1 ;
        skos:inScheme     <http://www.ebu.ch/metadata/ontologies/skos/ebu_ParentalGuidanceCodeCS> ;
        skos:changeNote   "" ;
        skos:historyNote  "" ;
        skos:example      "" .

parentalguidance:_64.1.5
        rdf:type          ebucore:TargetAudience ;
        skos:prefLabel    "14"@en ;
        skos:definition   "No one under the age of 14 admitted "@en ;
        skos:broader      parentalguidance:_64.1 ;
        skos:inScheme     <http://www.ebu.ch/metadata/ontologies/skos/ebu_ParentalGuidanceCodeCS> ;
        skos:changeNote   "" ;
        skos:historyNote  "" ;
        skos:example      "" .

parentalguidance:_64.1.6
        rdf:type          ebucore:TargetAudience ;
        skos:prefLabel    "16"@en ;
        skos:definition   "No one under the age of 16 admitted "@en ;
        skos:broader      parentalguidance:_64.1 ;
        skos:inScheme     <http://www.ebu.ch/metadata/ontologies/skos/ebu_ParentalGuidanceCodeCS> ;
        skos:changeNote   "" ;
        skos:historyNote  "" ;
        skos:example      "" .

parentalguidance:_64.1.7
        rdf:type          ebucore:TargetAudience ;
        skos:prefLabel    "18"@en ;
        skos:definition   "No one under the age of 18 admitted "@en ;
        skos:broader      parentalguidance:_64.1 ;
        skos:inScheme     <http://www.ebu.ch/metadata/ontologies/skos/ebu_ParentalGuidanceCodeCS> ;
        skos:changeNote   "" ;
        skos:historyNote  "" ;
        skos:example      "" .

parentalguidance:_65  rdf:type  ebucore:TargetAudience ;
        skos:prefLabel    "TH-BFVC"@en ;
        skos:scopeNote    "Region:Thailand"@en ;
        skos:definition   ""@en ;
        skos:inScheme     <http://www.ebu.ch/metadata/ontologies/skos/ebu_ParentalGuidanceCodeCS> ;
        skos:narrower     parentalguidance:_65.1 ;
        skos:changeNote   "Update" ;
        skos:historyNote  "2010-08-03" ;
        skos:example      "" ;
        dct:description   "Movie labs ratings: https://www.movielabs.com/md/ratings/v2.0/html/TH_BFVC_Ratings.html"@en ;
        skos:note         "Valid" .

parentalguidance:_65.1
        rdf:type          ebucore:TargetAudience ;
        skos:prefLabel    "Rating"@en ;
        skos:broader      parentalguidance:_65 ;
        skos:inScheme     <http://www.ebu.ch/metadata/ontologies/skos/ebu_ParentalGuidanceCodeCS> ;
        skos:narrower     parentalguidance:_65.1.1 ;
        skos:narrower     parentalguidance:_65.1.2 ;
        skos:narrower     parentalguidance:_65.1.3 ;
        skos:narrower     parentalguidance:_65.1.4 ;
        skos:narrower     parentalguidance:_65.1.5 ;
        skos:narrower     parentalguidance:_65.1.6 ;
        skos:changeNote   "" ;
        skos:historyNote  "" ;
        skos:example      "" .

parentalguidance:_65.1.1
        rdf:type          ebucore:TargetAudience ;
        skos:prefLabel    "P"@en ;
        skos:definition   "Promotional, film is educational and viewing is encouraged for\n         all Thai people.."@en ;
        skos:broader      parentalguidance:_65.1 ;
        skos:inScheme     <http://www.ebu.ch/metadata/ontologies/skos/ebu_ParentalGuidanceCodeCS> ;
        skos:changeNote   "" ;
        skos:historyNote  "" ;
        skos:example      "" .

parentalguidance:_65.1.2
        rdf:type          ebucore:TargetAudience ;
        skos:prefLabel    "G"@en ;
        skos:definition   "Suitable for general audiences "@en ;
        skos:broader      parentalguidance:_65.1 ;
        skos:inScheme     <http://www.ebu.ch/metadata/ontologies/skos/ebu_ParentalGuidanceCodeCS> ;
        skos:changeNote   "" ;
        skos:historyNote  "" ;
        skos:example      "" .

parentalguidance:_65.1.3
        rdf:type          ebucore:TargetAudience ;
        skos:prefLabel    "13+"@en ;
        skos:definition   "No one under the age of 13 admitted "@en ;
        skos:broader      parentalguidance:_65.1 ;
        skos:inScheme     <http://www.ebu.ch/metadata/ontologies/skos/ebu_ParentalGuidanceCodeCS> ;
        skos:changeNote   "" ;
        skos:historyNote  "" ;
        skos:example      "" .

parentalguidance:_65.1.4
        rdf:type          ebucore:TargetAudience ;
        skos:prefLabel    "15+"@en ;
        skos:definition   "No one under the age of 15 admitted "@en ;
        skos:broader      parentalguidance:_65.1 ;
        skos:inScheme     <http://www.ebu.ch/metadata/ontologies/skos/ebu_ParentalGuidanceCodeCS> ;
        skos:changeNote   "" ;
        skos:historyNote  "" ;
        skos:example      "" .

parentalguidance:_65.1.5
        rdf:type          ebucore:TargetAudience ;
        skos:prefLabel    "18+"@en ;
        skos:definition   "No one under the age of 18 admitted "@en ;
        skos:broader      parentalguidance:_65.1 ;
        skos:inScheme     <http://www.ebu.ch/metadata/ontologies/skos/ebu_ParentalGuidanceCodeCS> ;
        skos:changeNote   "" ;
        skos:historyNote  "" ;
        skos:example      "" .

parentalguidance:_65.1.6
        rdf:type          ebucore:TargetAudience ;
        skos:prefLabel    "20+"@en ;
        skos:definition   "For views over 20 years old only "@en ;
        skos:broader      parentalguidance:_65.1 ;
        skos:inScheme     <http://www.ebu.ch/metadata/ontologies/skos/ebu_ParentalGuidanceCodeCS> ;
        skos:changeNote   "" ;
        skos:historyNote  "" ;
        skos:example      "" .

parentalguidance:_66  rdf:type  ebucore:TargetAudience ;
        skos:prefLabel    "AE-UAB"@en ;
        skos:scopeNote    "Region:United Arab Emirates"@en ;
        skos:definition   ""@en ;
        skos:inScheme     <http://www.ebu.ch/metadata/ontologies/skos/ebu_ParentalGuidanceCodeCS> ;
        skos:narrower     parentalguidance:_66.1 ;
        skos:changeNote   "Correct subterm termId starting with 65.x into\n         66.x" ;
        skos:historyNote  "2019-06-24" ;
        skos:example      "" ;
        skos:note         "Valid" .

parentalguidance:_66.1
        rdf:type          ebucore:TargetAudience ;
        skos:prefLabel    "Rating"@en ;
        skos:broader      parentalguidance:_66 ;
        skos:inScheme     <http://www.ebu.ch/metadata/ontologies/skos/ebu_ParentalGuidanceCodeCS> ;
        skos:narrower     parentalguidance:_66.1.1 ;
        skos:narrower     parentalguidance:_66.1.2 ;
        skos:narrower     parentalguidance:_66.1.3 ;
        skos:narrower     parentalguidance:_66.1.4 ;
        skos:narrower     parentalguidance:_66.1.5 ;
        skos:changeNote   "" ;
        skos:historyNote  "" ;
        skos:example      "" .

parentalguidance:_66.1.1
        rdf:type          ebucore:TargetAudience ;
        skos:prefLabel    "G"@en ;
        skos:definition   "Suitable for general audiences "@en ;
        skos:broader      parentalguidance:_66.1 ;
        skos:inScheme     <http://www.ebu.ch/metadata/ontologies/skos/ebu_ParentalGuidanceCodeCS> ;
        skos:changeNote   "" ;
        skos:historyNote  "" ;
        skos:example      "" .

parentalguidance:_66.1.2
        rdf:type          ebucore:TargetAudience ;
        skos:prefLabel    "PG-13"@en ;
        skos:definition   "Under 13 not admitted unless accompanied by an individual over\n         13. Some material may not be suitable for children "@en ;
        skos:broader      parentalguidance:_66.1 ;
        skos:inScheme     <http://www.ebu.ch/metadata/ontologies/skos/ebu_ParentalGuidanceCodeCS> ;
        skos:changeNote   "" ;
        skos:historyNote  "" ;
        skos:example      "" .

parentalguidance:_66.1.3
        rdf:type          ebucore:TargetAudience ;
        skos:prefLabel    "PG15"@en ;
        skos:definition   "Under 15 not admitted unless accompanied by an individual over\n         15. Some material may not be suitable for children "@en ;
        skos:broader      parentalguidance:_66.1 ;
        skos:inScheme     <http://www.ebu.ch/metadata/ontologies/skos/ebu_ParentalGuidanceCodeCS> ;
        skos:changeNote   "" ;
        skos:historyNote  "" ;
        skos:example      "" .

parentalguidance:_66.1.4
        rdf:type          ebucore:TargetAudience ;
        skos:prefLabel    "15+"@en ;
        skos:definition   "No one under the age of 15 admitted "@en ;
        skos:broader      parentalguidance:_66.1 ;
        skos:inScheme     <http://www.ebu.ch/metadata/ontologies/skos/ebu_ParentalGuidanceCodeCS> ;
        skos:changeNote   "" ;
        skos:historyNote  "" ;
        skos:example      "" .

parentalguidance:_66.1.5
        rdf:type          ebucore:TargetAudience ;
        skos:prefLabel    "18+"@en ;
        skos:definition   "No one under the age of 18 admitted "@en ;
        skos:broader      parentalguidance:_66.1 ;
        skos:inScheme     <http://www.ebu.ch/metadata/ontologies/skos/ebu_ParentalGuidanceCodeCS> ;
        skos:changeNote   "" ;
        skos:historyNote  "" ;
        skos:example      "" .

parentalguidance:_67  rdf:type  ebucore:TargetAudience ;
        skos:prefLabel    "simple"@en ;
        skos:definition   ""@en ;
        skos:inScheme     <http://www.ebu.ch/metadata/ontologies/skos/ebu_ParentalGuidanceCodeCS> ;
        skos:narrower     parentalguidance:_67.1 ;
        skos:narrower     parentalguidance:_67.2 ;
        skos:historyNote  "2023-07-13" ;
        skos:note         "Valid" .

parentalguidance:_67.1
        rdf:type         ebucore:TargetAudience ;
        skos:prefLabel   "nonadult"@en ;
        skos:altLabel    "family"@en ;
        skos:altLabel    "children"@en ;
        skos:definition  "Viewing for all ages"@en ;
        skos:broader     parentalguidance:_67 ;
        skos:inScheme    <http://www.ebu.ch/metadata/ontologies/skos/ebu_ParentalGuidanceCodeCS> .

parentalguidance:_67.2
        rdf:type         ebucore:TargetAudience ;
        skos:prefLabel   "adult"@en ;
        skos:definition  "Only for adult viewing"@en ;
        skos:broader     parentalguidance:_67 ;
        skos:inScheme    <http://www.ebu.ch/metadata/ontologies/skos/ebu_ParentalGuidanceCodeCS> .

# https://movielabs.com/md/ratings/v2.5/CMR_Ratings_v2.5.xml
# https://cinema.cultura.gov.it/database-nuova-classificazione/
parentalguidance:_68  rdf:type  ebucore:TargetAudience ;
        skos:prefLabel    "IT-MBACT"@en ;
        skos:altLabel     "MBACT"@en ;
        skos:scopeNote    "Region:Italy"@en ;
        skos:definition   "Direzione generale Cinema e audiovisivo"@en ;
        skos:inScheme     <http://www.ebu.ch/metadata/ontologies/skos/ebu_ParentalGuidanceCodeCS> ;
        skos:narrower     parentalguidance:_68.1 ;
        skos:changeNote   "Created" ;
        skos:historyNote  "2024-04-10" ;
        skos:example      "" ;
        skos:note         "Valid" .

parentalguidance:_68.1
        rdf:type          ebucore:TargetAudience ;
        skos:prefLabel    "Rating"@en ;
        skos:definition   ""@en ;
        skos:broader      parentalguidance:_68;
        skos:inScheme     <http://www.ebu.ch/metadata/ontologies/skos/ebu_ParentalGuidanceCodeCS> ;
        skos:narrower     parentalguidance:_68.1.1 ;
        skos:narrower     parentalguidance:_68.1.2 ;
        skos:narrower     parentalguidance:_68.1.3 ;
        skos:narrower     parentalguidance:_68.1.4 ;
        skos:changeNote   "" ;
        skos:historyNote  "" ;
        skos:example      "" .

parentalguidance:_68.1.1
        rdf:type          ebucore:TargetAudience ;
        skos:prefLabel    "T"@en ;
        skos:definition   "Film for everyone"@en ;
        skos:definition   "Pellicola per tutti"@it ;
        skos:broader      parentalguidance:_68.1 ;
        skos:inScheme     <http://www.ebu.ch/metadata/ontologies/skos/ebu_ParentalGuidanceCodeCS> ;
        skos:changeNote   "" ;
        skos:historyNote  "" ;
        skos:example      "" .

parentalguidance:_68.1.2
        rdf:type          ebucore:TargetAudience ;
        skos:prefLabel    "VM6"@en ;
        skos:definition   "Opere non adatte ai minori di anni 6"@it ;
        skos:definition   "Works not suitable for children under 6 years"@en ;
        skos:broader      parentalguidance:_68.1 ;
        skos:inScheme     <http://www.ebu.ch/metadata/ontologies/skos/ebu_ParentalGuidanceCodeCS> ;
        skos:changeNote   "" ;
        skos:historyNote  "" ;
        skos:example      "" .

parentalguidance:_68.1.3
        rdf:type          ebucore:TargetAudience ;
        skos:prefLabel    "VM14"@en ;
        skos:definition   "14 anni"@it ;
        skos:definition   "14 years"@en ;
        skos:broader      parentalguidance:_68.1 ;
        skos:inScheme     <http://www.ebu.ch/metadata/ontologies/skos/ebu_ParentalGuidanceCodeCS> ;
        skos:changeNote   "" ;
        skos:historyNote  "" ;
        skos:example      "" .

parentalguidance:_68.1.4
        rdf:type          ebucore:TargetAudience ;
        skos:prefLabel    "VM18"@en ;
        skos:definition   "18 anni"@it ;
        skos:definition   "18 years"@en ;
        skos:broader      parentalguidance:_68.1 ;
        skos:inScheme     <http://www.ebu.ch/metadata/ontologies/skos/ebu_ParentalGuidanceCodeCS> ;
        skos:changeNote   "" ;
        skos:historyNote  "" ;
        skos:example      "" .


# https://movielabs.com/md/ratings/v2.5/CMR_Ratings_v2.5.xml
# https://movielabs.com/md/ratings/v2.4/xml/IT_AGCOM_Ratings.xml
# http://www.agcom.it/
parentalguidance:_69  rdf:type  ebucore:TargetAudience ;
        skos:prefLabel    "IT-AGCOM"@en ;
        skos:altLabel     "AGCOM"@en ;
        skos:scopeNote    "Region:Italy"@en ;
        skos:definition   "Direzione generale Cinema e audiovisivo"@en ;
        skos:inScheme     <http://www.ebu.ch/metadata/ontologies/skos/ebu_ParentalGuidanceCodeCS> ;
        skos:narrower     parentalguidance:_69.1 ;
        skos:changeNote   "Created" ;
        skos:historyNote  "2024-04-10" ;
        skos:example      "" ;
        skos:note         "Valid" .

parentalguidance:_69.1
        rdf:type          ebucore:TargetAudience ;
        skos:prefLabel    "Rating"@en ;
        skos:definition   ""@en ;
        skos:broader      parentalguidance:_69 ;
        skos:inScheme     <http://www.ebu.ch/metadata/ontologies/skos/ebu_ParentalGuidanceCodeCS> ;
        skos:narrower     parentalguidance:_69.1.1 ;
        skos:narrower     parentalguidance:_69.1.2 ;
        skos:narrower     parentalguidance:_69.1.3 ;
        skos:narrower     parentalguidance:_69.1.4 ;
        skos:changeNote   "" ;
        skos:historyNote  "" ;
        skos:example      "" .

parentalguidance:_69.1.1
        rdf:type          ebucore:TargetAudience ;
        skos:prefLabel    "T"@en ;
        skos:definition   "Film for everyone"@en ;
        skos:definition   "Pellicola per tutti"@it ;
        skos:broader      parentalguidance:_69.1 ;
        skos:inScheme     <http://www.ebu.ch/metadata/ontologies/skos/ebu_ParentalGuidanceCodeCS> ;
        skos:changeNote   "" ;
        skos:historyNote  "" ;
        skos:example      "" .

parentalguidance:_69.1.2
        rdf:type          ebucore:TargetAudience ;
        skos:prefLabel    "VM6"@en ;
        skos:definition   "Film Vietati ai minori di 6 anni"@it ;
        skos:definition   "Films prohibited to minors under 6 years"@en ;
        skos:broader      parentalguidance:_69.1 ;
        skos:inScheme     <http://www.ebu.ch/metadata/ontologies/skos/ebu_ParentalGuidanceCodeCS> ;
        skos:changeNote   "" ;
        skos:historyNote  "" ;
        skos:example      "" .

parentalguidance:_69.1.3
        rdf:type          ebucore:TargetAudience ;
        skos:prefLabel    "VM14"@en ;
        skos:definition   "Film Vietati ai minori di 14 anni"@it ;
        skos:definition   "Films prohibited to minors under 14 years"@en ;
        skos:broader      parentalguidance:_69.1 ;
        skos:inScheme     <http://www.ebu.ch/metadata/ontologies/skos/ebu_ParentalGuidanceCodeCS> ;
        skos:changeNote   "" ;
        skos:historyNote  "" ;
        skos:example      "" .

parentalguidance:_69.1.4
        rdf:type          ebucore:TargetAudience ;
        skos:prefLabel    "VM18"@en ;
        skos:definition   "Film Vietati ai minori di 18 anni"@it ;
        skos:definition   "Films prohibited to minors under 18 years"@en ;
        skos:broader      parentalguidance:_69.1 ;
        skos:inScheme     <http://www.ebu.ch/metadata/ontologies/skos/ebu_ParentalGuidanceCodeCS> ;
        skos:changeNote   "" ;
        skos:historyNote  "" ;
        skos:example      "" .


_:b0    rdf:first  parentalguidance:_31 ;
        rdf:rest   rdf:nil .

_:b1    rdf:first  parentalguidance:_19 ;
        rdf:rest   _:b0 .

_:b2    rdf:first  parentalguidance:_25 ;
        rdf:rest   _:b1 .

_:b3    rdf:first  parentalguidance:_27 ;
        rdf:rest   _:b2 .

_:b4    rdf:first  parentalguidance:_50 ;
        rdf:rest   _:b3 .

_:b5    rdf:first  parentalguidance:_48 ;
        rdf:rest   _:b4 .

parentalguidance:defaultSchemesList
        rdf:type         skos:OrderedCollection ;
        rdfs:label       "Default PG Schemes List"@en ;
        skos:definition  "The ordered list of Parental Guidance top concepts to be considered when no scheme is provided for a rating"@en ;
        skos:memberList  _:b5 .


parentalguidance:_70  rdf:type  ebucore:TargetAudience ;
        skos:prefLabel    "JP-EIRIN"@en ; # https://en.wikipedia.org/wiki/Eirin
        skos:prefLabel    "映倫"@ja ;
        skos:scopeNote    "Region:Japan"@en ;
        skos:definition   "Film Classification and Rating Organization"@en ;
        skos:definition   "映画倫理機構,  Eiga Rinri Kikō"@ja ;
        skos:inScheme     <http://www.ebu.ch/metadata/ontologies/skos/ebu_ParentalGuidanceCodeCS> ;
        skos:narrower     parentalguidance:_70.1 ;
        skos:narrower     parentalguidance:_70.2 ;
        skos:changeNote   "Create" ;
        skos:historyNote  "2024-07-24" ;
        skos:example      "" ;
        dct:description   "Ratings: https://www.eirin.jp/english/008.html"@en ;
        skos:note         "Valid" .

parentalguidance:_70.1
        rdf:type          ebucore:TargetAudience ;
        skos:prefLabel    "Rating"@en ;
        skos:prefLabel    "レーティングマーク"@ja ;
        skos:broader      parentalguidance:_70 ;
        skos:inScheme     <http://www.ebu.ch/metadata/ontologies/skos/ebu_ParentalGuidanceCodeCS> ;
        skos:narrower     parentalguidance:_70.1.1 ;
        skos:narrower     parentalguidance:_70.1.2 ;
        skos:narrower     parentalguidance:_70.1.3 ;
        skos:narrower     parentalguidance:_70.1.4 ;
        skos:changeNote   "" ;
        skos:historyNote  "" ;
        skos:example      "" .

parentalguidance:_70.1.1
        rdf:type          ebucore:TargetAudience ;
        skos:prefLabel    "G"@en ;
        skos:prefLabel    "映倫"@ja ;
        skos:definition   ""@ja ;
        skos:definition   "Anybody can view"@en ;
        skos:broader      parentalguidance:_70.1 ;
        skos:inScheme     <http://www.ebu.ch/metadata/ontologies/skos/ebu_ParentalGuidanceCodeCS> ;
        skos:changeNote   "" ;
        skos:historyNote  "" ;
        skos:example      "" .

parentalguidance:_70.1.2
        rdf:type          ebucore:TargetAudience ;
        skos:prefLabel    "PG12"@en ;
        skos:definition   "Parental advice and guidance recommended for under 12 years old"@en ;
        skos:broader      parentalguidance:_70.1 ;
        skos:inScheme     <http://www.ebu.ch/metadata/ontologies/skos/ebu_ParentalGuidanceCodeCS> ;
        skos:changeNote   "" ;
        skos:historyNote  "" ;
        skos:example      "" .

parentalguidance:_70.1.3
        rdf:type          ebucore:TargetAudience ;
        skos:prefLabel    "R15+"@en ; # https://en.wikipedia.org/wiki/Eirin
        skos:definition   "Viewing is prohibited for those under 15 years old"@en ;
        skos:broader      parentalguidance:_70.1 ;
        skos:inScheme     <http://www.ebu.ch/metadata/ontologies/skos/ebu_ParentalGuidanceCodeCS> ;
        skos:changeNote   "" ;
        skos:historyNote  "" ;
        skos:example      "" .

parentalguidance:_70.1.4
        rdf:type          ebucore:TargetAudience ;
        skos:prefLabel    "R18+"@en ;
        skos:definition   "Viewing is prohibited for those under 18 years old"@en ;
        skos:broader      parentalguidance:_70.1 ;
        skos:inScheme     <http://www.ebu.ch/metadata/ontologies/skos/ebu_ParentalGuidanceCodeCS> ;
        skos:changeNote   "" ;
        skos:historyNote  "" ;
        skos:example      "" .

parentalguidance:_70.2
        rdf:type          ebucore:TargetAudience ;
        skos:prefLabel    "Criteria"@en ;
        skos:prefLabel    "コンテンツアイコン"@ja ;
        skos:broader      parentalguidance:_70 ;
        skos:inScheme     <http://www.ebu.ch/metadata/ontologies/skos/ebu_ParentalGuidanceCodeCS> ;
        skos:narrower     parentalguidance:_70.2.1 ;
        skos:narrower     parentalguidance:_70.2.2 ;
        skos:narrower     parentalguidance:_70.2.3 ;
        skos:narrower     parentalguidance:_70.2.4 ;
        skos:narrower     parentalguidance:_70.2.5 ;
        skos:narrower     parentalguidance:_70.2.6 ;
        skos:narrower     parentalguidance:_70.2.7 ;
        skos:changeNote   "" ;
        skos:historyNote  "" ;
        skos:example      "" .

parentalguidance:_70.2.1
        rdf:type          ebucore:TargetAudience ;
        skos:prefLabel    "言語"@ja ;
        skos:prefLabel    "Language"@en ;
        skos:broader      parentalguidance:_70.2 ;
        skos:inScheme     <http://www.ebu.ch/metadata/ontologies/skos/ebu_ParentalGuidanceCodeCS> ;
        skos:changeNote   "" ;
        skos:historyNote  "" ;
        skos:example      "" .

parentalguidance:_70.2.2
        rdf:type          ebucore:TargetAudience ;
        skos:prefLabel    "セクシャル"@ja ;
        skos:prefLabel    "Sex"@en ;
        skos:broader      parentalguidance:_70.2 ;
        skos:inScheme     <http://www.ebu.ch/metadata/ontologies/skos/ebu_ParentalGuidanceCodeCS> ;
        skos:changeNote   "" ;
        skos:historyNote  "" ;
        skos:example      "" .

parentalguidance:_70.2.3
        rdf:type          ebucore:TargetAudience ;
        skos:prefLabel    "ヌード"@ja ;
        skos:prefLabel    "Nudity"@en ;
        skos:broader      parentalguidance:_70.2 ;
        skos:inScheme     <http://www.ebu.ch/metadata/ontologies/skos/ebu_ParentalGuidanceCodeCS> ;
        skos:changeNote   "" ;
        skos:historyNote  "" ;
        skos:example      "" .

parentalguidance:_70.2.4
        rdf:type          ebucore:TargetAudience ;
        skos:prefLabel    "暴力"@ja ;
        skos:prefLabel    "Violence"@en ;
        skos:broader      parentalguidance:_70.2 ;
        skos:inScheme     <http://www.ebu.ch/metadata/ontologies/skos/ebu_ParentalGuidanceCodeCS> ;
        skos:changeNote   "" ;
        skos:historyNote  "" ;
        skos:example      "" .

parentalguidance:_70.2.5
        rdf:type          ebucore:TargetAudience ;
        skos:prefLabel    "ホラー"@ja ;
        skos:prefLabel    "Horror"@en ;
        skos:broader      parentalguidance:_70.2 ;
        skos:inScheme     <http://www.ebu.ch/metadata/ontologies/skos/ebu_ParentalGuidanceCodeCS> ;
        skos:changeNote   "" ;
        skos:historyNote  "" ;
        skos:example      "" .

parentalguidance:_70.2.6
        rdf:type          ebucore:TargetAudience ;
        skos:prefLabel    "麻薬"@ja ;
        skos:prefLabel    "Drugs"@en ;
        skos:broader      parentalguidance:_70.2 ;
        skos:inScheme     <http://www.ebu.ch/metadata/ontologies/skos/ebu_ParentalGuidanceCodeCS> ;
        skos:changeNote   "" ;
        skos:historyNote  "" ;
        skos:example      "" .

parentalguidance:_70.2.7
        rdf:type          ebucore:TargetAudience ;
        skos:prefLabel    "犯罪"@ja ;
        skos:prefLabel    "Crime"@en ;
        skos:broader      parentalguidance:_70.2 ;
        skos:inScheme     <http://www.ebu.ch/metadata/ontologies/skos/ebu_ParentalGuidanceCodeCS> ;
        skos:changeNote   "" ;
        skos:historyNote  "" ;
        skos:example      "" .



# Ref for Russian ratings: https://movielabs.com/md/ratings/v2.4.5/html/RU_MKRF_Ratings.html
parentalguidance:_71  rdf:type  ebucore:TargetAudience ;
        skos:prefLabel    "RU-MKRF"@en ;
        skos:altLabel     "MKRF"@en ;
        skos:scopeNote    "Region:RUSSIA"@en ;
        skos:definition   "Ministry of Culture of the Russian Federation"@en ;
        skos:inScheme     <http://www.ebu.ch/metadata/ontologies/skos/ebu_ParentalGuidanceCodeCS> ;
        skos:narrower     parentalguidance:_71.1 ;
        skos:changeNote   "Created" ;
        skos:historyNote  "2024-11-15" ;
        skos:example      "" ;
        skos:note         "Valid" .

parentalguidance:_71.1
        rdf:type          ebucore:TargetAudience ;
        skos:prefLabel    "Rating"@en ;
        skos:definition   ""@en ;
        skos:broader      parentalguidance:_71 ;
        skos:inScheme     <http://www.ebu.ch/metadata/ontologies/skos/ebu_ParentalGuidanceCodeCS> ;
        skos:narrower     parentalguidance:_71.1.1 ;
        skos:narrower     parentalguidance:_71.1.2 ;
        skos:narrower     parentalguidance:_71.1.3 ;
        skos:narrower     parentalguidance:_71.1.4 ;
        skos:narrower     parentalguidance:_71.1.5 ;
        skos:changeNote   "" ;
        skos:historyNote  "" ;
        skos:example      "" .

parentalguidance:_71.1.1
        rdf:type          ebucore:TargetAudience ;
        skos:prefLabel    "0+"@en ;
        skos:definition   "Suitable for all ages"@en ;
        skos:broader      parentalguidance:_71.1 ;
        skos:inScheme     <http://www.ebu.ch/metadata/ontologies/skos/ebu_ParentalGuidanceCodeCS> ;
        skos:changeNote   "" ;
        skos:historyNote  "" ;
        skos:example      "" .

parentalguidance:_71.1.2
        rdf:type          ebucore:TargetAudience ;
        skos:prefLabel    "6+"@en ;
        skos:definition   "Media suitable for people aged 6 and older"@en ;
        skos:broader      parentalguidance:_71.1 ;
        skos:inScheme     <http://www.ebu.ch/metadata/ontologies/skos/ebu_ParentalGuidanceCodeCS> ;
        skos:changeNote   "" ;
        skos:historyNote  "" ;
        skos:example      "" .

parentalguidance:_71.1.3
        rdf:type          ebucore:TargetAudience ;
        skos:prefLabel    "12+"@en ;
        skos:definition   "Media suitable for people aged 12 and older"@en ;
        skos:broader      parentalguidance:_71.1 ;
        skos:inScheme     <http://www.ebu.ch/metadata/ontologies/skos/ebu_ParentalGuidanceCodeCS> ;
        skos:changeNote   "" ;
        skos:historyNote  "" ;
        skos:example      "" .

parentalguidance:_71.1.4
        rdf:type          ebucore:TargetAudience ;
        skos:prefLabel    "16+"@en ;
        skos:definition   "Media suitable for people aged 16 and older"@en ;
        skos:broader      parentalguidance:_71.1 ;
        skos:inScheme     <http://www.ebu.ch/metadata/ontologies/skos/ebu_ParentalGuidanceCodeCS> ;
        skos:changeNote   "" ;
        skos:historyNote  "" ;
        skos:example      "" .

parentalguidance:_71.1.5
        rdf:type          ebucore:TargetAudience ;
        skos:prefLabel    "18+"@en ;
        skos:definition   "Media suitable only for people aged 18 and older"@en ;
        skos:broader      parentalguidance:_71.1 ;
        skos:inScheme     <http://www.ebu.ch/metadata/ontologies/skos/ebu_ParentalGuidanceCodeCS> ;
        skos:changeNote   "" ;
        skos:historyNote  "" ;
        skos:example      "" .

parentalguidance:_72 rdf:type ebucore:TargetAudience ;
        skos:prefLabel "CA-TVPG"@en ;
        skos:altLabel "CA-V-Chip"@en ;
        skos:scopeNote "Region: Canada"@en ;
        skos:definition "The Canadian TV parental guidelines system (V-Chip)"@en ;
        skos:inScheme <http://www.ebu.ch/metadata/ontologies/skos/ebu_ParentalGuidanceCodeCS> ;
        skos:narrower parentalguidance:_72.1 .

parentalguidance:_72.1 rdf:type ebucore:TargetAudience ;
        skos:prefLabel "Ratings"@en ;
        skos:broader parentalguidance:_72 ;
        skos:inScheme <http://www.ebu.ch/metadata/ontologies/skos/ebu_ParentalGuidanceCodeCS> ;
        skos:narrower parentalguidance:_72.1.1 ;
        skos:narrower parentalguidance:_72.1.2 ;
        skos:narrower parentalguidance:_72.1.3 ;
        skos:narrower parentalguidance:_72.1.4 ;
        skos:narrower parentalguidance:_72.1.5 ;
        skos:narrower parentalguidance:_72.1.6 .

parentalguidance:_72.1.1 rdf:type ebucore:TargetAudience ;
        skos:prefLabel "C"@en ;
        skos:definition "Children – Suitable for ages under 8 years"@en ;
        skos:broader parentalguidance:_72.1 ;
        skos:inScheme <http://www.ebu.ch/metadata/ontologies/skos/ebu_ParentalGuidanceCodeCS> .

parentalguidance:_72.1.2 rdf:type ebucore:TargetAudience ;
        skos:prefLabel "C8+"@en ;
        skos:definition "Children Over 8 Years – Suitable for ages 8 and older"@en ;
        skos:broader parentalguidance:_72.1 ;
        skos:inScheme <http://www.ebu.ch/metadata/ontologies/skos/ebu_ParentalGuidanceCodeCS> .

parentalguidance:_72.1.3 rdf:type ebucore:TargetAudience ;
        skos:prefLabel "G"@en ;
        skos:definition "General – Suitable for all audiences"@en ;
        skos:broader parentalguidance:_72.1 ;
        skos:inScheme <http://www.ebu.ch/metadata/ontologies/skos/ebu_ParentalGuidanceCodeCS> .

parentalguidance:_72.1.4 rdf:type ebucore:TargetAudience ;
        skos:prefLabel "PG"@en ;
        skos:definition "Parental Guidance Suggested"@en ;
        skos:broader parentalguidance:_72.1 ;
        skos:inScheme <http://www.ebu.ch/metadata/ontologies/skos/ebu_ParentalGuidanceCodeCS> .

parentalguidance:_72.1.5 rdf:type ebucore:TargetAudience ;
        skos:prefLabel "14+"@en ;
        skos:definition "Parents Strongly Cautioned – Suitable for ages 14 and older"@en ;
        skos:broader parentalguidance:_72.1 ;
        skos:inScheme <http://www.ebu.ch/metadata/ontologies/skos/ebu_ParentalGuidanceCodeCS> .

parentalguidance:_72.1.6 rdf:type ebucore:TargetAudience ;
        skos:prefLabel "18+"@en ;
        skos:definition "Mature Audience – Suitable for ages 18 and older"@en ;
        skos:broader parentalguidance:_72.1 ;
        skos:inScheme <http://www.ebu.ch/metadata/ontologies/skos/ebu_ParentalGuidanceCodeCS> .