<rdf:RDF
    xmlns:rdf="http://www.w3.org/1999/02/22-rdf-syntax-ns#"
    xmlns:ebucore="http://www.ebu.ch/metadata/ontologies/ebucore/ebucore#"
    xmlns:ebucoreext="https://metadata.amagi.tv/ebu/amagi_ebucoreExtension#"
    xmlns:owl="http://www.w3.org/2002/07/owl#"
    xmlns:skos="http://www.w3.org/2004/02/skos/core#"
    xmlns:rdfs="http://www.w3.org/2000/01/rdf-schema#" > 
  <rdf:Description rdf:about="https://metadata.amagi.tv/ebu/amagi_ebucoreExtension#hasAnnotation">
    <rdfs:range rdf:resource="http://www.ebu.ch/metadata/ontologies/ebucore/ebucore#Annotation"/>
    <rdfs:domain rdf:resource="https://metadata.amagi.tv/ebu/amagi_ebucoreExtension#AIAugmentedMeta"/>
    <rdfs:comment xml:lang="en">To associate annotation with an Asset</rdfs:comment>
    <rdfs:label xml:lang="en">hasAnnotation</rdfs:label>
    <rdf:type rdf:resource="http://www.w3.org/1999/02/22-rdf-syntax-ns#Property"/>
  </rdf:Description>
  <rdf:Description rdf:about="https://metadata.amagi.tv/ebu/amagi_ebucoreExtension#targetPlatformId">
    <rdfs:comment xml:lang="en">A specific platform id to which a media resource is to be targetted</rdfs:comment>
    <rdfs:range rdf:resource="http://www.w3.org/2001/XMLSchema#string"/>
    <rdfs:domain rdf:resource="http://www.ebu.ch/metadata/ontologies/ebucore/ebucore#Resource"/>
    <rdfs:domain rdf:resource="http://www.ebu.ch/metadata/ontologies/ebucore/ebucore#MediaResource"/>
    <rdfs:label xml:lang="en">targetPlatformId</rdfs:label>
    <rdf:type rdf:resource="http://www.w3.org/1999/02/22-rdf-syntax-ns#Property"/>
  </rdf:Description>
  <rdf:Description rdf:about="https://metadata.amagi.tv/ebu/amagi_ebucoreExtension#Cuepoint">
    <rdfs:subClassOf rdf:resource="http://www.w3.org/2002/07/owl#Thing"/>
    <rdfs:comment xml:lang="en">To provide cuepoint metadata for an asset.</rdfs:comment>
    <rdf:label xml:lang="en">Cuepoint</rdf:label>
    <rdf:type rdf:resource="http://www.w3.org/2000/01/rdf-schema#Class"/>
  </rdf:Description>
  <rdf:Description rdf:about="https://metadata.amagi.tv/ebu/amagi_ebucoreExtension#targetChannelId">
    <rdfs:comment xml:lang="en">A specific channel id to which a media resource is to be targetted</rdfs:comment>
    <rdfs:range rdf:resource="http://www.w3.org/2001/XMLSchema#string"/>
    <rdfs:domain rdf:resource="http://www.ebu.ch/metadata/ontologies/ebucore/ebucore#Resource"/>
    <rdfs:domain rdf:resource="http://www.ebu.ch/metadata/ontologies/ebucore/ebucore#MediaResource"/>
    <rdfs:label xml:lang="en">targetChannelId</rdfs:label>
    <rdf:type rdf:resource="http://www.w3.org/1999/02/22-rdf-syntax-ns#Property"/>
  </rdf:Description>
  <rdf:Description rdf:about="https://metadata.amagi.tv/ebu/amagi_ebucoreExtension#hasPublicationCap">
    <rdfs:label xml:lang="en">hasPublicationCap</rdfs:label>
    <rdfs:subPropertyOf rdf:resource="http://www.ebu.ch/metadata/ontologies/ebucore/ebucore#isCoveredBy"/>
    <rdfs:comment xml:lang="en">To express publication limits to airing</rdfs:comment>
    <rdfs:comment xml:lang="en">Publication Caps.</rdfs:comment>
    <rdfs:domain rdf:resource="http://www.ebu.ch/metadata/ontologies/ebucore/ebucore#PublicationRestrictions"/>
    <rdfs:range rdf:resource="https://metadata.amagi.tv/ebu/amagi_ebucoreExtension#PublicationCap"/>
    <rdf:type rdf:resource="http://www.w3.org/1999/02/22-rdf-syntax-ns#Property"/>
  </rdf:Description>
  <rdf:Description rdf:about="https://metadata.amagi.tv/ebu/amagi_ebucoreExtension#releaseCountry">
    <skos:definition xml:lang="en">This property denotes the country where the asset is released.</skos:definition>
    <rdfs:label xml:lang="en">releaseCountry</rdfs:label>
    <rdfs:isDefinedBy rdf:resource="https://metadata.amagi.tv/ebu/amagi_ebucoreExtension"/>
    <rdfs:domain rdf:resource="https://metadata.amagi.tv/ebu/amagi_ebucoreExtension#Release"/>
    <rdfs:range rdf:resource="http://www.ebu.ch/metadata/ontologies/ebucore/ebucore#CountryCode"/>
    <rdfs:range rdf:resource="http://www.w3.org/2001/XMLSchema#string"/>
    <rdf:type rdf:resource="http://www.w3.org/1999/02/22-rdf-syntax-ns#Property"/>
  </rdf:Description>
  <rdf:Description rdf:about="https://metadata.amagi.tv/ebu/amagi_ebucoreExtension#endAssetOffsetIndex">
    <rdfs:range rdf:resource="http://www.w3.org/2001/XMLSchema#string"/>
    <rdfs:domain rdf:resource="http://www.ebu.ch/metadata/ontologies/ebucore/ebucore#Part"/>
    <rdfs:label xml:lang="en">endAssetOffsetIndex</rdfs:label>
    <rdfs:comment xml:lang="en">To identify the asset index whose start is the end of a collection part. It may have 'eos' to indicate end is the end of the last asset in a collection </rdfs:comment>
    <rdf:type rdf:resource="http://www.w3.org/1999/02/22-rdf-syntax-ns#Property"/>
  </rdf:Description>
  <rdf:Description rdf:about="https://metadata.amagi.tv/ebu/amagi_ebucoreExtension#eventNumber">
    <rdfs:label xml:lang="en">eventNumber</rdfs:label>
    <rdfs:comment xml:lang="en">The event number in a superEvent. e.g. match number, game number</rdfs:comment>
    <rdfs:range rdf:resource="http://www.w3.org/2001/XMLSchema#string"/>
    <rdfs:domain rdf:resource="http://www.ebu.ch/metadata/ontologies/ebucore/ebucore#Event"/>
    <rdf:type rdf:resource="http://www.w3.org/1999/02/22-rdf-syntax-ns#Property"/>
  </rdf:Description>
  <rdf:Description rdf:about="https://metadata.amagi.tv/ebu/amagi_ebucoreExtension#publicationPeriod">
    <rdfs:comment xml:lang="en">The publication period associated with the publicationCap for a given PublicationRestrictions instance. Period examples 6H, 1M, 2M, 3D, 1W, 10D, 1D6H, 1M15D where H-&gt;hours, M is month, D is day, W is week.</rdfs:comment>
    <rdfs:label xml:lang="en">publicationPeriod</rdfs:label>
    <rdfs:domain rdf:resource="https://metadata.amagi.tv/ebu/amagi_ebucoreExtension#PublicationCap"/>
    <rdfs:range rdf:resource="http://www.w3.org/2001/XMLSchema#string"/>
    <rdf:type rdf:resource="http://www.w3.org/1999/02/22-rdf-syntax-ns#Property"/>
  </rdf:Description>
  <rdf:Description rdf:about="https://metadata.amagi.tv/ebu/amagi_ebucoreExtension#startAssetOffsetIndex">
    <rdfs:range rdf:resource="http://www.w3.org/2001/XMLSchema#string"/>
    <rdfs:domain rdf:resource="http://www.ebu.ch/metadata/ontologies/ebucore/ebucore#Part"/>
    <rdfs:label xml:lang="en">startAssetOffsetIndex</rdfs:label>
    <rdfs:comment xml:lang="en">To identify the asset index whose start is the start of a collection part </rdfs:comment>
    <rdf:type rdf:resource="http://www.w3.org/1999/02/22-rdf-syntax-ns#Property"/>
  </rdf:Description>
  <rdf:Description rdf:about="https://metadata.amagi.tv/ebu/amagi_ebucoreExtension">
    <owl:imports rdf:resource="http://www.ebu.ch/metadata/ontologies/ebucore/ebucore"/>
    <rdf:type rdf:resource="http://www.w3.org/2002/07/owl#Ontology"/>
  </rdf:Description>
  <rdf:Description rdf:about="https://metadata.amagi.tv/ebu/amagi_ebucoreExtension#hasAIAugmentedMeta">
    <rdfs:comment xml:lang="en">Property to associate an asset with its AI augmented metadata.</rdfs:comment>
    <rdfs:label xml:lang="en">hasAIAugmentedMeta</rdfs:label>
    <rdfs:domain rdf:resource="http://www.ebu.ch/metadata/ontologies/ebucore/ebucore#Asset"/>
    <rdfs:range rdf:resource="https://metadata.amagi.tv/ebu/amagi_ebucoreExtension#AIAugmentedMeta"/>
    <rdf:type rdf:resource="http://www.w3.org/1999/02/22-rdf-syntax-ns#Property"/>
  </rdf:Description>
  <rdf:Description rdf:about="https://metadata.amagi.tv/ebu/amagi_ebucoreExtension#hasEtcAnnotationLocation">
    <rdfs:label xml:lang="en">hasEtcAnnotationLocation</rdfs:label>
    <rdfs:comment xml:lang="en">Range: A uri pointing to AI generated etc(entity, topic, categories) metadata</rdfs:comment>
    <rdfs:range rdf:resource="http://www.w3.org/2001/XMLSchema#string"/>
    <rdfs:domain rdf:resource="https://metadata.amagi.tv/ebu/amagi_ebucoreExtension#AIAugmentedMeta"/>
    <rdf:type rdf:resource="http://www.w3.org/1999/02/22-rdf-syntax-ns#Property"/>
  </rdf:Description>
  <rdf:Description rdf:about="https://metadata.amagi.tv/ebu/amagi_ebucoreExtension#targetPlatformBrandId">
    <rdfs:comment xml:lang="en">A specific platform brand id to which a media resource is to be targetted</rdfs:comment>
    <rdfs:range rdf:resource="http://www.w3.org/2001/XMLSchema#string"/>
    <rdfs:domain rdf:resource="http://www.ebu.ch/metadata/ontologies/ebucore/ebucore#Resource"/>
    <rdfs:domain rdf:resource="http://www.ebu.ch/metadata/ontologies/ebucore/ebucore#MediaResource"/>
    <rdfs:label xml:lang="en">targetPlatformBrandId</rdfs:label>
    <rdf:type rdf:resource="http://www.w3.org/1999/02/22-rdf-syntax-ns#Property"/>
  </rdf:Description>
  <rdf:Description rdf:about="https://metadata.amagi.tv/ebu/amagi_ebucoreExtension#appliesToPlatformId">
    <rdfs:label xml:lang="en">Applies To PlatformId</rdfs:label>
    <rdfs:comment xml:lang="en">Specifies the platform_id for which the platform guide params are defined.</rdfs:comment>
    <rdfs:range rdf:resource="http://www.w3.org/2001/XMLSchema#string"/>
    <rdfs:domain rdf:resource="https://metadata.amagi.tv/ebu/amagi_ebucoreExtension#PlatformGuideParams"/>
    <rdf:type rdf:resource="http://www.w3.org/1999/02/22-rdf-syntax-ns#Property"/>
  </rdf:Description>
  <rdf:Description rdf:about="http://www.ebu.ch/metadata/ontologies/ebucore/ebucore#Image">
    <rdfs:subClassOf rdf:resource="http://www.ebu.ch/metadata/ontologies/ebucore/ebucore#Resource"/>
  </rdf:Description>
  <rdf:Description rdf:about="https://metadata.amagi.tv/ebu/amagi_ebucoreExtension/ebucore#MusicalEvent">
    <rdfs:comment xml:lang="en">To describe a musical event.</rdfs:comment>
    <rdfs:label xml:lang="en">Musical event</rdfs:label>
    <rdfs:subClassOf rdf:resource="http://www.ebu.ch/metadata/ontologies/ebucore/ebucore#Event"/>
    <rdf:type rdf:resource="http://www.w3.org/2000/01/rdf-schema#Class"/>
  </rdf:Description>
  <rdf:Description rdf:about="https://metadata.amagi.tv/ebu/amagi_ebucoreExtension#hasCuepoint">
    <rdfs:comment xml:lang="en">Property to associate an asset with its cuepoint metadata.</rdfs:comment>
    <rdfs:label xml:lang="en">hasCuepoint</rdfs:label>
    <rdfs:domain rdf:resource="http://www.ebu.ch/metadata/ontologies/ebucore/ebucore#Asset"/>
    <rdfs:range rdf:resource="https://metadata.amagi.tv/ebu/amagi_ebucoreExtension#Cuepoint"/>
    <rdf:type rdf:resource="http://www.w3.org/1999/02/22-rdf-syntax-ns#Property"/>
  </rdf:Description>
  <rdf:Description rdf:about="https://metadata.amagi.tv/ebu/amagi_ebucoreExtension#PublicationRestrictions">
    <rdfs:subClassOf rdf:resource="http://www.ebu.ch/metadata/ontologies/ebucore/ebucore#Rights"/>
    <rdfs:comment xml:lang="en">To express restriction on the number of times an asset can be published.</rdfs:comment>
    <rdfs:label xml:lang="en">PublicationRestrictions</rdfs:label>
    <rdf:type rdf:resource="http://www.w3.org/2000/01/rdf-schema#Class"/>
  </rdf:Description>
  <rdf:Description rdf:about="https://metadata.amagi.tv/ebu/amagi_ebucoreExtension#hasVideoAnnotationLocation">
    <rdfs:label xml:lang="en">hasVideoAnnotationLocation</rdfs:label>
    <rdfs:comment xml:lang="en">Range: A uri pointing to AI generated video metadata</rdfs:comment>
    <rdfs:range rdf:resource="http://www.w3.org/2001/XMLSchema#string"/>
    <rdfs:domain rdf:resource="https://metadata.amagi.tv/ebu/amagi_ebucoreExtension#AIAugmentedMeta"/>
    <rdf:type rdf:resource="http://www.w3.org/1999/02/22-rdf-syntax-ns#Property"/>
  </rdf:Description>
  <rdf:Description rdf:about="https://metadata.amagi.tv/ebu/amagi_ebucoreExtension#subCategories">
    <rdfs:label xml:lang="en">Sub category</rdfs:label>
    <rdfs:comment xml:lang="en">A subcategory is a more specific classification within a broader category.</rdfs:comment>
    <rdfs:range rdf:resource="http://www.w3.org/2001/XMLSchema#string"/>
    <rdfs:domain rdf:resource="https://metadata.amagi.tv/ebu/amagi_ebucoreExtension#PlatformGuideParams"/>
    <rdf:type rdf:resource="http://www.w3.org/1999/02/22-rdf-syntax-ns#Property"/>
  </rdf:Description>
  <rdf:Description rdf:about="https://metadata.amagi.tv/ebu/amagi_ebucoreExtension#hasProductionCountry">
    <skos:definition xml:lang="en">This property denotes the country of the production studio.</skos:definition>
    <rdfs:label xml:lang="en">Production Country</rdfs:label>
    <rdfs:isDefinedBy rdf:resource="https://metadata.amagi.tv/ebu/amagi_ebucoreExtension"/>
    <rdfs:domain rdf:resource="http://www.ebu.ch/metadata/ontologies/ebucore/ebucore#Asset"/>
    <rdfs:range rdf:resource="http://www.ebu.ch/metadata/ontologies/ebucore/ebucore#CountryCode"/>
    <rdfs:range rdf:resource="http://www.w3.org/2001/XMLSchema#string"/>
    <rdf:type rdf:resource="http://www.w3.org/1999/02/22-rdf-syntax-ns#Property"/>
  </rdf:Description>
  <rdf:Description rdf:about="https://metadata.amagi.tv/ebu/amagi_ebucoreExtension#isDirectedToChildren">
    <skos:definition xml:lang="en">This property denotes whether the asset has been targeted to children.</skos:definition>
    <rdfs:label xml:lang="en">Is directed to children</rdfs:label>
    <rdfs:isDefinedBy rdf:resource="https://metadata.amagi.tv/ebu/amagi_ebucoreExtension"/>
    <rdfs:domain rdf:resource="http://www.ebu.ch/metadata/ontologies/ebucore/ebucore#Asset"/>
    <rdfs:range rdf:resource="http://www.w3.org/2001/XMLSchema#boolean"/>
    <rdf:type rdf:resource="http://www.w3.org/1999/02/22-rdf-syntax-ns#Property"/>
  </rdf:Description>
  <rdf:Description rdf:about="https://metadata.amagi.tv/ebu/amagi_ebucoreExtension#hasPublicationRestrictions">
    <rdfs:label xml:lang="en">hasPublicationRestrictions</rdfs:label>
    <rdfs:subPropertyOf rdf:resource="http://www.ebu.ch/metadata/ontologies/ebucore/ebucore#isCoveredBy"/>
    <rdfs:comment xml:lang="en">To express publication restrictions like limits to airing</rdfs:comment>
    <rdfs:comment xml:lang="en">PublicationRestrictions.</rdfs:comment>
    <rdfs:domain rdf:resource="http://www.ebu.ch/metadata/ontologies/ebucore/ebucore#Asset"/>
    <rdfs:domain rdf:resource="http://www.ebu.ch/metadata/ontologies/ebucore/ebucore#PublicationEvent"/>
    <rdfs:range rdf:resource="https://metadata.amagi.tv/ebu/amagi_ebucoreExtension#PublicationRestrictions"/>
    <rdf:type rdf:resource="http://www.w3.org/1999/02/22-rdf-syntax-ns#Property"/>
  </rdf:Description>
  <rdf:Description rdf:about="https://metadata.amagi.tv/ebu/amagi_ebucoreExtension#hasParticipatingTeam">
    <rdfs:domain rdf:resource="http://www.ebu.ch/metadata/ontologies/ebucore/ebucore#SportsEvent"/>
    <rdfs:comment xml:lang="en">range: Agent or string</rdfs:comment>
    <rdfs:label xml:lang="en">Participating Team</rdfs:label>
    <rdfs:range rdf:resource="http://www.w3.org/2001/XMLSchema#string"/>
    <rdfs:range rdf:resource="http://www.ebu.ch/metadata/ontologies/ebucore/ebucore#Team"/>
    <rdfs:comment xml:lang="en">To identify participating Agents.</rdfs:comment>
    <rdf:type rdf:resource="http://www.w3.org/1999/02/22-rdf-syntax-ns#Property"/>
  </rdf:Description>
  <rdf:Description rdf:about="https://metadata.amagi.tv/ebu/amagi_ebucoreExtension/ebucore#hasEventGenre">
    <rdfs:comment xml:lang="en">Range: string or Genre</rdfs:comment>
    <rdfs:range rdf:resource="http://www.ebu.ch/metadata/ontologies/ebucore/ebucore#Genre"/>
    <rdfs:comment xml:lang="en">The genre of content associated with the Event.</rdfs:comment>
    <rdfs:domain rdf:resource="http://www.ebu.ch/metadata/ontologies/ebucore/ebucore#Event"/>
    <rdfs:label xml:lang="en">Event genre</rdfs:label>
    <rdfs:range rdf:resource="http://www.w3.org/2001/XMLSchema#string"/>
    <rdf:type rdf:resource="http://www.w3.org/1999/02/22-rdf-syntax-ns#Property"/>
  </rdf:Description>
  <rdf:Description rdf:about="https://metadata.amagi.tv/ebu/amagi_ebucoreExtension#Cuepoint_Type">
    <rdfs:label xml:lang="en">Cuepoint type</rdfs:label>
    <rdfs:subClassOf rdf:resource="http://www.w3.org/2004/02/skos/core#Concept"/>
    <rdfs:comment xml:lang="en">To define a type or cuepoint.</rdfs:comment>
    <rdf:type rdf:resource="http://www.w3.org/2000/01/rdf-schema#Class"/>
  </rdf:Description>
  <rdf:Description rdf:about="https://metadata.amagi.tv/ebu/amagi_ebucoreExtension#currentNumberOfEpisodes">
    <rdfs:range rdf:resource="http://www.w3.org/2001/XMLSchema#integer"/>
    <rdfs:domain rdf:resource="http://www.ebu.ch/metadata/ontologies/ebucore/ebucore#Group"/>
    <rdfs:label xml:lang="en">Current number of episodes</rdfs:label>
    <rdfs:comment xml:lang="en">To provide the current number of episodes in a Season.</rdfs:comment>
    <rdf:type rdf:resource="http://www.w3.org/1999/02/22-rdf-syntax-ns#Property"/>
  </rdf:Description>
  <rdf:Description rdf:about="http://www.ebu.ch/metadata/ontologies/ebucore/ebucore#hasPart">
    <rdfs:range rdf:resource="http://www.ebu.ch/metadata/ontologies/ebucore/ebucore#Part"/>
    <rdfs:label xml:lang="en">Part</rdfs:label>
    <rdfs:comment xml:lang="en">To define Parts (segments, fragments, shots, etc.)
            within an EditorialObject.</rdfs:comment>
    <rdfs:domain rdf:resource="https://metadata.amagi.tv/ebu/amagi_ebucoreExtension#AIAugmentedMeta"/>
    <rdf:type rdf:resource="http://www.w3.org/1999/02/22-rdf-syntax-ns#Property"/>
  </rdf:Description>
  <rdf:Description rdf:about="https://metadata.amagi.tv/ebu/amagi_ebucoreExtension#PlatformGuideParams">
    <rdfs:subClassOf rdf:resource="http://www.w3.org/2002/07/owl#Thing"/>
    <rdfs:comment xml:lang="en">To provide platform guide params metadata for an asset.</rdfs:comment>
    <rdf:label xml:lang="en">PlatformGuideParams</rdf:label>
    <rdf:type rdf:resource="http://www.w3.org/2000/01/rdf-schema#Class"/>
  </rdf:Description>
  <rdf:Description rdf:about="http://www.ebu.ch/metadata/ontologies/ebucore/ebucore#width">
    <rdfs:domain rdf:resource="http://www.ebu.ch/metadata/ontologies/ebucore/ebucore#Image"/>
    <rdfs:range rdf:resource="http://www.w3.org/2001/XMLSchema#integer"/>
  </rdf:Description>
  <rdf:Description rdf:about="https://metadata.amagi.tv/ebu/amagi_ebucoreExtension#cuepointTimestamp">
    <rdfs:label xml:lang="en">Cuepoint timestamp</rdfs:label>
    <rdfs:comment xml:lang="en">The time when the Cuepoint occurs. Cuepoint examples 12.0, 55.55, 105.6. These float values are converted to strings</rdfs:comment>
    <rdfs:range rdf:resource="http://www.w3.org/2001/XMLSchema#string"/>
    <rdfs:domain rdf:resource="https://metadata.amagi.tv/ebu/amagi_ebucoreExtension#Cuepoint"/>
    <rdf:type rdf:resource="http://www.w3.org/1999/02/22-rdf-syntax-ns#Property"/>
  </rdf:Description>
  <rdf:Description rdf:about="http://www.ebu.ch/metadata/ontologies/ebucore/ebucore#height">
    <rdfs:domain rdf:resource="http://www.ebu.ch/metadata/ontologies/ebucore/ebucore#Image"/>
    <rdfs:range rdf:resource="http://www.w3.org/2001/XMLSchema#integer"/>
  </rdf:Description>
  <rdf:Description rdf:about="https://metadata.amagi.tv/ebu/amagi_ebucoreExtension#hasCountryOfOrigin">
    <skos:definition xml:lang="en">This property denotes the country where the content was filmed.</skos:definition>
    <rdfs:label xml:lang="en">Country Of Origin</rdfs:label>
    <rdfs:isDefinedBy rdf:resource="https://metadata.amagi.tv/ebu/amagi_ebucoreExtension"/>
    <rdfs:domain rdf:resource="http://www.ebu.ch/metadata/ontologies/ebucore/ebucore#Asset"/>
    <rdfs:range rdf:resource="http://www.ebu.ch/metadata/ontologies/ebucore/ebucore#CountryCode"/>
    <rdfs:range rdf:resource="http://www.w3.org/2001/XMLSchema#string"/>
    <rdf:type rdf:resource="http://www.w3.org/1999/02/22-rdf-syntax-ns#Property"/>
  </rdf:Description>
  <rdf:Description rdf:about="https://metadata.amagi.tv/ebu/amagi_ebucoreExtension#isTitled">
    <rdfs:domain rdf:resource="http://www.ebu.ch/metadata/ontologies/ebucore/ebucore#Image"/>
    <skos:definition xml:lang="en">This is set to true if an image is titled. default is false. Titled images are ones with text e.g. banner with movie name, series name etc</skos:definition>
    <rdfs:label xml:lang="en">isTitled</rdfs:label>
    <rdfs:range rdf:resource="http://www.w3.org/2001/XMLSchema#boolean"/>
  </rdf:Description>
  <rdf:Description rdf:about="https://metadata.amagi.tv/ebu/amagi_ebucoreExtension#publicationCap">
    <rdfs:comment xml:lang="en">To express restriction on total number of times the media can be published per interval. </rdfs:comment>
    <rdfs:label xml:lang="en">publicationCap</rdfs:label>
    <rdfs:domain rdf:resource="https://metadata.amagi.tv/ebu/amagi_ebucoreExtension#PublicationCap"/>
    <rdfs:range rdf:resource="http://www.w3.org/2001/XMLSchema#string"/>
    <rdf:type rdf:resource="http://www.w3.org/1999/02/22-rdf-syntax-ns#Property"/>
  </rdf:Description>
  <rdf:Description rdf:about="https://metadata.amagi.tv/ebu/amagi_ebucoreExtension#Category">
    <rdfs:label xml:lang="en">Subject</rdfs:label>
    <rdfs:subClassOf rdf:resource="http://www.w3.org/2004/02/skos/core#Concept"/>
    <rdfs:comment xml:lang="en">A term describing the high level categorization of content covered by the
            BusinessObject or resource. This is provided as free text in an annotation label or as an identifier pointing to a term in a classification scheme e.g. https://cv.iptc.org/newscodes/mediatopic</rdfs:comment>
    <rdf:type rdf:resource="http://www.w3.org/2000/01/rdf-schema#Class"/>
  </rdf:Description>
  <rdf:Description rdf:about="https://metadata.amagi.tv/ebu/amagi_ebucoreExtension#mediaResourceName">
    <rdfs:comment xml:lang="en">The name given to a media resource.</rdfs:comment>
    <rdfs:range rdf:resource="http://www.w3.org/2001/XMLSchema#string"/>
    <rdfs:domain rdf:resource="http://www.ebu.ch/metadata/ontologies/ebucore/ebucore#MediaResource"/>
    <rdfs:label xml:lang="en">Resource name</rdfs:label>
    <rdf:type rdf:resource="http://www.w3.org/1999/02/22-rdf-syntax-ns#Property"/>
  </rdf:Description>
  <rdf:Description rdf:about="https://metadata.amagi.tv/ebu/amagi_ebucoreExtension/ebucore#sponsor">
    <rdfs:label xml:lang="en">sponsor</rdfs:label>
    <rdfs:comment xml:lang="en">Sponsor of an event. Equivalent to https://schema.org/sponsor. Example: Adidas AG is sponsor of 2014 FIFA World Cup</rdfs:comment>
    <rdfs:range rdf:resource="http://www.ebu.ch/metadata/ontologies/ebucore/ebucore#Agent"/>
    <rdfs:domain rdf:resource="http://www.ebu.ch/metadata/ontologies/ebucore/ebucore#Event"/>
    <rdf:type rdf:resource="http://www.w3.org/1999/02/22-rdf-syntax-ns#Property"/>
  </rdf:Description>
  <rdf:Description rdf:about="https://metadata.amagi.tv/ebu/amagi_ebucoreExtension#hasPlatformGuideParams">
    <rdfs:comment xml:lang="en">Specifies the category and its subcategories for particular platform.</rdfs:comment>
    <rdfs:label xml:lang="en">hasPlatformGuideParams</rdfs:label>
    <rdfs:domain rdf:resource="http://www.ebu.ch/metadata/ontologies/ebucore/ebucore#Asset"/>
    <rdfs:range rdf:resource="https://metadata.amagi.tv/ebu/amagi_ebucoreExtension#PlatformGuideParams"/>
    <rdf:type rdf:resource="http://www.w3.org/1999/02/22-rdf-syntax-ns#Property"/>
  </rdf:Description>
  <rdf:Description rdf:about="https://metadata.amagi.tv/ebu/amagi_ebucoreExtension#hasEventRelatedPicture">
    <rdfs:comment xml:lang="en">A link/locator to a picture related to an Event.</rdfs:comment>
    <rdfs:range rdf:resource="http://www.ebu.ch/metadata/ontologies/ebucore/ebucore#Picture"/>
    <rdfs:domain rdf:resource="http://www.ebu.ch/metadata/ontologies/ebucore/ebucore#Event"/>
    <rdfs:label xml:lang="en">Event Related picture</rdfs:label>
    <rdf:type rdf:resource="http://www.w3.org/1999/02/22-rdf-syntax-ns#Property"/>
  </rdf:Description>
  <rdf:Description rdf:about="https://metadata.amagi.tv/ebu/amagi_ebucoreExtension#mainCategory">
    <rdfs:label xml:lang="en">Main category</rdfs:label>
    <rdfs:comment xml:lang="en">A category is a broad classification that groups similar types of content or products within a particular platform.</rdfs:comment>
    <rdfs:range rdf:resource="http://www.w3.org/2001/XMLSchema#string"/>
    <rdfs:domain rdf:resource="https://metadata.amagi.tv/ebu/amagi_ebucoreExtension#PlatformGuideParams"/>
    <rdf:type rdf:resource="http://www.w3.org/1999/02/22-rdf-syntax-ns#Property"/>
  </rdf:Description>
  <rdf:Description rdf:about="https://metadata.amagi.tv/ebu/amagi_ebucoreExtension#audioChannelLayout">
    <rdfs:comment xml:lang="en">The arrangement and spatial configuration of audio channels within an audio stream. Possible values are mono, stereo, 2.1, 3, quad, 3.1, 4.1, 5.1, 7.1. These values are derived from the standard channel layouts listed at https://trac.ffmpeg.org/wiki/AudioChannelManipulation#Listchannelnamesandstandardchannellayouts</rdfs:comment>
    <rdfs:range rdf:resource="http://www.w3.org/2001/XMLSchema#string"/>
    <rdfs:domain rdf:resource="http://www.ebu.ch/metadata/ontologies/ebucore/ebucore#AudioTrack"/>
    <rdfs:label xml:lang="en">Audio Channel Layout</rdfs:label>
    <rdf:type rdf:resource="http://www.w3.org/1999/02/22-rdf-syntax-ns#Property"/>
  </rdf:Description>
  <rdf:Description rdf:about="https://metadata.amagi.tv/ebu/amagi_ebucoreExtension#Release">
    <rdfs:subClassOf rdf:resource="http://www.w3.org/2002/07/owl#Thing"/>
    <rdfs:comment xml:lang="en">To provide release metadata for an asset.</rdfs:comment>
    <rdfs:label xml:lang="en">Release</rdfs:label>
    <rdf:type rdf:resource="http://www.w3.org/2000/01/rdf-schema#Class"/>
  </rdf:Description>
  <rdf:Description rdf:about="https://metadata.amagi.tv/ebu/amagi_ebucoreExtension#hasCuepointType">
    <rdfs:label xml:lang="en">Cuepoint type</rdfs:label>
    <rdfs:range rdf:resource="http://www.w3.org/2001/XMLSchema#anyURI"/>
    <rdfs:range rdf:resource="https://metadata.amagi.tv/ebu/amagi_ebucoreExtension#Cuepoint_Type"/>
    <rdfs:comment xml:lang="en">A type of Cuepoint.</rdfs:comment>
    <rdfs:range rdf:resource="http://www.w3.org/2001/XMLSchema#string"/>
    <rdfs:domain rdf:resource="https://metadata.amagi.tv/ebu/amagi_ebucoreExtension#Cuepoint"/>
    <rdf:type rdf:resource="http://www.w3.org/1999/02/22-rdf-syntax-ns#Property"/>
  </rdf:Description>
  <rdf:Description rdf:about="https://metadata.amagi.tv/ebu/amagi_ebucoreExtension#VideoAnnotation">
    <rdfs:subClassOf rdf:resource="http://www.ebu.ch/metadata/ontologies/ebucore/ebucore#Annotation"/>
    <rdfs:comment xml:lang="en">A class specific to the annotation of a video asset.</rdfs:comment>
    <rdfs:label xml:lang="en">VideoAnnotation</rdfs:label>
    <rdf:type rdf:resource="http://www.w3.org/2000/01/rdf-schema#Class"/>
  </rdf:Description>
  <rdf:Description rdf:about="http://www.ebu.ch/metadata/ontologies/ebucore/ebucore#dateReleased">
    <rdfs:domain rdf:resource="https://metadata.amagi.tv/ebu/amagi_ebucoreExtension#Release"/>
  </rdf:Description>
  <rdf:Description rdf:about="https://metadata.amagi.tv/ebu/amagi_ebucoreExtension#hasRelease">
    <rdfs:comment xml:lang="en">Property to associate an asset with its release metadata.</rdfs:comment>
    <rdfs:label xml:lang="en">hasRelease</rdfs:label>
    <rdfs:domain rdf:resource="http://www.ebu.ch/metadata/ontologies/ebucore/ebucore#Asset"/>
    <rdfs:range rdf:resource="https://metadata.amagi.tv/ebu/amagi_ebucoreExtension#Release"/>
    <rdf:type rdf:resource="http://www.w3.org/1999/02/22-rdf-syntax-ns#Property"/>
  </rdf:Description>
  <rdf:Description rdf:about="https://metadata.amagi.tv/ebu/amagi_ebucoreExtension#maxPublicationEvents">
    <rdfs:comment xml:lang="en">To express restriction on the maximum number of publication events for an asset in a given date range.</rdfs:comment>
    <rdfs:label xml:lang="en">maxPublicationEvents</rdfs:label>
    <rdfs:domain rdf:resource="http://www.ebu.ch/metadata/ontologies/ebucore/ebucore#UsageRestrictions"/>
    <rdfs:range rdf:resource="http://www.w3.org/2001/XMLSchema#integer"/>
    <rdf:type rdf:resource="http://www.w3.org/1999/02/22-rdf-syntax-ns#Property"/>
  </rdf:Description>
  <rdf:Description rdf:about="https://metadata.amagi.tv/ebu/amagi_ebucoreExtension#scopeNote">
    <skos:scopeNote xml:lang="en">This property may be used directly to annotate any owl:thing within ebucore scope</skos:scopeNote>
    <skos:definition xml:lang="en">A note to denote the scope of a grounded entity. Specifically useful to denote the manual-edits, active-meta</skos:definition>
    <rdfs:label xml:lang="en">scopeNote</rdfs:label>
    <rdfs:isDefinedBy rdf:resource="https://metadata.amagi.tv/ebu/amagi_ebucoreExtension"/>
    <rdf:type rdf:resource="http://www.w3.org/2002/07/owl#AnnotationProperty"/>
    <rdf:type rdf:resource="http://www.w3.org/1999/02/22-rdf-syntax-ns#Property"/>
  </rdf:Description>
  <rdf:Description rdf:about="https://metadata.amagi.tv/ebu/amagi_ebucoreExtension/ebucore#superEvent">
    <rdfs:label xml:lang="en">superEvent</rdfs:label>
    <rdfs:domain rdf:resource="http://www.ebu.ch/metadata/ontologies/ebucore/ebucore#Event"/>
    <rdfs:range rdf:resource="http://www.ebu.ch/metadata/ontologies/ebucore/ebucore#Event"/>
    <rdfs:comment xml:lang="en">To identify parent event to which an event belongs to. Equivalent to https://schema.org/superEvent</rdfs:comment>
    <rdf:type rdf:resource="http://www.w3.org/1999/02/22-rdf-syntax-ns#Property"/>
  </rdf:Description>
  <rdf:Description rdf:about="https://metadata.amagi.tv/ebu/amagi_ebucoreExtension#SportsEvent">
    <rdfs:comment xml:lang="en">To describe a sports event.</rdfs:comment>
    <rdfs:label xml:lang="en">Sports event</rdfs:label>
    <rdfs:subClassOf rdf:resource="http://www.ebu.ch/metadata/ontologies/ebucore/ebucore#Event"/>
    <rdf:type rdf:resource="http://www.w3.org/2000/01/rdf-schema#Class"/>
  </rdf:Description>
  <rdf:Description rdf:about="https://metadata.amagi.tv/ebu/amagi_ebucoreExtension#isAttributedTo">
    <skos:definition xml:lang="en">This property allows to denote the attribution of an asset's metadata to its source url. The source urls could be media rss feed url or a source csv location.</skos:definition>
    <rdfs:label xml:lang="en">SourceAttribution</rdfs:label>
    <rdfs:isDefinedBy rdf:resource="https://metadata.amagi.tv/ebu/amagi_ebucoreExtension"/>
    <rdfs:domain rdf:resource="http://www.ebu.ch/metadata/ontologies/ebucore/ebucore#Asset"/>
    <rdfs:range rdf:resource="http://www.w3.org/2001/XMLSchema#anyURI"/>
    <rdfs:range rdf:resource="http://www.w3.org/2001/XMLSchema#string"/>
    <rdf:type rdf:resource="http://www.w3.org/1999/02/22-rdf-syntax-ns#Property"/>
  </rdf:Description>
  <rdf:Description rdf:about="https://metadata.amagi.tv/ebu/amagi_ebucoreExtension/ebucore#PoliticalEvent">
    <rdfs:comment xml:lang="en">To describe a political event, e.g. election campaign, debate etc.</rdfs:comment>
    <rdfs:label xml:lang="en">Political event</rdfs:label>
    <rdfs:subClassOf rdf:resource="http://www.ebu.ch/metadata/ontologies/ebucore/ebucore#Event"/>
    <rdf:type rdf:resource="http://www.w3.org/2000/01/rdf-schema#Class"/>
  </rdf:Description>
  <rdf:Description rdf:about="https://metadata.amagi.tv/ebu/amagi_ebucoreExtension/ebucore#organizer">
    <rdfs:label xml:lang="en">organizer</rdfs:label>
    <rdfs:comment xml:lang="en">Organizer of an event. Equivalent to https://schema.org/organizer. Example: FIFA is organizer of 2014 FIFA World Cup</rdfs:comment>
    <rdfs:range rdf:resource="http://www.ebu.ch/metadata/ontologies/ebucore/ebucore#Agent"/>
    <rdfs:domain rdf:resource="http://www.ebu.ch/metadata/ontologies/ebucore/ebucore#Event"/>
    <rdf:type rdf:resource="http://www.w3.org/1999/02/22-rdf-syntax-ns#Property"/>
  </rdf:Description>
  <rdf:Description rdf:about="http://www.ebu.ch/metadata/ontologies/ebucore/ebucore#annotationId">
    <rdfs:range rdf:resource="http://www.ebu.ch/metadata/ontologies/ebucore/ebucore#Identifier"/>
  </rdf:Description>
  <rdf:Description rdf:about="https://metadata.amagi.tv/ebu/amagi_ebucoreExtension#AIAugmentedMeta">
    <rdfs:subClassOf rdf:resource="http://www.w3.org/2002/07/owl#Thing"/>
    <rdfs:comment xml:lang="en">To provide AI augmented metadata for an asset.</rdfs:comment>
    <rdfs:label xml:lang="en">AIAugmentedMeta</rdfs:label>
    <rdf:type rdf:resource="http://www.w3.org/2000/01/rdf-schema#Class"/>
  </rdf:Description>
  <rdf:Description rdf:about="https://metadata.amagi.tv/ebu/amagi_ebucoreExtension#PublicationCap">
    <rdfs:subClassOf rdf:resource="http://www.w3.org/2002/07/owl#Thing"/>
    <rdfs:comment xml:lang="en">To provide information to restrict publications in a given interval of time</rdfs:comment>
    <rdfs:label xml:lang="en">PublicationCap</rdfs:label>
    <rdf:type rdf:resource="http://www.w3.org/2000/01/rdf-schema#Class"/>
  </rdf:Description>
  <rdf:Description rdf:about="https://metadata.amagi.tv/ebu/amagi_ebucoreExtension#Entity">
    <rdfs:label xml:lang="en">Entity</rdfs:label>
    <owl:equivalentClass rdf:resource="http://www.ebu.ch/metadata/ontologies/ebucore/ebucore#Keyword"/>
    <rdfs:subClassOf rdf:resource="http://www.w3.org/2004/02/skos/core#Concept"/>
    <rdfs:comment xml:lang="en">To proivde key entites associated with an asset.</rdfs:comment>
    <rdf:type rdf:resource="http://www.w3.org/2000/01/rdf-schema#Class"/>
  </rdf:Description>
  <rdf:Description rdf:about="https://metadata.amagi.tv/ebu/amagi_ebucoreExtension#Graphic">
    <rdfs:subClassOf rdf:resource="http://www.ebu.ch/metadata/ontologies/ebucore/ebucore#EditorialObject"/>
    <rdfs:comment xml:lang="en">Entity to represent the graphic to be used as overlay</rdfs:comment>
    <rdfs:label xml:lang="en">Graphic</rdfs:label>
    <rdf:type rdf:resource="http://www.w3.org/2000/01/rdf-schema#Class"/>
  </rdf:Description>
  <rdf:Description rdf:about="https://metadata.amagi.tv/ebu/amagi_ebucoreExtension#userDefinedFps">
    <rdfs:domain rdf:resource="http://www.ebu.ch/metadata/ontologies/ebucore/ebucore#Asset"/>
    <rdfs:range rdf:resource="http://www.w3.org/2001/XMLSchema#string" />
    <rdfs:comment xml:lang="en">The unit used to express the user provided frame rate of a MediaResource in frames/second associated with an ebucore asset.</rdfs:comment>
    <rdfs:label xml:lang="en">User Defined Frame Rate</rdfs:label>
    <rdf:type rdf:resource="http://www.w3.org/1999/02/22-rdf-syntax-ns#Property"/>
  </rdf:Description>
  <rdf:Description rdf:about="https://metadata.amagi.tv/ebu/amagi_ebucoreExtension#isPatched">
    <rdfs:domain rdf:resource="http://www.ebu.ch/metadata/ontologies/ebucore/ebucore#Resource"/>
    <rdfs:range rdf:resource="http://www.w3.org/2001/XMLSchema#boolean" />
    <rdfs:comment xml:lang="en">Used to denote if an artefact has been added through patch.</rdfs:comment>
    <rdfs:label xml:lang="en">Is Patched</rdfs:label>
    <rdf:type rdf:resource="http://www.w3.org/1999/02/22-rdf-syntax-ns#Property"/>
  </rdf:Description>
    <rdf:Description rdf:about="https://metadata.amagi.tv/ebu/amagi_ebucoreExtension#CustomKeyValue">
    <rdfs:subClassOf rdf:resource="http://www.w3.org/2002/07/owl#Thing"/>
    <rdfs:comment xml:lang="en">Class to represent specific key value pairs</rdfs:comment>
    <rdfs:label xml:lang="en">CustomKeyValue</rdfs:label>
    <rdf:type rdf:resource="http://www.w3.org/2000/01/rdf-schema#Class"/>
  </rdf:Description>
  <rdf:Description rdf:about="https://metadata.amagi.tv/ebu/amagi_ebucoreExtension#customKey">
    <rdfs:label xml:lang="en">Custom Key Value</rdfs:label>
    <rdfs:domain rdf:resource="https://metadata.amagi.tv/ebu/amagi_ebucoreExtension#CustomKeyValue"/>
    <rdfs:comment xml:lang="en">Key string of CustomKeyValue</rdfs:comment>
    <rdfs:range rdf:resource="http://www.w3.org/2001/XMLSchema#string"/>
    <rdf:type rdf:resource="http://www.w3.org/1999/02/22-rdf-syntax-ns#Property"/>
  </rdf:Description>
    <rdf:Description rdf:about="https://metadata.amagi.tv/ebu/amagi_ebucoreExtension#customValue">
    <rdfs:label xml:lang="en">custom value</rdfs:label>
    <rdfs:domain rdf:resource="https://metadata.amagi.tv/ebu/amagi_ebucoreExtension#CustomKeyValue"/>
    <rdfs:comment xml:lang="en">Value string of CustomKeyValue</rdfs:comment>
    <rdfs:range rdf:resource="http://www.w3.org/2001/XMLSchema#string"/>
    <rdf:type rdf:resource="http://www.w3.org/1999/02/22-rdf-syntax-ns#Property"/>
  </rdf:Description>
</rdf:RDF>
